@prefix : <http://bigg-project.eu/ontology#> .
@prefix cp: <http://www.w3.org/2015/03/inspire/cp#> .
@prefix dc: <http://purl.org/dc/elements/1.1/> .
@prefix gn: <https://www.geonames.org/ontology#> .
@prefix owl: <http://www.w3.org/2002/07/owl#> .
@prefix rdf: <http://www.w3.org/1999/02/22-rdf-syntax-ns#> .
@prefix ssn: <http://www.w3.org/ns/ssn/> .
@prefix xml: <http://www.w3.org/XML/1998/namespace> .
@prefix xsd: <http://www.w3.org/2001/XMLSchema#> .
@prefix bigg: <http://bigg-project.eu/ontology#> .
@prefix foaf: <http://xmlns.com/foaf/0.1/> .
@prefix prov: <http://www.w3.org/ns/prov#> .
@prefix rdfs: <http://www.w3.org/2000/01/rdf-schema#> .
@prefix skos: <http://www.w3.org/2004/02/skos/core#> .
@prefix sosa: <http://www.w3.org/ns/sosa/> .
@prefix time: <http://www.w3.org/2006/time#> .
@prefix geosp: <http://www.opengis.net/ont/geosparql#> .
@prefix icaen: <http://bigg-project.eu/data#> .
@prefix saref: <https://saref.etsi.org/core/> .
@prefix vcard: <http://www.w3.org/2006/vcard/ns#> .
@prefix wgs84: <http://www.w3.org/2003/01/geo/wgs84_pos#> .
@prefix s4agri: <https://saref.etsi.org/saref4agri/> .
@prefix s4bldg: <https://saref.etsi.org/saref4bldg/> .
@prefix s4city: <https://saref.etsi.org/saref4city/> .
@prefix s4syst: <https://saref.etsi.org/saref4syst/> .
@prefix s4watr: <https://saref.etsi.org/saref4watr/> .
@prefix schema: <https://schema.org/> .
@prefix dcterms: <http://purl.org/dc/terms/> .
@base <http://bigg-project.eu/ontology#> .

<http://bigg-project.eu/ontology#> rdf:type owl:Ontology ;
                                    owl:imports <http://www.w3.org/2006/time#2016> .

#################################################################
#    Annotation properties
#################################################################

###  http://purl.org/dc/elements/1.1/date
dc:date rdf:type owl:AnnotationProperty .


###  http://purl.org/dc/elements/1.1/description
dc:description rdf:type owl:AnnotationProperty .


###  http://purl.org/dc/elements/1.1/title
dc:title rdf:type owl:AnnotationProperty .


###  http://purl.org/dc/terms/abstract
dcterms:abstract rdf:type owl:AnnotationProperty .


###  http://purl.org/dc/terms/contributor
dcterms:contributor rdf:type owl:AnnotationProperty .


###  http://purl.org/dc/terms/created
dcterms:created rdf:type owl:AnnotationProperty .


###  http://purl.org/dc/terms/creator
dcterms:creator rdf:type owl:AnnotationProperty .


###  http://purl.org/dc/terms/dateCopyrighted
dcterms:dateCopyrighted rdf:type owl:AnnotationProperty .


###  http://purl.org/dc/terms/description
dcterms:description rdf:type owl:AnnotationProperty .


###  http://purl.org/dc/terms/issued
dcterms:issued rdf:type owl:AnnotationProperty .


###  http://purl.org/dc/terms/license
dcterms:license rdf:type owl:AnnotationProperty .


###  http://purl.org/dc/terms/modified
dcterms:modified rdf:type owl:AnnotationProperty .


###  http://purl.org/dc/terms/publisher
dcterms:publisher rdf:type owl:AnnotationProperty .


###  http://purl.org/dc/terms/replaces
dcterms:replaces rdf:type owl:AnnotationProperty .


###  http://purl.org/dc/terms/rights
dcterms:rights rdf:type owl:AnnotationProperty .


###  http://purl.org/dc/terms/rightsHolder
dcterms:rightsHolder rdf:type owl:AnnotationProperty .


###  http://purl.org/dc/terms/source
dcterms:source rdf:type owl:AnnotationProperty .


###  http://purl.org/dc/terms/title
dcterms:title rdf:type owl:AnnotationProperty .


###  http://purl.org/vocab/vann/preferredNamespacePrefix
<http://purl.org/vocab/vann/preferredNamespacePrefix> rdf:type owl:AnnotationProperty .


###  http://purl.org/vocab/vann/preferredNamespaceUri
<http://purl.org/vocab/vann/preferredNamespaceUri> rdf:type owl:AnnotationProperty .


###  http://www.w3.org/2001/XMLSchema#pattern
xsd:pattern rdf:type owl:AnnotationProperty .


###  http://www.w3.org/2003/01/geo/wgs84_pos#alt
wgs84:alt rdf:type owl:AnnotationProperty ;
          rdfs:domain wgs84:SpatialThing .


###  http://www.w3.org/2003/01/geo/wgs84_pos#lat
wgs84:lat rdf:type owl:AnnotationProperty ;
          rdfs:domain wgs84:SpatialThing .


###  http://www.w3.org/2003/01/geo/wgs84_pos#location
wgs84:location rdf:type owl:AnnotationProperty ;
               rdfs:range wgs84:SpatialThing .


###  http://www.w3.org/2003/01/geo/wgs84_pos#long
wgs84:long rdf:type owl:AnnotationProperty .


###  http://www.w3.org/2004/02/skos/core#changeNote
skos:changeNote rdf:type owl:AnnotationProperty .


###  http://www.w3.org/2004/02/skos/core#definition
skos:definition rdf:type owl:AnnotationProperty .


###  http://www.w3.org/2004/02/skos/core#editorialNote
skos:editorialNote rdf:type owl:AnnotationProperty .


###  http://www.w3.org/2004/02/skos/core#example
skos:example rdf:type owl:AnnotationProperty .


###  http://www.w3.org/2004/02/skos/core#historyNote
skos:historyNote rdf:type owl:AnnotationProperty .


###  http://www.w3.org/2004/02/skos/core#note
skos:note rdf:type owl:AnnotationProperty .


###  http://www.w3.org/2004/02/skos/core#prefLabel
skos:prefLabel rdf:type owl:AnnotationProperty .


###  http://www.w3.org/2004/02/skos/core#scopeNote
skos:scopeNote rdf:type owl:AnnotationProperty .


###  http://www.w3.org/ns/prov#hadPrimarySource
prov:hadPrimarySource rdf:type owl:AnnotationProperty .


###  http://xmlns.com/foaf/0.1/PersonalProfileDocument
foaf:PersonalProfileDocument rdf:type owl:AnnotationProperty .


###  http://xmlns.com/foaf/0.1/homepage
foaf:homepage rdf:type owl:AnnotationProperty .


###  http://xmlns.com/foaf/0.1/name
foaf:name rdf:type owl:AnnotationProperty .


###  https://schema.org/affiliation
schema:affiliation rdf:type owl:AnnotationProperty .


###  https://schema.org/email
schema:email rdf:type owl:AnnotationProperty .


###  https://schema.org/name
schema:name rdf:type owl:AnnotationProperty .


###  https://schema.org/url
schema:url rdf:type owl:AnnotationProperty .


#################################################################
#    Datatypes
#################################################################

###  http://www.opengis.net/ont/geosparql#dggsLiteral
geosp:dggsLiteral rdf:type rdfs:Datatype ;
                  rdfs:isDefinedBy geosp: ,
                                   <http://www.opengis.net/spec/geosparql/1.1/req/geometry-extension/dggs-literal> ;
                  rdfs:seeAlso <http://www.opengis.net/doc/AS/dggs/2.0> ;
                  skos:definition "A textual serialization of a Discrete Global Grid (DGGS) Geometry object."@en ;
                  skos:example <http://www.opengis.net/spec/geosparql/1.1/specification.html#B.1.2.4> ,
                               " \"<https://w3id.org/dggs/auspix> OrdinateList (R3234)\"^^<http://www.opengis.net/ont/geosparql#dggsLiteral>" ;
                  skos:prefLabel "DGGS Literal"@en ;
                  skos:scopeNote "This datatype is not expected to be used directly but to serve as an abstract datatype for a series of specific DGGS literal types, for specific DGGS implementations" .


###  http://www.opengis.net/ont/geosparql#geoJSONLiteral
geosp:geoJSONLiteral rdf:type rdfs:Datatype ;
                     rdfs:isDefinedBy geosp: ,
                                      <http://www.opengis.net/spec/geosparql/1.1/req/geometry-extension/geojson-literal> ;
                     rdfs:seeAlso <https://tools.ietf.org/html/rfc7946> ;
                     skos:definition "A GeoJSON serialization of a Geometry object."@en ;
                     skos:example <http://www.opengis.net/spec/geosparql/1.1/specification.html#B.1.2.4> ;
                     skos:prefLabel "GeoJSON Literal"@en .


###  http://www.opengis.net/ont/geosparql#gmlLiteral
geosp:gmlLiteral rdf:type rdfs:Datatype ;
                 rdfs:isDefinedBy geosp: ,
                                  <http://www.opengis.net/spec/geosparql/1.0/req/geometry-extension/gml-literal> ,
                                  <http://www.opengis.net/spec/geosparql/1.1/req/geometry-extension/gml-literal> ;
                 rdfs:seeAlso <https://portal.ogc.org/files/?artifact_id=20509> ;
                 skos:definition "A GML serialization of a Geometry object."@en ;
                 skos:example <http://www.opengis.net/spec/geosparql/1.1/specification.html#B.1.2.4> ;
                 skos:prefLabel "GML Literal"@en .


###  http://www.opengis.net/ont/geosparql#kmlLiteral
geosp:kmlLiteral rdf:type rdfs:Datatype ;
                 rdfs:isDefinedBy geosp: ,
                                  <http://www.opengis.net/spec/geosparql/1.1/req/geometry-extension/kml-literal> ;
                 rdfs:seeAlso <https://www.ogc.org/standards/kml/> ;
                 skos:definition "A KML serialization of a Geometry object."@en ;
                 skos:example <http://www.opengis.net/spec/geosparql/1.1/specification.html#B.1.2.4> ;
                 skos:prefLabel "KML Literal"@en .


###  http://www.opengis.net/ont/geosparql#wktLiteral
geosp:wktLiteral rdf:type rdfs:Datatype ;
                 rdfs:isDefinedBy geosp: ,
                                  <http://www.opengis.net/spec/geosparql/1.0/req/geometry-extension/wkt-literal> ,
                                  <http://www.opengis.net/spec/geosparql/1.1/req/geometry-extension/wkt-literal> ;
                 rdfs:seeAlso <https://portal.ogc.org/files/?artifact_id=25355> ;
                 skos:definition "A Well-known Text serialization of a Geometry object."@en ;
                 skos:example <http://www.opengis.net/spec/geosparql/1.1/specification.html#B.2.2.2> ;
                 skos:prefLabel "Well-known Text Literal"@en .


###  http://www.w3.org/2001/XMLSchema#date
xsd:date rdf:type rdfs:Datatype .


###  http://www.w3.org/2001/XMLSchema#dateTimeStamp
xsd:dateTimeStamp rdfs:label "sello de tiempo"@es .


###  http://www.w3.org/2001/XMLSchema#duration
xsd:duration rdf:type rdfs:Datatype .


###  http://www.w3.org/2001/XMLSchema#gDay
xsd:gDay rdf:type rdfs:Datatype .


###  http://www.w3.org/2001/XMLSchema#gMonth
xsd:gMonth rdf:type rdfs:Datatype .


###  http://www.w3.org/2001/XMLSchema#gYear
xsd:gYear rdf:type rdfs:Datatype .


###  http://www.w3.org/2001/XMLSchema#gYearMonth
xsd:gYearMonth rdf:type rdfs:Datatype .


###  http://www.w3.org/2006/time#generalDay
time:generalDay rdf:type rdfs:Datatype ;
                rdfs:comment """Day of month - formulated as a text string with a pattern constraint to reproduce the same lexical form as gDay, except that values up to 99 are permitted, in order to support calendars with more than 31 days in a month. 
Note that the value-space is not defined, so a generic OWL2 processor cannot compute ordering relationships of values of this type."""@en ,
                             """Día del mes - formulado como una cadena de texto con una restricción patrón para reproducir la misma forma léxica que gDay, excepto que se permiten valores hasta el 99, con el propósito de proporcionar soporte a calendarios con meses con más de 31 días.
            Nótese que el espacio de valores no está definido, por tanto, un procesador genérico de OWL2 no puede computar relaciones de orden de valores de este tipo."""@es ;
                rdfs:label "Día generalizado"@es ,
                           "Generalized day"@en ;
                skos:definition """Day of month - formulated as a text string with a pattern constraint to reproduce the same lexical form as gDay, except that values up to 99 are permitted, in order to support calendars with more than 31 days in a month. 
Note that the value-space is not defined, so a generic OWL2 processor cannot compute ordering relationships of values of this type."""@en ,
                                """Día del mes - formulado como una cadena de texto con una restricción patrón para reproducir la misma forma léxica que gDay, excepto que se permiten valores hasta el 99, con el propósito de proporcionar soporte a calendarios con meses con más de 31 días.
            Nótese que el espacio de valores no está definido, por tanto, un procesador genérico de OWL2 no puede computar relaciones de orden de valores de este tipo."""@es .


###  http://www.w3.org/2006/time#generalMonth
time:generalMonth rdf:type rdfs:Datatype ;
                  rdfs:comment """Mes del año - formulado como una cadena de texto con una restricción patrón para reproducir la misma forma léxica que gMonth, excepto que se permiten valores hasta el 20, con el propósito de proporcionar soporte a calendarios con años con más de 12 meses.
            Nótese que el espacio de valores no está definido, por tanto, un procesador genérico de OWL2 no puede computar relaciones de orden de valores de este tipo."""@es ,
                               """Month of year - formulated as a text string with a pattern constraint to reproduce the same lexical form as gMonth, except that values up to 20 are permitted, in order to support calendars with more than 12 months in the year. 
Note that the value-space is not defined, so a generic OWL2 processor cannot compute ordering relationships of values of this type."""@en ;
                  rdfs:label "Generalized month"@en ,
                             "Mes generalizado"@es ;
                  skos:definition """Mes del año - formulado como una cadena de texto con una restricción patrón para reproducir la misma forma léxica que gMonth, excepto que se permiten valores hasta el 20, con el propósito de proporcionar soporte a calendarios con años con más de 12 meses.
            Nótese que el espacio de valores no está definido, por tanto, un procesador genérico de OWL2 no puede computar relaciones de orden de valores de este tipo."""@es ,
                                  """Month of year - formulated as a text string with a pattern constraint to reproduce the same lexical form as gMonth, except that values up to 20 are permitted, in order to support calendars with more than 12 months in the year. 
Note that the value-space is not defined, so a generic OWL2 processor cannot compute ordering relationships of values of this type."""@en .


###  http://www.w3.org/2006/time#generalYear
time:generalYear rdf:type rdfs:Datatype ;
                 rdfs:comment """Número de año - formulado como una cadena de texto con una restricción patrón para reproducir la misma forma léxica que gYear, aunque no está restringido a valores del calendario gregoriano.
            Nótese que el espacio de valores no está definido, por tanto, un procesador genérico de OWL2 no puede computar relaciones de orden de valores de este tipo."""@es ,
                              """Year number - formulated as a text string with a pattern constraint to reproduce the same lexical form as gYear, but not restricted to values from the Gregorian calendar. 
Note that the value-space is not defined, so a generic OWL2 processor cannot compute ordering relationships of values of this type."""@en ;
                 rdfs:label "Año generalizado"@es ,
                            "Generalized year"@en ;
                 skos:definition """Número de año - formulado como una cadena de texto con una restricción patrón para reproducir la misma forma léxica que gYear, aunque no está restringido a valores del calendario gregoriano.
            Nótese que el espacio de valores no está definido, por tanto, un procesador genérico de OWL2 no puede computar relaciones de orden de valores de este tipo."""@es ,
                                 """Year number - formulated as a text string with a pattern constraint to reproduce the same lexical form as gYear, but not restricted to values from the Gregorian calendar. 
Note that the value-space is not defined, so a generic OWL2 processor cannot compute ordering relationships of values of this type."""@en .


#################################################################
#    Object Properties
#################################################################

###  http://bigg-project.eu/ontology#manages
bigg:manages rdf:type owl:ObjectProperty ;
             rdfs:comment "manages"@en ;
             rdfs:label "manages"@en .


###  http://purl.obolibrary.org/obo/TAXRANK_1000000
<http://purl.obolibrary.org/obo/TAXRANK_1000000> rdf:type owl:ObjectProperty ;
                                                 rdfs:label "has taxon rank"@en .


###  http://schema.org/affiliation
<http://schema.org/affiliation> rdf:type owl:ObjectProperty .


###  http://www.opengis.net/ont/geosparql#defaultGeometry
geosp:defaultGeometry rdf:type owl:ObjectProperty ;
                      owl:equivalentProperty geosp:hasDefaultGeometry ;
                      rdfs:subPropertyOf geosp:hasGeometry ;
                      rdfs:domain geosp:Feature ;
                      rdfs:range geosp:Geometry ;
                      rdfs:isDefinedBy geosp: ,
                                       <http://www.opengis.net/spec/geosparql/1.1/req/geometry-extension/feature-properties> ;
                      skos:definition "The default Geometry to be used in spatial calculations. It is usually the most detailed Geometry."@en ;
                      skos:example <http://www.opengis.net/spec/geosparql/1.1/specification.html#B.1.2.2> ,
                                   <http://www.opengis.net/spec/geosparql/1.1/specification.html#B.2.1> ;
                      skos:note "Duplicate properties defaultGeometry and hasDefaultGeometry exist because of an inconsistency between ontology and documentation in GeoSPARQL 1.0. Only hasDefaultGeometry is described in the documention." ;
                      skos:prefLabel "default geometry"@en .


###  http://www.opengis.net/ont/geosparql#ehContains
geosp:ehContains rdf:type owl:ObjectProperty ;
                 rdfs:domain geosp:SpatialObject ;
                 rdfs:range geosp:SpatialObject ;
                 rdfs:isDefinedBy geosp: ,
                                  <http://www.opengis.net/spec/geosparql/1.0/req/geometry-extension/eh-spatial-relations> ,
                                  <http://www.opengis.net/spec/geosparql/1.1/req/geometry-extension/eh-spatial-relations> ;
                 rdfs:seeAlso <http://dbpedia.org/resource/DE-9IM> ;
                 skos:definition "States that the subject SpatialObject spatially contains the object SpatialObject. DE-9IM: T*TFF*FF*"@en ;
                 skos:prefLabel "contains"@en .


###  http://www.opengis.net/ont/geosparql#ehCoveredBy
geosp:ehCoveredBy rdf:type owl:ObjectProperty ;
                  rdfs:domain geosp:SpatialObject ;
                  rdfs:range geosp:SpatialObject ;
                  rdfs:isDefinedBy geosp: ,
                                   <http://www.opengis.net/spec/geosparql/1.0/req/geometry-extension/eh-spatial-relations> ,
                                   <http://www.opengis.net/spec/geosparql/1.1/req/geometry-extension/eh-spatial-relations> ;
                  rdfs:seeAlso <http://dbpedia.org/resource/DE-9IM> ;
                  skos:definition "States that the subject SpatialObject is spatially covered by the object SpatialObject. DE-9IM: TFF*TFT**"@en ;
                  skos:prefLabel "covered by"@en .


###  http://www.opengis.net/ont/geosparql#ehCovers
geosp:ehCovers rdf:type owl:ObjectProperty ;
               rdfs:domain geosp:SpatialObject ;
               rdfs:range geosp:SpatialObject ;
               rdfs:isDefinedBy geosp: ,
                                <http://www.opengis.net/spec/geosparql/1.0/req/geometry-extension/eh-spatial-relations> ,
                                <http://www.opengis.net/spec/geosparql/1.1/req/geometry-extension/eh-spatial-relations> ;
               rdfs:seeAlso <http://dbpedia.org/resource/DE-9IM> ;
               skos:definition "States that the subject SpatialObject spatially covers the object SpatialObject. DE-9IM: T*TFT*FF*"@en ;
               skos:prefLabel "covers"@en .


###  http://www.opengis.net/ont/geosparql#ehDisjoint
geosp:ehDisjoint rdf:type owl:ObjectProperty ;
                 owl:equivalentProperty geosp:sfDisjoint ;
                 rdfs:domain geosp:SpatialObject ;
                 rdfs:range geosp:SpatialObject ;
                 rdfs:isDefinedBy geosp: ,
                                  <http://www.opengis.net/spec/geosparql/1.0/req/geometry-extension/eh-spatial-relations> ,
                                  <http://www.opengis.net/spec/geosparql/1.1/req/geometry-extension/eh-spatial-relations> ;
                 rdfs:seeAlso <http://dbpedia.org/resource/DE-9IM> ;
                 skos:definition "States that the subject SpatialObject is spatially disjoint from the object SpatialObject. DE-9IM: FF*FF****"@en ;
                 skos:prefLabel "disjoint"@en .


###  http://www.opengis.net/ont/geosparql#ehEquals
geosp:ehEquals rdf:type owl:ObjectProperty ;
               owl:equivalentProperty geosp:sfEquals ;
               rdfs:domain geosp:SpatialObject ;
               rdfs:range geosp:SpatialObject ;
               rdfs:isDefinedBy geosp: ,
                                <http://www.opengis.net/spec/geosparql/1.0/req/geometry-extension/eh-spatial-relations> ,
                                <http://www.opengis.net/spec/geosparql/1.1/req/geometry-extension/eh-spatial-relations> ;
               rdfs:seeAlso <http://dbpedia.org/resource/DE-9IM> ;
               skos:definition "States that the subject SpatialObject spatially equals the object SpatialObject. DE-9IM: TFFFTFFFT"@en ;
               skos:prefLabel "equals"@en .


###  http://www.opengis.net/ont/geosparql#ehInside
geosp:ehInside rdf:type owl:ObjectProperty ;
               rdfs:domain geosp:SpatialObject ;
               rdfs:range geosp:SpatialObject ;
               rdfs:isDefinedBy geosp: ,
                                <http://www.opengis.net/spec/geosparql/1.0/req/geometry-extension/eh-spatial-relations> ,
                                <http://www.opengis.net/spec/geosparql/1.1/req/geometry-extension/eh-spatial-relations> ;
               rdfs:seeAlso <http://dbpedia.org/resource/DE-9IM> ;
               skos:definition "States that the subject SpatialObject is spatially inside the object SpatialObject. DE-9IM: TFF*FFT**"@en ;
               skos:prefLabel "inside"@en .


###  http://www.opengis.net/ont/geosparql#ehMeet
geosp:ehMeet rdf:type owl:ObjectProperty ;
             owl:equivalentProperty geosp:sfTouches ;
             rdfs:domain geosp:SpatialObject ;
             rdfs:range geosp:SpatialObject ;
             rdfs:isDefinedBy geosp: ,
                              <http://www.opengis.net/spec/geosparql/1.0/req/geometry-extension/eh-spatial-relations> ,
                              <http://www.opengis.net/spec/geosparql/1.1/req/geometry-extension/eh-spatial-relations> ;
             rdfs:seeAlso <http://dbpedia.org/resource/DE-9IM> ;
             skos:definition "States that the subject SpatialObject spatially meets the object SpatialObject. DE-9IM: FT******* ^ F**T***** ^ F***T****"@en ;
             skos:prefLabel "meet"@en .


###  http://www.opengis.net/ont/geosparql#ehOverlap
geosp:ehOverlap rdf:type owl:ObjectProperty ;
                rdfs:domain geosp:SpatialObject ;
                rdfs:range geosp:SpatialObject ;
                rdfs:isDefinedBy geosp: ,
                                 <http://www.opengis.net/spec/geosparql/1.0/req/geometry-extension/eh-spatial-relations> ,
                                 <http://www.opengis.net/spec/geosparql/1.1/req/geometry-extension/eh-spatial-relations> ;
                rdfs:seeAlso <http://dbpedia.org/resource/DE-9IM> ;
                skos:definition "States that the subject SpatialObject spatially overlaps the object SpatialObject. DE-9IM: T*T***T**"@en ;
                skos:prefLabel "overlap"@en .


###  http://www.opengis.net/ont/geosparql#hasArea
geosp:hasArea rdf:type owl:ObjectProperty ;
              rdfs:subPropertyOf geosp:hasSize ;
              rdfs:domain geosp:SpatialObject ;
              rdfs:isDefinedBy geosp: ,
                               <http://www.opengis.net/spec/geosparql/1.1/req/geometry-extension/spatial-object-properties> ;
              skos:definition "The area of a Spatial Object."@en ;
              skos:example <http://www.opengis.net/spec/geosparql/1.1/specification.html#B.1.1.2.4> ,
                           <http://www.opengis.net/spec/geosparql/1.1/specification.html#B.1.2.2> ;
              skos:prefLabel "has area"@en .


###  http://www.opengis.net/ont/geosparql#hasBoundingBox
geosp:hasBoundingBox rdf:type owl:ObjectProperty ;
                     rdfs:subPropertyOf geosp:hasGeometry ;
                     rdfs:domain geosp:Feature ;
                     rdfs:range geosp:Geometry ;
                     rdfs:isDefinedBy geosp: ,
                                      <http://www.opengis.net/spec/geosparql/1.1/req/geometry-extension/feature-properties> ;
                     skos:definition "The minimum or smallest bounding or enclosing box of a given Feature."@en ;
                     skos:example <http://www.opengis.net/spec/geosparql/1.1/specification.html#B.1.2.2> ;
                     skos:prefLabel "has bounding box"@en ;
                     skos:scopeNote "The target is a Geometry that defines a rectilinear region whose edges are aligned with the axes of the coordinate reference system, which exactly contains the Feature, for example an instance of http://www.opengis.net/ont/sf#envelope."@en .


###  http://www.opengis.net/ont/geosparql#hasCentroid
geosp:hasCentroid rdf:type owl:ObjectProperty ;
                  rdfs:subPropertyOf geosp:hasGeometry ;
                  rdfs:domain geosp:Feature ;
                  rdfs:range geosp:Geometry ;
                  rdfs:isDefinedBy geosp: ,
                                   <http://www.opengis.net/spec/geosparql/1.1/req/geometry-extension/feature-properties> ;
                  skos:definition "The arithmetic mean position of all the Geometry points of a given Feature."@en ;
                  skos:example <http://www.opengis.net/spec/geosparql/1.1/specification.html#B.1.2.2> ;
                  skos:prefLabel "has centroid"@en ;
                  skos:scopeNote "The target Geometry shall describe a point, for example an instance of http://www.opengis.net/ont/sf#Point."@en .


###  http://www.opengis.net/ont/geosparql#hasDefaultGeometry
geosp:hasDefaultGeometry rdf:type owl:ObjectProperty ;
                         rdfs:subPropertyOf geosp:hasGeometry ;
                         rdfs:domain geosp:Feature ;
                         rdfs:range geosp:Geometry ;
                         rdfs:isDefinedBy geosp: ,
                                          <http://www.opengis.net/spec/geosparql/1.0/req/geometry-extension/feature-properties> ,
                                          <http://www.opengis.net/spec/geosparql/1.1/req/geometry-extension/feature-properties> ;
                         skos:definition "The default Geometry to be used in spatial calculations. It is usually the most detailed Geometry."@en ;
                         skos:note "Duplicate properties defaultGeometry and hasDefaultGeometry exist because of an inconsistency between ontology and documentation in GeoSPARQL 1.0. Only hasDefaultGeometry is described in the documention." ;
                         skos:prefLabel "has default geometry"@en .


###  http://www.opengis.net/ont/geosparql#hasGeometry
geosp:hasGeometry rdf:type owl:ObjectProperty ;
                  rdfs:domain geosp:Feature ;
                  rdfs:range geosp:Geometry ;
                  rdfs:comment "A spatial representation for a given feature."@en ;
                  rdfs:isDefinedBy geosp: ,
                                   <http://www.opengis.net/spec/geosparql/1.0/req/geometry-extension/feature-properties> ,
                                   <http://www.opengis.net/spec/geosparql/1.1/req/geometry-extension/feature-properties> ;
                  rdfs:label "has geometry"@en ,
                             "hasGeometry"@en ;
                  skos:definition "A spatial representation for a given Feature."@en ;
                  skos:example <http://www.opengis.net/spec/geosparql/1.1/specification.html#B.1.1.2.2> ,
                               <http://www.opengis.net/spec/geosparql/1.1/specification.html#B.1.1.2.3> ,
                               <http://www.opengis.net/spec/geosparql/1.1/specification.html#B.1.1.2.4> ,
                               <http://www.opengis.net/spec/geosparql/1.1/specification.html#B.1.1.2.5> ,
                               <http://www.opengis.net/spec/geosparql/1.1/specification.html#B.1.1.2.6> ,
                               <http://www.opengis.net/spec/geosparql/1.1/specification.html#B.1.1.2.8> ,
                               <http://www.opengis.net/spec/geosparql/1.1/specification.html#B.1.1.3.2> ,
                               <http://www.opengis.net/spec/geosparql/1.1/specification.html#B.1.1.3.3> ,
                               <http://www.opengis.net/spec/geosparql/1.1/specification.html#B.1.2.2> ,
                               <http://www.opengis.net/spec/geosparql/1.1/specification.html#B.1.2.3> ,
                               <http://www.opengis.net/spec/geosparql/1.1/specification.html#B.1.2.4> ,
                               <http://www.opengis.net/spec/geosparql/1.1/specification.html#B.2> ;
                  skos:prefLabel "has geometry"@en .


###  http://www.opengis.net/ont/geosparql#hasLength
geosp:hasLength rdf:type owl:ObjectProperty ;
                rdfs:subPropertyOf geosp:hasSize ;
                rdfs:domain geosp:SpatialObject ;
                rdfs:isDefinedBy geosp: ,
                                 <http://www.opengis.net/spec/geosparql/1.1/req/geometry-extension/spatial-object-properties> ;
                skos:definition "The length of a Spatial Object."@en ;
                skos:example <http://www.opengis.net/spec/geosparql/1.1/specification.html#B.1.1.2.7> ,
                             <http://www.opengis.net/spec/geosparql/1.1/specification.html#B.1.2.2> ;
                skos:prefLabel "has length"@en .


###  http://www.opengis.net/ont/geosparql#hasPerimeterLength
geosp:hasPerimeterLength rdf:type owl:ObjectProperty ;
                         rdfs:subPropertyOf geosp:hasSize ;
                         rdfs:domain geosp:SpatialObject ;
                         rdfs:isDefinedBy geosp: ,
                                          <http://www.opengis.net/spec/geosparql/1.1/req/geometry-extension/spatial-object-properties> ;
                         skos:definition "The length of the perimeter of a Spatial Object."@en ;
                         skos:example <http://www.opengis.net/spec/geosparql/1.1/specification.html#B.1.1.1.2> ;
                         skos:prefLabel "has perimeter length"@en .


###  http://www.opengis.net/ont/geosparql#hasSize
geosp:hasSize rdf:type owl:ObjectProperty ;
              rdfs:domain geosp:SpatialObject ;
              rdfs:isDefinedBy geosp: ,
                               <http://www.opengis.net/spec/geosparql/1.0/req/topology-vocab-extension/spatial-object-properties> ,
                               <http://www.opengis.net/spec/geosparql/1.1/req/topology-vocab-extension/spatial-object-properties> ;
              skos:definition "Subproperties of this property are used to indicate the size of a Spatial Object as a measurement or estimate of one or more dimensions of the Spatial Object's spatial presence."@en ;
              skos:note "The recommended way to specify size is by using a subproperty of hasMetricSize. Subproperties of hasSize can be used if more complex expressions are necessary, for example if the unit of length can not be converted to meter, or if additional data are needed to describe the measurement or estimate."@en ;
              skos:prefLabel "has size"@en .


###  http://www.opengis.net/ont/geosparql#hasSpatialAccuracy
geosp:hasSpatialAccuracy rdf:type owl:ObjectProperty ;
                         rdfs:domain geosp:Geometry ;
                         rdfs:isDefinedBy geosp: ,
                                          <http://www.opengis.net/spec/geosparql/1.1/req/geometry-extension/geometry-properties> ;
                         skos:definition "The positional accuracy of the coordinates of a Geometry."@en ;
                         skos:example <http://www.opengis.net/spec/geosparql/1.1/specification.html#B.1.2.3> ;
                         skos:note "Spatial accuracy is applicable when a Geometry is used to represent a Feature. It is expressed as a distance that indicates the truthfullness of the positions (coordinates) that define the Geometry. In this case accuracy defines a zone surrounding each coordinate within wich the real positions are known to be. The accuracy value defines this zone as a distance from the coordinate(s) in all directions (e.g. a line, a circle or a sphere, depending on spatial dimension)."@en ;
                         skos:prefLabel "has spatial accuracy"@en .


###  http://www.opengis.net/ont/geosparql#hasSpatialResolution
geosp:hasSpatialResolution rdf:type owl:ObjectProperty ;
                           rdfs:domain geosp:Geometry ;
                           rdfs:isDefinedBy geosp: ,
                                            <http://www.opengis.net/spec/geosparql/1.1/req/geometry-extension/feature-properties> ;
                           skos:definition "The spatial resolution of a Geometry."@en ;
                           skos:example <http://www.opengis.net/spec/geosparql/1.1/specification.html#B.1.2.2> ;
                           skos:note "Spatial resolution specifies the level of detail of a Geometry. It the smallest distinguishable distance between spatially adjacent coordinates."@en ;
                           skos:prefLabel "has spatial resolution"@en .


###  http://www.opengis.net/ont/geosparql#hasVolume
geosp:hasVolume rdf:type owl:ObjectProperty ;
                rdfs:subPropertyOf geosp:hasSize ;
                rdfs:domain geosp:SpatialObject ;
                rdfs:isDefinedBy geosp: ,
                                 <http://www.opengis.net/spec/geosparql/1.1/req/geometry-extension/spatial-object-properties> ;
                skos:definition "The volume of a three-dimensional Spatial Object."@en ;
                skos:example <http://www.opengis.net/spec/geosparql/1.1/specification.html#B.1.2.2> ;
                skos:prefLabel "has volume"@en .


###  http://www.opengis.net/ont/geosparql#rcc8dc
geosp:rcc8dc rdf:type owl:ObjectProperty ;
             rdfs:domain geosp:SpatialObject ;
             rdfs:range geosp:SpatialObject ;
             rdfs:isDefinedBy geosp: ,
                              <http://www.opengis.net/spec/geosparql/1.0/req/topology-vocab-extension/rcc8-spatial-relations> ,
                              <http://www.opengis.net/spec/geosparql/1.1/req/topology-vocab-extension/rcc8-spatial-relations> ;
             rdfs:seeAlso <http://dbpedia.org/resource/DE-9IM> ;
             skos:definition "States that the subject SpatialObject is spatially disjoint from the object SpatialObject. DE-9IM: FFTFFTTTT"@en ;
             skos:prefLabel "disconnected"@en .


###  http://www.opengis.net/ont/geosparql#rcc8ec
geosp:rcc8ec rdf:type owl:ObjectProperty ;
             rdfs:domain geosp:SpatialObject ;
             rdfs:range geosp:SpatialObject ;
             rdfs:isDefinedBy geosp: ,
                              <http://www.opengis.net/spec/geosparql/1.0/req/topology-vocab-extension/rcc8-spatial-relations> ,
                              <http://www.opengis.net/spec/geosparql/1.1/req/topology-vocab-extension/rcc8-spatial-relations> ;
             rdfs:seeAlso <http://dbpedia.org/resource/DE-9IM> ;
             skos:definition "States that the subject SpatialObject spatially meets the object SpatialObject. DE-9IM: FFTFTTTTT"@en ;
             skos:prefLabel "externally connected"@en .


###  http://www.opengis.net/ont/geosparql#rcc8eq
geosp:rcc8eq rdf:type owl:ObjectProperty ;
             rdfs:domain geosp:SpatialObject ;
             rdfs:range geosp:SpatialObject ;
             rdfs:isDefinedBy geosp: ,
                              <http://www.opengis.net/spec/geosparql/1.0/req/topology-vocab-extension/rcc8-spatial-relations> ,
                              <http://www.opengis.net/spec/geosparql/1.1/req/topology-vocab-extension/rcc8-spatial-relations> ;
             rdfs:seeAlso <http://dbpedia.org/resource/DE-9IM> ;
             skos:definition "States that the subject SpatialObject spatially equals the object SpatialObject. DE-9IM: TFFFTFFFT"@en ;
             skos:prefLabel "equals"@en .


###  http://www.opengis.net/ont/geosparql#rcc8ntpp
geosp:rcc8ntpp rdf:type owl:ObjectProperty ;
               rdfs:domain geosp:SpatialObject ;
               rdfs:range geosp:SpatialObject ;
               rdfs:isDefinedBy geosp: ,
                                <http://www.opengis.net/spec/geosparql/1.0/req/topology-vocab-extension/rcc8-spatial-relations> ,
                                <http://www.opengis.net/spec/geosparql/1.1/req/topology-vocab-extension/rcc8-spatial-relations> ;
               rdfs:seeAlso <http://dbpedia.org/resource/DE-9IM> ;
               skos:definition "States that the subject SpatialObject is spatially inside the object SpatialObject. DE-9IM: TFFTFFTTT"@en ;
               skos:prefLabel "non-tangential proper part"@en .


###  http://www.opengis.net/ont/geosparql#rcc8ntppi
geosp:rcc8ntppi rdf:type owl:ObjectProperty ;
                rdfs:domain geosp:SpatialObject ;
                rdfs:range geosp:SpatialObject ;
                rdfs:isDefinedBy geosp: ,
                                 <http://www.opengis.net/spec/geosparql/1.0/req/topology-vocab-extension/rcc8-spatial-relations> ,
                                 <http://www.opengis.net/spec/geosparql/1.1/req/topology-vocab-extension/rcc8-spatial-relations> ;
                rdfs:seeAlso <http://dbpedia.org/resource/DE-9IM> ;
                skos:definition "States that the subject SpatialObject spatially contains the object SpatialObject. DE-9IM: TTTFFTFFT"@en ;
                skos:prefLabel "non-tangential proper part inverse"@en .


###  http://www.opengis.net/ont/geosparql#rcc8po
geosp:rcc8po rdf:type owl:ObjectProperty ;
             rdfs:domain geosp:SpatialObject ;
             rdfs:range geosp:SpatialObject ;
             rdfs:isDefinedBy geosp: ,
                              <http://www.opengis.net/spec/geosparql/1.0/req/topology-vocab-extension/rcc8-spatial-relations> ,
                              <http://www.opengis.net/spec/geosparql/1.1/req/topology-vocab-extension/rcc8-spatial-relations> ;
             rdfs:seeAlso <http://dbpedia.org/resource/DE-9IM> ;
             skos:definition "States that the subject SpatialObject spatially overlaps the object SpatialObject. DE-9IM: TTTTTTTTT"@en ;
             skos:prefLabel "partially overlapping"@en .


###  http://www.opengis.net/ont/geosparql#rcc8tpp
geosp:rcc8tpp rdf:type owl:ObjectProperty ;
              rdfs:domain geosp:SpatialObject ;
              rdfs:range geosp:SpatialObject ;
              rdfs:isDefinedBy geosp: ,
                               <http://www.opengis.net/spec/geosparql/1.0/req/topology-vocab-extension/rcc8-spatial-relations> ,
                               <http://www.opengis.net/spec/geosparql/1.1/req/topology-vocab-extension/rcc8-spatial-relations> ;
              rdfs:seeAlso <http://dbpedia.org/resource/DE-9IM> ;
              skos:definition "States that the subject SpatialObject is spatially covered by the object SpatialObject. DE-9IM: TFFTTFTTT"@en ;
              skos:prefLabel "tangential proper part"@en .


###  http://www.opengis.net/ont/geosparql#rcc8tppi
geosp:rcc8tppi rdf:type owl:ObjectProperty ;
               rdfs:domain geosp:SpatialObject ;
               rdfs:range geosp:SpatialObject ;
               rdfs:isDefinedBy geosp: ,
                                <http://www.opengis.net/spec/geosparql/1.0/req/topology-vocab-extension/rcc8-spatial-relations> ,
                                <http://www.opengis.net/spec/geosparql/1.1/req/topology-vocab-extension/rcc8-spatial-relations> ;
               rdfs:seeAlso <http://dbpedia.org/resource/DE-9IM> ;
               skos:definition "States that the subject SpatialObject spatially covers the object SpatialObject. DE-9IM: TTTFTTFFT"@en ;
               skos:prefLabel "tangential proper part inverse"@en .


###  http://www.opengis.net/ont/geosparql#sfContains
geosp:sfContains rdf:type owl:ObjectProperty ;
                 rdfs:domain geosp:SpatialObject ;
                 rdfs:range geosp:SpatialObject ;
                 rdfs:comment "Exists if the subject SpatialObject spatially contains the object SpatialObject. DE-9IM: T*****FF*"@en ;
                 rdfs:isDefinedBy <http://www.opengis.net/ont/geosparql> ,
                                  geosp: ,
                                  <http://www.opengis.net/spec/geosparql/1.0> ,
                                  <http://www.opengis.net/spec/geosparql/1.0/req/topology-vocab-extension/rcc8-spatial-relations> ,
                                  <http://www.opengis.net/spec/geosparql/1.1/req/topology-vocab-extension/rcc8-spatial-relations> ;
                 rdfs:label "contains"@en ,
                            "sfContains"@en ;
                 rdfs:seeAlso <http://dbpedia.org/resource/DE-9IM> ;
                 skos:definition "States that the subject SpatialObject spatially contains the object SpatialObject. DE-9IM: T*****FF*"@en ;
                 skos:prefLabel "contains"@en .


###  http://www.opengis.net/ont/geosparql#sfCrosses
geosp:sfCrosses rdf:type owl:ObjectProperty ;
                rdfs:domain geosp:SpatialObject ;
                rdfs:range geosp:SpatialObject ;
                rdfs:isDefinedBy geosp: ,
                                 <http://www.opengis.net/spec/geosparql/1.0/req/topology-vocab-extension/sf-spatial-relations> ,
                                 <http://www.opengis.net/spec/geosparql/1.1/req/topology-vocab-extension/sf-spatial-relations> ;
                rdfs:seeAlso <http://dbpedia.org/resource/DE-9IM> ;
                skos:definition "States that the subject SpatialObject spatially crosses the object SpatialObject. DE-9IM: T*T******"@en ;
                skos:prefLabel "crosses"@en .


###  http://www.opengis.net/ont/geosparql#sfDisjoint
geosp:sfDisjoint rdf:type owl:ObjectProperty ;
                 rdfs:domain geosp:SpatialObject ;
                 rdfs:range geosp:SpatialObject ;
                 rdfs:isDefinedBy geosp: ,
                                  <http://www.opengis.net/spec/geosparql/1.0/req/topology-vocab-extension/sf-spatial-relations> ,
                                  <http://www.opengis.net/spec/geosparql/1.1/req/topology-vocab-extension/sf-spatial-relations> ;
                 rdfs:seeAlso <http://dbpedia.org/resource/DE-9IM> ;
                 skos:definition "States that the subject SpatialObject is spatially disjoint from the object SpatialObject. DE-9IM: FF*FF****"@en ;
                 skos:prefLabel "disjoint"@en .


###  http://www.opengis.net/ont/geosparql#sfEquals
geosp:sfEquals rdf:type owl:ObjectProperty ;
               rdfs:domain geosp:SpatialObject ;
               rdfs:range geosp:SpatialObject ;
               rdfs:isDefinedBy geosp: ,
                                <http://www.opengis.net/spec/geosparql/1.0/req/topology-vocab-extension/sf-spatial-relations> ,
                                <http://www.opengis.net/spec/geosparql/1.1/req/topology-vocab-extension/sf-spatial-relations> ;
               rdfs:seeAlso <http://dbpedia.org/resource/DE-9IM> ;
               skos:definition "States that the subject SpatialObject spatially equals the object SpatialObject. DE-9IM: TFFFTFFFT"@en ;
               skos:prefLabel "equals"@en .


###  http://www.opengis.net/ont/geosparql#sfIntersects
geosp:sfIntersects rdf:type owl:ObjectProperty ;
                   rdfs:domain geosp:SpatialObject ;
                   rdfs:range geosp:SpatialObject ;
                   rdfs:isDefinedBy geosp: ,
                                    <http://www.opengis.net/spec/geosparql/1.0/req/topology-vocab-extension/sf-spatial-relations> ,
                                    <http://www.opengis.net/spec/geosparql/1.1/req/topology-vocab-extension/sf-spatial-relations> ;
                   rdfs:seeAlso <http://dbpedia.org/resource/DE-9IM> ;
                   skos:definition "States that the subject SpatialObject is not spatially disjoint from the object SpatialObject. DE-9IM: T******** ^ *T******* ^ ***T***** ^ ****T****"@en ;
                   skos:prefLabel "intersects"@en .


###  http://www.opengis.net/ont/geosparql#sfOverlaps
geosp:sfOverlaps rdf:type owl:ObjectProperty ;
                 rdfs:domain geosp:SpatialObject ;
                 rdfs:range geosp:SpatialObject ;
                 rdfs:isDefinedBy geosp: ,
                                  <http://www.opengis.net/spec/geosparql/1.0/req/topology-vocab-extension/sf-spatial-relations> ,
                                  <http://www.opengis.net/spec/geosparql/1.1/req/topology-vocab-extension/sf-spatial-relations> ;
                 rdfs:seeAlso <http://dbpedia.org/resource/DE-9IM> ;
                 skos:definition "States that the subject SpatialObject spatially overlaps the object SpatialObject. DE-9IM: T*T***T**"@en ;
                 skos:prefLabel "overlaps"@en .


###  http://www.opengis.net/ont/geosparql#sfTouches
geosp:sfTouches rdf:type owl:ObjectProperty ;
                rdfs:domain geosp:SpatialObject ;
                rdfs:range geosp:SpatialObject ;
                rdfs:isDefinedBy geosp: ,
                                 <http://www.opengis.net/spec/geosparql/1.0/req/topology-vocab-extension/sf-spatial-relations> ,
                                 <http://www.opengis.net/spec/geosparql/1.1/req/topology-vocab-extension/sf-spatial-relations> ;
                rdfs:seeAlso <http://dbpedia.org/resource/DE-9IM> ;
                skos:definition "States that the subject SpatialObject spatially touches the object SpatialObject. DE-9IM: FT******* ^ F**T***** ^ F***T****"@en ;
                skos:prefLabel "touches"@en .


###  http://www.opengis.net/ont/geosparql#sfWithin
geosp:sfWithin rdf:type owl:ObjectProperty ;
               rdfs:domain geosp:SpatialObject ;
               rdfs:range geosp:SpatialObject ;
               rdfs:comment "Exists if the subject SpatialObject is spatially within the object SpatialObject. DE-9IM: T*F**F***"@en ;
               rdfs:isDefinedBy <http://www.opengis.net/ont/geosparql> ,
                                geosp: ,
                                <http://www.opengis.net/spec/geosparql/1.0> ,
                                <http://www.opengis.net/spec/geosparql/1.0/req/topology-vocab-extension/sf-spatial-relations> ,
                                <http://www.opengis.net/spec/geosparql/1.1/req/topology-vocab-extension/sf-spatial-relations> ;
               rdfs:label "sfWithin"@en ,
                          "within"@en ;
               rdfs:seeAlso <http://dbpedia.org/resource/DE-9IM> ;
               skos:definition "States that the subject SpatialObject is spatially within the object SpatialObject. DE-9IM: T*F**F***"@en ;
               skos:prefLabel "within"@en .


###  http://www.w3.org/2000/01/rdf-schema#member
rdfs:member rdf:type owl:ObjectProperty .


###  http://www.w3.org/2003/01/geo/wgs84_pos#location
wgs84:location rdf:type owl:ObjectProperty ;
               rdfs:subPropertyOf foaf:based_near .


###  http://www.w3.org/2003/01/geo/wgs84_pos#long
wgs84:long rdf:type owl:ObjectProperty ;
           rdfs:domain wgs84:SpatialThing .


###  http://www.w3.org/2006/time#after
time:after rdf:type owl:ObjectProperty ;
           owl:inverseOf time:before ;
           rdfs:domain time:TemporalEntity ;
           rdfs:range time:TemporalEntity ;
           rdfs:comment "Asume una dirección en el tiempo. Si una entidad temporal T1 está después de otra entidad temporal T2, entonces el principio de T1 está después del final de T2."@es ,
                        "Gives directionality to time. If a temporal entity T1 is after another temporal entity T2, then the beginning of T1 is after the end of T2."@en ;
           rdfs:label "after"@en ,
                      "después"@es ;
           skos:definition "Asume una dirección en el tiempo. Si una entidad temporal T1 está después de otra entidad temporal T2, entonces el principio de T1 está después del final de T2."@es ,
                           "Gives directionality to time. If a temporal entity T1 is after another temporal entity T2, then the beginning of T1 is after the end of T2."@en .


###  http://www.w3.org/2006/time#before
time:before rdf:type owl:ObjectProperty ,
                     owl:TransitiveProperty ;
            rdfs:domain time:TemporalEntity ;
            rdfs:range time:TemporalEntity ;
            rdfs:comment "Asume una dirección en el tiempo. Si una entidad temporal T1 está antes que otra entidad temporal T2, entonces el final de T1 está antes que el principio de T2. Así, \"antes\" se puede considerar básica para instantes y derivada para intervalos."@es ,
                         "Gives directionality to time. If a temporal entity T1 is before another temporal entity T2, then the end of T1 is before the beginning of T2. Thus, \"before\" can be considered to be basic to instants and derived for intervals."@en ;
            rdfs:label "antes"@es ,
                       "before"@en ;
            skos:definition "Asume una dirección en el tiempo. Si una entidad temporal T1 está antes que otra entidad temporal T2, entonces el final de T1 está antes que el principio de T2. Así, \"antes\" se puede considerar básica para instantes y derivada para intervalos."@es ,
                            "Gives directionality to time. If a temporal entity T1 is before another temporal entity T2, then the end of T1 is before the beginning of T2. Thus, \"before\" can be considered to be basic to instants and derived for intervals."@en .


###  http://www.w3.org/2006/time#dayOfWeek
time:dayOfWeek rdf:type owl:ObjectProperty ;
               rdfs:domain time:GeneralDateTimeDescription ;
               rdfs:range time:DayOfWeek ;
               rdfs:comment "El día de la semana, cuyo valor es un miembro de la clase 'día de la semana'." ,
                            "The day of week, whose value is a member of the class time:DayOfWeek"@en ;
               rdfs:label "day of week"@en ,
                          "día de la semana"@es ;
               skos:definition "El día de la semana, cuyo valor es un miembro de la clase 'día de la semana'."@es ,
                               "The day of week, whose value is a member of the class time:DayOfWeek"@en .


###  http://www.w3.org/2006/time#hasBeginning
time:hasBeginning rdf:type owl:ObjectProperty ;
                  rdfs:subPropertyOf time:hasTime ;
                  rdfs:domain time:TemporalEntity ;
                  rdfs:range time:Instant ;
                  rdfs:comment "Beginning of a temporal entity"@en ,
                               "Comienzo de una entidad temporal."@es ;
                  rdfs:label "has beginning"@en ,
                             "tiene principio"@es ;
                  skos:definition "Beginning of a temporal entity."@en ,
                                  "Comienzo de una entidad temporal."@es .


###  http://www.w3.org/2006/time#hasDateTimeDescription
time:hasDateTimeDescription rdf:type owl:ObjectProperty ;
                            rdfs:domain time:DateTimeInterval ;
                            rdfs:range time:GeneralDateTimeDescription ;
                            rdfs:comment "Valor de intervalo de fecha-hora expresado como un valor estructurado. El principio y el final del intervalo coincide con los límites del elemento más corto en la descripción."@es ,
                                         "Value of DateTimeInterval expressed as a structured value. The beginning and end of the interval coincide with the limits of the shortest element in the description."@en ;
                            rdfs:label "has Date-Time description"@en ,
                                       "tiene descripción fecha-hora"@es ;
                            skos:definition "Valor de intervalo de fecha-hora expresado como un valor estructurado. El principio y el final del intervalo coincide con los límites del elemento más corto en la descripción."@es ,
                                            "Value of DateTimeInterval expressed as a structured value. The beginning and end of the interval coincide with the limits of the shortest element in the description."@en .


###  http://www.w3.org/2006/time#hasDuration
time:hasDuration rdf:type owl:ObjectProperty ;
                 rdfs:subPropertyOf time:hasTemporalDuration ;
                 rdfs:range time:Duration ;
                 rdfs:comment "Duración de una entidad temporal, expresada como un valor escalado o un valor nominal."@es ,
                              "Duration of a temporal entity, expressed as a scaled value or nominal value"@en ;
                 rdfs:label "has duration"@en ,
                            "tiene duración"@es ;
                 skos:definition "Duración de una entidad temporal, evento o actividad, o cosa, expresada como un valor escalado."@es ,
                                 "Duration of a temporal entity, event or activity, or thing, expressed as a scaled value"@en .


###  http://www.w3.org/2006/time#hasDurationDescription
time:hasDurationDescription rdf:type owl:ObjectProperty ;
                            rdfs:subPropertyOf time:hasTemporalDuration ;
                            rdfs:range time:GeneralDurationDescription ;
                            rdfs:comment "Duración de una entidad temporal, expresada utilizando una descripción estructurada."@es ,
                                         "Duration of a temporal entity, expressed using a structured description"@en ;
                            rdfs:label "has duration description"@en ,
                                       "tiene descripción de duración"@es ;
                            skos:definition "Duración de una entidad temporal, expresada utilizando una descripción estructurada."@es ,
                                            "Duration of a temporal entity, expressed using a structured description"@en .


###  http://www.w3.org/2006/time#hasEnd
time:hasEnd rdf:type owl:ObjectProperty ;
            rdfs:subPropertyOf time:hasTime ;
            rdfs:domain time:TemporalEntity ;
            rdfs:range time:Instant ;
            rdfs:comment "End of a temporal entity."@en ,
                         "Final de una entidad temporal."@es ;
            rdfs:label "has end"@en ,
                       "tiene fin"@es ;
            skos:definition "End of a temporal entity."@en ,
                            "Final de una entidad temporal."@es .


###  http://www.w3.org/2006/time#hasTRS
time:hasTRS rdf:type owl:ObjectProperty ,
                     owl:FunctionalProperty ;
            rdfs:domain [ rdf:type owl:Class ;
                          owl:unionOf ( time:GeneralDurationDescription
                                        time:TemporalPosition
                                      )
                        ] ;
            rdfs:range time:TRS ;
            rdfs:comment "El sistema de referencia temporal utilizado por una posición temporal o descripción de extensión."@es ,
                         "The temporal reference system used by a temporal position or extent description. "@en ;
            rdfs:label "Temporal reference system used"@en ,
                       "sistema de referencia temporal utilizado"@es ;
            skos:definition "El sistema de referencia temporal utilizado por una posición temporal o descripción de extensión."@es ,
                            "The temporal reference system used by a temporal position or extent description. "@en .


###  http://www.w3.org/2006/time#hasTemporalDuration
time:hasTemporalDuration rdf:type owl:ObjectProperty ;
                         rdfs:domain time:TemporalEntity ;
                         rdfs:range time:TemporalDuration ;
                         rdfs:comment "Duración de una entidad temporal."@es ,
                                      "Duration of a temporal entity."@en ;
                         rdfs:label "has temporal duration"@en ,
                                    "tiene duración temporal"@es ;
                         skos:definition "Duración de una entidad temporal."@es ,
                                         "Duration of a temporal entity."@en .


###  http://www.w3.org/2006/time#hasTime
time:hasTime rdf:type owl:ObjectProperty ;
             rdfs:range time:TemporalEntity ;
             rdfs:comment "Proporciona soporte a la asociación de una entidad temporal (instante o intervalo) a cualquier cosa."@es ,
                          "Supports the association of a temporal entity (instant or interval) to any thing"@en ;
             rdfs:label "has time"@en ,
                        "tiene tiempo"@es ;
             skos:definition "Proporciona soporte a la asociación de una entidad temporal (instante o intervalo) a cualquier cosa."@es ,
                             "Supports the association of a temporal entity (instant or interval) to any thing"@en ;
             skos:editorialNote "Característica arriesgada -añadida en la revisión del 2017 que no ha sido todavía utilizada de forma amplia."@es ,
                                "Feature at risk - added in 2017 revision, and not yet widely used. "@en .


###  http://www.w3.org/2006/time#inDateTime
time:inDateTime rdf:type owl:ObjectProperty ;
                rdfs:subPropertyOf time:inTemporalPosition ;
                rdfs:domain time:Instant ;
                rdfs:range time:GeneralDateTimeDescription ;
                rdfs:comment "Posición de un instante, expresada utilizando una descripción estructurada."@es ,
                             "Position of an instant, expressed using a structured description"@en ;
                rdfs:label "en descripción de fecha-hora"@es ,
                           "in date-time description"@en ;
                skos:definition "Posición de un instante, expresada utilizando una descripción estructurada."@es ,
                                "Position of an instant, expressed using a structured description"@en .


###  http://www.w3.org/2006/time#inTemporalPosition
time:inTemporalPosition rdf:type owl:ObjectProperty ;
                        rdfs:domain time:Instant ;
                        rdfs:range time:TemporalPosition ;
                        rdfs:comment "Posición de un instante de tiempo."@es ,
                                     "Position of a time instant"@en ;
                        rdfs:label "Temporal position"@en ,
                                   "posición temporal"@es ;
                        skos:definition "Posición de un instante de tiempo."@es ,
                                        "Position of a time instant"@en .


###  http://www.w3.org/2006/time#inTimePosition
time:inTimePosition rdf:type owl:ObjectProperty ;
                    rdfs:subPropertyOf time:inTemporalPosition ;
                    rdfs:domain time:Instant ;
                    rdfs:range time:TimePosition ;
                    rdfs:comment "Posición de un instante, expresada como una coordenada temporal o un valor nominal."@es ,
                                 "Position of an instant, expressed as a temporal coordinate or nominal value"@en ;
                    rdfs:label "Time position"@en ,
                               "posición de tiempo"@es ;
                    skos:definition "Posición de un instante, expresada como una coordenada temporal o un valor nominal."@es ,
                                    "Position of a time instant expressed as a TimePosition"@en .


###  http://www.w3.org/2006/time#inside
time:inside rdf:type owl:ObjectProperty ;
            rdfs:domain time:Interval ;
            rdfs:range time:Instant ;
            rdfs:comment "An instant that falls inside the interval. It is not intended to include beginnings and ends of intervals."@en ,
                         "Un instante que cae dentro del intervalo. Se asume que no es ni el principio ni el final de ningún intervalo."@es ;
            rdfs:label "has time instant inside"@en ,
                       "tiene instante de tiempo dentro"@es ;
            skos:definition "An instant that falls inside the interval. It is not intended to include beginnings and ends of intervals."@en ,
                            "Un instante que cae dentro del intervalo. Se asume que no es ni el principio ni el final de ningún intervalo."@es .


###  http://www.w3.org/2006/time#intervalAfter
time:intervalAfter rdf:type owl:ObjectProperty ;
                   rdfs:subPropertyOf time:after ,
                                      time:intervalDisjoint ;
                   owl:inverseOf time:intervalBefore ;
                   rdfs:domain time:ProperInterval ;
                   rdfs:range time:ProperInterval ;
                   rdfs:comment "If a proper interval T1 is intervalAfter another proper interval T2, then the beginning of T1 is after the end of T2."@en ,
                                "Si un intervalo propio T1 es posterior a otro intervalo propio T2, entonces el principio de T1 está después que el final de T2." ;
                   rdfs:label "interval after"@en ,
                              "intervalo posterior"@es ;
                   skos:definition "If a proper interval T1 is intervalAfter another proper interval T2, then the beginning of T1 is after the end of T2."@en ,
                                   "Si un intervalo propio T1 es posterior a otro intervalo propio T2, entonces el principio de T1 está después que el final de T2."@es .


###  http://www.w3.org/2006/time#intervalBefore
time:intervalBefore rdf:type owl:ObjectProperty ;
                    rdfs:subPropertyOf time:before ,
                                       time:intervalDisjoint ;
                    rdfs:domain time:ProperInterval ;
                    rdfs:range time:ProperInterval ;
                    rdfs:comment "If a proper interval T1 is intervalBefore another proper interval T2, then the end of T1 is before the beginning of T2."@en ,
                                 "Si un intervalo propio T1 está antes que otro intervalo propio T2, entonces el final de T1 está antes que el principio de T2."@es ;
                    rdfs:label "interval before"@en ,
                               "intervalo anterior"@es ;
                    skos:definition "If a proper interval T1 is intervalBefore another proper interval T2, then the end of T1 is before the beginning of T2."@en ,
                                    "Si un intervalo propio T1 está antes que otro intervalo propio T2, entonces el final de T1 está antes que el principio de T2."@es .


###  http://www.w3.org/2006/time#intervalContains
time:intervalContains rdf:type owl:ObjectProperty ;
                      owl:inverseOf time:intervalDuring ;
                      rdfs:domain time:ProperInterval ;
                      rdfs:range time:ProperInterval ;
                      rdfs:comment "If a proper interval T1 is intervalContains another proper interval T2, then the beginning of T1 is before the beginning of T2, and the end of T1 is after the end of T2."@en ,
                                   "Si un intervalo propio T1 contiene otro intervalo propio T2, entonces el principio de T1 está antes que el principio de T2, y el final de T1 está después del final de T2."@es ;
                      rdfs:label "interval contains"@en ,
                                 "intervalo contiene"@es ;
                      skos:definition "If a proper interval T1 is intervalContains another proper interval T2, then the beginning of T1 is before the beginning of T2, and the end of T1 is after the end of T2."@en ,
                                      "Si un intervalo propio T1 contiene otro intervalo propio T2, entonces el principio de T1 está antes que el principio de T2, y el final de T1 está después del final de T2."@es .


###  http://www.w3.org/2006/time#intervalDisjoint
time:intervalDisjoint rdf:type owl:ObjectProperty ;
                      rdfs:domain time:ProperInterval ;
                      rdfs:range time:ProperInterval ;
                      rdfs:comment "If a proper interval T1 is intervalDisjoint another proper interval T2, then the beginning of T1 is after the end of T2, or the end of T1 is before the beginning of T2, i.e. the intervals do not overlap in any way, but their ordering relationship is not known."@en ,
                                   "Si un intervalo propio T1 es disjunto con otro intervalo propio T2, entonces el principio de T1 está después del final de T2, o el final de T1 está antes que el principio de T2, es decir, los intervalos no se solapan de ninguna forma, aunque su relación de orden no se conozca."@es ;
                      rdfs:label "interval disjoint"@en ,
                                 "intervalo disjunto"@es ;
                      skos:definition "If a proper interval T1 is intervalDisjoint another proper interval T2, then the beginning of T1 is after the end of T2, or the end of T1 is before the beginning of T2, i.e. the intervals do not overlap in any way, but their ordering relationship is not known."@en ,
                                      "Si un intervalo propio T1 es disjunto con otro intervalo propio T2, entonces el principio de T1 está después del final de T2, o el final de T1 está antes que el principio de T2, es decir, los intervalos no se solapan de ninguna forma, aunque su relación de orden no se conozca."@es ;
                      skos:note "Esta relación entre intervalos no estaba incluida en las 13 relaciones básicas definidas por Allen (1984), pero está definida en T.3 como la unión de 'intervalo anterior' con 'intervalo posterior'. Sin embargo, esto está fuera de la expresividad de OWL2, por tanto, está implementado como una propiedad explícita, con 'intervalo anterior' e 'intervalo posterior' como sub-propiedades."@es ,
                                "This interval relation is not included in the 13 basic relationships defined in Allen (1984), but is defined in (T.3) as the union of :intervalBefore v :intervalAfter . However, that is outside OWL2 expressivity, so is implemented as an explicit property, with :intervalBefore , :intervalAfter as sub-properties"@en .


###  http://www.w3.org/2006/time#intervalDuring
time:intervalDuring rdf:type owl:ObjectProperty ;
                    rdfs:subPropertyOf time:intervalIn ;
                    rdfs:domain time:ProperInterval ;
                    rdfs:range time:ProperInterval ;
                    rdfs:comment "If a proper interval T1 is intervalDuring another proper interval T2, then the beginning of T1 is after the beginning of T2, and the end of T1 is before the end of T2."@en ,
                                 "Si un intervalo propio T1 está durante otro intervalo propio T2, entonces del principio de T1 está después del principio de T2, y el final de T1 está antes que el final de T2."@es ;
                    rdfs:label "interval during"@en ,
                               "intervalo durante"@es ;
                    skos:definition "If a proper interval T1 is intervalDuring another proper interval T2, then the beginning of T1 is after the beginning of T2, and the end of T1 is before the end of T2."@en ,
                                    "Si un intervalo propio T1 está durante otro intervalo propio T2, entonces del principio de T1 está después del principio de T2, y el final de T1 está antes que el final de T2."@es .


###  http://www.w3.org/2006/time#intervalEquals
time:intervalEquals rdf:type owl:ObjectProperty ;
                    rdfs:domain time:ProperInterval ;
                    rdfs:range time:ProperInterval ;
                    owl:propertyDisjointWith time:intervalIn ;
                    rdfs:comment "If a proper interval T1 is intervalEquals another proper interval T2, then the beginning of T1 is coincident with the beginning of T2, and the end of T1 is coincident with the end of T2."@en ,
                                 "Si un intervalo propio T1 es igual a otro intervalo propio T2, entonces el principio de T1 coincide con el principio de T2, y el final de T1 coincide con el final de T2."@es ;
                    rdfs:label "interval equals"@en ,
                               "intervalo igual"@es ;
                    skos:definition "If a proper interval T1 is intervalEquals another proper interval T2, then the beginning of T1 is coincident with the beginning of T2, and the end of T1 is coincident with the end of T2."@en ,
                                    "Si un intervalo propio T1 es igual a otro intervalo propio T2, entonces el principio de T1 coincide con el principio de T2, y el final de T1 coincide con el final de T2."@es .


###  http://www.w3.org/2006/time#intervalFinishedBy
time:intervalFinishedBy rdf:type owl:ObjectProperty ;
                        owl:inverseOf time:intervalFinishes ;
                        rdfs:domain time:ProperInterval ;
                        rdfs:range time:ProperInterval ;
                        rdfs:comment "If a proper interval T1 is intervalFinishedBy another proper interval T2, then the beginning of T1 is before the beginning of T2, and the end of T1 is coincident with the end of T2."@en ,
                                     "Si un intervalo propio T1 está terminado por otro intervalo propio T2, entonces el principio de T1 está antes que el principio de T2, y el final de T1 coincide con el final de T2."@es ;
                        rdfs:label "interval finished by"@en ,
                                   "intervalo terminado por"@es ;
                        skos:definition "If a proper interval T1 is intervalFinishedBy another proper interval T2, then the beginning of T1 is before the beginning of T2, and the end of T1 is coincident with the end of T2."@en ,
                                        "Si un intervalo propio T1 está terminado por otro intervalo propio T2, entonces el principio de T1 está antes que el principio de T2, y el final de T1 coincide con el final de T2."@es .


###  http://www.w3.org/2006/time#intervalFinishes
time:intervalFinishes rdf:type owl:ObjectProperty ;
                      rdfs:subPropertyOf time:intervalIn ;
                      rdfs:domain time:ProperInterval ;
                      rdfs:range time:ProperInterval ;
                      rdfs:comment "If a proper interval T1 is intervalFinishes another proper interval T2, then the beginning of T1 is after the beginning of T2, and the end of T1 is coincident with the end of T2."@en ,
                                   "Si un intervalo propio T1 termina otro intervalo propio T2, entonces del principio de T1 está después del principio de T2, y el final de T1 coincide con el final de T2."@es ;
                      rdfs:label "interval finishes"@en ,
                                 "intervalo termina"@es ;
                      skos:definition "If a proper interval T1 is intervalFinishes another proper interval T2, then the beginning of T1 is after the beginning of T2, and the end of T1 is coincident with the end of T2."@en ,
                                      "Si un intervalo propio T1 termina otro intervalo propio T2, entonces del principio de T1 está después del principio de T2, y el final de T1 coincide con el final de T2."@es .


###  http://www.w3.org/2006/time#intervalIn
time:intervalIn rdf:type owl:ObjectProperty ;
                rdfs:domain time:ProperInterval ;
                rdfs:range time:ProperInterval ;
                rdfs:comment "If a proper interval T1 is intervalIn another proper interval T2, then the beginning of T1 is after the beginning of T2 or is coincident with the beginning of T2, and the end of T1 is before the end of T2, or is coincident with the end of T2, except that end of T1 may not be coincident with the end of T2 if the beginning of T1 is coincident with the beginning of T2."@en ,
                             "Si un intervalo propio T1 es un intervalo interior a otro intervalo propio T2, entonces el principio de T1 está después del principio de T2 o coincide con el principio de T2, y el final de T1 está antes que el final de T2, o coincide con el final de T2, excepto que el final de T1 puede no coincidir con el final de T2 si el principio de T1 coincide con el principio de T2."@es ;
                rdfs:label "interval in"@en ,
                           "intervalo interior"@es ;
                skos:definition "If a proper interval T1 is intervalIn another proper interval T2, then the beginning of T1 is after the beginning of T2 or is coincident with the beginning of T2, and the end of T1 is before the end of T2, or is coincident with the end of T2, except that end of T1 may not be coincident with the end of T2 if the beginning of T1 is coincident with the beginning of T2."@en ,
                                "Si un intervalo propio T1 es un intervalo interior a otro intervalo propio T2, entonces el principio de T1 está después del principio de T2 o coincide con el principio de T2, y el final de T1 está antes que el final de T2, o coincide con el final de T2, excepto que el final de T1 puede no coincidir con el final de T2 si el principio de T1 coincide con el principio de T2."@es ;
                skos:note "Esta relación entre intervalos no estaba incluida en las 13 relaciones básicas definidas por Allen (1984), pero se hace referencia a ella como \"una relación importante\" en Allen y Ferguson (1997). Es la unión disjunta de 'intervalo empieza', 'intervalo durante' y con 'intervalo termina'. Sin embargo, esto está fuera de la expresividad de OWL2, por tanto, se implementa como una propiedad explícita, con 'intervalo empieza', 'intervalo durante' e 'intervalo termina' como sub-propiedades."@es ,
                          "This interval relation is not included in the 13 basic relationships defined in Allen (1984), but is referred to as 'an important relationship' in Allen and Ferguson (1997). It is the disjoint union of :intervalStarts v :intervalDuring v :intervalFinishes . However, that is outside OWL2 expressivity, so is implemented as an explicit property, with :intervalStarts , :intervalDuring , :intervalFinishes as sub-properties"@en .


###  http://www.w3.org/2006/time#intervalMeets
time:intervalMeets rdf:type owl:ObjectProperty ;
                   owl:inverseOf time:intervalMetBy ;
                   rdfs:domain time:ProperInterval ;
                   rdfs:range time:ProperInterval ;
                   rdfs:comment "If a proper interval T1 is intervalMeets another proper interval T2, then the end of T1 is coincident with the beginning of T2."@en ,
                                "Si un intervalo propio T1 se encuentra con otro intervalo propio T2, entonces el final de T1 coincide con el principio de T2."@es ;
                   rdfs:label "interval meets"@en ,
                              "intervalo se encuentra"@es ;
                   skos:definition "If a proper interval T1 is intervalMeets another proper interval T2, then the end of T1 is coincident with the beginning of T2."@en ,
                                   "Si un intervalo propio T1 se encuentra con otro intervalo propio T2, entonces el final de T1 coincide con el principio de T2."@es .


###  http://www.w3.org/2006/time#intervalMetBy
time:intervalMetBy rdf:type owl:ObjectProperty ;
                   rdfs:domain time:ProperInterval ;
                   rdfs:range time:ProperInterval ;
                   rdfs:comment "If a proper interval T1 is intervalMetBy another proper interval T2, then the beginning of T1 is coincident with the end of T2."@en ,
                                "Si un intervalo propio T1 es 'intervalo encontrado por' otro intervalo propio T2, entonces el principio de T1 coincide con el final de T2."@es ;
                   rdfs:label "interval met by"@en ,
                              "intervalo encontrado por"@es ;
                   skos:definition "If a proper interval T1 is intervalMetBy another proper interval T2, then the beginning of T1 is coincident with the end of T2."@en ,
                                   "Si un intervalo propio T1 es 'intervalo encontrado por' otro intervalo propio T2, entonces el principio de T1 coincide con el final de T2."@es .


###  http://www.w3.org/2006/time#intervalOverlappedBy
time:intervalOverlappedBy rdf:type owl:ObjectProperty ;
                          owl:inverseOf time:intervalOverlaps ;
                          rdfs:domain time:ProperInterval ;
                          rdfs:range time:ProperInterval ;
                          rdfs:comment "If a proper interval T1 is intervalOverlappedBy another proper interval T2, then the beginning of T1 is after the beginning of T2, the beginning of T1 is before the end of T2, and the end of T1 is after the end of T2."@en ,
                                       "Si un intervalo propio T1 es 'intervalo solapado por' otro intervalo propio T2, entonces el principio de T1 es posterior al principio de T2, y el principio de T1 es anterior al final de T2, y el final de T1 es posterior al final de T2."@es ;
                          rdfs:label "interval overlapped by"@en ,
                                     "intervalo solapado por"@es ;
                          skos:definition "If a proper interval T1 is intervalOverlappedBy another proper interval T2, then the beginning of T1 is after the beginning of T2, the beginning of T1 is before the end of T2, and the end of T1 is after the end of T2."@en ,
                                          "Si un intervalo propio T1 es 'intervalo solapado por' otro intervalo propio T2, entonces el principio de T1 es posterior al principio de T2, y el principio de T1 es anterior al final de T2, y el final de T1 es posterior al final de T2."@es .


###  http://www.w3.org/2006/time#intervalOverlaps
time:intervalOverlaps rdf:type owl:ObjectProperty ;
                      rdfs:domain time:ProperInterval ;
                      rdfs:range time:ProperInterval ;
                      rdfs:comment "Asume una dirección en el tiempo. Si una entidad temporal T1 está después de otra entidad temporal T2, entonces el principio de T1 está después del final de T2."@es ,
                                   "If a proper interval T1 is intervalOverlaps another proper interval T2, then the beginning of T1 is before the beginning of T2, the end of T1 is after the beginning of T2, and the end of T1 is before the end of T2."@en ,
                                   "Si un intervalo propio T1 se solapa con otro intervalo propio T2, entonces el principio de T1 es anterior al principio de T2, el final de T1 es posterior al principio de T2, y el final de T1 es anterior al final de T2."@es ;
                      rdfs:label "interval overlaps"@en ,
                                 "intervalo se solapa"@es ;
                      skos:definition "If a proper interval T1 is intervalOverlaps another proper interval T2, then the beginning of T1 is before the beginning of T2, the end of T1 is after the beginning of T2, and the end of T1 is before the end of T2."@en ,
                                      "Si un intervalo propio T1 se solapa con otro intervalo propio T2, entonces el principio de T1 es anterior al principio de T2, el final de T1 es posterior al principio de T2, y el final de T1 es anterior al final de T2."@es .


###  http://www.w3.org/2006/time#intervalStartedBy
time:intervalStartedBy rdf:type owl:ObjectProperty ;
                       owl:inverseOf time:intervalStarts ;
                       rdfs:domain time:ProperInterval ;
                       rdfs:range time:ProperInterval ;
                       rdfs:comment "If a proper interval T1 is intervalStarted another proper interval T2, then the beginning of T1 is coincident with the beginning of T2, and the end of T1 is after the end of T2."@en ,
                                    "Si un intervalo propio T1 es empezado por otro intervalo propio T2, entonces el principio de T1 coincide con el principio de T2, y el final de T1 es posterior al final de T2."@es ;
                       rdfs:label "interval started by"@en ;
                       skos:definition "If a proper interval T1 is intervalStarted another proper interval T2, then the beginning of T1 is coincident with the beginning of T2, and the end of T1 is after the end of T2."@en ,
                                       "Si un intervalo propio T1 es empezado por otro intervalo propio T2, entonces el principio de T1 coincide con el principio de T2, y el final de T1 es posterior al final de T2."@es .


###  http://www.w3.org/2006/time#intervalStarts
time:intervalStarts rdf:type owl:ObjectProperty ;
                    rdfs:subPropertyOf time:intervalIn ;
                    rdfs:domain time:ProperInterval ;
                    rdfs:range time:ProperInterval ;
                    rdfs:comment "If a proper interval T1 is intervalStarts another proper interval T2, then the beginning of T1 is coincident with the beginning of T2, and the end of T1 is before the end of T2."@en ,
                                 "Si un intervalo propio T1 empieza otro intervalo propio T2, entonces del principio de T1 con el principio de T2, y el final de T1 es anterior al final de T2."@es ;
                    rdfs:label "interval starts"@en ,
                               "intervalo empieza"@es ;
                    skos:definition "If a proper interval T1 is intervalStarts another proper interval T2, then the beginning of T1 is coincident with the beginning of T2, and the end of T1 is before the end of T2."@en ,
                                    "Si un intervalo propio T1 empieza otro intervalo propio T2, entonces del principio de T1 con el final de T2, y el final de T1 es anterior al final de T2."@es .


###  http://www.w3.org/2006/time#monthOfYear
time:monthOfYear rdf:type owl:ObjectProperty ;
                 rdfs:domain time:GeneralDateTimeDescription ;
                 rdfs:range time:MonthOfYear ;
                 rdfs:comment "El mes del año, cuyo valor es un miembro de la clase 'mes del año'."@es ,
                              "The month of the year, whose value is a member of the class time:MonthOfYear"@en ;
                 rdfs:label "mes del año"@es ,
                            "month of year"@en ;
                 skos:definition "El mes del año, cuyo valor es un miembro de la clase 'mes del año'."@es ,
                                 "The month of the year, whose value is a member of the class time:MonthOfYear"@en ;
                 skos:editorialNote "Característica arriesgada - añadida en la revisión de 2017, y todavía no ampliamente utilizada."@es ,
                                    "Feature at risk - added in 2017 revision, and not yet widely used. "@en .


###  http://www.w3.org/2006/time#timeZone
time:timeZone rdf:type owl:ObjectProperty ;
              rdfs:domain time:GeneralDateTimeDescription ;
              rdfs:range time:TimeZone ;
              rdfs:comment "The time zone for clock elements in the temporal position"@en ;
              rdfs:label "en huso horario"@es ,
                         "in time zone"@en ;
              skos:historyNote """En la versión original de OWL-Time de 2006, el rango de 'en huso horario' se definió en un espacio de nombres diferente \"http://www.w3.org/2006/timezone#\".
            Un axioma de alineación permite que los datos codificados de acuerdo con la versión anterior sean consistentes con la ontología actualizada."""@es ,
                               """In the original 2006 version of OWL-Time, the range of time:timeZone was a TimeZone class in a separate namespace \"http://www.w3.org/2006/timezone#\". 
An alignment axiom 
	tzont:TimeZone rdfs:subClassOf time:TimeZone . 
allows data encoded according to the previous version to be consistent with the updated ontology. """ ;
              skos:note """IANA maintains a database of timezones. These are well maintained and generally considered authoritative, but individual items are not available at individual URIs, so cannot be used directly in data expressed using OWL-Time.

DBPedia provides a set of resources corresponding to the IANA timezones, with a URI for each (e.g. http://dbpedia.org/resource/Australia/Eucla). The World Clock service also provides a list of time zones with the description of each available as an individual webpage with a convenient individual URI (e.g. https://www.timeanddate.com/time/zones/acwst). These or other, similar, resources might be used as a value of the time:timeZone property.""" ,
                        """IANA mantiene una base de datos de husos horarios. Éstas están bien mantenidas y generalmente se consideran autorizadas, pero los ítems individuales no están disponibles en URIs individuales, por tanto, no se pueden utilizar directamente en datos expresados utilizando OWL-Time.
            La BDPedia proporciona un conjunto de recursos correspondientes a los husos horarios de IANA, con una URI para cada uno (por ejemplo, http://dbpedia.org/resource/Australia/Eucla). El Servicio de Reloj Mundial también proporciona una lista de husos horarios con la descripción de cada uno de los disponibles como una página Web individual con una URI adecuada individual (por ejemplo, https://www.timeanddate.com/time/zones/acwst). Éstos, y otros recursos similares, se puden usar como un valor de la propiedad 'huso horario'."""@es .


###  http://www.w3.org/2006/time#unitType
time:unitType rdf:type owl:ObjectProperty ;
              rdfs:domain [ rdf:type owl:Class ;
                            owl:unionOf ( time:Duration
                                          time:GeneralDateTimeDescription
                                        )
                          ] ;
              rdfs:range time:TemporalUnit ;
              rdfs:comment "La unidad de tiempo que proporciona la precisión de un valor fecha-hora o la escala de una extensión temporal."@es ,
                           "The temporal unit which provides the precision of a date-time value or scale of a temporal extent"@en ;
              rdfs:label "temporal unit type"@en ,
                         "tipo de unidad temporal"@es .


###  http://www.w3.org/ns/sosa/hosts
sosa:hosts rdf:type owl:ObjectProperty ;
           owl:inverseOf sosa:isHostedBy ;
           rdfs:comment "Relation between a platform and the systems it hosts."@en ;
           rdfs:isDefinedBy sosa: ;
           rdfs:label "host"@en .


###  http://www.w3.org/ns/sosa/isHostedBy
sosa:isHostedBy rdf:type owl:ObjectProperty ;
                rdfs:comment "Relation between a system and its hosting platform."@en ;
                rdfs:isDefinedBy sosa: ;
                rdfs:label "is hosted by"@en .


###  http://www.w3.org/ns/ssn/deployedOnPlatform
ssn:deployedOnPlatform rdf:type owl:ObjectProperty ;
                       owl:inverseOf ssn:inDeployment ;
                       rdfs:comment "Relation between a deployment and the platform(s) involved in the deployment."@en ;
                       rdfs:isDefinedBy ssn: ;
                       rdfs:label "deployed on platform"@en .


###  http://www.w3.org/ns/ssn/deployedSystem
ssn:deployedSystem rdf:type owl:ObjectProperty ;
                   owl:inverseOf ssn:hasDeployment ;
                   rdfs:comment "Relation between a deployment and the system deployed."@en ;
                   rdfs:isDefinedBy ssn: ;
                   rdfs:label "deployed system"@en .


###  http://www.w3.org/ns/ssn/hasDeployment
ssn:hasDeployment rdf:type owl:ObjectProperty ;
                  rdfs:isDefinedBy ssn: ;
                  rdfs:label "has deployment"@en .


###  http://www.w3.org/ns/ssn/hasSubSystem
ssn:hasSubSystem rdf:type owl:ObjectProperty ;
                 rdfs:isDefinedBy ssn: ;
                 rdfs:label "has subsystem"@en .


###  http://www.w3.org/ns/ssn/inDeployment
ssn:inDeployment rdf:type owl:ObjectProperty ;
                 rdfs:comment "Relation between a platform and the deployment(s) that takes place in the platform."@en ;
                 rdfs:isDefinedBy ssn: ;
                 rdfs:label "in deployment"@en .


###  http://xmlns.com/foaf/0.1/based_near
foaf:based_near rdf:type owl:ObjectProperty .


###  http://xmlns.com/foaf/0.1/member
foaf:member rdf:type owl:ObjectProperty ;
            rdfs:label "member"@en .


###  https://saref.etsi.org/core/accomplishes
saref:accomplishes rdf:type owl:ObjectProperty ;
                   owl:inverseOf saref:isAccomplishedBy ;
                   rdfs:range saref:Task ;
                   rdfs:comment "A relationship between a certain entity (e.g., a device) and the task it accomplishes"@en ;
                   rdfs:isDefinedBy saref: ;
                   rdfs:label "accomplishes"@en .


###  https://saref.etsi.org/core/actsUpon
saref:actsUpon rdf:type owl:ObjectProperty ;
               rdfs:domain saref:Command ;
               rdfs:range saref:State ;
               rdfs:comment "A relationship between a command and a state"@en ;
               rdfs:isDefinedBy saref: ;
               rdfs:label "acts upon"@en .


###  https://saref.etsi.org/core/consistsOf
saref:consistsOf rdf:type owl:ObjectProperty ;
                 rdfs:comment "A relationship indicating a composite entity that consists of other entities (e.g., a temperature/humidity sensor that consists of a temperature sensor and a humidity sensor)"@en ;
                 rdfs:label "consists of"@en .


###  https://saref.etsi.org/core/controlsProperty
saref:controlsProperty rdf:type owl:ObjectProperty ;
                       rdfs:domain saref:Device ;
                       rdfs:range saref:Property ;
                       rdfs:comment "A relationship specifying the property that can be controlled by a certain device"@en ;
                       rdfs:isDefinedBy saref: ;
                       rdfs:label "controls property"@en .


###  https://saref.etsi.org/core/hasCommand
saref:hasCommand rdf:type owl:ObjectProperty ;
                 owl:inverseOf saref:isCommandOf ;
                 rdfs:domain saref:Function ;
                 rdfs:range saref:Command ;
                 rdfs:comment "A relationship between a function and a command"@en ,
                              "A relationship between an entity (such as a function) and a command"@en ;
                 rdfs:isDefinedBy saref: ;
                 rdfs:label "has command"@en .


###  https://saref.etsi.org/core/hasFunction
saref:hasFunction rdf:type owl:ObjectProperty ;
                  rdfs:domain saref:Device ;
                  rdfs:range saref:Function ;
                  rdfs:comment "A relationship identifying the function of a device"@en ,
                               "A relationship identifying the type of function of a device"@en ;
                  rdfs:isDefinedBy saref: ;
                  rdfs:label "has function"@en .


###  https://saref.etsi.org/core/hasMeasurement
saref:hasMeasurement rdf:type owl:ObjectProperty ;
                     owl:inverseOf saref:isMeasurementOf ;
                     rdfs:domain saref:FeatureOfInterest ;
                     rdfs:range saref:Measurement ;
                     rdfs:comment "A relationship between a feature of interest and a measurement about it"@en ,
                                  "Relation betwwen a feature of interest and the measurments that are about it."@en ;
                     rdfs:isDefinedBy saref: ;
                     rdfs:label "has measurement"@en ,
                                "is feature of interest of"@en .


###  https://saref.etsi.org/core/hasMeterReading
saref:hasMeterReading rdf:type owl:ObjectProperty ;
                      rdfs:domain saref:MeteringFunction ;
                      rdfs:range saref:Measurement ;
                      rdfs:comment "A relationship between a metering function and the measurement of the reading"@en ;
                      rdfs:label "has meter reading"@en .


###  https://saref.etsi.org/core/hasMeterReadingType
saref:hasMeterReadingType rdf:type owl:ObjectProperty ;
                          rdfs:domain saref:MeteringFunction ;
                          rdfs:range saref:Property ;
                          rdfs:comment "A relationship identifying the reading type of a metering function (e.g., Water, Gas, Pressure , Energy , Power, etc.)"@en ;
                          rdfs:label "has meter reading type"@en .


###  https://saref.etsi.org/core/hasPrice
saref:hasPrice rdf:type owl:ObjectProperty ;
               rdfs:range saref:Price ;
               rdfs:comment "A relationship indentifying the price associated to an entity"@en ;
               rdfs:label "has price"@en .


###  https://saref.etsi.org/core/hasProfile
saref:hasProfile rdf:type owl:ObjectProperty ;
                 rdfs:domain saref:Device ;
                 rdfs:range saref:Profile ;
                 rdfs:comment "A relationship associating a profile to a certain device"@en ;
                 rdfs:label "has profile"@en .


###  https://saref.etsi.org/core/hasProperty
saref:hasProperty rdf:type owl:ObjectProperty ;
                  owl:inverseOf saref:isPropertyOf ;
                  rdfs:domain saref:FeatureOfInterest ;
                  rdfs:range saref:Property ;
                  rdfs:comment "A relationship between a feature of interest and a property of that feature"@en ,
                               "Relation between a feature of interest and its properties."@en ;
                  rdfs:isDefinedBy saref: ;
                  rdfs:label "has property"@en .


###  https://saref.etsi.org/core/hasSensingRange
saref:hasSensingRange rdf:type owl:ObjectProperty ;
                      rdfs:domain saref:SensingFunction ;
                      rdfs:range saref:Measurement ;
                      rdfs:comment "A relationship between a sensing function and a measurement identifying the range of a sensor detection"@en ;
                      rdfs:label "has sensing range"@en .


###  https://saref.etsi.org/core/hasSensorType
saref:hasSensorType rdf:type owl:ObjectProperty ;
                    rdfs:domain saref:SensingFunction ;
                    rdfs:range saref:Property ;
                    rdfs:comment "A relationship identifying the sensing type of a sensor detection (i.e., Temperature, Occupancy, Humidity, Motion , Smoke, Pressure, etc.) "@en ;
                    rdfs:label "has sensor type"@en .


###  https://saref.etsi.org/core/hasState
saref:hasState rdf:type owl:ObjectProperty ;
               rdfs:domain saref:Device ;
               rdfs:range saref:State ;
               rdfs:comment "A relationship identifying the type of state of a device"@en ;
               rdfs:isDefinedBy saref: ;
               rdfs:label "has state"@en .


###  https://saref.etsi.org/core/hasThresholdMeasurement
saref:hasThresholdMeasurement rdf:type owl:ObjectProperty ;
                              rdfs:domain saref:EventFunction ;
                              rdfs:range saref:Measurement ;
                              rdfs:comment "A relationship associated with an event function to notify that a certain threshold measurement has been exceeded"@en ;
                              rdfs:label "has threshold measurement"@en .


###  https://saref.etsi.org/core/hasTime
saref:hasTime rdf:type owl:ObjectProperty ;
              rdfs:range saref:Time ;
              rdfs:comment "A relationship to associate time information to an entity"@en ;
              rdfs:label "has time"@en .


###  https://saref.etsi.org/core/hasTypicalConsumption
saref:hasTypicalConsumption rdf:type owl:ObjectProperty ;
                            rdfs:comment "A relationship identifying the typical (energy or power) consumption of a device"@en ;
                            rdfs:label "has typical consumption"@en .


###  https://saref.etsi.org/core/isAbout
saref:isAbout rdf:type owl:ObjectProperty ;
              rdfs:comment "A relationship identifying what an entity, such as a profile, is about"@en ;
              rdfs:label "isAbout"@en .


###  https://saref.etsi.org/core/isAccomplishedBy
saref:isAccomplishedBy rdf:type owl:ObjectProperty ;
                       rdfs:domain saref:Task ;
                       rdfs:comment "A relationship identifying an entity (e.g., a device) that can accomplish a task."@en ,
                                    "A relationship indentifying the task accomplished by a certain entity (e.g., a device)"@en ;
                       rdfs:isDefinedBy saref: ;
                       rdfs:label "is accomplished by"@en .


###  https://saref.etsi.org/core/isCommandOf
saref:isCommandOf rdf:type owl:ObjectProperty ;
                  rdfs:domain saref:Command ;
                  rdfs:range saref:Function ;
                  rdfs:comment "A relationship between a command and a function."@en ;
                  rdfs:isDefinedBy saref: ;
                  rdfs:label "is command of"@en .


###  https://saref.etsi.org/core/isControlledByDevice
saref:isControlledByDevice rdf:type owl:ObjectProperty ;
                           rdfs:domain saref:Property ;
                           rdfs:range saref:Device ;
                           rdfs:comment "A relationship specifying the devices that can control a certain property"@en ;
                           rdfs:isDefinedBy saref: ;
                           rdfs:label "is controlled by device"@en .


###  https://saref.etsi.org/core/isMeasuredByDevice
saref:isMeasuredByDevice rdf:type owl:ObjectProperty ;
                         rdfs:domain saref:Property ;
                         rdfs:range saref:Device ;
                         rdfs:comment "A relationship specifying the devices that can measure a certain property"@en ;
                         rdfs:isDefinedBy saref: ;
                         rdfs:label "is measured by device"@en .


###  https://saref.etsi.org/core/isMeasuredIn
saref:isMeasuredIn rdf:type owl:ObjectProperty ;
                   rdfs:domain saref:Measurement ;
                   rdfs:range saref:UnitOfMeasure ;
                   rdfs:comment "A relation between a measurement and the unit of measure in which the measurement value is expressed."@en ,
                                "A relationship identifying the unit of measure used for a certain entity."@en ;
                   rdfs:isDefinedBy saref: ,
                                    "https://saref.etsi.org/core/" ;
                   rdfs:label "is measured in"@en .


###  https://saref.etsi.org/core/isMeasurementOf
saref:isMeasurementOf rdf:type owl:ObjectProperty ;
                      rdfs:domain saref:Measurement ;
                      rdfs:range saref:FeatureOfInterest ;
                      rdfs:comment "A relationship between a measurement and the feature of interest whose quality was measured"@en ,
                                   "Relation between a measurement and the feature of interest being measured."@en ;
                      rdfs:isDefinedBy saref: ;
                      rdfs:label "has feature of interest"@en ,
                                 "is measurement of"@en ,
                                 "isMeasurementOf"@en .


###  https://saref.etsi.org/core/isOfferedBy
saref:isOfferedBy rdf:type owl:ObjectProperty ;
                  owl:inverseOf saref:offers ;
                  rdfs:domain saref:Service ;
                  rdfs:range saref:Device ;
                  rdfs:comment "A relationship between a service and a device that offers the service"@en ;
                  rdfs:label "is offered by"@en .


###  https://saref.etsi.org/core/isPropertyOf
saref:isPropertyOf rdf:type owl:ObjectProperty ;
                   rdfs:domain saref:Property ;
                   rdfs:range saref:FeatureOfInterest ;
                   rdfs:comment "A relationship between a property and the feature of interest it belongs to"@en ,
                                "Relation between a property and a feature of interest in which such property appears."@en ;
                   rdfs:isDefinedBy saref: ;
                   rdfs:label "is property of"@en .


###  https://saref.etsi.org/core/isUsedFor
saref:isUsedFor rdf:type owl:ObjectProperty ;
                rdfs:comment "A relationship specifying the commodity for which a device is used for"@en ;
                rdfs:label "is used for"@en .


###  https://saref.etsi.org/core/makesMeasurement
saref:makesMeasurement rdf:type owl:ObjectProperty ;
                       owl:inverseOf saref:measurementMadeBy ;
                       rdfs:domain saref:Device ;
                       rdfs:range saref:Measurement ;
                       rdfs:comment "A relation between a device and the measurements it makes. Such measurement will link together the value of the measurement, its unit of measure and the property to which it relates."@en ;
                       rdfs:isDefinedBy saref: ;
                       rdfs:label "makes measurement"@en .


###  https://saref.etsi.org/core/measurementMadeBy
saref:measurementMadeBy rdf:type owl:ObjectProperty ;
                        rdfs:domain saref:Measurement ;
                        rdfs:range saref:Device ;
                        rdfs:comment "A relation between a measurement and the device that made it."@en ,
                                     "Relation between a measurement and the device that made it."@en ;
                        rdfs:isDefinedBy saref: ;
                        rdfs:label "measurement made by"@en .


###  https://saref.etsi.org/core/measuresProperty
saref:measuresProperty rdf:type owl:ObjectProperty ;
                       rdfs:domain saref:Device ;
                       rdfs:range saref:Property ;
                       rdfs:comment "A relationship specifying the property that can be measured by a certain device"@en ;
                       rdfs:isDefinedBy saref: ;
                       rdfs:label "measures property"@en .


###  https://saref.etsi.org/core/offers
saref:offers rdf:type owl:ObjectProperty ;
             rdfs:domain saref:Device ;
             rdfs:range saref:Service ;
             rdfs:comment "A relationship between a device and a service"@en ;
             rdfs:label "offers"@en .


###  https://saref.etsi.org/core/relatesToMeasurement
saref:relatesToMeasurement rdf:type owl:ObjectProperty ;
                           owl:inverseOf saref:relatesToProperty ;
                           rdfs:domain saref:Property ;
                           rdfs:range saref:Measurement ;
                           rdfs:comment "A relationship between a property and the measurements it relates to"@en ;
                           rdfs:isDefinedBy saref: ;
                           rdfs:label "relates to measurement"@en .


###  https://saref.etsi.org/core/relatesToProperty
saref:relatesToProperty rdf:type owl:ObjectProperty ;
                        rdfs:domain saref:Measurement ;
                        rdfs:range saref:Property ;
                        rdfs:comment "A relation between a measurement and the property such measurement is about."@en ,
                                     "A relationship between a measurement and the property it relates to"@en ;
                        rdfs:isDefinedBy saref: ,
                                         "https://saref.etsi.org/core/" ;
                        rdfs:label "relates to property"@en .


###  https://saref.etsi.org/core/represents
saref:represents rdf:type owl:ObjectProperty ;
                 rdfs:domain saref:Service ;
                 rdfs:range saref:Function ;
                 rdfs:comment "A relationship between a service and a function."@en ;
                 rdfs:label "represents"@en .


###  https://saref.etsi.org/saref4agri/contains
s4agri:contains rdf:type owl:ObjectProperty ;
                rdfs:subPropertyOf geosp:sfContains ;
                owl:inverseOf s4agri:isContainedIn ;
                rdfs:comment "contains"@en ;
                rdfs:label "contains"@en .


###  https://saref.etsi.org/saref4agri/generates
s4agri:generates rdf:type owl:ObjectProperty ;
                 rdfs:subPropertyOf saref:hasProperty ;
                 rdfs:comment "A relation to represent the yield generated by a Crop."@en ;
                 rdfs:label "generates"@en .


###  https://saref.etsi.org/saref4agri/hasDeploymentPeriod
s4agri:hasDeploymentPeriod rdf:type owl:ObjectProperty ;
                           rdfs:comment "Relation to indicate the temporal duration or period of a deployment."@en ,
                                        "has deployment period"@en ;
                           rdfs:label "has deployment period"@en .


###  https://saref.etsi.org/saref4agri/hasID
s4agri:hasID rdf:type owl:ObjectProperty ;
             rdfs:subPropertyOf owl:topObjectProperty ;
             rdfs:range s4agri:ID ;
             rdfs:comment "A relation to express the unique identifier of an animal."@en ;
             rdfs:label "has id"@en .


###  https://saref.etsi.org/saref4agri/hasMember
s4agri:hasMember rdf:type owl:ObjectProperty ;
                 owl:inverseOf s4agri:isMemberOf ;
                 rdfs:comment "A relation to represent  the members of an AnimalGroup."@en ;
                 rdfs:label "has member"@en .


###  https://saref.etsi.org/saref4agri/hasReceived
s4agri:hasReceived rdf:type owl:ObjectProperty ;
                   owl:inverseOf s4agri:receives ;
                   rdfs:comment "has received"@en ;
                   rdfs:label "has received"@en .


###  https://saref.etsi.org/saref4agri/isContainedIn
s4agri:isContainedIn rdf:type owl:ObjectProperty ;
                     rdfs:comment "is contained in"@en ;
                     rdfs:label "is contained in"@en .


###  https://saref.etsi.org/saref4agri/isDeployedAtSpace
s4agri:isDeployedAtSpace rdf:type owl:ObjectProperty ;
                         rdfs:comment "Relation to indicate the geographical componet of a deployment."@en ,
                                      "is deployed at space"@en ;
                         rdfs:label "is deployed at space"@en .


###  https://saref.etsi.org/saref4agri/isLocatedIn
s4agri:isLocatedIn rdf:type owl:ObjectProperty ;
                   owl:inverseOf s4agri:isLocationOf ;
                   rdfs:comment "A relation to express the physical location of a saref4agri entity (e.g., an animal)"@en ;
                   rdfs:label "is located in"@en .


###  https://saref.etsi.org/saref4agri/isLocationOf
s4agri:isLocationOf rdf:type owl:ObjectProperty ;
                    rdfs:comment "is location of"@en ;
                    rdfs:label "is location of"@en .


###  https://saref.etsi.org/saref4agri/isMemberOf
s4agri:isMemberOf rdf:type owl:ObjectProperty ;
                  rdfs:comment "A relation to express that an animal can be part of groups."@en ;
                  rdfs:label "is member of"@en .


###  https://saref.etsi.org/saref4agri/managesFarm
s4agri:managesFarm rdf:type owl:ObjectProperty ;
                   rdfs:comment "manages farm"@en ;
                   rdfs:label "manages farm"@en .


###  https://saref.etsi.org/saref4agri/receives
s4agri:receives rdf:type owl:ObjectProperty ;
                rdfs:subPropertyOf saref:hasMeasurement ;
                rdfs:comment "A relation to represent the intake/consumption of certain substances in a Crop."@en ;
                rdfs:label "receives"@en .


###  https://saref.etsi.org/saref4bldg/airFlowRateMax
s4bldg:airFlowRateMax rdf:type owl:ObjectProperty ;
                      rdfs:comment "Maximum allowable air flow rate. Usually measured in m3/s."@en ;
                      rdfs:label "air flow rate range max"@en .


###  https://saref.etsi.org/saref4bldg/airFlowRateMin
s4bldg:airFlowRateMin rdf:type owl:ObjectProperty ;
                      rdfs:comment "Minimum allowable air flow rate. Usually measured in m3/s."@en ;
                      rdfs:label "air flow rate range min"@en .


###  https://saref.etsi.org/saref4bldg/ambientDesignDryBulbTemperature
s4bldg:ambientDesignDryBulbTemperature rdf:type owl:ObjectProperty ;
                                       rdfs:comment "Ambient design dry bulb temperature used for selecting the cooling tower. Usually measured in degrees Kelvin (K)."@en ;
                                       rdfs:label "ambient design dry bulb temperature"@en .


###  https://saref.etsi.org/saref4bldg/ambientDesignWetBulbTemperature
s4bldg:ambientDesignWetBulbTemperature rdf:type owl:ObjectProperty ;
                                       rdfs:comment "Ambient design wet bulb temperature used for selecting the cooling tower. Usually measured in degrees Kelvin (K)."@en ;
                                       rdfs:label "ambient design wet bulb temperature"@en .


###  https://saref.etsi.org/saref4bldg/apparentPowerMax
s4bldg:apparentPowerMax rdf:type owl:ObjectProperty ;
                        rdfs:comment "Maximum apparent power/capacity in VA (volt ampere). Usually measured in Watts (W, J/s)."@en ;
                        rdfs:label "maximum apparent power"@en .


###  https://saref.etsi.org/saref4bldg/audioVolume
s4bldg:audioVolume rdf:type owl:ObjectProperty ;
                   rdfs:comment "Indicates discrete audio volume levels and corresponding sound power offsets, if applicable. Missing values may be interpolated. Measured in watts."@en ;
                   rdfs:label "audio volume"@en .


###  https://saref.etsi.org/saref4bldg/basinReserveVolume
s4bldg:basinReserveVolume rdf:type owl:ObjectProperty ;
                          rdfs:comment "Volume between operating and overflow levels in cooling tower basin. Usually measured in cubic metre (m3)."@en ;
                          rdfs:label "basin reserve volume"@en .


###  https://saref.etsi.org/saref4bldg/bladeThickness
s4bldg:bladeThickness rdf:type owl:ObjectProperty ;
                      rdfs:comment "The thickness of the damper blade. Usually measured in millimeters (mm)."@en ;
                      rdfs:label "blade thickness"@en .


###  https://saref.etsi.org/saref4bldg/bodyMass
s4bldg:bodyMass rdf:type owl:ObjectProperty ;
                rdfs:comment "Overall body mass of the heater. Usually measured in kilograms (kg) or grams (g)."@en ;
                rdfs:label "body mass"@en .


###  https://saref.etsi.org/saref4bldg/capacityWeight
s4bldg:capacityWeight rdf:type owl:ObjectProperty ;
                      rdfs:comment "Capacity of the transport element measured by weight. Usually measured in kilograms (kg) or grams (g)."@en ;
                      rdfs:label "capacity weight"@en .


###  https://saref.etsi.org/saref4bldg/closeOffRating
s4bldg:closeOffRating rdf:type owl:ObjectProperty ;
                      rdfs:comment "Close off rating. Usually measured in Pascals (Pa, N/m2)."@en ;
                      rdfs:label "close off rating"@en .


###  https://saref.etsi.org/saref4bldg/coilLength
s4bldg:coilLength rdf:type owl:ObjectProperty ;
                  rdfs:comment "Length of coil. Usually measured in millimeters (mm)."@en ;
                  rdfs:label "coil length"@en .


###  https://saref.etsi.org/saref4bldg/coilWidth
s4bldg:coilWidth rdf:type owl:ObjectProperty ;
                 rdfs:comment "Width of coil. Usually measured in millimeters (mm"@en ;
                 rdfs:label "coil width"@en .


###  https://saref.etsi.org/saref4bldg/colorTemperature
s4bldg:colorTemperature rdf:type owl:ObjectProperty ;
                        rdfs:comment "The color temperature of any source of radiation is defined as the temperature (in Kelvin) of a black-body or Planckian radiator whose radiation has the same chromaticity as the source of radiation. Often the values are only approximate color temperatures as the black-body radiator cannot emit radiation of every chromaticity value. The color temperatures of the commonest artificial light sources range from less than 3000K (warm white) to 4000K (intermediate) and over 5000K (daylight). Usually measured in degrees Kelvin (K)."@en ;
                        rdfs:label "color temperature"@en .


###  https://saref.etsi.org/saref4bldg/compressorSpeed
s4bldg:compressorSpeed rdf:type owl:ObjectProperty ;
                       rdfs:comment "Compressor speed. Usually measured in cycles/s."@en ;
                       rdfs:label "compressor speed"@en .


###  https://saref.etsi.org/saref4bldg/connectionSize
s4bldg:connectionSize rdf:type owl:ObjectProperty ;
                      rdfs:comment "The connection size of the to and from the pump. Usually measured in millimeters (mm)."@en ;
                      rdfs:label "connection size"@en .


###  https://saref.etsi.org/saref4bldg/contains
s4bldg:contains rdf:type owl:ObjectProperty ;
                owl:inverseOf s4bldg:isContainedIn ;
                rdf:type owl:TransitiveProperty ;
                rdfs:comment "A relation between a physical space and the objects located in such space."@en ;
                rdfs:label "contains"@en .


###  https://saref.etsi.org/saref4bldg/contributedLuminousFlux
s4bldg:contributedLuminousFlux rdf:type owl:ObjectProperty ;
                               rdfs:comment "Luminous flux is a photometric measure of radiant flux, i.e. the volume of light emitted from a light source. Luminous flux is measured either for the interior as a whole or for a part of the interior (partial luminous flux for a solid angle). All other photometric parameters are derivatives of luminous flux. Luminous flux is measured in lumens (lm). The luminous flux is given as a nominal value for each lamp. Usually measured in Lumen (lm, Candela Steradian)."@en ;
                               rdfs:label "contributed luminous flux"@en .


###  https://saref.etsi.org/saref4bldg/coverLength
s4bldg:coverLength rdf:type owl:ObjectProperty ;
                   rdfs:comment "The length measured along the x-axis in the local coordinate system or the radius (in the case of a circular shape in plan) of the cover of the oil interceptor. Usually measured in millimeters (mm)."@en ;
                   rdfs:label "cover length"@en .


###  https://saref.etsi.org/saref4bldg/coverWidth
s4bldg:coverWidth rdf:type owl:ObjectProperty ;
                  rdfs:comment "The length measured along the x-axis in the local coordinate system of the cover of the oil interceptor. Usually measured in millimeters (mm)."@en ;
                  rdfs:label "cover width"@en .


###  https://saref.etsi.org/saref4bldg/effectiveCapacity
s4bldg:effectiveCapacity rdf:type owl:ObjectProperty ;
                         rdfs:comment "The total effective or actual volumetric capacity of the tank. Usually measured in cubic metre (m3).B3"@en ;
                         rdfs:label "effective capacity"@en .


###  https://saref.etsi.org/saref4bldg/electricGeneratorEfficiency
s4bldg:electricGeneratorEfficiency rdf:type owl:ObjectProperty ;
                                   rdfs:comment "The ratio of output capacity to intake capacity."@en ;
                                   rdfs:label "electric generator efficiency"@en .


###  https://saref.etsi.org/saref4bldg/electricMotorEfficiency
s4bldg:electricMotorEfficiency rdf:type owl:ObjectProperty ;
                               rdfs:comment "The ratio of output capacity to intake capacity."@en ;
                               rdfs:label "electric motor efficiency"@en .


###  https://saref.etsi.org/saref4bldg/externalSurfaceArea
s4bldg:externalSurfaceArea rdf:type owl:ObjectProperty ;
                           rdfs:comment "External surface area (both primary and secondary area). Usually measured in square metre (m2)."@en ;
                           rdfs:label "external surface area"@en .


###  https://saref.etsi.org/saref4bldg/faceArea
s4bldg:faceArea rdf:type owl:ObjectProperty ;
                rdfs:comment "Face area open to the airstream. Usually measured in square metre (m2)."@en ;
                rdfs:label "face area"@en .


###  https://saref.etsi.org/saref4bldg/finalResistance
s4bldg:finalResistance rdf:type owl:ObjectProperty ;
                       rdfs:comment "Filter fluid resistance when replacement is required (i.e., Pressure drop at the maximum air flowrate across the filter when the filter needs replacement per ASHRAE Standard 52.1). Usually measured in Pascals (Pa, N/m2)."@en ;
                       rdfs:label "final resistance"@en .


###  https://saref.etsi.org/saref4bldg/firstCurvatureRadius
s4bldg:firstCurvatureRadius rdf:type owl:ObjectProperty ;
                            rdfs:comment "FirstCurvatureRadius should be defined as the base or left side radius of curvature value. Usually measured in millimeters (mm)."@en ;
                            rdfs:label "first curvature radius"@en .


###  https://saref.etsi.org/saref4bldg/flowCoefficient
s4bldg:flowCoefficient rdf:type owl:ObjectProperty ;
                       rdfs:comment "Flow coefficient (the quantity of fluid that passes through a fully open valve at unit pressure drop), typically expressed as the Kv or Cv value for the valve."@en ;
                       rdfs:label "flow coefficient"@en .


###  https://saref.etsi.org/saref4bldg/flowResistanceMax
s4bldg:flowResistanceMax rdf:type owl:ObjectProperty ;
                         rdfs:comment "Allowable range of frictional resistance against which the fluid is being pumped. Usually measured in Pascals (Pa, N/m2)."@en ;
                         rdfs:label "flow resistance range"@en .


###  https://saref.etsi.org/saref4bldg/flowResistanceMin
s4bldg:flowResistanceMin rdf:type owl:ObjectProperty ;
                         rdfs:comment "Allowable range of frictional resistance against which the fluid is being pumped. Usually measured in Pascals (Pa, N/m2)."@en ;
                         rdfs:label "flow resistance range"@en .


###  https://saref.etsi.org/saref4bldg/fluidFlowRateMax
s4bldg:fluidFlowRateMax rdf:type owl:ObjectProperty ;
                        rdfs:comment "Possible range of fluid flowrate that can be delivered. Usually measured in m3/s."@en ;
                        rdfs:label "fluid flow rate range"@en .


###  https://saref.etsi.org/saref4bldg/fluidFlowRateMin
s4bldg:fluidFlowRateMin rdf:type owl:ObjectProperty ;
                        rdfs:comment "Possible range of fluid flowrate that can be delivered. Usually measured in m3/s."@en ;
                        rdfs:label "fluid flow rate range"@en .


###  https://saref.etsi.org/saref4bldg/foulingFactor
s4bldg:foulingFactor rdf:type owl:ObjectProperty ;
                     rdfs:comment "Fouling factor of the tubes in the tube bundle. Usually measured in m2 Kelvin/Watt."@en ;
                     rdfs:label "fouling factor"@en .


###  https://saref.etsi.org/saref4bldg/frameDepth
s4bldg:frameDepth rdf:type owl:ObjectProperty ;
                  rdfs:comment "The length (or depth) of the damper frame. Usually measured in millimeters (mm)."@en ;
                  rdfs:label "frame depth"@en .


###  https://saref.etsi.org/saref4bldg/frameThickness
s4bldg:frameThickness rdf:type owl:ObjectProperty ;
                      rdfs:comment "The thickness of the damper frame material. Usually measured in millimeters (mm)."@en ;
                      rdfs:label "frame thickness"@en .


###  https://saref.etsi.org/saref4bldg/hasSpace
s4bldg:hasSpace rdf:type owl:ObjectProperty ;
                owl:inverseOf s4bldg:isSpaceOf ;
                rdf:type owl:TransitiveProperty ;
                rdfs:comment "Relation between a building or a building space and the spaces it can be divided into."@en ;
                rdfs:label "has space"@en .


###  https://saref.etsi.org/saref4bldg/heatExchangeArea
s4bldg:heatExchangeArea rdf:type owl:ObjectProperty ;
                        rdfs:comment "Heat exchange area. Usually measured in square metre (m2)."@en ;
                        rdfs:label "heat exchange area"@en .


###  https://saref.etsi.org/saref4bldg/heatTransferSurfaceArea
s4bldg:heatTransferSurfaceArea rdf:type owl:ObjectProperty ;
                               rdfs:comment "Total heat transfer area of the vessel. Usually measured in square metre (m2)."@en ;
                               rdfs:label "heat transfer surface area"@en .


###  https://saref.etsi.org/saref4bldg/height
s4bldg:height rdf:type owl:ObjectProperty ;
              rdfs:comment "Height of the vibration isolator before tha application of load. Usually measured in millimeters (mm)."@en ;
              rdfs:label "height"@en .


###  https://saref.etsi.org/saref4bldg/horizontalSpacing
s4bldg:horizontalSpacing rdf:type owl:ObjectProperty ;
                         rdfs:comment "Horizontal spacing between tubes in the tube bundle. Usually measured in millimeters (mm)."@en ;
                         rdfs:label "horizontal spacing"@en .


###  https://saref.etsi.org/saref4bldg/hydraulicDiameter
s4bldg:hydraulicDiameter rdf:type owl:ObjectProperty ;
                         rdfs:comment "Hydraulic diameter. Usually measured in millimeters (mm)."@en ;
                         rdfs:label "hydraulic diameter"@en .


###  https://saref.etsi.org/saref4bldg/idealCapacity
s4bldg:idealCapacity rdf:type owl:ObjectProperty ;
                     rdfs:comment "Compressor capacity under ideal conditions. Usually measured in Watts (W, J/s)."@en ;
                     rdfs:label "ideal capacity"@en .


###  https://saref.etsi.org/saref4bldg/idealShaftPower
s4bldg:idealShaftPower rdf:type owl:ObjectProperty ;
                       rdfs:comment "Compressor shaft power under ideal conditions. Usually measured in Watts (W, J/s)."@en ;
                       rdfs:label "ideal shaft power"@en .


###  https://saref.etsi.org/saref4bldg/imaginaryImpedanceRatio
s4bldg:imaginaryImpedanceRatio rdf:type owl:ObjectProperty ;
                               rdfs:comment "The ratio between the imaginary part of the zero sequence impedance and the imaginary part of the positive impedance (i.e. imaginary part of the short-circuit voltage) of the transformer. Used for three-phase transformer which includes a N-conductor."@en ;
                               rdfs:label "imaginary impedance ratio"@en .


###  https://saref.etsi.org/saref4bldg/impellerDiameter
s4bldg:impellerDiameter rdf:type owl:ObjectProperty ;
                        rdfs:comment "Diameter of compressor impeller - used to scale performance of geometrically similar compressors. Usually measured in millimeters (mm)."@en ;
                        rdfs:label "impeller diameter"@en .


###  https://saref.etsi.org/saref4bldg/inLineRowSpacing
s4bldg:inLineRowSpacing rdf:type owl:ObjectProperty ;
                        rdfs:comment "In-line tube row spacing. Usually measured in millimeters (mm)."@en ;
                        rdfs:label "in line row spacing"@en .


###  https://saref.etsi.org/saref4bldg/initialResistance
s4bldg:initialResistance rdf:type owl:ObjectProperty ;
                         rdfs:comment "Initial new filter fluid resistance (i.e., pressure drop at the maximum air flowrate across the filter when the filter is new per ASHRAE Standard 52.1). Usually measured in Pascals (Pa, N/m2)."@en ;
                         rdfs:label "initial resistance"@en .


###  https://saref.etsi.org/saref4bldg/inletConnectionSize
s4bldg:inletConnectionSize rdf:type owl:ObjectProperty ;
                           rdfs:comment "Size of the inlet connection. Usually measured in millimeters (mm)."@en ;
                           rdfs:label "inlet connection size"@en .


###  https://saref.etsi.org/saref4bldg/insideDiameter
s4bldg:insideDiameter rdf:type owl:ObjectProperty ;
                      rdfs:comment "Actual inner diameter of the tube in the tube bundle. Usually measured in millimeters (mm)."@en ;
                      rdfs:label "inside diameter"@en .


###  https://saref.etsi.org/saref4bldg/internalRefrigerantVolume
s4bldg:internalRefrigerantVolume rdf:type owl:ObjectProperty ;
                                 rdfs:comment "Internal volume of evaporator (refrigerant side). Usually measured in cubic metre (m3)."@en ;
                                 rdfs:label "internal refrigerant volume"@en .


###  https://saref.etsi.org/saref4bldg/internalSurfaceArea
s4bldg:internalSurfaceArea rdf:type owl:ObjectProperty ;
                           rdfs:comment "Internal surface area. Usually measured in square metre (m2)."@en ;
                           rdfs:label "internal surface area"@en .


###  https://saref.etsi.org/saref4bldg/internalWaterVolume
s4bldg:internalWaterVolume rdf:type owl:ObjectProperty ;
                           rdfs:comment "Internal volume of evaporator (water side). Usually measured in cubic metre (m3)."@en ;
                           rdfs:label "internal water volume"@en .


###  https://saref.etsi.org/saref4bldg/isContainedIn
s4bldg:isContainedIn rdf:type owl:ObjectProperty ,
                              owl:TransitiveProperty ;
                     rdfs:comment "A relation between an object and the physical space in which it is located."@en ;
                     rdfs:label "is contained in"@en .


###  https://saref.etsi.org/saref4bldg/isSpaceOf
s4bldg:isSpaceOf rdf:type owl:ObjectProperty ,
                          owl:TransitiveProperty ;
                 rdfs:comment "Relation between a building space and the building or building space it belongs to."@en ;
                 rdfs:label "isSpaceOf"@en .


###  https://saref.etsi.org/saref4bldg/isolatorCompressibility
s4bldg:isolatorCompressibility rdf:type owl:ObjectProperty ;
                               rdfs:comment "The compressibility of the vibration isolator."@en ;
                               rdfs:label "isolator compressibility"@en .


###  https://saref.etsi.org/saref4bldg/isolatorStaticDeflection
s4bldg:isolatorStaticDeflection rdf:type owl:ObjectProperty ;
                                rdfs:comment "Static deflection of the vibration isolator. Usually measured in millimeters (mm)."@en ;
                                rdfs:label "isolator static deflection"@en .


###  https://saref.etsi.org/saref4bldg/lampMaintenanceFactor
s4bldg:lampMaintenanceFactor rdf:type owl:ObjectProperty ;
                             rdfs:comment "Non recoverable losses of luminous flux of a lamp due to lamp depreciation i.e. the decreasing of light output of a luminaire due to aging and dirt."@en ;
                             rdfs:label "lamp maintenance factor"@en .


###  https://saref.etsi.org/saref4bldg/leakageFullyClosed
s4bldg:leakageFullyClosed rdf:type owl:ObjectProperty ;
                          rdfs:comment "Leakage when fully closed. Usually measured in m3/s."@en ;
                          rdfs:label "leakage fully closed"@en .


###  https://saref.etsi.org/saref4bldg/length
s4bldg:length rdf:type owl:ObjectProperty ;
              rdfs:comment "The finished length of the device. Usually measured in millimeters (mm)."@en ;
              rdfs:label "length"@en .


###  https://saref.etsi.org/saref4bldg/liftElevationDifference
s4bldg:liftElevationDifference rdf:type owl:ObjectProperty ;
                               rdfs:comment "Elevation difference between cooling tower sump and the top of the tower. Usually measured in millimeters (mm)."@en ;
                               rdfs:label "lift elevation difference"@en .


###  https://saref.etsi.org/saref4bldg/lightEmitterNominalPower
s4bldg:lightEmitterNominalPower rdf:type owl:ObjectProperty ;
                                rdfs:comment "Light emitter nominal power. Usually measured in Watts (W, J/s)."@en ;
                                rdfs:label "light emitter nominal power"@en .


###  https://saref.etsi.org/saref4bldg/limitingTerminalSize
s4bldg:limitingTerminalSize rdf:type owl:ObjectProperty ;
                            rdfs:comment "The maximum terminal size capacity of the device. Usually measured in square metre (m2)."@en ;
                            rdfs:label "limiting terminal size"@en .


###  https://saref.etsi.org/saref4bldg/lockedRotorCurrent
s4bldg:lockedRotorCurrent rdf:type owl:ObjectProperty ;
                          rdfs:comment "Input current when a motor armature is energized but not rotating. Usually measured in Ampere (A)."@en ;
                          rdfs:label "locked rotor current"@en .


###  https://saref.etsi.org/saref4bldg/netPositiveSuctionHead
s4bldg:netPositiveSuctionHead rdf:type owl:ObjectProperty ;
                              rdfs:comment "Minimum liquid pressure at the pump inlet to prevent cavitation. Usually measured in Pascals (Pa, N/m2)."@en ;
                              rdfs:label "net positive suction head"@en .


###  https://saref.etsi.org/saref4bldg/nominalAirFlowRate
s4bldg:nominalAirFlowRate rdf:type owl:ObjectProperty ;
                          rdfs:comment "Nominal rate of air flow. Usually measured in m3/s."@en ;
                          rdfs:label "nominal air flow rate"@en .


###  https://saref.etsi.org/saref4bldg/nominalBodyDepth
s4bldg:nominalBodyDepth rdf:type owl:ObjectProperty ;
                        rdfs:comment "Nominal or quoted =length, measured along the z-axis of the local coordinate system of the object, of the body of the object. Usually measured in millimeters (mm)."@en ;
                        rdfs:label "nominal body depth"@en .


###  https://saref.etsi.org/saref4bldg/nominalBodyLength
s4bldg:nominalBodyLength rdf:type owl:ObjectProperty ;
                         rdfs:comment "Nominal or quoted length, measured along the x-axis of the local coordinate system of the object, of the body of the object. Usually measured in millimeters (mm)."@en ;
                         rdfs:label "nominal body length"@en .


###  https://saref.etsi.org/saref4bldg/nominalBodyWidth
s4bldg:nominalBodyWidth rdf:type owl:ObjectProperty ;
                        rdfs:comment "Nominal or quoted length, measured along the y-axis of the local coordinate system of the object, of the body of the object. Usually measured in millimeters (mm)."@en ;
                        rdfs:label "nominal body width"@en .


###  https://saref.etsi.org/saref4bldg/nominalCapacity
s4bldg:nominalCapacity rdf:type owl:ObjectProperty ;
                       rdfs:comment "Nominal capacity. Usually measured in Watts (W, J/s)."@en ;
                       rdfs:label "nominal capacity"@en .


###  https://saref.etsi.org/saref4bldg/nominalCondensingTemperature
s4bldg:nominalCondensingTemperature rdf:type owl:ObjectProperty ;
                                    rdfs:comment "Chiller condensing temperature. Usually measured in degrees Kelvin (K)."@en ;
                                    rdfs:label "nominal condensing temperature"@en .


###  https://saref.etsi.org/saref4bldg/nominalCoolingCapacity
s4bldg:nominalCoolingCapacity rdf:type owl:ObjectProperty ;
                              rdfs:comment "Nominal cooling capacity. Usually measured in Watts (W, J/s)."@en ;
                              rdfs:label "nominal cooling capacity"@en .


###  https://saref.etsi.org/saref4bldg/nominalDepth
s4bldg:nominalDepth rdf:type owl:ObjectProperty ;
                    rdfs:comment "The nominal depth of the tank. Note: Not required for a horizontal cylindrical tank. Usually measured in millimeters (mm)."@en ;
                    rdfs:label "nominal depth"@en .


###  https://saref.etsi.org/saref4bldg/nominalDiameter
s4bldg:nominalDiameter rdf:type owl:ObjectProperty ;
                       rdfs:comment "Nominal diameter or width of the tubes in the tube bundle. Usually measured in millimeters (mm)."@en ;
                       rdfs:label "nominal diameter"@en .


###  https://saref.etsi.org/saref4bldg/nominalEfficiency
s4bldg:nominalEfficiency rdf:type owl:ObjectProperty ;
                         rdfs:comment "Nominal chiller efficiency under nominal conditions. "@en ;
                         rdfs:label "nominal efficiency"@en .


###  https://saref.etsi.org/saref4bldg/nominalEnergyConsumption
s4bldg:nominalEnergyConsumption rdf:type owl:ObjectProperty ;
                                rdfs:comment "Nominal fuel consumption rate required to produce the total boiler heat output. Usually measured in Watts (W, J/s)."@en ;
                                rdfs:label "nominal energy consumption"@en .


###  https://saref.etsi.org/saref4bldg/nominalEvaporatingTemmperature
s4bldg:nominalEvaporatingTemmperature rdf:type owl:ObjectProperty ;
                                      rdfs:comment "Chiller evaporating temperature.Usually measured in degrees Kelvin (K)."@en ;
                                      rdfs:label "nominal evaporating temmperature"@en .


###  https://saref.etsi.org/saref4bldg/nominalFilterFaceVelocity
s4bldg:nominalFilterFaceVelocity rdf:type owl:ObjectProperty ;
                                 rdfs:comment "Filter face velocity. Usually measured in m/s."@en ;
                                 rdfs:label "nominal filter face velocity"@en .


###  https://saref.etsi.org/saref4bldg/nominalFlowRate
s4bldg:nominalFlowRate rdf:type owl:ObjectProperty ;
                       rdfs:comment "Nominal fluid flow rate through the filter. Usually measured in m3/s."@en ;
                       rdfs:label "nominal flow rate"@en .


###  https://saref.etsi.org/saref4bldg/nominalFrequency
s4bldg:nominalFrequency rdf:type owl:ObjectProperty ;
                        rdfs:comment "The nominal frequency of the supply. Usually measured in cycles/s or Hertz (Hz)."@en ;
                        rdfs:label "nominal frequency"@en .


###  https://saref.etsi.org/saref4bldg/nominalHeatRejectionRate
s4bldg:nominalHeatRejectionRate rdf:type owl:ObjectProperty ;
                                rdfs:comment "Sum of the refrigeration effect and the heat equivalent of the power input to the compressor. Usually measured in Watts (W, J/s)."@en ;
                                rdfs:label "nominal heat rejection rate"@en .


###  https://saref.etsi.org/saref4bldg/nominalHeatTransferArea
s4bldg:nominalHeatTransferArea rdf:type owl:ObjectProperty ;
                               rdfs:comment "Nominal heat transfer surface area associated with nominal overall heat transfer coefficient. Usually measured in square metre (m2)."@en ;
                               rdfs:label "nominal heat transfer area"@en .


###  https://saref.etsi.org/saref4bldg/nominalHeatTransferCoefficient
s4bldg:nominalHeatTransferCoefficient rdf:type owl:ObjectProperty ;
                                      rdfs:comment "Nominal overall heat transfer coefficient associated with nominal heat transfer area. Usually measured in Watts/m2 Kelvin."@en ;
                                      rdfs:label "nominal heat transfer coefficient"@en .


###  https://saref.etsi.org/saref4bldg/nominalHeatingCapacity
s4bldg:nominalHeatingCapacity rdf:type owl:ObjectProperty ;
                              rdfs:comment "Nominal heating capacity. Usually measured in Watts (W, J/s)."@en ;
                              rdfs:label "nominal heating capacity"@en .


###  https://saref.etsi.org/saref4bldg/nominalLatentCapacity
s4bldg:nominalLatentCapacity rdf:type owl:ObjectProperty ;
                             rdfs:comment "Nominal latent capacity. Usually measured in Watts (W, J/s)."@en ;
                             rdfs:label "nominal latent capacity"@en .


###  https://saref.etsi.org/saref4bldg/nominalLengthOrDiameter
s4bldg:nominalLengthOrDiameter rdf:type owl:ObjectProperty ;
                               rdfs:comment "The nominal length or, in the case of a vertical cylindrical tank, the nominal diameter of the tank. Usually measured in millimeters (mm)."@en ;
                               rdfs:label "nominal length or diameter"@en .


###  https://saref.etsi.org/saref4bldg/nominalMediaSurfaceVelocity
s4bldg:nominalMediaSurfaceVelocity rdf:type owl:ObjectProperty ;
                                   rdfs:comment "Average fluid velocity at the media surface. Usually measured in m/s."@en ;
                                   rdfs:label "nominal media surface velocity"@en .


###  https://saref.etsi.org/saref4bldg/nominalMoistureGain
s4bldg:nominalMoistureGain rdf:type owl:ObjectProperty ;
                           rdfs:comment "Nominal rate of water vapor added into the airstream. Usually measured in kg/s."@en ;
                           rdfs:label "nominal moisture gain"@en .


###  https://saref.etsi.org/saref4bldg/nominalPartLoadRatio
s4bldg:nominalPartLoadRatio rdf:type owl:ObjectProperty ;
                            rdfs:comment "Allowable part load ratio range."@en ;
                            rdfs:label "nominal part load ratio"@en .


###  https://saref.etsi.org/saref4bldg/nominalParticleGeometricMeanDiameter
s4bldg:nominalParticleGeometricMeanDiameter rdf:type owl:ObjectProperty ;
                                            rdfs:comment "Particle geometric mean diameter associated with nominal efficiency. Usually measured in millimeters (mm)."@en ;
                                            rdfs:label "nominal particle geometric mean diameter"@en .


###  https://saref.etsi.org/saref4bldg/nominalParticleGeometricStandardDeviation
s4bldg:nominalParticleGeometricStandardDeviation rdf:type owl:ObjectProperty ;
                                                 rdfs:comment "Particle geometric standard deviation associated with nominal efficiency. "@en ;
                                                 rdfs:label "nominal particle geometric standard deviation"@en .


###  https://saref.etsi.org/saref4bldg/nominalPowerConsumption
s4bldg:nominalPowerConsumption rdf:type owl:ObjectProperty ;
                               rdfs:comment "Nominal total power consumption. Usually measured in Watts (W, J/s)."@en ;
                               rdfs:label "nominal power consumption"@en .


###  https://saref.etsi.org/saref4bldg/nominalPowerRate
s4bldg:nominalPowerRate rdf:type owl:ObjectProperty ;
                        rdfs:comment "Nominal fan power rate.Usually measured in Watts (W, J/s)."@en ;
                        rdfs:label "nominal power rate"@en .


###  https://saref.etsi.org/saref4bldg/nominalPressureDrop
s4bldg:nominalPressureDrop rdf:type owl:ObjectProperty ;
                           rdfs:comment "Total pressure drop across the filter. Usually measured in Pascals (Pa, N/m2)."@en ;
                           rdfs:label "nominal pressure drop"@en .


###  https://saref.etsi.org/saref4bldg/nominalReturnWaterTemperatureCooling
s4bldg:nominalReturnWaterTemperatureCooling rdf:type owl:ObjectProperty ;
                                            rdfs:comment "Nominal return water temperature (refers to nominal cooling capacity). Usually measured in degrees Kelvin (K)."@en ;
                                            rdfs:label "nominal return water temperature cooling"@en .


###  https://saref.etsi.org/saref4bldg/nominalReturnWaterTemperatureHeating
s4bldg:nominalReturnWaterTemperatureHeating rdf:type owl:ObjectProperty ;
                                            rdfs:comment "Nominal return water temperature (refers to nominal heating capacity). Usually measured in degrees Kelvin (K)."@en ;
                                            rdfs:label "nominal return water temperature heating"@en .


###  https://saref.etsi.org/saref4bldg/nominalRotationSpeed
s4bldg:nominalRotationSpeed rdf:type owl:ObjectProperty ;
                            rdfs:comment "Nominal fan wheel speed. Usually measured in cycles/s."@en ;
                            rdfs:label "nominal rotation speed"@en .


###  https://saref.etsi.org/saref4bldg/nominalSensibleCapacity
s4bldg:nominalSensibleCapacity rdf:type owl:ObjectProperty ;
                               rdfs:comment "Nominal sensible capacity. Usually measured in Watts (W, J/s)."@en ;
                               rdfs:label "nominal sensible capacity"@en .


###  https://saref.etsi.org/saref4bldg/nominalSorroundingHumidityCooling
s4bldg:nominalSorroundingHumidityCooling rdf:type owl:ObjectProperty ;
                                         rdfs:comment "Nominal surrounding humidity (refers to nominal cooling capacity). Usually measured in degrees Kelvin (K)."@en ;
                                         rdfs:label "nominal sorrounding humidity cooling"@en .


###  https://saref.etsi.org/saref4bldg/nominalSorroundingTemperatureCooling
s4bldg:nominalSorroundingTemperatureCooling rdf:type owl:ObjectProperty ;
                                            rdfs:comment "Nominal surrounding temperature (refers to nominal cooling capacity). Usually measured in degrees Kelvin (K)."@en ;
                                            rdfs:label "nominal sorrounding temperature cooling"@en .


###  https://saref.etsi.org/saref4bldg/nominalSorroundingTemperatureHeating
s4bldg:nominalSorroundingTemperatureHeating rdf:type owl:ObjectProperty ;
                                            rdfs:comment "Nominal surrounding temperature (refers to nominal heating capacity). Usually measured in degrees Kelvin (K)."@en ;
                                            rdfs:label "nominal sorrounding temperature heating"@en .


###  https://saref.etsi.org/saref4bldg/nominalStaticPressure
s4bldg:nominalStaticPressure rdf:type owl:ObjectProperty ;
                             rdfs:comment "The static pressure within the air stream that the fan must overcome to insure designed circulation of air. Usually measured in Pascals (Pa, N/m2)."@en ;
                             rdfs:label "nominal static pressure"@en .


###  https://saref.etsi.org/saref4bldg/nominalSupplyVoltage
s4bldg:nominalSupplyVoltage rdf:type owl:ObjectProperty ;
                            rdfs:comment "The nominal voltage of the supply. Usually measured in Volts (V, W/A)."@en ;
                            rdfs:label "nominal supply voltage"@en .


###  https://saref.etsi.org/saref4bldg/nominalSupplyVoltageMax
s4bldg:nominalSupplyVoltageMax rdf:type owl:ObjectProperty ;
                               rdfs:comment "The maximum and minimum allowed voltage of the supply e.g. boundaries of 380V/440V may be applied for a nominal voltage of 400V."@en ;
                               rdfs:label "nominal supply voltage offset"@en .


###  https://saref.etsi.org/saref4bldg/nominalSupplyVoltageMin
s4bldg:nominalSupplyVoltageMin rdf:type owl:ObjectProperty ;
                               rdfs:comment "The maximum and minimum allowed voltage of the supply e.g. boundaries of 380V/440V may be applied for a nominal voltage of 400V."@en ;
                               rdfs:label "nominal supply voltage offset"@en .


###  https://saref.etsi.org/saref4bldg/nominalSupplyWaterTemperatureCooling
s4bldg:nominalSupplyWaterTemperatureCooling rdf:type owl:ObjectProperty ;
                                            rdfs:comment "Nominal supply water temperature (refers to nominal cooling capacity). Usually measured in degrees Kelvin (K)."@en ;
                                            rdfs:label "nominal supply water temperature cooling"@en .


###  https://saref.etsi.org/saref4bldg/nominalSupplyWaterTemperatureHeating
s4bldg:nominalSupplyWaterTemperatureHeating rdf:type owl:ObjectProperty ;
                                            rdfs:comment "Nominal supply water temperature (refers to nominal heating capacity). Usually measured in degrees Kelvin (K)."@en ;
                                            rdfs:label "nominal supply water temperature heating"@en .


###  https://saref.etsi.org/saref4bldg/nominalTotalPressure
s4bldg:nominalTotalPressure rdf:type owl:ObjectProperty ;
                            rdfs:comment "Nominal total pressure rise across the fan. Usually measured in Pascals (Pa, N/m2)."@en ;
                            rdfs:label "nominal total pressure"@en .


###  https://saref.etsi.org/saref4bldg/nominalUa
s4bldg:nominalUa rdf:type owl:ObjectProperty ;
                 rdfs:comment "Nominal UA value."@en ;
                 rdfs:label "nominal ua"@en .


###  https://saref.etsi.org/saref4bldg/nominalVolumetricCapacity
s4bldg:nominalVolumetricCapacity rdf:type owl:ObjectProperty ;
                                 rdfs:comment "The total nominal or design volumetric capacity of the tank. Usually measured in cubic metre (m3)."@en ;
                                 rdfs:label "nominal volumetric capacity"@en .


###  https://saref.etsi.org/saref4bldg/nominalWaterFlowCooling
s4bldg:nominalWaterFlowCooling rdf:type owl:ObjectProperty ;
                               rdfs:comment "Nominal water flow (refers to nominal cooling capacity). Usually measured in m3/s."@en ;
                               rdfs:label "nominal water flow cooling"@en .


###  https://saref.etsi.org/saref4bldg/nominalWaterFlowHeating
s4bldg:nominalWaterFlowHeating rdf:type owl:ObjectProperty ;
                               rdfs:comment "Nominal water flow (refers to nominal heating capacity). Usually measured in m3/s."@en ;
                               rdfs:label "nominal water flow heating"@en .


###  https://saref.etsi.org/saref4bldg/nominalWidthOrDiameter
s4bldg:nominalWidthOrDiameter rdf:type owl:ObjectProperty ;
                              rdfs:comment "The nominal width or, in the case of a horizontal cylindrical tank, the nominal diameter of the tank. Note: Not required for a vertical cylindrical tank. Usually measured in millimeters (mm)."@en ;
                              rdfs:label "nominal width or diameter"@en .


###  https://saref.etsi.org/saref4bldg/nomminalRotationSpeed
s4bldg:nomminalRotationSpeed rdf:type owl:ObjectProperty ;
                             rdfs:comment "Pump rotational speed under nominal conditions. Usually measured in cycles/s."@en ;
                             rdfs:label "nomminal rotation speed"@en .


###  https://saref.etsi.org/saref4bldg/openPressureDrop
s4bldg:openPressureDrop rdf:type owl:ObjectProperty ;
                        rdfs:comment "Total pressure drop across damper. Usually measured in Pascals (Pa, N/m2)."@en ;
                        rdfs:label "open pressure drop"@en .


###  https://saref.etsi.org/saref4bldg/operatingWeight
s4bldg:operatingWeight rdf:type owl:ObjectProperty ;
                       rdfs:comment "Operating weight of the tank including all of its contents. Usually measured in kilograms (kg) or grams (g)."@en ;
                       rdfs:label "operating weight"@en .


###  https://saref.etsi.org/saref4bldg/operationTemperatureMax
s4bldg:operationTemperatureMax rdf:type owl:ObjectProperty ;
                               rdfs:comment "Allowable operation ambient (air, fluid) temperature range. Usually measured in degrees Kelvin (K)."@en ;
                               rdfs:label "operation temperature range"@en .


###  https://saref.etsi.org/saref4bldg/operationTemperatureMin
s4bldg:operationTemperatureMin rdf:type owl:ObjectProperty ;
                               rdfs:comment "Allowable operation ambient (air, fluid) temperature range. Usually measured in degrees Kelvin (K)."@en ;
                               rdfs:label "operation temperature range"@en .


###  https://saref.etsi.org/saref4bldg/operationalRiterial
s4bldg:operationalRiterial rdf:type owl:ObjectProperty ;
                           rdfs:comment "Time of operation at maximum operational ambient air temperature. Measured in seconds (s) or days (d) or other units of time."@en ;
                           rdfs:label "operational riterial"@en .


###  https://saref.etsi.org/saref4bldg/outletConnectionSize
s4bldg:outletConnectionSize rdf:type owl:ObjectProperty ;
                            rdfs:comment "Size of the outlet connection. Usually measured in millimeters (mm)."@en ;
                            rdfs:label "outlet connection size"@en .


###  https://saref.etsi.org/saref4bldg/outletTemperatureMax
s4bldg:outletTemperatureMax rdf:type owl:ObjectProperty ;
                            rdfs:comment "Allowable outlet temperature of either the water or the steam. Usually measured in degrees Kelvin (K)."@en ;
                            rdfs:label "outlet temperature range"@en .


###  https://saref.etsi.org/saref4bldg/outletTemperatureMin
s4bldg:outletTemperatureMin rdf:type owl:ObjectProperty ;
                            rdfs:comment "Allowable outlet temperature of either the water or the steam. Usually measured in degrees Kelvin (K)."@en ;
                            rdfs:label "outlet temperature range"@en .


###  https://saref.etsi.org/saref4bldg/outputCapacity
s4bldg:outputCapacity rdf:type owl:ObjectProperty ;
                      rdfs:comment "Total nominal heat output as listed by the manufacturer. Usually measured in Watts (W, J/s)."@en ;
                      rdfs:label "output capacity"@en .


###  https://saref.etsi.org/saref4bldg/outsideDiameter
s4bldg:outsideDiameter rdf:type owl:ObjectProperty ;
                       rdfs:comment "Actual outside diameter of the tube in the tube bundle. Usually measured in millimeters (mm)."@en ;
                       rdfs:label "outside diameter"@en .


###  https://saref.etsi.org/saref4bldg/partLoadRatioMax
s4bldg:partLoadRatioMax rdf:type owl:ObjectProperty ;
                        rdfs:comment "Maximum part load ratio as a fraction of nominal capacity."@en ;
                        rdfs:label "maximum part load ratio"@en .


###  https://saref.etsi.org/saref4bldg/partLoadRatioMin
s4bldg:partLoadRatioMin rdf:type owl:ObjectProperty ;
                        rdfs:comment "Minimum part load ratio as a fraction of nominal capacity."@en ;
                        rdfs:label "minimum part load ratio"@en .


###  https://saref.etsi.org/saref4bldg/powerOutputMax
s4bldg:powerOutputMax rdf:type owl:ObjectProperty ;
                      rdfs:comment "The maximum output power rating of the engine. Usually measured in Watts (W, J/s)."@en ;
                      rdfs:label "maximum power output"@en .


###  https://saref.etsi.org/saref4bldg/pressureRating
s4bldg:pressureRating rdf:type owl:ObjectProperty ;
                      rdfs:comment "Nominal pressure rating of the boiler as rated by the agency having jurisdiction. Usually measured in Pascals (Pa, N/m2)."@en ;
                      rdfs:label "pressure rating"@en .


###  https://saref.etsi.org/saref4bldg/primaryAirFlowRateMax
s4bldg:primaryAirFlowRateMax rdf:type owl:ObjectProperty ;
                             rdfs:comment "Maximum primary airflow that can be delivered. Usually measured in m3/s."@en ;
                             rdfs:label "primary air flow rate range"@en .


###  https://saref.etsi.org/saref4bldg/primaryAirFlowRateMin
s4bldg:primaryAirFlowRateMin rdf:type owl:ObjectProperty ;
                             rdfs:comment "Minimum primary airflow that can be delivered. Usually measured in m3/s."@en ;
                             rdfs:label "primary air flow rate range"@en .


###  https://saref.etsi.org/saref4bldg/primaryApparentPower
s4bldg:primaryApparentPower rdf:type owl:ObjectProperty ;
                            rdfs:comment "The power in VA (volt ampere) that has been transformed and that runs into the transformer on the primary side. Usually measured in Watts (W, J/s)."@en ;
                            rdfs:label "primary apparent power"@en .


###  https://saref.etsi.org/saref4bldg/primaryCurrent
s4bldg:primaryCurrent rdf:type owl:ObjectProperty ;
                      rdfs:comment "The current that is going to be transformed and that runs into the transformer on the primary side. Usually measured in Ampere (A)."@en ;
                      rdfs:label "primary current"@en .


###  https://saref.etsi.org/saref4bldg/primaryFrequency
s4bldg:primaryFrequency rdf:type owl:ObjectProperty ;
                        rdfs:comment "The frequency that is going to be transformed and that runs into the transformer on the primary side. Usually measured in cycles/s or Hertz (Hz)."@en ;
                        rdfs:label "primary frequency"@en .


###  https://saref.etsi.org/saref4bldg/primaryVoltage
s4bldg:primaryVoltage rdf:type owl:ObjectProperty ;
                      rdfs:comment "The voltage that is going to be transformed and that runs into the transformer on the primary side. Usually measured in Volts (V, W/A)."@en ;
                      rdfs:label "primary voltage"@en .


###  https://saref.etsi.org/saref4bldg/pumpFlowRateMax
s4bldg:pumpFlowRateMax rdf:type owl:ObjectProperty ;
                       rdfs:comment "Allowable range of volume of fluid being pumped against the resistance specified. Usually measured in kg/s."@en ;
                       rdfs:label "pump flow rate range"@en .


###  https://saref.etsi.org/saref4bldg/pumpFlowRateMin
s4bldg:pumpFlowRateMin rdf:type owl:ObjectProperty ;
                       rdfs:comment "Allowable range of volume of fluid being pumped against the resistance specified. Usually measured in kg/s."@en ;
                       rdfs:label "pump flow rate range"@en .


###  https://saref.etsi.org/saref4bldg/realImpedanceRatio
s4bldg:realImpedanceRatio rdf:type owl:ObjectProperty ;
                          rdfs:comment "The ratio between the real part of the zero sequence impedance and the real part of the positive impedance (i.e. real part of the short-circuit voltage) of the transformer. Used for three-phase transformer which includes a N-conductor."@en ;
                          rdfs:label "real impedance ratio"@en .


###  https://saref.etsi.org/saref4bldg/secondCurvatureRadius
s4bldg:secondCurvatureRadius rdf:type owl:ObjectProperty ;
                             rdfs:comment "SecondCurvatureRadius should be defined as the top or right side radius of curvature value. Usually measured in millimeters (mm)."@en ;
                             rdfs:label "second curvature radius"@en .


###  https://saref.etsi.org/saref4bldg/secondaryAirFlowRateMax
s4bldg:secondaryAirFlowRateMax rdf:type owl:ObjectProperty ;
                               rdfs:comment "Maximum secondary airflow that can be delivered. Usually measured in Pascals (Pa, N/m2)."@en ;
                               rdfs:label "secondary air flow rate range"@en .


###  https://saref.etsi.org/saref4bldg/secondaryAirFlowRateMin
s4bldg:secondaryAirFlowRateMin rdf:type owl:ObjectProperty ;
                               rdfs:comment "Maximum secondary airflow that can be delivered. Usually measured in Pascals (Pa, N/m2)."@en ;
                               rdfs:label "secondary air flow rate range"@en .


###  https://saref.etsi.org/saref4bldg/secondaryApparentPower
s4bldg:secondaryApparentPower rdf:type owl:ObjectProperty ;
                              rdfs:comment "The power in VA (volt ampere) that has been transformed and is running out of the transformer on the secondary side. Usually measured in Watts (W, J/s)."@en ;
                              rdfs:label "secondary apparent power"@en .


###  https://saref.etsi.org/saref4bldg/secondaryCurrent
s4bldg:secondaryCurrent rdf:type owl:ObjectProperty ;
                        rdfs:comment "The current that has been transformed and is running out of the transformer on the secondary side. Usually measured in Ampere (A)."@en ;
                        rdfs:label "secondary current"@en .


###  https://saref.etsi.org/saref4bldg/secondaryFrequency
s4bldg:secondaryFrequency rdf:type owl:ObjectProperty ;
                          rdfs:comment "The frequency that has been transformed and is running out of the transformer on the secondary side. Usually measured in cycles/s or Hertz (Hz)."@en ;
                          rdfs:label "secondary frequency"@en .


###  https://saref.etsi.org/saref4bldg/secondaryVoltage
s4bldg:secondaryVoltage rdf:type owl:ObjectProperty ;
                        rdfs:comment "The voltage that has been transformed and is running out of the transformer on the secondary side. Usually measured in Volts (V, W/A)."@en ;
                        rdfs:label "secondary voltage"@en .


###  https://saref.etsi.org/saref4bldg/shortCircuitVoltage
s4bldg:shortCircuitVoltage rdf:type owl:ObjectProperty ;
                           rdfs:comment "A complex number that specifies the real and imaginary parts of the short-circuit voltage at rated current of a transformer given in %."@en ;
                           rdfs:label "short circuit voltage"@en .


###  https://saref.etsi.org/saref4bldg/size
s4bldg:size rdf:type owl:ObjectProperty ;
            rdfs:comment "The size of the connection to the valve (or to each connection for faucets, mixing valves, etc.). Usually measured in millimeters (mm)."@en ;
            rdfs:label "size"@en .


###  https://saref.etsi.org/saref4bldg/solarReflectance
s4bldg:solarReflectance rdf:type owl:ObjectProperty ;
                        rdfs:comment "(Rsol): The ratio of incident solar radiation that is reflected by a shading system (also named _e). Note the following equation Asol + Rsol + Tsol = 1"@en ;
                        rdfs:label "solar reflectance"@en .


###  https://saref.etsi.org/saref4bldg/solarTransmittance
s4bldg:solarTransmittance rdf:type owl:ObjectProperty ;
                          rdfs:comment "(Tsol) The ratio of incident solar radiation that directly passes through a shading system (also named _e). Note the following equation Asol + Rsol + Tsol = 1"@en ;
                          rdfs:label "solar transmittance"@en .


###  https://saref.etsi.org/saref4bldg/spectrumMax
s4bldg:spectrumMax rdf:type owl:ObjectProperty ;
                   rdfs:comment "The spectrum of radiation describes its composition with regard to wavelength. Light, for example, as the portion of electromagnetic radiation that is visible to the human eye, is radiation with wavelengths in the range of approx. 380 to 780 nm (1 nm = 10 m). The corresponding range of colours varies from violet to indigo, blue, green, yellow, orange, and red. These colours form a continuous spectrum, in which the various spectral sectors merge into each other."@en ;
                   rdfs:label "maximum spectrum"@en .


###  https://saref.etsi.org/saref4bldg/spectrumMin
s4bldg:spectrumMin rdf:type owl:ObjectProperty ;
                   rdfs:comment "The spectrum of radiation describes its composition with regard to wavelength. Light, for example, as the portion of electromagnetic radiation that is visible to the human eye, is radiation with wavelengths in the range of approx. 380 to 780 nm (1 nm = 10 m). The corresponding range of colours varies from violet to indigo, blue, green, yellow, orange, and red. These colours form a continuous spectrum, in which the various spectral sectors merge into each other."@en ;
                   rdfs:label "minimum spectrum"@en .


###  https://saref.etsi.org/saref4bldg/staggeredRowSpacing
s4bldg:staggeredRowSpacing rdf:type owl:ObjectProperty ;
                           rdfs:comment "Staggered tube row spacing. Usually measured in millimeters (mm)."@en ;
                           rdfs:label "staggered row spacing"@en .


###  https://saref.etsi.org/saref4bldg/startCurrentFactor
s4bldg:startCurrentFactor rdf:type owl:ObjectProperty ;
                          rdfs:comment "IEC. Start current factor defines how large the peek starting current will become on the engine. StartCurrentFactor is multiplied to NominalCurrent and we get the start current."@en ;
                          rdfs:label "start current factor"@en .


###  https://saref.etsi.org/saref4bldg/startingTime
s4bldg:startingTime rdf:type owl:ObjectProperty ;
                    rdfs:comment "The time (in s) needed for the motor to reach its rated speed with its driven equipment attached, starting from standstill and at the nominal voltage applied at its terminals."@en ;
                    rdfs:label "starting time"@en .


###  https://saref.etsi.org/saref4bldg/supportedWeightMax
s4bldg:supportedWeightMax rdf:type owl:ObjectProperty ;
                          rdfs:comment "The maximum weight that can be carried by the vibration isolator. Usually measured in kilograms (kg) or grams (g)."@en ;
                          rdfs:label "maximum supported weight"@en .


###  https://saref.etsi.org/saref4bldg/teTime
s4bldg:teTime rdf:type owl:ObjectProperty ;
              rdfs:comment "The maximum time (in s) at which the motor could run with locked rotor when the motor is used in an EX-environment. The time indicates that a protective device should trip before this time when the starting current of the motor is slowing through the device."@en ;
              rdfs:label "te time"@en .


###  https://saref.etsi.org/saref4bldg/temperatureRating
s4bldg:temperatureRating rdf:type owl:ObjectProperty ;
                         rdfs:comment "Temperature rating. Usually measured in degrees Kelvin (K)."@en ;
                         rdfs:label "temperature rating"@en .


###  https://saref.etsi.org/saref4bldg/testPressure
s4bldg:testPressure rdf:type owl:ObjectProperty ;
                    rdfs:comment "The maximum pressure to which the valve has been subjected under test. Usually measured in Pascals (Pa, N/m2)."@en ;
                    rdfs:label "test pressure"@en .


###  https://saref.etsi.org/saref4bldg/thermalConductivity
s4bldg:thermalConductivity rdf:type owl:ObjectProperty ;
                           rdfs:comment "Fouling factor of the tubes in the tube bundle. Usually measured in m2 Kelvin/Watt."@en ;
                           rdfs:label "thermal conductivity"@en .


###  https://saref.etsi.org/saref4bldg/thermalEfficiency
s4bldg:thermalEfficiency rdf:type owl:ObjectProperty ;
                         rdfs:comment "Overall Thermal Efficiency is defined as gross energy output of the heat transfer device divided by the energy input."@en ;
                         rdfs:label "thermal efficiency"@en .


###  https://saref.etsi.org/saref4bldg/thermalMassHeatCapacity
s4bldg:thermalMassHeatCapacity rdf:type owl:ObjectProperty ;
                               rdfs:comment "Product of component mass and specific heat."@en ;
                               rdfs:label "thermal mass heat capacity"@en .


###  https://saref.etsi.org/saref4bldg/thermalTransmittance
s4bldg:thermalTransmittance rdf:type owl:ObjectProperty ;
                            rdfs:comment "Rate at which energy is transmitted through a body. Usually measured in Watts/m2 Kelvin."@en ;
                            rdfs:label "thermal transmittance"@en .


###  https://saref.etsi.org/saref4bldg/ventilatingPipeSize
s4bldg:ventilatingPipeSize rdf:type owl:ObjectProperty ;
                           rdfs:comment "Size of the ventilating pipe(s). Usually measured in millimeters (mm)."@en ;
                           rdfs:label "ventilating pipe size"@en .


###  https://saref.etsi.org/saref4bldg/verticalSpacing
s4bldg:verticalSpacing rdf:type owl:ObjectProperty ;
                       rdfs:comment "Vertical spacing between tubes in the tube bundle.Usually measured in millimeters (mm)."@en ;
                       rdfs:label "vertical spacing"@en .


###  https://saref.etsi.org/saref4bldg/vibrationTransmissibility
s4bldg:vibrationTransmissibility rdf:type owl:ObjectProperty ;
                                 rdfs:comment "The vibration transmissibility percentage."@en ;
                                 rdfs:label "vibration transmissibility"@en .


###  https://saref.etsi.org/saref4bldg/visibleLightReflectance
s4bldg:visibleLightReflectance rdf:type owl:ObjectProperty ;
                               rdfs:comment "Fraction of the visible light that is reflected by the glazing at normal incidence. It is a value without unit."@en ;
                               rdfs:label "visible light reflectance"@en .


###  https://saref.etsi.org/saref4bldg/visibleLightTransmittance
s4bldg:visibleLightTransmittance rdf:type owl:ObjectProperty ;
                                 rdfs:comment "Fraction of the visible light that passes the shading system at normal incidence. It is a value without unit."@en ;
                                 rdfs:label "visible light transmittance"@en .


###  https://saref.etsi.org/saref4bldg/volumen
s4bldg:volumen rdf:type owl:ObjectProperty ;
               rdfs:comment "Total volume of fluid in the tubes and their headers. Usually measured in cubic metre (m3)."@en ;
               rdfs:label "volumen"@en .


###  https://saref.etsi.org/saref4bldg/waterInletTemperatureMax
s4bldg:waterInletTemperatureMax rdf:type owl:ObjectProperty ;
                                rdfs:comment "Allowable water inlet temperature range. Usually measured in degrees Kelvin (K)."@en ;
                                rdfs:label "water inlet temperature range"@en .


###  https://saref.etsi.org/saref4bldg/waterInletTemperatureMin
s4bldg:waterInletTemperatureMin rdf:type owl:ObjectProperty ;
                                rdfs:comment "Allowable water inlet temperature range. Usually measured in degrees Kelvin (K)."@en ;
                                rdfs:label "water inlet temperature range"@en .


###  https://saref.etsi.org/saref4bldg/waterPressureMax
s4bldg:waterPressureMax rdf:type owl:ObjectProperty ;
                        rdfs:comment "Allowable water circuit working pressure range. Usually measured in Pascals (Pa, N/m2)."@en ;
                        rdfs:label "water pressure range"@en .


###  https://saref.etsi.org/saref4bldg/waterPressureMin
s4bldg:waterPressureMin rdf:type owl:ObjectProperty ;
                        rdfs:comment "Allowable water circuit working pressure range. Usually measured in Pascals (Pa, N/m2)."@en ;
                        rdfs:label "water pressure range"@en .


###  https://saref.etsi.org/saref4bldg/waterRequirement
s4bldg:waterRequirement rdf:type owl:ObjectProperty ;
                        rdfs:comment "Make-up water requirement. Usually measured in m3/s."@en ;
                        rdfs:label "water requirement"@en .


###  https://saref.etsi.org/saref4bldg/waterStorageCapacity
s4bldg:waterStorageCapacity rdf:type owl:ObjectProperty ;
                            rdfs:comment "Water storage capacity. Usually measured in cubic metre (m3)."@en ;
                            rdfs:label "water storage capacity"@en .


###  https://saref.etsi.org/saref4bldg/weight
s4bldg:weight rdf:type owl:ObjectProperty ;
              rdfs:comment "The weight of the device. Usually measured in kilograms (kg) or grams (g)."@en ;
              rdfs:label "weight"@en .


###  https://saref.etsi.org/saref4bldg/workingPressure
s4bldg:workingPressure rdf:type owl:ObjectProperty ;
                       rdfs:comment "The normally expected maximum working pressure of the valve. Usually measured in Pascals (Pa, N/m2)."@en ;
                       rdfs:label "working pressure"@en .


###  https://saref.etsi.org/saref4bldg/workingPressureMax
s4bldg:workingPressureMax rdf:type owl:ObjectProperty ;
                          rdfs:comment "Maximum working pressure. Usually measured in Pascals (Pa, N/m2)."@en ;
                          rdfs:label "maximum working pressure"@en .


###  https://saref.etsi.org/saref4bldg/workingPressureMin
s4bldg:workingPressureMin rdf:type owl:ObjectProperty ;
                          rdfs:comment "Allowable minimum working pressure (relative to ambient pressure). Usually measured in Pascals (Pa, N/m2)."@en ;
                          rdfs:label "minimum working pressure"@en .


###  https://saref.etsi.org/saref4city/assesses
s4city:assesses rdf:type owl:ObjectProperty ;
                rdfs:isDefinedBy s4city: ;
                rdfs:label "assesses"@en .


###  https://saref.etsi.org/saref4city/hasCalculationPeriod
s4city:hasCalculationPeriod rdf:type owl:ObjectProperty ;
                            rdfs:isDefinedBy s4city: ;
                            rdfs:label "has calculation period"@en .


###  https://saref.etsi.org/saref4city/hasKPI
s4city:hasKPI rdf:type owl:ObjectProperty ;
              owl:inverseOf s4city:isKPIOf ;
              rdfs:isDefinedBy s4city: ;
              rdfs:label "has key performance indicator"@en .


###  https://saref.etsi.org/saref4city/isAssessedBy
s4city:isAssessedBy rdf:type owl:ObjectProperty ;
                    rdfs:isDefinedBy s4city: ;
                    rdfs:label "is assessed by"@en .


###  https://saref.etsi.org/saref4city/isDerivedFrom
s4city:isDerivedFrom rdf:type owl:ObjectProperty ;
                     rdfs:isDefinedBy s4city: ;
                     rdfs:label "is derived from"@en .


###  https://saref.etsi.org/saref4city/isKPIOf
s4city:isKPIOf rdf:type owl:ObjectProperty ;
               rdfs:isDefinedBy s4city: ;
               rdfs:label "is key performance indicator of"@en .


###  https://saref.etsi.org/saref4city/quantifiesKPI
s4city:quantifiesKPI rdf:type owl:ObjectProperty ;
                     rdfs:isDefinedBy s4city: ;
                     rdfs:label "quantifies KPI"@en .


###  https://saref.etsi.org/saref4city/refersToFeature
s4city:refersToFeature rdf:type owl:ObjectProperty ;
                       rdfs:comment "Relation between a KPI assessment and the geographical feature it refers to"@en ;
                       rdfs:isDefinedBy s4city: ;
                       rdfs:label "refers to feature"@en .


###  https://saref.etsi.org/saref4city/refersToTime
s4city:refersToTime rdf:type owl:ObjectProperty ;
                    rdfs:isDefinedBy s4city: ;
                    rdfs:label "refers to time"@en .


###  https://saref.etsi.org/saref4syst/connectedThrough
s4syst:connectedThrough rdf:type owl:ObjectProperty ;
                        owl:inverseOf s4syst:connectsSystem ;
                        rdfs:domain s4syst:System ;
                        rdfs:range s4syst:Connection ;
                        owl:propertyChainAxiom ( s4syst:connectsAt
                                                 s4syst:connectsSystemThrough
                                               ) ;
                        rdfs:comment "Links a system to one of its connections to other systems."@en ;
                        rdfs:label "connected through"@en .


###  https://saref.etsi.org/saref4syst/connectedTo
s4syst:connectedTo rdf:type owl:ObjectProperty ,
                            owl:SymmetricProperty ;
                   rdfs:domain s4syst:System ;
                   rdfs:range s4syst:System ;
                   rdfs:comment "Links a system to a system it is connected to. Connected systems interact in some way. The exact meaning of \"interact\" is defined by sub properties of s4syst:connectedTo. Property s4syst:connectedTo is symmetric. This property can be qualified using class s4syst:Connection, which connects the two systems. If there is a connection between several systems, then one may infer these systems are pairwise connected."@en ;
                   rdfs:label "connected to"@en .


###  https://saref.etsi.org/saref4syst/connectionPointOf
s4syst:connectionPointOf rdf:type owl:ObjectProperty ;
                         owl:inverseOf s4syst:connectsAt ;
                         rdf:type owl:FunctionalProperty ;
                         rdfs:domain s4syst:ConnectionPoint ;
                         rdfs:range s4syst:System ;
                         rdfs:comment "Links a connection point to the one and only one system it belongs to."@en ;
                         rdfs:label "connection point to"@en .


###  https://saref.etsi.org/saref4syst/connectsAt
s4syst:connectsAt rdf:type owl:ObjectProperty ,
                           owl:InverseFunctionalProperty ;
                  rdfs:domain s4syst:System ;
                  rdfs:range s4syst:ConnectionPoint ;
                  rdfs:comment "Links a system to one of the connection points at which it connects."@en ;
                  rdfs:label "connects at"@en .


###  https://saref.etsi.org/saref4syst/connectsSystem
s4syst:connectsSystem rdf:type owl:ObjectProperty ;
                      rdfs:domain s4syst:Connection ;
                      rdfs:range s4syst:System ;
                      owl:propertyChainAxiom ( s4syst:connectsSystemAt
                                               s4syst:connectionPointOf
                                             ) ;
                      rdfs:comment "Links a connection to one of the systems it connects."@en ;
                      rdfs:label "connects system"@en .


###  https://saref.etsi.org/saref4syst/connectsSystemAt
s4syst:connectsSystemAt rdf:type owl:ObjectProperty ;
                        owl:inverseOf s4syst:connectsSystemThrough ;
                        rdfs:domain s4syst:Connection ;
                        rdfs:range s4syst:ConnectionPoint ;
                        rdfs:comment "Links a connection to one of the connection points at which it connects a system."@en ;
                        rdfs:label "connects system at"@en .


###  https://saref.etsi.org/saref4syst/connectsSystemThrough
s4syst:connectsSystemThrough rdf:type owl:ObjectProperty ;
                             rdfs:domain s4syst:ConnectionPoint ;
                             rdfs:range s4syst:Connection ;
                             rdfs:comment "Links a connection point to one of the connections through which it connects its system."@en ;
                             rdfs:label "connects system through"@en .


###  https://saref.etsi.org/saref4syst/hasSubSystem
s4syst:hasSubSystem rdf:type owl:ObjectProperty ;
                    owl:inverseOf s4syst:subSystemOf ;
                    rdf:type owl:TransitiveProperty ;
                    rdfs:domain s4syst:System ;
                    rdfs:range s4syst:System ;
                    rdfs:comment "Links a system to one of its sub systems."@en ;
                    rdfs:isDefinedBy s4syst: ;
                    rdfs:label "has sub system"@en ,
                               "has sub-system"@en .


###  https://saref.etsi.org/saref4syst/subSystemOf
s4syst:subSystemOf rdf:type owl:ObjectProperty ,
                            owl:TransitiveProperty ;
                   rdfs:domain s4syst:System ;
                   rdfs:range s4syst:System ;
                   rdfs:comment "Links a system to its super system. Properties of subsystems somehow contribute to the properties of the super system. The exact meaning of \"contribute is defined by sub properties of s4syst:subSystemOf. Property s4syst:subSystemOf is transitive."@en ;
                   rdfs:label "sub system of"@en .


###  https://saref.etsi.org/saref4watr/appliesTo
s4watr:appliesTo rdf:type owl:ObjectProperty ;
                 rdfs:domain s4watr:Tariff ;
                 rdfs:range s4watr:WaterMeter ;
                 rdfs:comment "The water meter to which a tariff applies to."@en ;
                 rdfs:label "applies to"@en .


###  https://saref.etsi.org/saref4watr/controlsFeature
s4watr:controlsFeature rdf:type owl:ObjectProperty ;
                       rdfs:domain saref:Device ;
                       rdfs:range saref:FeatureOfInterest ;
                       rdfs:comment "A relationship specifying the features of interest that are controlled by a device."@en ;
                       rdfs:label "controls feature"@en .


###  https://saref.etsi.org/saref4watr/featureIsControlledByDevice
s4watr:featureIsControlledByDevice rdf:type owl:ObjectProperty ;
                                   rdfs:domain saref:FeatureOfInterest ;
                                   rdfs:range saref:Device ;
                                   rdfs:comment "A relationship specifying the devices that control a feature of interest."@en ;
                                   rdfs:label "feature is controlled by device"@en .


###  https://saref.etsi.org/saref4watr/featureIsMeasuredByDevice
s4watr:featureIsMeasuredByDevice rdf:type owl:ObjectProperty ;
                                 rdfs:domain saref:FeatureOfInterest ;
                                 rdfs:range saref:Device ;
                                 rdfs:comment "A relationship specifying the devices that measure a feature of interest."@en ;
                                 rdfs:label "feature is measured by device"@en .


###  https://saref.etsi.org/saref4watr/forAbsoluteTimeAtDay
s4watr:forAbsoluteTimeAtDay rdf:type owl:ObjectProperty ;
                            rdfs:domain s4watr:TimeBasedTariff ;
                            rdfs:range time:Interval ;
                            rdfs:comment "The time interval in each day for which a tariff is applied (e.g., 8:00 to 10:00)."@en ;
                            rdfs:label "for absolute time at day"@en .


###  https://saref.etsi.org/saref4watr/forWeekDay
s4watr:forWeekDay rdf:type owl:ObjectProperty ;
                  rdfs:domain s4watr:TimeBasedTariff ;
                  rdfs:range time:DayOfWeek ;
                  rdfs:comment "The day of the week for which a tariff is applied (e.g., each Saturday and Sunday)."@en ;
                  rdfs:label "for week day"@en .


###  https://saref.etsi.org/saref4watr/hasBillingPeriod
s4watr:hasBillingPeriod rdf:type owl:ObjectProperty ;
                        rdfs:domain s4watr:Tariff ;
                        rdfs:range time:TemporalDuration ;
                        rdfs:comment "The billing period of a tariff."@en ;
                        rdfs:label "has billing period"@en .


###  https://saref.etsi.org/saref4watr/hasDuration
s4watr:hasDuration rdf:type owl:ObjectProperty ;
                   rdfs:domain s4watr:Tariff ;
                   rdfs:range time:TemporalDuration ;
                   rdfs:comment "The duration of a tariff."@en ;
                   rdfs:label "has duration"@en .


###  https://saref.etsi.org/saref4watr/hasPeriod
s4watr:hasPeriod rdf:type owl:ObjectProperty ;
                 rdfs:domain s4watr:Tariff ;
                 rdfs:range time:TemporalDuration ;
                 rdfs:comment "The period of a tariff."@en ;
                 rdfs:label "has period"@en .


###  https://saref.etsi.org/saref4watr/hasPhenomenonTime
s4watr:hasPhenomenonTime rdf:type owl:ObjectProperty ;
                         rdfs:domain saref:Measurement ;
                         rdfs:range time:TemporalEntity ;
                         rdfs:comment "The time for which the value of a measurement applies to the feature of interest."@en ;
                         rdfs:label "has phenomenon time"@en .


###  https://saref.etsi.org/saref4watr/isDesignedFor
s4watr:isDesignedFor rdf:type owl:ObjectProperty ;
                     rdfs:comment "The type of water for which an infrastructure is designed for."@en ;
                     rdfs:label "is designed for"@en .


###  https://saref.etsi.org/saref4watr/isIntendedFor
s4watr:isIntendedFor rdf:type owl:ObjectProperty ;
                     rdfs:comment "The intended use of the infrastructure."@en ;
                     rdfs:label "is intended for"@en .


###  https://saref.etsi.org/saref4watr/measuresFeature
s4watr:measuresFeature rdf:type owl:ObjectProperty ;
                       rdfs:domain saref:Device ;
                       rdfs:range saref:FeatureOfInterest ;
                       rdfs:comment "A relationship specifying the features of interest that are measured by a device."@en ;
                       rdfs:label "measures feature"@en .


###  https://www.geonames.org/ontology#parentADM2
gn:parentADM2 rdf:type owl:ObjectProperty .


###  https://www.geonames.org/ontology#parentADM3
gn:parentADM3 rdf:type owl:ObjectProperty .


#################################################################
#    Data properties
#################################################################

###  http://schema.org/familyName
<http://schema.org/familyName> rdf:type owl:DatatypeProperty .


###  http://schema.org/givenName
<http://schema.org/givenName> rdf:type owl:DatatypeProperty .


###  http://schema.org/name
<http://schema.org/name> rdf:type owl:DatatypeProperty .


###  http://www.opengis.net/ont/geosparql#asDGGS
geosp:asDGGS rdf:type owl:DatatypeProperty ;
             rdfs:subPropertyOf geosp:hasSerialization ;
             rdfs:domain geosp:Geometry ;
             rdfs:range geosp:dggsLiteral ;
             rdfs:isDefinedBy geosp: ,
                              <http://www.opengis.net/spec/geosparql/1.1/req/geometry-extension/geometry-as-dggs-literal> ;
             skos:definition "The Discrete Global Grid System (DGGS) serialization of a Geometry"@en ;
             skos:example <http://www.opengis.net/spec/geosparql/1.1/specification.html#B.1.2.4> ;
             skos:prefLabel "as DGGS"@en .


###  http://www.opengis.net/ont/geosparql#asGML
geosp:asGML rdf:type owl:DatatypeProperty ;
            rdfs:subPropertyOf geosp:hasSerialization ;
            rdfs:domain geosp:Geometry ;
            rdfs:range geosp:gmlLiteral ;
            rdfs:isDefinedBy geosp: ,
                             <http://www.opengis.net/spec/geosparql/1.0/req/geometry-extension/geometry-as-gml-literal> ,
                             <http://www.opengis.net/spec/geosparql/1.1/req/geometry-extension/geometry-as-gml-literal> ;
            skos:definition "The GML serialization of a Geometry"@en ;
            skos:example <http://www.opengis.net/spec/geosparql/1.1/specification.html#B.1.2.4> ;
            skos:prefLabel "as GML"@en .


###  http://www.opengis.net/ont/geosparql#asGeoJSON
geosp:asGeoJSON rdf:type owl:DatatypeProperty ;
                rdfs:subPropertyOf geosp:hasSerialization ;
                rdfs:domain geosp:Geometry ;
                rdfs:range geosp:geoJSONLiteral ;
                rdfs:isDefinedBy geosp: ,
                                 <http://www.opengis.net/spec/geosparql/1.1/req/geometry-extension/geometry-as-geojson-literal> ;
                rdfs:seeAlso <https://tools.ietf.org/html/rfc7946> ;
                skos:definition "The GeoJSON serialization of a Geometry"@en ;
                skos:example <http://www.opengis.net/spec/geosparql/1.1/specification.html#B.1.2.4> ;
                skos:prefLabel "as GeoJSON"@en .


###  http://www.opengis.net/ont/geosparql#asKML
geosp:asKML rdf:type owl:DatatypeProperty ;
            rdfs:subPropertyOf geosp:hasSerialization ;
            rdfs:domain geosp:Geometry ;
            rdfs:range geosp:kmlLiteral ;
            rdfs:isDefinedBy geosp: ,
                             <http://www.opengis.net/spec/geosparql/1.1/req/geometry-extension/geometry-as-kml-literal> ;
            rdfs:seeAlso <https://www.ogc.org/standards/kml> ;
            skos:definition "The KML serialization of a Geometry"@en ;
            skos:example <http://www.opengis.net/spec/geosparql/1.1/specification.html#B.1.2.4> ;
            skos:prefLabel "as KML"@en .


###  http://www.opengis.net/ont/geosparql#asWKT
geosp:asWKT rdf:type owl:DatatypeProperty ;
            rdfs:subPropertyOf geosp:hasSerialization ;
            rdfs:domain geosp:Geometry ;
            rdfs:range geosp:wktLiteral ;
            rdfs:isDefinedBy geosp: ,
                             <http://www.opengis.net/spec/geosparql/1.0/req/geometry-extension/geometry-as-wkt-literal> ,
                             <http://www.opengis.net/spec/geosparql/1.1/req/geometry-extension/geometry-as-wkt-literal> ;
            skos:definition "The WKT serialization of a Geometry"@en ;
            skos:example <http://www.opengis.net/spec/geosparql/1.1/specification.html#B.1.1.2.2> ,
                         <http://www.opengis.net/spec/geosparql/1.1/specification.html#B.1.1.2.3> ,
                         <http://www.opengis.net/spec/geosparql/1.1/specification.html#B.1.1.2.4> ,
                         <http://www.opengis.net/spec/geosparql/1.1/specification.html#B.1.1.2.5> ,
                         <http://www.opengis.net/spec/geosparql/1.1/specification.html#B.1.1.2.6> ,
                         <http://www.opengis.net/spec/geosparql/1.1/specification.html#B.1.1.2.8> ,
                         <http://www.opengis.net/spec/geosparql/1.1/specification.html#B.1.1.3.1> ,
                         <http://www.opengis.net/spec/geosparql/1.1/specification.html#B.1.1.3.2> ,
                         <http://www.opengis.net/spec/geosparql/1.1/specification.html#B.1.1.3.3> ,
                         <http://www.opengis.net/spec/geosparql/1.1/specification.html#B.1.2.2> ,
                         <http://www.opengis.net/spec/geosparql/1.1/specification.html#B.2.1> ,
                         <http://www.opengis.net/spec/geosparql/1.1/specification.html#B.2.2.4> ;
            skos:prefLabel "as WKT"@en .


###  http://www.opengis.net/ont/geosparql#coordinateDimension
geosp:coordinateDimension rdf:type owl:DatatypeProperty ;
                          rdfs:domain geosp:Geometry ;
                          rdfs:range xsd:integer ;
                          rdfs:isDefinedBy geosp: ,
                                           <http://www.opengis.net/spec/geosparql/1.1/req/geometry-extension/geometry-properties> ;
                          skos:definition "The number of measurements or axes needed to describe the position of this Geometry in a coordinate system."@en ;
                          skos:example <http://www.opengis.net/spec/geosparql/1.1/specification.html#B.1.2.3> ;
                          skos:prefLabel "coordinate dimension"@en .


###  http://www.opengis.net/ont/geosparql#dimension
geosp:dimension rdf:type owl:DatatypeProperty ;
                rdfs:domain geosp:Geometry ;
                rdfs:range xsd:integer ;
                rdfs:isDefinedBy geosp: ,
                                 <http://www.opengis.net/spec/geosparql/1.1/req/geometry-extension/geometry-properties> ;
                skos:definition "The topological dimension of this geometric object, which must be less than or equal to the coordinate dimension. In non-homogeneous collections, this will return the largest topological dimension of the contained objects."@en ;
                skos:example <http://www.opengis.net/spec/geosparql/1.1/specification.html#B.1.2.3> ;
                skos:prefLabel "dimension"@en .


###  http://www.opengis.net/ont/geosparql#hasMetricArea
geosp:hasMetricArea rdf:type owl:DatatypeProperty ;
                    rdfs:subPropertyOf geosp:hasMetricSize ;
                    rdfs:domain geosp:SpatialObject ;
                    rdfs:range xsd:double ;
                    rdfs:isDefinedBy geosp: ,
                                     <http://www.opengis.net/spec/geosparql/1.1/req/geometry-extension/spatial-object-properties> ;
                    skos:definition "The area of a Spatial Object in square meters."@en ;
                    skos:example <http://www.opengis.net/spec/geosparql/1.1/specification.html#B.1.1.2.3> ,
                                 <http://www.opengis.net/spec/geosparql/1.1/specification.html#B.1.1.2.9> ,
                                 <http://www.opengis.net/spec/geosparql/1.1/specification.html#B.1.1.3.3> ,
                                 <http://www.opengis.net/spec/geosparql/1.1/specification.html#B.1.2.2> ;
                    skos:prefLabel "has area in square meters"@en .


###  http://www.opengis.net/ont/geosparql#hasMetricLength
geosp:hasMetricLength rdf:type owl:DatatypeProperty ;
                      rdfs:subPropertyOf geosp:hasMetricSize ;
                      rdfs:domain geosp:SpatialObject ;
                      rdfs:range xsd:double ;
                      rdfs:isDefinedBy geosp: ,
                                       <http://www.opengis.net/spec/geosparql/1.1/req/geometry-extension/spatial-object-properties> ;
                      skos:definition "The length of a Spatial Object in meters."@en ;
                      skos:example <http://www.opengis.net/spec/geosparql/1.1/specification.html#B.1.2.2> ;
                      skos:prefLabel "has length in meters"@en .


###  http://www.opengis.net/ont/geosparql#hasMetricPerimeterLength
geosp:hasMetricPerimeterLength rdf:type owl:DatatypeProperty ;
                               rdfs:subPropertyOf geosp:hasMetricSize ;
                               rdfs:domain geosp:SpatialObject ;
                               rdfs:range xsd:double ;
                               rdfs:isDefinedBy geosp: ,
                                                <http://www.opengis.net/spec/geosparql/1.1/req/geometry-extension/spatial-object-properties> ;
                               skos:definition "The length of the perimeter of a Spatial Object in meters."@en ;
                               skos:example <http://www.opengis.net/spec/geosparql/1.1/specification.html#B.1.1.1.2> ;
                               skos:prefLabel "has perimeter length in meters"@en .


###  http://www.opengis.net/ont/geosparql#hasMetricSize
geosp:hasMetricSize rdf:type owl:DatatypeProperty ;
                    rdfs:domain geosp:SpatialObject ;
                    rdfs:range xsd:double ;
                    rdfs:isDefinedBy geosp: ,
                                     <http://www.opengis.net/spec/geosparql/1.1/req/geometry-extension/spatial-object-properties> ;
                    skos:definition "Subproperties of this property are used to indicate the size of a Spatial Object, as a measurement or estimate of one or more dimensions of the Spatial Object's spatial presence. Units are always metric (meter, square meter or cubic meter)."@en ;
                    skos:prefLabel "has metric size"@en .


###  http://www.opengis.net/ont/geosparql#hasMetricSpatialAccuracy
geosp:hasMetricSpatialAccuracy rdf:type owl:DatatypeProperty ;
                               rdfs:domain geosp:Geometry ;
                               rdfs:range xsd:double ;
                               rdfs:isDefinedBy geosp: ,
                                                <http://www.opengis.net/spec/geosparql/1.1/req/geometry-extension/geometry-properties> ;
                               skos:definition "The positional accuracy of the coordinates of a Geometry in meters."@en ;
                               skos:example <http://www.opengis.net/spec/geosparql/1.1/specification.html#B.1.2.3> ;
                               skos:note "Spatial accuracy is applicable when a Geometry is used to represent a Feature. It is expressed as a distance that indicates the truthfullness of the positions (coordinates) that define the Geometry. In this case accuracy defines a zone surrounding each coordinate within wich the real positions are known to be. The accuracy value defines this zone as a distance from the coordinate(s) in all directions (e.g. a line, a circle or a sphere, depending on spatial dimension)."@en ;
                               skos:prefLabel "has spatial accuracy in meters"@en .


###  http://www.opengis.net/ont/geosparql#hasMetricSpatialResolution
geosp:hasMetricSpatialResolution rdf:type owl:DatatypeProperty ;
                                 rdfs:domain geosp:Geometry ;
                                 rdfs:range xsd:double ;
                                 rdfs:isDefinedBy geosp: ,
                                                  <http://www.opengis.net/spec/geosparql/1.1/req/geometry-extension/geometry-properties> ;
                                 skos:definition "The spatial resolution of a Geometry in meters."@en ;
                                 skos:example <http://www.opengis.net/spec/geosparql/1.1/specification.html#B.1.1.2.6> ,
                                              <http://www.opengis.net/spec/geosparql/1.1/specification.html#B.1.2.2> ;
                                 skos:note "Spatial resolution specifies the level of detail of a Geometry. It the smallest dinstinguishable distance between spatially adjacent coordinates."@en ;
                                 skos:prefLabel "has spatial resolution in meters"@en .


###  http://www.opengis.net/ont/geosparql#hasMetricVolume
geosp:hasMetricVolume rdf:type owl:DatatypeProperty ;
                      rdfs:subPropertyOf geosp:hasMetricSize ;
                      rdfs:domain geosp:SpatialObject ;
                      rdfs:range xsd:double ;
                      rdfs:isDefinedBy geosp: ,
                                       <http://www.opengis.net/spec/geosparql/1.1/req/geometry-extension/spatial-object-properties> ;
                      skos:definition "The volume of a Spatial Object in cubic meters."@en ;
                      skos:example <http://www.opengis.net/spec/geosparql/1.1/specification.html#B.1.1.2.9> ,
                                   <http://www.opengis.net/spec/geosparql/1.1/specification.html#B.1.2.2> ;
                      skos:prefLabel "has volume in cubic meters"@en .


###  http://www.opengis.net/ont/geosparql#hasSerialization
geosp:hasSerialization rdf:type owl:DatatypeProperty ;
                       rdfs:domain geosp:Geometry ;
                       rdfs:range rdfs:Literal ;
                       rdfs:isDefinedBy geosp: ,
                                        <http://www.opengis.net/spec/geosparql/1.0/req/geometry-extension/geometry-properties> ,
                                        <http://www.opengis.net/spec/geosparql/1.1/req/geometry-extension/geometry-properties> ;
                       skos:definition "Connects a Geometry object with its text-based serialization."@en ;
                       skos:example <http://www.opengis.net/spec/geosparql/1.1/specification.html#B.1.2.3> ;
                       skos:prefLabel "has serialization"@en .


###  http://www.opengis.net/ont/geosparql#isEmpty
geosp:isEmpty rdf:type owl:DatatypeProperty ;
              rdfs:domain geosp:Geometry ;
              rdfs:range xsd:boolean ;
              rdfs:isDefinedBy geosp: ,
                               <http://www.opengis.net/spec/geosparql/1.0/req/geometry-extension/geometry-properties> ,
                               <http://www.opengis.net/spec/geosparql/1.1/req/geometry-extension/geometry-properties> ;
              skos:definition "(true) if this geometric object is the empty Geometry. If true, then this geometric object represents the empty point set for the coordinate space."@en ;
              skos:example <http://www.opengis.net/spec/geosparql/1.1/specification.html#B.1.2.3> ;
              skos:prefLabel "is empty"@en .


###  http://www.opengis.net/ont/geosparql#isSimple
geosp:isSimple rdf:type owl:DatatypeProperty ;
               rdfs:domain geosp:Geometry ;
               rdfs:range xsd:boolean ;
               rdfs:isDefinedBy geosp: ,
                                <http://www.opengis.net/spec/geosparql/1.0/req/geometry-extension/geometry-properties> ,
                                <http://www.opengis.net/spec/geosparql/1.1/req/geometry-extension/geometry-properties> ;
               rdfs:seeAlso <https://portal.ogc.org/files/?artifact_id=25355> ;
               skos:definition "(true) if this geometric object has no anomalous geometric points, such as self intersection or self tangency."@en ;
               skos:example <http://www.opengis.net/spec/geosparql/1.1/specification.html#B.1.2.3> ;
               skos:prefLabel "is simple"@en .


###  http://www.opengis.net/ont/geosparql#spatialDimension
geosp:spatialDimension rdf:type owl:DatatypeProperty ;
                       rdfs:domain geosp:Geometry ;
                       rdfs:range xsd:integer ;
                       rdfs:isDefinedBy geosp: ,
                                        <http://www.opengis.net/spec/geosparql/1.0/req/geometry-extension/geometry-properties> ,
                                        <http://www.opengis.net/spec/geosparql/1.1/req/geometry-extension/geometry-properties> ;
                       skos:definition "The number of measurements or axes needed to describe the spatial position of this Geometry in a coordinate system."@en ;
                       skos:example <http://www.opengis.net/spec/geosparql/1.1/specification.html#B.1.2.3> ;
                       skos:prefLabel "spatial dimension"@en .


###  http://www.w3.org/2003/01/geo/wgs84_pos#alt
wgs84:alt rdf:type owl:DatatypeProperty .


###  http://www.w3.org/2003/01/geo/wgs84_pos#lat
wgs84:lat rdf:type owl:DatatypeProperty .


###  http://www.w3.org/2006/time#day
time:day rdf:type owl:DatatypeProperty ;
         rdfs:domain time:GeneralDateTimeDescription ;
         rdfs:comment """Day position in a calendar-clock system.

The range of this property is not specified, so can be replaced by any specific representation of a calendar day from any calendar. """@en ,
                      "Posición de día en un sistema calendario-reloj."@es ;
         rdfs:label "day"@en ,
                    "día"@es ;
         skos:definition """Day position in a calendar-clock system.

The range of this property is not specified, so can be replaced by any specific representation of a calendar day from any calendar. """@en ,
                         """Posición de día en un sistema calendario-reloj.

El rango de esta propiedad no está especificado, por tanto, se puede reemplazar por una representación específica de un día de calendario de cualquier calendario."""@es .


###  http://www.w3.org/2006/time#dayOfYear
time:dayOfYear rdf:type owl:DatatypeProperty ;
               rdfs:domain time:GeneralDateTimeDescription ;
               rdfs:range xsd:nonNegativeInteger ;
               rdfs:comment "El número de día en el año."@es ,
                            "The number of the day within the year"@en ;
               rdfs:label "day of year"@en ,
                          "día del año"@es ;
               skos:definition "El número de día en el año."@es ,
                               "The number of the day within the year"@en .


###  http://www.w3.org/2006/time#days
time:days rdf:type owl:DatatypeProperty ;
          rdfs:domain time:GeneralDurationDescription ;
          rdfs:range xsd:decimal ;
          rdfs:comment "Longitud de, o elemento de la longitud de, una extensión temporal expresada en días."@es ,
                       "length of, or element of the length of, a temporal extent expressed in days"@en ;
          rdfs:label "days duration"@en ,
                     "duración en días"@es ;
          skos:definition "Longitud de, o elemento de la longitud de, una extensión temporal expresada en días."@es ,
                          "length of, or element of the length of, a temporal extent expressed in days"@en .


###  http://www.w3.org/2006/time#hasXSDDuration
time:hasXSDDuration rdf:type owl:DatatypeProperty ;
                    rdfs:domain time:TemporalEntity ;
                    rdfs:range xsd:duration ;
                    rdfs:comment "Extensión de una entidad temporal, expresada utilizando xsd:duration."@es ,
                                 "Extent of a temporal entity, expressed using xsd:duration"@en ;
                    rdfs:label "has XSD duration"@en ,
                               "tiene duración XSD"@es ;
                    skos:definition "Extensión de una entidad temporal, expresada utilizando xsd:duration."@es ,
                                    "Extent of a temporal entity, expressed using xsd:duration"@en ;
                    skos:editorialNote "Característica arriesgada - añadida en la revisión de 2017, y todavía no ampliamente utilizada."@es ,
                                       "Feature at risk - added in 2017 revision, and not yet widely used. "@en .


###  http://www.w3.org/2006/time#hour
time:hour rdf:type owl:DatatypeProperty ;
          rdfs:domain time:GeneralDateTimeDescription ;
          rdfs:range xsd:nonNegativeInteger ;
          rdfs:comment "Hour position in a calendar-clock system."@en ,
                       "Posición de hora en un sistema calendario-reloj."@es ;
          rdfs:label "hora"@es ,
                     "hour"@en ;
          skos:definition "Hour position in a calendar-clock system."@en ,
                          "Posición de hora en un sistema calendario-reloj."@es .


###  http://www.w3.org/2006/time#hours
time:hours rdf:type owl:DatatypeProperty ;
           rdfs:domain time:GeneralDurationDescription ;
           rdfs:range xsd:decimal ;
           rdfs:comment "Longitud de, o elemento de la longitud de, una extensión temporal expresada en horas."@es ,
                        "length of, or element of the length of, a temporal extent expressed in hours"@en ;
           rdfs:label "duración en horas"@es ,
                      "hours duration"@en ;
           skos:definition "Longitud de, o elemento de la longitud de, una extensión temporal expresada en horas."@es ,
                           "length of, or element of the length of, a temporal extent expressed in hours"@en .


###  http://www.w3.org/2006/time#inXSDDate
time:inXSDDate rdf:type owl:DatatypeProperty ;
               rdfs:domain time:Instant ;
               rdfs:range xsd:date ;
               rdfs:comment "Posición de un instante, expresado utilizando xsd:date."@es ,
                            "Position of an instant, expressed using xsd:date"@en ;
               rdfs:label "en fecha XSD"@es ,
                          "in XSD date"@en ;
               skos:definition "Posición de un instante, expresado utilizando xsd:date."@es ,
                               "Position of an instant, expressed using xsd:date"@en .


###  http://www.w3.org/2006/time#inXSDDateTime
time:inXSDDateTime rdf:type owl:DatatypeProperty ;
                   rdfs:domain time:Instant ;
                   rdfs:range xsd:dateTime ;
                   rdfs:comment "Posición de un instante, expresado utilizando xsd:dateTime."@es ,
                                "Position of an instant, expressed using xsd:dateTime"@en ;
                   rdfs:label "en fecha-tiempo XSD"@es ,
                              "in XSD Date-Time"@en ;
                   owl:deprecated "true"^^xsd:boolean ;
                   skos:definition "Posición de un instante, expresado utilizando xsd:dateTime."@es ,
                                   "Position of an instant, expressed using xsd:dateTime"@en ;
                   skos:note "La propiedad 'en fecha-hora XSD' ha sido reemplazada por 'en fecha-sello de tiempo XSD' que hace obligatorio el campo 'huso horario'."@es ,
                             "The property :inXSDDateTime is replaced by :inXSDDateTimeStamp which makes the time-zone field mandatory."@en .


###  http://www.w3.org/2006/time#inXSDDateTimeStamp
time:inXSDDateTimeStamp rdf:type owl:DatatypeProperty ;
                        rdfs:domain time:Instant ;
                        rdfs:range xsd:dateTimeStamp ;
                        rdfs:comment "Posición de un instante, expresado utilizando xsd:dateTimeStamp."@es ,
                                     "Position of an instant, expressed using xsd:dateTimeStamp"@en ;
                        rdfs:label "en fecha-sello de tiempo XSD"@es ,
                                   "in XSD Date-Time-Stamp"@en ;
                        skos:definition "Posición de un instante, expresado utilizando xsd:dateTimeStamp."@es ,
                                        "Position of an instant, expressed using xsd:dateTimeStamp"@en .


###  http://www.w3.org/2006/time#inXSDgYear
time:inXSDgYear rdf:type owl:DatatypeProperty ;
                rdfs:domain time:Instant ;
                rdfs:range xsd:gYear ;
                rdfs:comment "Posición de un instante, expresado utilizando xsd:gYear."@es ,
                             "Position of an instant, expressed using xsd:gYear"@en ;
                rdfs:label "en año gregoriano XSD"@es ,
                           "in XSD g-Year"@en ;
                skos:definition "Posición de un instante, expresado utilizando xsd:gYear."@es ,
                                "Position of an instant, expressed using xsd:gYear"@en .


###  http://www.w3.org/2006/time#inXSDgYearMonth
time:inXSDgYearMonth rdf:type owl:DatatypeProperty ;
                     rdfs:domain time:Instant ;
                     rdfs:range xsd:gYearMonth ;
                     rdfs:comment "Posición de un instante, expresado utilizando xsd:gYearMonth."@es ,
                                  "Position of an instant, expressed using xsd:gYearMonth"@en ;
                     rdfs:label "en año-mes gregoriano XSD"@es ,
                                "in XSD g-YearMonth"@en ;
                     skos:definition "Posición de un instante, expresado utilizando xsd:gYearMonth."@es ,
                                     "Position of an instant, expressed using xsd:gYearMonth"@en .


###  http://www.w3.org/2006/time#minute
time:minute rdf:type owl:DatatypeProperty ;
            rdfs:domain time:GeneralDateTimeDescription ;
            rdfs:range xsd:nonNegativeInteger ;
            rdfs:comment "Minute position in a calendar-clock system."@en ,
                         "Posición de minuto en un sistema calendario-reloj."@es ;
            rdfs:label "minute"@en ,
                       "minuto"@es ;
            skos:definition "Minute position in a calendar-clock system."@en ,
                            "Posición de minuto en un sistema calendario-reloj."@es .


###  http://www.w3.org/2006/time#minutes
time:minutes rdf:type owl:DatatypeProperty ;
             rdfs:domain time:GeneralDurationDescription ;
             rdfs:range xsd:decimal ;
             rdfs:comment "Longitud de, o elemento de la longitud de, una extensión temporal expresada en minutos."@es ,
                          "length, or element of, a temporal extent expressed in minutes"@en ;
             rdfs:label "minutes"@en ,
                        "minutos"@es ;
             skos:definition "Longitud de, o elemento de la longitud de, una extensión temporal expresada en minutos."@es ,
                             "length, or element of, a temporal extent expressed in minutes"@en .


###  http://www.w3.org/2006/time#month
time:month rdf:type owl:DatatypeProperty ;
           rdfs:domain time:GeneralDateTimeDescription ;
           rdfs:comment """Month position in a calendar-clock system.

The range of this property is not specified, so can be replaced by any specific representation of a calendar month from any calendar. """@en ,
                        """Posición de mes en un sistema calendario-reloj.
    El rango de esta propiedad no está especificado, por tanto, se puede reemplazar por cualquier representación específica de un mes de calendario de un calendario cualquiera."""@es ;
           rdfs:label "mes"@es ,
                      "month"@en ;
           skos:definition """Month position in a calendar-clock system.

The range of this property is not specified, so can be replaced by any specific representation of a calendar month from any calendar. """@en ,
                           """Posición de mes en un sistema calendario-reloj.
            El rango de esta propiedad no está especificado, por tanto, se puede reemplazar por cualquier representación específica de un mes de calendario de un calendario cualquiera."""@es .


###  http://www.w3.org/2006/time#months
time:months rdf:type owl:DatatypeProperty ;
            rdfs:domain time:GeneralDurationDescription ;
            rdfs:range xsd:decimal ;
            rdfs:comment "Longitud de, o elemento de la longitud de, una extensión temporal expresada en meses."@es ,
                         "length of, or element of the length of, a temporal extent expressed in months"@en ;
            rdfs:label "duración en meses"@es ,
                       "months duration"@en ;
            skos:definition "Longitud de, o elemento de la longitud de, una extensión temporal expresada en meses."@es ,
                            "length of, or element of the length of, a temporal extent expressed in months"@en .


###  http://www.w3.org/2006/time#nominalPosition
time:nominalPosition rdf:type owl:DatatypeProperty ;
                     rdfs:domain time:TimePosition ;
                     rdfs:range xsd:string ;
                     rdfs:comment "El valor (nominal) que indica posición temporal en un sistema de referencia ordinal."@es ,
                                  "The (nominal) value indicating temporal position in an ordinal reference system "@en ;
                     rdfs:label "Name of temporal position"@en ,
                                "nombre de posición temporal"@es ;
                     skos:definition "El valor (nominal) que indica posición temporal en un sistema de referencia ordinal."@es ,
                                     "The (nominal) value indicating temporal position in an ordinal reference system "@en .


###  http://www.w3.org/2006/time#numericDuration
time:numericDuration rdf:type owl:DatatypeProperty ;
                     rdfs:domain time:Duration ;
                     rdfs:range xsd:decimal ;
                     rdfs:comment "Valor de una extensión temporal expresada como un número decimal escalado por una unidad de tiempo."@es ,
                                  "Value of a temporal extent expressed as a decimal number scaled by a temporal unit"@en ;
                     rdfs:label "Numeric value of temporal duration"@en ,
                                "valor numérico de duración temporal"@es ;
                     skos:definition "Valor de una extensión temporal expresada como un número decimal escalado por una unidad de tiempo."@es ,
                                     "Value of a temporal extent expressed as a decimal number scaled by a temporal unit"@en .


###  http://www.w3.org/2006/time#numericPosition
time:numericPosition rdf:type owl:DatatypeProperty ;
                     rdfs:domain time:TimePosition ;
                     rdfs:range xsd:decimal ;
                     rdfs:comment "El valor (numérico) que indica posición temporal en un sistema de referencia ordinal."@es ,
                                  "The (numeric) value indicating position within a temporal coordinate system "@en ;
                     rdfs:label "Numeric value of temporal position"@en ,
                                "valor numérico de posición temporal"@es ;
                     skos:definition "El valor (numérico) que indica posición temporal en un sistema de referencia ordinal."@es ,
                                     "The (numeric) value indicating position within a temporal coordinate system "@en .


###  http://www.w3.org/2006/time#second
time:second rdf:type owl:DatatypeProperty ;
            rdfs:domain time:GeneralDateTimeDescription ;
            rdfs:range xsd:decimal ;
            rdfs:comment "Posición de segundo en un sistema calendario-reloj."@es ,
                         "Second position in a calendar-clock system."@en ;
            rdfs:label "second"@en ,
                       "segundo"@es .


###  http://www.w3.org/2006/time#seconds
time:seconds rdf:type owl:DatatypeProperty ;
             rdfs:domain time:GeneralDurationDescription ;
             rdfs:range xsd:decimal ;
             rdfs:comment "Longitud de, o elemento de la longitud de, una extensión temporal expresada en segundos."@es ,
                          "length of, or element of the length of, a temporal extent expressed in seconds"@en ;
             rdfs:label "duración en segundos"@es ,
                        "seconds duration"@en ;
             rdfs:seeAlso <http://www.bipm.org/en/publications/si-brochure/second.html> .


###  http://www.w3.org/2006/time#week
time:week rdf:type owl:DatatypeProperty ;
          rdfs:domain time:GeneralDateTimeDescription ;
          rdfs:range xsd:nonNegativeInteger ;
          rdfs:comment "Número de semana en el año."@es ,
                       "Week number within the year."@en ;
          rdfs:label "semana"@es ,
                     "week"@en ;
          skos:note "Weeks are numbered differently depending on the calendar in use and the local language or cultural conventions (locale). ISO-8601 specifies that the first week of the year includes at least four days, and that Monday is the first day of the week. In that system, week 1 is the week that contains the first Thursday in the year."@en ;
          skos:scopeNote "Las semanas están numeradas de forma diferente dependiendo del calendario en uso y de las convenciones lingüísticas y culturales locales (locale en inglés). El ISO-8601 especifica que la primera semana del año incluye al menos cuatro días, y que el lunes es el primer día de la semana. En ese sistema, la semana 1 es la semana que contiene el primer jueves del año."@es .


###  http://www.w3.org/2006/time#weeks
time:weeks rdf:type owl:DatatypeProperty ;
           rdfs:domain time:GeneralDurationDescription ;
           rdfs:range xsd:decimal ;
           rdfs:comment "Longitud de, o elemento de la longitud de, una extensión temporal expresada en semanas."@es ,
                        "length of, or element of the length of, a temporal extent expressed in weeks"@en ;
           rdfs:label "duración en semanas"@es ,
                      "weeks duration"@en .


###  http://www.w3.org/2006/time#xsdDateTime
time:xsdDateTime rdf:type owl:DatatypeProperty ;
                 rdfs:domain time:DateTimeInterval ;
                 rdfs:range xsd:dateTime ;
                 rdfs:comment "Valor de 'intervalo de fecha-hora' expresado como un valor compacto."@es ,
                              "Value of DateTimeInterval expressed as a compact value."@en ;
                 rdfs:label "has XSD date-time"@en ,
                            "tiene fecha-hora XSD"@es ;
                 owl:deprecated "true"^^xsd:boolean ;
                 skos:note "Using xsd:dateTime in this place means that the duration of the interval is implicit: it corresponds to the length of the smallest non-zero element of the date-time literal. However, this rule cannot be used for intervals whose duration is more than one rank smaller than the starting time - e.g. the first minute or second of a day, the first hour of a month, or the first day of a year. In these cases the desired interval cannot be distinguished from the interval corresponding to the next rank up. Because of this essential ambiguity, use of this property is not recommended and it is deprecated."@en ,
                           "Utilizando xsd:dateTime en este lugar significa que la duración del intervalo está implícita: se corresponde con la longitud del elemento más pequeño distinto de cero del literal fecha-hora. Sin embargo, esta regla no se puede utilizar para intervalos cuya duración es mayor que un rango más pequeño que el tiempo de comienzo - p.ej. el primer minuto o segundo del día, la primera hora del mes, o el primer día del año. En estos casos el intervalo deseado no se puede distinguir del intervalo correspondiente al próximo rango más alto. Debido a esta ambigüedad esencial, no se recomienda el uso de esta propiedad y está desaprobada." .


###  http://www.w3.org/2006/time#year
time:year rdf:type owl:DatatypeProperty ;
          rdfs:domain time:GeneralDateTimeDescription ;
          rdfs:comment """Posición de año en un sistema calendario-reloj.

l rango de esta propiedad no está especificado, por tanto, se puede reemplazar por cualquier representación específica de un año de calendario de un calendario cualquiera."""@es ,
                       """Year position in a calendar-clock system.

The range of this property is not specified, so can be replaced by any specific representation of a calendar year from any calendar. """@en ;
          rdfs:label "year"@en .


###  http://www.w3.org/2006/time#years
time:years rdf:type owl:DatatypeProperty ;
           rdfs:domain time:GeneralDurationDescription ;
           rdfs:range xsd:decimal ;
           rdfs:comment "Longitud de, o elemento de la longitud de, una extensión temporal expresada en años."@es ,
                        "length of, or element of the length of, a temporal extent expressed in years"@en ;
           rdfs:label "duración en años"@es ,
                      "years duration"@en .


###  http://www.w3.org/2006/vcard/ns#street-address
vcard:street-address rdf:type owl:DatatypeProperty .


###  http://www.w3.org/2008/05/skos#notation
<http://www.w3.org/2008/05/skos#notation> rdf:type owl:DatatypeProperty .


###  http://www.w3.org/2015/03/inspire/cp#nationalCadastralReference
cp:nationalCadastralReference rdf:type owl:DatatypeProperty ;
                              rdfs:subPropertyOf <http://www.w3.org/2008/05/skos#notation> ;
                              rdfs:domain cp:CadastralParcel ;
                              rdfs:range xsd:string ;
                              rdfs:comment "Thematic identifier at national level, generally the full national code of the basic property unit. Must ensure the link to the national cadastral register or equivalent."@en ;
                              rdfs:isDefinedBy <http://www.w3.org/2015/03/inspire/cp> ;
                              rdfs:label "national cadastral reference"@en .


###  https://saref.etsi.org/core/hasDescription
saref:hasDescription rdf:type owl:DatatypeProperty ;
                     rdfs:range xsd:string ;
                     rdfs:comment "A relationship providing a description of an entity (e.g., device)"@en ,
                                  "A relationship providing a description of an entity (e.g., device). The value is expected to be a string or a string with language tag."@en ,
                                  "DEPRECATED: The use of rdfs:comment is recommended instead."@en ;
                     rdfs:isDefinedBy saref: ;
                     rdfs:label "has description"@en ;
                     owl:deprecated "true"^^xsd:boolean .


###  https://saref.etsi.org/core/hasManufacturer
saref:hasManufacturer rdf:type owl:DatatypeProperty ;
                      rdfs:range xsd:string ;
                      rdfs:comment "A relationship identifying the manufacturer of an entity (e.g., device)"@en ,
                                   "A relationship identifying the manufacturer of an entity (e.g., device). The value is expected to be a string or a string with language tag."@en ;
                      rdfs:isDefinedBy saref: ;
                      rdfs:label "has manufacturer"@en .


###  https://saref.etsi.org/core/hasModel
saref:hasModel rdf:type owl:DatatypeProperty ;
               rdfs:range xsd:string ;
               rdfs:comment "A relationship identifying the model of an entity (e.g., device)"@en ,
                            "A relationship identifying the model of an entity (e.g., device). The value is expected to be a string or a string with language tag."@en ;
               rdfs:isDefinedBy saref: ;
               rdfs:label "has model"@en .


###  https://saref.etsi.org/core/hasTimestamp
saref:hasTimestamp rdf:type owl:DatatypeProperty ,
                            owl:FunctionalProperty ;
                   rdfs:range xsd:dateTime ;
                   rdfs:comment "A relationship stating the timestamp of an entity (e.g. a measurement)."@en ;
                   rdfs:isDefinedBy saref: ,
                                    "https://saref.etsi.org/core/" ;
                   rdfs:label "has timestamp"@en .


###  https://saref.etsi.org/core/hasValue
saref:hasValue rdf:type owl:DatatypeProperty ;
               rdfs:comment "A relationship defining the value of a certain property, e.g., energy or power"@en ,
                            "A relationship defining the value of a certain property, e.g., energy or power. Note that, even if numeric values are expected to enable reasoning, measurement values could use other datatypes."@en ;
               rdfs:isDefinedBy saref: ;
               rdfs:label "has value"@en .


###  https://saref.etsi.org/saref4agri/hasBirthDate
s4agri:hasBirthDate rdf:type owl:DatatypeProperty ;
                    rdfs:range xsd:dateTime ;
                    rdfs:comment "A relation to express the birth date of an animal."@en ;
                    rdfs:label "has birth date"@en .


###  https://saref.etsi.org/saref4agri/hasDeathDate
s4agri:hasDeathDate rdf:type owl:DatatypeProperty ;
                    rdfs:range xsd:dateTime ;
                    rdfs:comment "A relation to express the death date of an animal."@en ;
                    rdfs:label "has death date"@en .


###  https://saref.etsi.org/saref4agri/hasHarvestDate
s4agri:hasHarvestDate rdf:type owl:DatatypeProperty ;
                      rdfs:subPropertyOf owl:topDataProperty ;
                      rdfs:range xsd:dateTime ;
                      rdfs:comment "A relation to express the day the crop is harvested."@en ;
                      rdfs:label "has harvest date"@en .


###  https://saref.etsi.org/saref4agri/hasName
s4agri:hasName rdf:type owl:DatatypeProperty ;
               rdfs:range xsd:string ;
               rdfs:comment "A relation to express the name of an entity (e.g.,animal)."@en ;
               rdfs:label "has name"@en .


###  https://saref.etsi.org/saref4agri/hasPlantDate
s4agri:hasPlantDate rdf:type owl:DatatypeProperty ;
                    rdfs:subPropertyOf owl:topDataProperty ;
                    rdfs:range xsd:dateTime ;
                    rdfs:comment "A relation to express the day the crop is planted."@en ;
                    rdfs:label "has plant date"@en .


###  https://saref.etsi.org/saref4bldg/accessType
s4bldg:accessType rdf:type owl:DatatypeProperty ;
                  rdfs:range xsd:string ;
                  rdfs:comment "Defines the types of access (or cover) to a tank that may be specified. Note that covers are generally specified for rectangular tanks. For cylindrical tanks, access will normally be via a manhole."@en ;
                  rdfs:label "access type"@en .


###  https://saref.etsi.org/saref4bldg/application
s4bldg:application rdf:type owl:DatatypeProperty ;
                   rdfs:range xsd:string ;
                   rdfs:comment "Humidifier application. Fixed: Humidifier installed in a ducted flow distribution system. Portable: Humidifier is not installed in a ducted flow distribution system."@en ;
                   rdfs:label "application"@en .


###  https://saref.etsi.org/saref4bldg/arrangement
s4bldg:arrangement rdf:type owl:DatatypeProperty ;
                   rdfs:range xsd:string ;
                   rdfs:comment "Defines the basic flow arrangements for the heat exchanger: COUNTERFLOW: Counterflow heat exchanger arrangement. CROSSFLOW: Crossflow heat exchanger arrangement. PARALLELFLOW: Parallel flow heat exchanger arrangement. MULTIPASS: Multipass flow heat exchanger arrangement. OTHER: Other type of heat exchanger flow arrangement not defined above."@en ;
                   rdfs:label "arrangement"@en .


###  https://saref.etsi.org/saref4bldg/bladeAction
s4bldg:bladeAction rdf:type owl:DatatypeProperty ;
                   rdfs:range xsd:string ;
                   rdfs:comment "Blade action."@en ;
                   rdfs:label "blade action"@en .


###  https://saref.etsi.org/saref4bldg/bladeEdge
s4bldg:bladeEdge rdf:type owl:DatatypeProperty ;
                 rdfs:range xsd:string ;
                 rdfs:comment "Blade edge."@en ;
                 rdfs:label "blade edge"@en .


###  https://saref.etsi.org/saref4bldg/bladeShape
s4bldg:bladeShape rdf:type owl:DatatypeProperty ;
                  rdfs:range xsd:string ;
                  rdfs:comment "Blade shape. Flat means triple V-groove."@en ;
                  rdfs:label "blade shape"@en .


###  https://saref.etsi.org/saref4bldg/capacityControl
s4bldg:capacityControl rdf:type owl:DatatypeProperty ;
                       rdfs:range xsd:string ;
                       rdfs:comment "FanCycling: Fan is cycled on and off to control duty. TwoSpeedFan: Fan is switched between low and high speed to control duty. VariableSpeedFan: Fan speed is varied to control duty. DampersControl: Dampers modulate the air flow to control duty. BypassValveControl: Bypass valve modulates the water flow to control duty. MultipleSeriesPumps: Turn on/off multiple series pump to control duty. TwoSpeedPump: Switch between high/low pump speed to control duty. VariableSpeedPump: vary pump speed to control duty."@en ;
                       rdfs:label "capacity control"@en .


###  https://saref.etsi.org/saref4bldg/capacityControlType
s4bldg:capacityControlType rdf:type owl:DatatypeProperty ;
                           rdfs:range xsd:string ;
                           rdfs:comment "InletVane: Control by adjusting inlet vane. VariableSpeedDrive: Control by variable speed drive. BladePitchAngle: Control by adjusting blade pitch angle. TwoSpeed: Control by switch between high and low speed. DischargeDamper: Control by modulating discharge damper."@en ;
                           rdfs:label "capacity control type"@en .


###  https://saref.etsi.org/saref4bldg/capacityPeople
s4bldg:capacityPeople rdf:type owl:DatatypeProperty ;
                      rdfs:range xsd:nonNegativeInteger ;
                      rdfs:comment "Capacity of the transportation element measured in numbers of person."@en ;
                      rdfs:label "capacity people"@en .


###  https://saref.etsi.org/saref4bldg/circuitType
s4bldg:circuitType rdf:type owl:DatatypeProperty ;
                   rdfs:range xsd:string ;
                   rdfs:comment "OpenCircuit: Exposes water directly to the cooling atmosphere. CloseCircuit: The fluid is separated from the atmosphere by a heat exchanger. Wet: The air stream or the heat exchange surface is evaporatively cooled. Dry: No evaporation into the air stream. DryWet: A combination of a dry tower and a wet tower."@en ;
                   rdfs:label "circuit type"@en .


###  https://saref.etsi.org/saref4bldg/colorAppearance
s4bldg:colorAppearance rdf:type owl:DatatypeProperty ;
                       rdfs:range xsd:string ;
                       rdfs:comment "In both the DIN and CIE standards, artificial light sources are classified in terms of their color appearance. To the human eye they all appear to be white the difference can only be detected by direct comparison. Visual performance is not directly affected by differences in color appearance."@en ;
                       rdfs:label "color appearance"@en .


###  https://saref.etsi.org/saref4bldg/colorRenderingIndex
s4bldg:colorRenderingIndex rdf:type owl:DatatypeProperty ;
                           rdfs:range xsd:integer ;
                           rdfs:comment "The CRI indicates how well a light source renders eight standard colors compared to perfect reference lamp with the same color temperature. The CRI scale ranges from 1 to 100, with 100 representing perfect rendering properties."@en ;
                           rdfs:label "color rendering index"@en .


###  https://saref.etsi.org/saref4bldg/controlStrategy
s4bldg:controlStrategy rdf:type owl:DatatypeProperty ;
                       rdfs:range xsd:string ;
                       rdfs:comment "FixedExitingWaterTemp: The capacity is controlled to maintain a fixed exiting water temperature. WetBulbTempReset: The set-point is reset based on the wet-bulb temperature."@en ;
                       rdfs:label "control strategy"@en .


###  https://saref.etsi.org/saref4bldg/endShapeType
s4bldg:endShapeType rdf:type owl:DatatypeProperty ;
                    rdfs:range xsd:string ;
                    rdfs:comment "Defines the types of end shapes that can be used for preformed tanks. The convention for reading these enumerated values is that for a vertical cylinder, the first value is the base and the second is the top for a horizontal cylinder, the order of reading should be left to right. For a speherical tank, the value UNSET should be used.B5"@en ;
                    rdfs:label "end shape type"@en .


###  https://saref.etsi.org/saref4bldg/energySource
s4bldg:energySource rdf:type owl:DatatypeProperty ;
                    rdfs:range xsd:string ;
                    rdfs:comment "Enumeration defining the energy source or fuel cumbusted to generate heat."@en ,
                                 "The source of energy."@en ;
                    rdfs:label "energy source"@en .


###  https://saref.etsi.org/saref4bldg/evaporationCoolant
s4bldg:evaporationCoolant rdf:type owl:DatatypeProperty ;
                          rdfs:range xsd:string ;
                          rdfs:comment "The fluid used for the coolant in the evaporator."@en ;
                          rdfs:label "evaporation coolant"@en .


###  https://saref.etsi.org/saref4bldg/evaporationMediumType
s4bldg:evaporationMediumType rdf:type owl:DatatypeProperty ;
                             rdfs:range xsd:string ;
                             rdfs:comment "ColdLiquid: Evaporator is using liquid type of fluid to exchange heat with refrigerant. ColdAir: Evaporator is using air to exchange heat with refrigerant."@en ;
                             rdfs:label "evaporation medium type"@en .


###  https://saref.etsi.org/saref4bldg/failPosition
s4bldg:failPosition rdf:type owl:DatatypeProperty ;
                    rdfs:range xsd:string ;
                    rdfs:comment "Specifies the required fail-safe position of the actuator."@en ;
                    rdfs:label "fail position"@en .


###  https://saref.etsi.org/saref4bldg/finishColor
s4bldg:finishColor rdf:type owl:DatatypeProperty ;
                   rdfs:range xsd:string ;
                   rdfs:comment "Finish color for cooled beam."@en ;
                   rdfs:label "finish color"@en .


###  https://saref.etsi.org/saref4bldg/fireExit
s4bldg:fireExit rdf:type owl:DatatypeProperty ;
                rdfs:range xsd:boolean ;
                rdfs:comment "Indication whether this object is designed to serve as an exit in the case of fire (TRUE) or not (FALSE). Here whether the transport element (in case of e.g., a lift) is designed to serve as a fire exit, e.g., for fire escape purposes."@en ;
                rdfs:label "fire exit"@en .


###  https://saref.etsi.org/saref4bldg/flowArrangement
s4bldg:flowArrangement rdf:type owl:DatatypeProperty ;
                       rdfs:range xsd:string ;
                       rdfs:comment "CounterFlow: Air and water flow enter in different directions. CrossFlow: Air and water flow are perpendicular. ParallelFlow: air and water flow enter in same directions."@en ;
                       rdfs:label "flow arrangement"@en .


###  https://saref.etsi.org/saref4bldg/frameSize
s4bldg:frameSize rdf:type owl:DatatypeProperty ;
                 rdfs:range xsd:string ;
                 rdfs:comment "Designation of the frame size according to the named range of frame sizes designated at the place of use or according to a given standard."@en ;
                 rdfs:label "frame size"@en .


###  https://saref.etsi.org/saref4bldg/frameType
s4bldg:frameType rdf:type owl:DatatypeProperty ;
                 rdfs:range xsd:string ;
                 rdfs:comment "The type of frame used by the damper (e.g., Standard, Single Flange, Single Reversed Flange, Double Flange, etc.)."@en ;
                 rdfs:label "frame type"@en .


###  https://saref.etsi.org/saref4bldg/hasDefrost
s4bldg:hasDefrost rdf:type owl:DatatypeProperty ;
                  rdfs:range xsd:boolean ;
                  rdfs:comment "Whether the heat exchanger has defrost function or not."@en ;
                  rdfs:label "has defrost"@en .


###  https://saref.etsi.org/saref4bldg/hasExteriorInsulation
s4bldg:hasExteriorInsulation rdf:type owl:DatatypeProperty ;
                             rdfs:range xsd:boolean ;
                             rdfs:comment "TRUE if the silencer has exterior insulation. FALSE if it does not."@en ;
                             rdfs:label "has exterior insulation"@en .


###  https://saref.etsi.org/saref4bldg/hasHotGasBypass
s4bldg:hasHotGasBypass rdf:type owl:DatatypeProperty ;
                       rdfs:range xsd:boolean ;
                       rdfs:comment "Whether or not hot gas bypass is provided for the compressor. TRUE = Yes, FALSE = No."@en ;
                       rdfs:label "has hot gas bypass"@en .


###  https://saref.etsi.org/saref4bldg/hasLock
s4bldg:hasLock rdf:type owl:DatatypeProperty ;
               rdfs:range xsd:boolean ;
               rdfs:comment "Indication of whether a switching device has a key operated lock (=TRUE) or not (= FALSE)."@en ;
               rdfs:label "has lock"@en .


###  https://saref.etsi.org/saref4bldg/hasPartWinding
s4bldg:hasPartWinding rdf:type owl:DatatypeProperty ;
                      rdfs:range xsd:boolean ;
                      rdfs:comment "Indication of whether the motor is single speed, i.e. has a single winding (= FALSE) or multi-speed i.e.has part winding (= TRUE) ."@en ;
                      rdfs:label "has part winding"@en .


###  https://saref.etsi.org/saref4bldg/hasTurbulator
s4bldg:hasTurbulator rdf:type owl:DatatypeProperty ;
                     rdfs:range xsd:boolean ;
                     rdfs:comment "TRUE if the tube has a turbulator, FALSE if it does not."@en ;
                     rdfs:label "has turbulator"@en .


###  https://saref.etsi.org/saref4bldg/heatTransferDimension
s4bldg:heatTransferDimension rdf:type owl:DatatypeProperty ;
                             rdfs:range xsd:string ;
                             rdfs:comment "Indicates how heat is transmitted according to the shape of the space heater."@en ;
                             rdfs:label "heat transfer dimension"@en .


###  https://saref.etsi.org/saref4bldg/heatTransferMedium
s4bldg:heatTransferMedium rdf:type owl:DatatypeProperty ;
                          rdfs:range xsd:string ;
                          rdfs:comment "Enumeration defining the heat transfer medium if applicable."@en ;
                          rdfs:label "heat transfer medium"@en .


###  https://saref.etsi.org/saref4bldg/heatTransferTypeEnum
s4bldg:heatTransferTypeEnum rdf:type owl:DatatypeProperty ;
                            rdfs:range xsd:string ;
                            rdfs:comment "Type of heat transfer between the two air streams."@en ;
                            rdfs:label "heat transfer type enum"@en .


###  https://saref.etsi.org/saref4bldg/integratedLightingType
s4bldg:integratedLightingType rdf:type owl:DatatypeProperty ;
                              rdfs:range xsd:string ;
                              rdfs:comment "Integrated lighting in cooled beam."@en ;
                              rdfs:label "integrated lighting type"@en .


###  https://saref.etsi.org/saref4bldg/internalControl
s4bldg:internalControl rdf:type owl:DatatypeProperty ;
                       rdfs:range xsd:string ;
                       rdfs:comment "Internal modulation control."@en ;
                       rdfs:label "internal control"@en .


###  https://saref.etsi.org/saref4bldg/isExternal
s4bldg:isExternal rdf:type owl:DatatypeProperty ;
                  rdfs:range xsd:boolean ;
                  rdfs:comment "Indication whether the element is designed for use in the exterior (TRUE) or not (FALSE). If (TRUE) it is an external element and faces the outside of the building."@en ;
                  rdfs:label "is external"@en .


###  https://saref.etsi.org/saref4bldg/isFreeHanging
s4bldg:isFreeHanging rdf:type owl:DatatypeProperty ;
                     rdfs:range xsd:boolean ;
                     rdfs:comment "Is it free hanging type (not mounted in a false ceiling)?"@en ;
                     rdfs:label "is free hanging"@en .


###  https://saref.etsi.org/saref4bldg/isGuarded
s4bldg:isGuarded rdf:type owl:DatatypeProperty ;
                 rdfs:range xsd:boolean ;
                 rdfs:comment "Indication of whether the motor enclosure is guarded (= TRUE) or not (= FALSE)."@en ;
                 rdfs:label "is guarded"@en .


###  https://saref.etsi.org/saref4bldg/isIlluminated
s4bldg:isIlluminated rdf:type owl:DatatypeProperty ;
                     rdfs:range xsd:boolean ;
                     rdfs:comment "An indication of whether there is an illuminated indicator to show that the switch is on (=TRUE) or not (= FALSE)."@en ;
                     rdfs:label "is illuminated"@en .


###  https://saref.etsi.org/saref4bldg/isNeutralPrimaryTerminalAvailable
s4bldg:isNeutralPrimaryTerminalAvailable rdf:type owl:DatatypeProperty ;
                                         rdfs:range xsd:boolean ;
                                         rdfs:comment "An indication of whether the neutral point of the primary winding is available as a terminal (=TRUE) or not (= FALSE)."@en ;
                                         rdfs:label "is neutral primary terminal available"@en .


###  https://saref.etsi.org/saref4bldg/isNeutralSecondaryTerminalAvailable
s4bldg:isNeutralSecondaryTerminalAvailable rdf:type owl:DatatypeProperty ;
                                           rdfs:range xsd:boolean ;
                                           rdfs:comment "An indication of whether the neutral point of the secondary winding is available as a terminal (=TRUE) or not (= FALSE)."@en ;
                                           rdfs:label "is neutral secondary terminal available"@en .


###  https://saref.etsi.org/saref4bldg/isPluggableOutlet
s4bldg:isPluggableOutlet rdf:type owl:DatatypeProperty ;
                         rdfs:range xsd:boolean ;
                         rdfs:comment "Indication of whether the outlet accepts a loose plug connection (= TRUE) or whether it is directly connected (= FALSE) or whether the form of connection has not yet been determined (= UNKNOWN)."@en ;
                         rdfs:label "is pluggable outlet"@en .


###  https://saref.etsi.org/saref4bldg/isWaterStorageHeater
s4bldg:isWaterStorageHeater rdf:type owl:DatatypeProperty ;
                            rdfs:range xsd:boolean ;
                            rdfs:comment "This is used to identify if the boiler has storage capacity (TRUE). If FALSE, then there is no storage capacity built into the boiler, such as an instantaneous hot water heater."@en ;
                            rdfs:label "is water storage heater"@en .


###  https://saref.etsi.org/saref4bldg/lampBallastType
s4bldg:lampBallastType rdf:type owl:DatatypeProperty ;
                       rdfs:range xsd:string ;
                       rdfs:comment "The type of ballast used to stabilise gas discharge by limiting the current during operation and to deliver the necessary striking voltage for starting. Ballasts are needed to operate Discharge Lamps such as Fluorescent, Compact Fluorescent, High-pressure Mercury, Metal Halide and High-pressure Sodium Lamps. Magnetic ballasts are chokes which limit the current passing through a lamp connected in series on the principle of self-induction. The resultant current and power are decisive for the efficient operation of the lamp. A specially designed ballast is required for every type of lamp to comply with lamp rating in terms of Luminous Flux, Color Appearance and service life. The two types of magnetic ballasts for fluorescent lamps are KVG Conventional (EC-A series) and VVG Low-loss ballasts (EC-B series). Low-loss ballasts have a higher efficiency, which means reduced ballast losses and a lower thermal load. Electronic ballasts are used to run fluorescent lamps at high frequencies (approx. 35 - 40 kHz)."@en ;
                       rdfs:label "lamp ballast type"@en .


###  https://saref.etsi.org/saref4bldg/lampCompensationType
s4bldg:lampCompensationType rdf:type owl:DatatypeProperty ;
                            rdfs:range xsd:string ;
                            rdfs:comment "Identifies the form of compensation used for power factor correction and radio suppression."@en ;
                            rdfs:label "lamp compensation type"@en .


###  https://saref.etsi.org/saref4bldg/legend
s4bldg:legend rdf:type owl:DatatypeProperty ;
              rdfs:range xsd:string ;
              rdfs:comment "A text inscribed or applied to the switch as a legend to indicate purpose or function."@en ;
              rdfs:label "legend"@en .


###  https://saref.etsi.org/saref4bldg/manualOverride
s4bldg:manualOverride rdf:type owl:DatatypeProperty ;
                      rdfs:range xsd:boolean ;
                      rdfs:comment "Identifies whether hand-operated operation is provided as an override (= TRUE) or not (= FALSE). Note that this value should be set to FALSE by default in the case of a Hand Operated Actuator."@en ;
                      rdfs:label "manual override"@en .


###  https://saref.etsi.org/saref4bldg/mechanicalOperated
s4bldg:mechanicalOperated rdf:type owl:DatatypeProperty ;
                          rdfs:range xsd:boolean ;
                          rdfs:comment "Indication whether the element is operated machanically (TRUE) or not, i.e. manually (FALSE)."@en ;
                          rdfs:label "mechanical operated"@en .


###  https://saref.etsi.org/saref4bldg/mediaSource
s4bldg:mediaSource rdf:type owl:DatatypeProperty ;
                   rdfs:range xsd:string ;
                   rdfs:comment "Indicates media sources and corresponding names of ports (DistributionPort with FlowDirection=SINK and PredefinedType=AUDIOVISUAL) or aggregated audio/video components (AudioVisualAppliance)."@en ;
                   rdfs:label "media source"@en .


###  https://saref.etsi.org/saref4bldg/motorDriveType
s4bldg:motorDriveType rdf:type owl:DatatypeProperty ;
                      rdfs:range xsd:string ;
                      rdfs:comment "Motor drive type: DIRECTDRIVE: Direct drive. BELTDRIVE: Belt drive. COUPLING: Coupling. OTHER: Other type of motor drive. UNKNOWN: Unknown motor drive type. "@en ;
                      rdfs:label "motor drive type"@en .


###  https://saref.etsi.org/saref4bldg/motorEnclosureType
s4bldg:motorEnclosureType rdf:type owl:DatatypeProperty ;
                          rdfs:range xsd:string ;
                          rdfs:comment "A list of the available types of motor enclosure from which that required may be selected."@en ;
                          rdfs:label "motor enclosure type"@en .


###  https://saref.etsi.org/saref4bldg/numberOfBlades
s4bldg:numberOfBlades rdf:type owl:DatatypeProperty ;
                      rdfs:range xsd:integer ;
                      rdfs:comment "Number of blades."@en ;
                      rdfs:label "number of blades"@en .


###  https://saref.etsi.org/saref4bldg/numberOfCells
s4bldg:numberOfCells rdf:type owl:DatatypeProperty ;
                     rdfs:range xsd:integer ;
                     rdfs:comment "Number of cells in one cooling tower unit."@en ;
                     rdfs:label "number of cells"@en .


###  https://saref.etsi.org/saref4bldg/numberOfCircuits
s4bldg:numberOfCircuits rdf:type owl:DatatypeProperty ;
                        rdfs:range xsd:integer ;
                        rdfs:comment "Number of parallel fluid tube circuits."@en ;
                        rdfs:label "number of circuits"@en .


###  https://saref.etsi.org/saref4bldg/numberOfGangs
s4bldg:numberOfGangs rdf:type owl:DatatypeProperty ;
                     rdfs:range xsd:integer ;
                     rdfs:comment "Number of gangs/buttons on this switch."@en ;
                     rdfs:label "number of gangs"@en .


###  https://saref.etsi.org/saref4bldg/numberOfPanels
s4bldg:numberOfPanels rdf:type owl:DatatypeProperty ;
                      rdfs:range xsd:integer ;
                      rdfs:comment "Number of panels."@en ;
                      rdfs:label "number of panels"@en .


###  https://saref.etsi.org/saref4bldg/numberOfRows
s4bldg:numberOfRows rdf:type owl:DatatypeProperty ;
                    rdfs:range xsd:integer ;
                    rdfs:comment "Number of tube rows in the tube bundle assembly."@en ;
                    rdfs:label "number of rows"@en .


###  https://saref.etsi.org/saref4bldg/numberOfSections
s4bldg:numberOfSections rdf:type owl:DatatypeProperty ;
                        rdfs:range xsd:integer ;
                        rdfs:comment "Number of sections used."@en ;
                        rdfs:label "number of sections"@en .


###  https://saref.etsi.org/saref4bldg/numberOsSockets
s4bldg:numberOsSockets rdf:type owl:DatatypeProperty ;
                       rdfs:range xsd:integer ;
                       rdfs:comment "The number of sockets that may be connected. In case of inconsistency, sockets defined on ports take precedence."@en ;
                       rdfs:label "number os sockets"@en .


###  https://saref.etsi.org/saref4bldg/operatingMode
s4bldg:operatingMode rdf:type owl:DatatypeProperty ;
                     rdfs:range xsd:string ;
                     rdfs:comment "Identifies the operating mode of the boiler."@en ;
                     rdfs:label "operating mode"@en .


###  https://saref.etsi.org/saref4bldg/operation
s4bldg:operation rdf:type owl:DatatypeProperty ;
                 rdfs:range xsd:string ;
                 rdfs:comment "The operational mechanism for the damper operation."@en ;
                 rdfs:label "operation"@en .


###  https://saref.etsi.org/saref4bldg/orientation
s4bldg:orientation rdf:type owl:DatatypeProperty ;
                   rdfs:range xsd:string ;
                   rdfs:comment "The intended orientation for the damper as specified by the manufacturer."@en ;
                   rdfs:label "orientation"@en .


###  https://saref.etsi.org/saref4bldg/patternType
s4bldg:patternType rdf:type owl:DatatypeProperty ;
                   rdfs:range xsd:string ;
                   rdfs:comment "Defines the types of pattern (or shape of a tank that may be specified."@en ;
                   rdfs:label "pattern type"@en .


###  https://saref.etsi.org/saref4bldg/pipeConnectionEnum
s4bldg:pipeConnectionEnum rdf:type owl:DatatypeProperty ;
                          rdfs:range xsd:string ;
                          rdfs:comment "The manner in which the pipe connection is made to the cooled beam."@en ;
                          rdfs:label "pipe connection enum"@en .


###  https://saref.etsi.org/saref4bldg/placementType
s4bldg:placementType rdf:type owl:DatatypeProperty ;
                     rdfs:range xsd:string ;
                     rdfs:comment "Indicates how the device is designed to be placed."@en ;
                     rdfs:label "placement type"@en .


###  https://saref.etsi.org/saref4bldg/powerSource
s4bldg:powerSource rdf:type owl:DatatypeProperty ;
                   rdfs:range xsd:string ;
                   rdfs:comment "Type of power driving the compressor."@en ;
                   rdfs:label "power source"@en .


###  https://saref.etsi.org/saref4bldg/readOutType
s4bldg:readOutType rdf:type owl:DatatypeProperty ;
                   rdfs:range xsd:string ;
                   rdfs:comment "Indication of the form that readout from the meter takes. In the case of a dial read out, this may comprise multiple dials that give a cumulative reading and/or a mechanical odometer."@en ;
                   rdfs:label "read out type"@en .


###  https://saref.etsi.org/saref4bldg/refrigerantClass
s4bldg:refrigerantClass rdf:type owl:DatatypeProperty ;
                        rdfs:range xsd:string ;
                        rdfs:comment "Refrigerant class used by the compressor. CFC: Chlorofluorocarbons. HCFC: Hydrochlorofluorocarbons. HFC: Hydrofluorocarbons."@en ;
                        rdfs:label "refrigerant class"@en .


###  https://saref.etsi.org/saref4bldg/remoteReading
s4bldg:remoteReading rdf:type owl:DatatypeProperty ;
                     rdfs:range xsd:boolean ;
                     rdfs:comment "Indicates whether the meter has a connection for remote reading through connection of a communication device (set TRUE) or not (set FALSE)."@en ;
                     rdfs:label "remote reading"@en .


###  https://saref.etsi.org/saref4bldg/roughness
s4bldg:roughness rdf:type owl:DatatypeProperty ;
                 rdfs:range xsd:string ;
                 rdfs:comment "A measure of the vertical deviations of the surface."@en ;
                 rdfs:label "roughness"@en .


###  https://saref.etsi.org/saref4bldg/secondaryCurrentType
s4bldg:secondaryCurrentType rdf:type owl:DatatypeProperty ;
                            rdfs:range xsd:string ;
                            rdfs:comment "A list of the secondary current types that can result from transformer output."@en ;
                            rdfs:label "secondary current type"@en .


###  https://saref.etsi.org/saref4bldg/shadingDeviceType
s4bldg:shadingDeviceType rdf:type owl:DatatypeProperty ;
                         rdfs:range xsd:string ;
                         rdfs:comment "Specifies the type of shading device."@en ;
                         rdfs:label "shading device type"@en .


###  https://saref.etsi.org/saref4bldg/sprayType
s4bldg:sprayType rdf:type owl:DatatypeProperty ;
                 rdfs:range xsd:string ;
                 rdfs:comment "SprayFilled: Water is sprayed into airflow. SplashTypeFill: water cascades over successive rows of splash bars. FilmTypeFill: water flows in a thin layer over closely spaced sheets."@en ;
                 rdfs:label "spray type"@en .


###  https://saref.etsi.org/saref4bldg/standard
s4bldg:standard rdf:type owl:DatatypeProperty ;
                rdfs:range xsd:string ;
                rdfs:comment "The designation of the standard applicable for the definition of the characteristics of the unit."@en ;
                rdfs:label "standard"@en .


###  https://saref.etsi.org/saref4bldg/storageType
s4bldg:storageType rdf:type owl:DatatypeProperty ;
                   rdfs:range xsd:string ;
                   rdfs:comment "Defines the general material category intended to be stored."@en ;
                   rdfs:label "storage type"@en .


###  https://saref.etsi.org/saref4bldg/switchFunction
s4bldg:switchFunction rdf:type owl:DatatypeProperty ;
                      rdfs:range xsd:string ;
                      rdfs:comment "Indicates types of switches which differs in functionality."@en ;
                      rdfs:label "switch function"@en .


###  https://saref.etsi.org/saref4bldg/temperatureClassification
s4bldg:temperatureClassification rdf:type owl:DatatypeProperty ;
                                 rdfs:range xsd:string ;
                                 rdfs:comment "Enumeration defining the temperature classification of the space heater surface temperature. low temperature - surface temperature is relatively low, usually heated by hot water or electricity. high temperature - surface temperature is relatively high, usually heated by gas or steam."@en ;
                                 rdfs:label "temperature classification"@en .


###  https://saref.etsi.org/saref4bldg/transformerVectorGroup
s4bldg:transformerVectorGroup rdf:type owl:DatatypeProperty ;
                              rdfs:range xsd:string ;
                              rdfs:comment "List of the possible vector groups for the transformer from which that required may be set. Values in the enumeration list follow a standard international code where the first letter describes how the primary windings are connected, the second letter describes how the secondary windings are connected, and the numbers describe the rotation of voltages and currents from the primary to the secondary side in multiples of 30 degrees. D: means that the windings are delta-connected. Y: means that the windings are star-connected. Z: means that the windings are zig-zag connected (a special start-connected providing low reactance of the transformer). The connectivity is only relevant for three-phase transformers."@en ;
                              rdfs:label "transformer vector group"@en .


###  https://saref.etsi.org/saref4bldg/valveMechanism
s4bldg:valveMechanism rdf:type owl:DatatypeProperty ;
                      rdfs:range xsd:string ;
                      rdfs:comment "The mechanism by which the valve function is achieved where: BALL: Valve that has a ported ball that can be turned relative to the body seat ports. BUTTERFLY: Valve in which a streamlined disc pivots about a diametric axis. CONFIGUREDGATE: Screwdown valve in which the closing gate is shaped in a configured manner to have a more precise control of pressure and flow change across the valve. GLAND: Valve with a tapered seating, in which a rotatable plug is retained by means of a gland and gland packing. GLOBE: Screwdown valve that has a spherical body. LUBRICATEDPLUG: Plug valve in which a lubricant is injected under pressure between the plug face and the body. NEEDLE: Valve for regulating the flow in or from a pipe, in which a slender cone moves along the axis of flow to close against a fixed conical seat. PARALLELSLIDE: Screwdown valve that has a machined plate that slides in formed grooves to form a seal. PLUG: Valve that has a ported plug that can be turned relative to the body seat ports. WEDGEGATE: Screwdown valve that has a wedge shaped plate fitting into tapered guides to form a seal."@en ;
                      rdfs:label "valve mechanism"@en .


###  https://saref.etsi.org/saref4bldg/valveOperation
s4bldg:valveOperation rdf:type owl:DatatypeProperty ;
                      rdfs:range xsd:string ;
                      rdfs:comment "The method of valve operation where: DROPWEIGHT: A valve that is closed by the action of a weighted lever being released, the weight normally being prevented from dropping by being held by a wire, the closure normally being made by the action of heat on a fusible link in the wire FLOAT: A valve that is opened and closed by the action of a float that rises and falls with water level. The float may be a ball attached to a lever or other mechanism HYDRAULIC: A valve that is opened and closed by hydraulic actuation LEVER: A valve that is opened and closed by the action of a lever rotating the gate within the valve. LOCKSHIELD: A valve that requires the use of a special lockshield key for opening and closing, the operating mechanism being protected by a shroud during normal operation. MOTORIZED: A valve that is opened and closed by the action of an electric motor on an actuator PNEUMATIC: A valve that is opened and closed by pneumatic actuation SOLENOID: A valve that is normally held open by a magnetic field in a coil acting on the gate but that is closed immediately if the electrical current generating the magnetic field is removed. SPRING: A valve that is normally held in position by the pressure of a spring on a plate but that may be caused to open if the pressure of the fluid is sufficient to overcome the spring pressure. THERMOSTATIC: A valve in which the ports are opened or closed to maintain a required predetermined temperature. WHEEL: A valve that is opened and closed by the action of a wheel moving the gate within the valve."@en ;
                      rdfs:label "valve operation"@en .


###  https://saref.etsi.org/saref4bldg/valvePattern
s4bldg:valvePattern rdf:type owl:DatatypeProperty ;
                    rdfs:range xsd:string ;
                    rdfs:comment "The configuration of the ports of a valve according to either the linear route taken by a fluid flowing through the valve or by the number of ports where: SINGLEPORT: Valve that has a single entry port from the system that it serves, the exit port being to the surrounding environment. ANGLED_2_PORT: Valve in which the direction of flow is changed through 90 degrees. STRAIGHT_2_PORT: Valve in which the flow is straight through. STRAIGHT_3_PORT: Valve with three separate ports. CROSSOVER_4_PORT: Valve with 4 separate ports."@en ;
                    rdfs:label "valve pattern"@en .


###  https://saref.etsi.org/saref4bldg/waterFlowControlSystemType
s4bldg:waterFlowControlSystemType rdf:type owl:DatatypeProperty ;
                                  rdfs:range xsd:string ;
                                  rdfs:comment "Factory fitted waterflow control system."@en ;
                                  rdfs:label "water flow control system type"@en .


###  https://saref.etsi.org/saref4city/hasCreationDate
s4city:hasCreationDate rdf:type owl:DatatypeProperty ;
                       rdfs:range xsd:dateTime ;
                       rdfs:isDefinedBy s4city: ;
                       rdfs:label "has creation date"@en .


###  https://saref.etsi.org/saref4city/hasExpirationDate
s4city:hasExpirationDate rdf:type owl:DatatypeProperty ;
                         rdfs:range xsd:dateTime ;
                         rdfs:isDefinedBy s4city: ;
                         rdfs:label "has expiration date"@en .


###  https://saref.etsi.org/saref4city/hasLastUpdateDate
s4city:hasLastUpdateDate rdf:type owl:DatatypeProperty ;
                         rdfs:range xsd:dateTime ;
                         rdfs:isDefinedBy s4city: ;
                         rdfs:label "has last update date"@en .


###  https://saref.etsi.org/saref4watr/forDayInMonth
s4watr:forDayInMonth rdf:type owl:DatatypeProperty ;
                     rdfs:domain s4watr:TimeBasedTariff ;
                     rdfs:range xsd:gDay ;
                     rdfs:comment "The day of the month for which a tariff is applied (e.g., each 15)."@en ;
                     rdfs:label "for day in month"@en .


###  https://saref.etsi.org/saref4watr/forFinancialConsumption
s4watr:forFinancialConsumption rdf:type owl:DatatypeProperty ;
                               rdfs:domain s4watr:ConsumptionBasedTariff ;
                               rdfs:comment "The financial consumption related to a tariff (e.g., prepaid tariffs)."@en ;
                               rdfs:label "for financial consumption"@en .


###  https://saref.etsi.org/saref4watr/forVolumeConsumption
s4watr:forVolumeConsumption rdf:type owl:DatatypeProperty ;
                            rdfs:domain s4watr:ConsumptionBasedTariff ;
                            rdfs:comment "The volume consumption related to a tariff (e.g., after consumption of 900 litres)."@en ;
                            rdfs:label "for volume consumption"@en .


###  https://saref.etsi.org/saref4watr/forVolumeFlow
s4watr:forVolumeFlow rdf:type owl:DatatypeProperty ;
                     rdfs:domain s4watr:ThresholdBasedTariff ;
                     rdfs:comment "The volume flow related to a tariff."@en ;
                     rdfs:label "for volume flow"@en .


###  https://saref.etsi.org/saref4watr/hasBillingDate
s4watr:hasBillingDate rdf:type owl:DatatypeProperty ;
                      rdfs:domain s4watr:Tariff ;
                      rdfs:range xsd:dateTime ;
                      rdfs:comment "The billing date of a tariff."@en ;
                      rdfs:label "has billing date"@en .


###  https://saref.etsi.org/saref4watr/hasFabricationNumber
s4watr:hasFabricationNumber rdf:type owl:DatatypeProperty ;
                            rdfs:range rdfs:Literal ;
                            rdfs:comment "The fabrication number of a device."@en ;
                            rdfs:label "has fabrication number"@en .


###  https://saref.etsi.org/saref4watr/hasFirmwareVersion
s4watr:hasFirmwareVersion rdf:type owl:DatatypeProperty ;
                          rdfs:range rdfs:Literal ;
                          rdfs:comment "The firmware version of a device."@en ;
                          rdfs:label "has firmware version"@en .


###  https://saref.etsi.org/saref4watr/hasHardwareVersion
s4watr:hasHardwareVersion rdf:type owl:DatatypeProperty ;
                          rdfs:range rdfs:Literal ;
                          rdfs:comment "The hardware version of a device."@en ;
                          rdfs:label "has hardware version"@en .


###  https://saref.etsi.org/saref4watr/hasStartTimestamp
s4watr:hasStartTimestamp rdf:type owl:DatatypeProperty ;
                         rdfs:domain s4watr:Tariff ;
                         rdfs:range xsd:dateTime ;
                         rdfs:comment "The start date and time of a tariff."@en ;
                         rdfs:label "has start timestamp"@en .


###  https://saref.etsi.org/saref4watr/hasVersion
s4watr:hasVersion rdf:type owl:DatatypeProperty ;
                  rdfs:range rdfs:Literal ;
                  rdfs:comment "The version of a device."@en ;
                  rdfs:label "has version"@en .


###  https://saref.etsi.org/saref4watr/operatesAtRadioFrequency
s4watr:operatesAtRadioFrequency rdf:type owl:DatatypeProperty ;
                                rdfs:comment "The radio frequency at which a device operates."@en ;
                                rdfs:label "operates at radio frequency"@en .


###  https://saref.etsi.org/saref4watr/requiresPower
s4watr:requiresPower rdf:type owl:DatatypeProperty ;
                     rdfs:comment "The power required by a device."@en ;
                     rdfs:label "requires power"@en .


###  https://www.geonames.org/ontology#name
gn:name rdf:type owl:DatatypeProperty .


###  https://www.geonames.org/ontology#postalCode
gn:postalCode rdf:type owl:DatatypeProperty .


#################################################################
#    Classes
#################################################################

###  http://bigg-project.eu/ontology#Area
bigg:Area rdf:type owl:Class ;
          rdfs:subClassOf saref:Property ;
          rdfs:comment "A saref:Property related to some measurements that are characterized by a certain value measured in an energy unit (such as Kilowatt_Hour or Watt_hour). Furter specializations of the saref:Energy class can be found in the SAREF4ENER extension, where classes such as EnergyMax, EnergyMin and EnergyExpected are defined. "@en .


###  http://bigg-project.eu/ontology#EnergyAsset
bigg:EnergyAsset rdf:type owl:Class ;
                 rdfs:subClassOf geosp:Feature ,
                                 saref:FeatureOfInterest ,
                                 s4syst:System ;
                 rdfs:comment "A energy asset is a physical entity used in the process of transporting, treating, storing and distributing energy."@en ;
                 rdfs:label "Energy asset"@en .


###  http://bigg-project.eu/ontology#EnergyDevice
bigg:EnergyDevice rdf:type owl:Class ;
                  rdfs:subClassOf bigg:EnergyAsset ,
                                  saref:Device ;
                  rdfs:comment "An energy device is a device that is also an energy asset."@en ;
                  rdfs:label "Energy device"@en .


###  http://bigg-project.eu/ontology#EnergyMeter
bigg:EnergyMeter rdf:type owl:Class ;
                 rdfs:subClassOf bigg:EnergyDevice ,
                                 saref:Meter ,
                                 [ rdf:type owl:Restriction ;
                                   owl:onProperty saref:measuresProperty ;
                                   owl:someValuesFrom saref:Energy
                                 ] ,
                                 [ rdf:type owl:Restriction ;
                                   owl:onProperty saref:hasProperty ;
                                   owl:allValuesFrom s4watr:WaterMeterProperty
                                 ] ,
                                 [ rdf:type owl:Restriction ;
                                   owl:onProperty s4watr:hasFabricationNumber ;
                                   owl:maxCardinality "1"^^xsd:nonNegativeInteger
                                 ] ,
                                 [ rdf:type owl:Restriction ;
                                   owl:onProperty s4watr:hasFirmwareVersion ;
                                   owl:maxCardinality "1"^^xsd:nonNegativeInteger
                                 ] ,
                                 [ rdf:type owl:Restriction ;
                                   owl:onProperty s4watr:hasHardwareVersion ;
                                   owl:maxCardinality "1"^^xsd:nonNegativeInteger
                                 ] ,
                                 [ rdf:type owl:Restriction ;
                                   owl:onProperty s4watr:hasVersion ;
                                   owl:maxCardinality "1"^^xsd:nonNegativeInteger
                                 ] ;
                 rdfs:comment "A energy meter is an instrument intended to measure continuously, memorize, and display the amouint of energy passing through the meter."@en ;
                 rdfs:label "Energy meter"@en .


###  http://bigg-project.eu/ontology#Patrimony
bigg:Patrimony rdf:type owl:Class ;
               rdfs:subClassOf geosp:Feature ,
                               [ rdf:type owl:Restriction ;
                                 owl:onProperty s4agri:contains ;
                                 owl:someValuesFrom s4agri:Building
                               ] ,
                               [ rdf:type owl:Restriction ;
                                 owl:onProperty s4agri:contains ;
                                 owl:someValuesFrom s4agri:Parcel
                               ] ,
                               [ rdf:type owl:Restriction ;
                                 owl:onProperty s4agri:hasName ;
                                 owl:maxCardinality "1"^^xsd:nonNegativeInteger
                               ] ;
               rdfs:comment "A set of real properties which can contain buildings and parcels."@en .


###  http://purl.obolibrary.org/obo/TAXRANK_0000000
<http://purl.obolibrary.org/obo/TAXRANK_0000000> rdf:type owl:Class ;
                                                 rdfs:label "Taxon rank"@en .


###  http://www.opengis.net/ont/geosparql#Feature
geosp:Feature rdf:type owl:Class ;
              rdfs:subClassOf geosp:SpatialObject ,
                              [ rdf:type owl:Restriction ;
                                owl:onProperty geosp:hasGeometry ;
                                owl:allValuesFrom geosp:Geometry
                              ] ;
              owl:disjointWith geosp:Geometry ;
              rdfs:comment "This class represents the top-level feature type. This class is equivalent to GFI_Feature defined in ISO 19156:2011, and it is superclass of all feature types."@en ;
              rdfs:isDefinedBy <http://www.opengis.net/ont/geosparql> ,
                               <http://www.opengis.net/ont/gml> ,
                               geosp: ,
                               <http://www.opengis.net/spec/geosparql/1.0/req/core/feature-class> ,
                               <http://www.opengis.net/spec/geosparql/1.1/req/core/feature-class> ;
              rdfs:label "Feature"@en ;
              skos:definition "A discrete spatial phenomenon in a universe of discourse."@en ;
              skos:example <http://www.opengis.net/spec/geosparql/1.1/specification.html#B.1.1.2.1> ,
                           <http://www.opengis.net/spec/geosparql/1.1/specification.html#B.1.1.2.2> ,
                           <http://www.opengis.net/spec/geosparql/1.1/specification.html#B.1.1.2.3> ,
                           <http://www.opengis.net/spec/geosparql/1.1/specification.html#B.1.1.2.4> ,
                           <http://www.opengis.net/spec/geosparql/1.1/specification.html#B.1.1.2.5> ,
                           <http://www.opengis.net/spec/geosparql/1.1/specification.html#B.1.1.2.6> ,
                           <http://www.opengis.net/spec/geosparql/1.1/specification.html#B.1.1.2.7> ,
                           <http://www.opengis.net/spec/geosparql/1.1/specification.html#B.1.1.2.8> ,
                           <http://www.opengis.net/spec/geosparql/1.1/specification.html#B.1.1.2.9> ,
                           <http://www.opengis.net/spec/geosparql/1.1/specification.html#B.1.1.3.2> ,
                           <http://www.opengis.net/spec/geosparql/1.1/specification.html#B.1.1.3.3> ,
                           <http://www.opengis.net/spec/geosparql/1.1/specification.html#B.1.2.2> ,
                           <http://www.opengis.net/spec/geosparql/1.1/specification.html#B.1.2.3> ,
                           <http://www.opengis.net/spec/geosparql/1.1/specification.html#B.1.2.4> ;
              skos:note "A Feature represents a uniquely identifiable phenomenon, for example a river or an apple. While such phenomena (and therefore the Features used to represent them) are bounded, their boundaries may be crisp (e.g., the declared boundaries of a state), vague (e.g., the delineation of a valley versus its neighboring mountains), and change with time (e.g., a storm front). While discrete in nature, Features may be created from continuous observations, such as an isochrone that determines the region that can be reached by ambulance within 5 minutes."@en ;
              skos:prefLabel "Feature"@en .


###  http://www.opengis.net/ont/geosparql#FeatureCollection
geosp:FeatureCollection rdf:type owl:Class ;
                        rdfs:subClassOf geosp:SpatialObjectCollection ,
                                        [ rdf:type owl:Restriction ;
                                          owl:onProperty rdfs:member ;
                                          owl:allValuesFrom geosp:Feature
                                        ] ;
                        rdfs:isDefinedBy geosp: ,
                                         <http://www.opengis.net/spec/geosparql/1.1/req/core/feature-collection-class> ;
                        skos:definition "Any collection of individual Features."@en ;
                        skos:example <http://www.opengis.net/spec/geosparql/1.1/specification.html#B.1.1.6> ;
                        skos:prefLabel "Feature Collection"@en .


###  http://www.opengis.net/ont/geosparql#Geometry
geosp:Geometry rdf:type owl:Class ;
               rdfs:subClassOf geosp:SpatialObject ;
               rdfs:comment "The class represents the top-level geometry type. This class is equivalent to the UML class GM_Object defined in ISO 19107, and it is superclass of all geometry types."@en ;
               rdfs:isDefinedBy <http://www.opengis.net/ont/geosparql> ,
                                geosp: ,
                                <http://www.opengis.net/spec/geosparql/1.0/req/geometry-extension/geometry-class> ,
                                <http://www.opengis.net/spec/geosparql/1.1/req/geometry-extension/geometry-class> ;
               rdfs:label "Geometry"@en ;
               skos:definition "A coherent set of direct positions in Euclidian space. A direct position holds the coordinates for a position within a Coordinate Reference System (CRS)."@en ;
               skos:example <http://www.opengis.net/spec/geosparql/1.1/specification.html#B.1.1.2.2> ,
                            <http://www.opengis.net/spec/geosparql/1.1/specification.html#B.1.1.2.3> ,
                            <http://www.opengis.net/spec/geosparql/1.1/specification.html#B.1.1.2.4> ,
                            <http://www.opengis.net/spec/geosparql/1.1/specification.html#B.1.1.2.5> ,
                            <http://www.opengis.net/spec/geosparql/1.1/specification.html#B.1.1.2.6> ,
                            <http://www.opengis.net/spec/geosparql/1.1/specification.html#B.1.1.2.8> ,
                            <http://www.opengis.net/spec/geosparql/1.1/specification.html#B.1.1.3.1> ,
                            <http://www.opengis.net/spec/geosparql/1.1/specification.html#B.1.1.3.2> ,
                            <http://www.opengis.net/spec/geosparql/1.1/specification.html#B.1.1.3.3> ,
                            <http://www.opengis.net/spec/geosparql/1.1/specification.html#B.1.2.2> ,
                            <http://www.opengis.net/spec/geosparql/1.1/specification.html#B.1.2.3> ,
                            <http://www.opengis.net/spec/geosparql/1.1/specification.html#B.1.2.4> ;
               skos:note "Geometry can be used as a representation of the shape, extent or location of a Feature, or can exist as a self-contained entity."@en ;
               skos:prefLabel "Geometry"@en .


###  http://www.opengis.net/ont/geosparql#GeometryCollection
geosp:GeometryCollection rdf:type owl:Class ;
                         rdfs:subClassOf geosp:SpatialObjectCollection ,
                                         [ rdf:type owl:Restriction ;
                                           owl:onProperty rdfs:member ;
                                           owl:allValuesFrom geosp:Geometry
                                         ] ;
                         rdfs:isDefinedBy geosp: ,
                                          <http://www.opengis.net/spec/geosparql/1.1/req/core/geometry-collection-class> ;
                         skos:definition "Any collection of individual Geometries."@en ;
                         skos:example <http://www.opengis.net/spec/geosparql/1.1/specification.html#B.1.1.7> ;
                         skos:prefLabel "Geometry Collection"@en .


###  http://www.opengis.net/ont/geosparql#SpatialObject
geosp:SpatialObject rdf:type owl:Class ;
                    rdfs:subClassOf [ rdf:type owl:Restriction ;
                                      owl:onProperty geosp:hasGeometry ;
                                      owl:allValuesFrom geosp:Geometry
                                    ] ,
                                    [ rdf:type owl:Restriction ;
                                      owl:onProperty geosp:sfContains ;
                                      owl:allValuesFrom geosp:SpatialObject
                                    ] ,
                                    [ rdf:type owl:Restriction ;
                                      owl:onProperty geosp:sfWithin ;
                                      owl:allValuesFrom geosp:SpatialObject
                                    ] ,
                                    [ rdf:type owl:Restriction ;
                                      owl:onProperty wgs84:location ;
                                      owl:allValuesFrom wgs84:Point
                                    ] ;
                    rdfs:comment "The class spatial-object represents everything that can have a spatial representation. It is superclass of feature and geometry."@en ;
                    rdfs:isDefinedBy <http://www.opengis.net/ont/geosparql> ,
                                     geosp: ,
                                     <http://www.opengis.net/spec/geosparql/1.0/req/core/spatial-object-class> ,
                                     <http://www.opengis.net/spec/geosparql/1.1/req/core/spatial-object-class> ;
                    rdfs:label "Spatial object"@en ,
                               "SpatialObject"@en ;
                    skos:definition "Anything spatial (having or being a shape, position or an extent)."@en ;
                    skos:example <http://www.opengis.net/spec/geosparql/1.1/specification.html#B.1.1.1.1> ,
                                 <http://www.opengis.net/spec/geosparql/1.1/specification.html#B.1.1.1.2> ;
                    skos:note "Subclasses are expected to be used for instance data."@en ;
                    skos:prefLabel "Spatial Object"@en .


###  http://www.opengis.net/ont/geosparql#SpatialObjectCollection
geosp:SpatialObjectCollection rdf:type owl:Class ;
                              rdfs:subClassOf rdfs:Container ,
                                              [ rdf:type owl:Restriction ;
                                                owl:onProperty rdfs:member ;
                                                owl:allValuesFrom geosp:SpatialObject
                                              ] ;
                              rdfs:isDefinedBy geosp: ,
                                               <http://www.opengis.net/spec/geosparql/1.1/req/core/spatial-object-collection-class> ;
                              skos:definition "Any collection of individual Spatial Objects. It is superclass of Feature Collection and Geometry Collection."@en ;
                              skos:prefLabel "Spatial Object Collection"@en .


###  http://www.opengis.net/ont/sf#Point
<http://www.opengis.net/ont/sf#Point> rdf:type owl:Class ;
                                      rdfs:subClassOf geosp:Geometry ;
                                      rdfs:isDefinedBy <http://www.opengis.net/ont/sf#> ;
                                      rdfs:label "Point"@en .


###  http://www.opengis.net/ont/sf#Polygon
<http://www.opengis.net/ont/sf#Polygon> rdf:type owl:Class ;
                                        rdfs:subClassOf geosp:Geometry ;
                                        rdfs:isDefinedBy <http://www.opengis.net/ont/sf#> ;
                                        rdfs:label "Polygon"@en .


###  http://www.w3.org/2000/01/rdf-schema#Container
rdfs:Container rdf:type owl:Class .


###  http://www.w3.org/2003/01/geo/wgs84_pos#Point
wgs84:Point rdf:type owl:Class ;
            rdfs:subClassOf geosp:Geometry ,
                            wgs84:SpatialThing ;
            rdfs:comment """ 
Uniquely identified by lat/long/alt. i.e.

spaciallyIntersects(P1, P2) :- lat(P1, LAT), long(P1, LONG), alt(P1, ALT),
  lat(P2, LAT), long(P2, LONG), alt(P2, ALT).

sameThing(P1, P2) :- type(P1, Point), type(P2, Point), spaciallyIntersects(P1, P2).
  """ ,
                         "A point, typically described using a coordinate system relative to Earth, such as WGS84."@en ,
                         """A point, typically described using a coordinate system relative to Earth, such as WGS84.
  """ ;
            rdfs:isDefinedBy wgs84: ;
            rdfs:label "Point"@en ,
                       "point" .


###  http://www.w3.org/2003/01/geo/wgs84_pos#SpatialThing
wgs84:SpatialThing rdf:type owl:Class ;
                   rdfs:comment """Anything with spatial extent, i.e. size, shape, or position.
 e.g. people, places, bowling balls, as well as abstract areas like cubes.
""" ;
                   rdfs:label "SpatialThing" .


###  http://www.w3.org/2006/time#DateTimeDescription
time:DateTimeDescription rdf:type owl:Class ;
                         rdfs:subClassOf time:GeneralDateTimeDescription ,
                                         [ rdf:type owl:Restriction ;
                                           owl:onProperty time:hasTRS ;
                                           owl:hasValue <http://www.opengis.net/def/uom/ISO-8601/0/Gregorian>
                                         ] ,
                                         [ rdf:type owl:Restriction ;
                                           owl:onProperty time:day ;
                                           owl:allValuesFrom xsd:gDay
                                         ] ,
                                         [ rdf:type owl:Restriction ;
                                           owl:onProperty time:month ;
                                           owl:allValuesFrom xsd:gMonth
                                         ] ,
                                         [ rdf:type owl:Restriction ;
                                           owl:onProperty time:year ;
                                           owl:allValuesFrom xsd:gYear
                                         ] ;
                         rdfs:comment "Descripción de fecha y tiempo estructurada con valores separados para los diferentes elementos de un sistema calendario-reloj. El sistema de referencia temporal está fijado al calendario gregoriano, y el rango de las propiedades año, mes, día restringidas a los correspondientes tipos del XML Schema xsd:gYear, xsd:gMonth y xsd:gDay respectivamente."@es ,
                                      "Description of date and time structured with separate values for the various elements of a calendar-clock system. The temporal reference system is fixed to Gregorian Calendar, and the range of year, month, day properties restricted to corresponding XML Schema types xsd:gYear, xsd:gMonth and xsd:gDay, respectively."@en ;
                         rdfs:label "Date-Time description"@en ,
                                    "descripción de fecha-tiempo"@es ;
                         skos:definition "Descripción de fecha y tiempo estructurada con valores separados para los diferentes elementos de un sistema calendario-reloj. El sistema de referencia temporal está fijado al calendario gregoriano, y el rango de las propiedades año, mes, día restringidas a los correspondientes tipos del XML Schema xsd:gYear, xsd:gMonth y xsd:gDay respectivamente."@es ,
                                         "Description of date and time structured with separate values for the various elements of a calendar-clock system. The temporal reference system is fixed to Gregorian Calendar, and the range of year, month, day properties restricted to corresponding XML Schema types xsd:gYear, xsd:gMonth and xsd:gDay, respectively."@en .


###  http://www.w3.org/2006/time#DateTimeInterval
time:DateTimeInterval rdf:type owl:Class ;
                      rdfs:subClassOf time:ProperInterval ;
                      rdfs:comment "'intervalo de fecha-hora' es una subclase de 'intervalo propio', definida utilizando el multi-elemento 'descripción de fecha-hora'."@es ,
                                   "DateTimeInterval is a subclass of ProperInterval, defined using the multi-element DateTimeDescription."@en ;
                      rdfs:label "Date-time interval"@en ,
                                 "intervalo de fecha-hora"@es ;
                      skos:definition "'intervalo de fecha-hora' es una subclase de 'intervalo propio', definida utilizando el multi-elemento 'descripción de fecha-hora'."@es ,
                                      "DateTimeInterval is a subclass of ProperInterval, defined using the multi-element DateTimeDescription."@en ;
                      skos:note "'intervalo de fecha-hora' se puede utilizar sólo para un intervalo cuyos límites coinciden con un elemento de fecha-hora alineados con el calendario y la zona horaria indicados. Por ejemplo, aunque ambos tienen una duración de un día, el intervalo de 24 horas que empieza en la media noche del comienzo del 8 mayo en Europa Central se puede expresar como un 'intervalo de fecha-hora', el intervalo de 24 horas que empieza a las 1:30pm no."@es ,
                                ":DateTimeInterval can only be used for an interval whose limits coincide with a date-time element aligned to the calendar and timezone indicated. For example, while both have a duration of one day, the 24-hour interval beginning at midnight at the beginning of 8 May in Central Europe can be expressed as a :DateTimeInterval, but the 24-hour interval starting at 1:30pm cannot."@en .


###  http://www.w3.org/2006/time#DayOfWeek
time:DayOfWeek rdf:type owl:Class ;
               rdfs:subClassOf owl:Thing ;
               rdfs:comment "El día de la semana"@es ,
                            "The day of week"@en ,
                            "The day of week."@en ;
               rdfs:isDefinedBy time: ;
               rdfs:label "Day of week"@en ,
                          "día de la semana"@es ;
               skos:changeNote """Remove enumeration from definition, in order to allow other days to be used when required in other calendars. 
NOTE: existing days are still present as members of the class, but the class membership is now open. 

In the original OWL-Time the following constraint appeared: 
  owl:oneOf (
      time:Monday
      time:Tuesday
      time:Wednesday
      time:Thursday
      time:Friday
      time:Saturday
      time:Sunday
    ) ;"""@en ;
               skos:definition "El día de la semana"@es ,
                               "The day of week"@en ;
               skos:note "La pertenencia a la clase 'día de la semana' está abierta, para permitir longitudes de semana alternativas y diferentes nombres de días."@es ,
                         "Membership of the class :DayOfWeek is open, to allow for alternative week lengths and different day names."@en .


###  http://www.w3.org/2006/time#Duration
time:Duration rdf:type owl:Class ;
              rdfs:subClassOf time:TemporalDuration ,
                              [ rdf:type owl:Restriction ;
                                owl:onProperty time:unitType ;
                                owl:cardinality "1"^^xsd:nonNegativeInteger
                              ] ,
                              [ rdf:type owl:Restriction ;
                                owl:onProperty time:numericDuration ;
                                owl:cardinality "1"^^xsd:nonNegativeInteger
                              ] ;
              rdfs:comment "Duración de una extensión temporal expresada como un número escalado por una unidad temporal."@es ,
                           "Duration of a temporal extent expressed as a number scaled by a temporal unit"@en ;
              rdfs:label "Time duration"@en ,
                         "duración de tiempo" ;
              skos:definition "Duración de una extensión temporal expresada como un número escalado por una unidad temporal."@es ,
                              "Duration of a temporal extent expressed as a number scaled by a temporal unit"@en ;
              skos:note "Alternativa a 'descripción de tiempo' para proporcionar descripción soporte a una duración temporal diferente a utilizar un sistema de calendario/reloj."@es ,
                        "Alternative to time:DurationDescription to support description of a temporal duration other than using a calendar/clock system."@en .


###  http://www.w3.org/2006/time#DurationDescription
time:DurationDescription rdf:type owl:Class ;
                         rdfs:subClassOf time:GeneralDurationDescription ,
                                         [ rdf:type owl:Restriction ;
                                           owl:onProperty time:hasTRS ;
                                           owl:hasValue <http://www.opengis.net/def/uom/ISO-8601/0/Gregorian>
                                         ] ,
                                         [ rdf:type owl:Restriction ;
                                           owl:onProperty time:days ;
                                           owl:allValuesFrom xsd:decimal
                                         ] ,
                                         [ rdf:type owl:Restriction ;
                                           owl:onProperty time:hours ;
                                           owl:allValuesFrom xsd:decimal
                                         ] ,
                                         [ rdf:type owl:Restriction ;
                                           owl:onProperty time:minutes ;
                                           owl:allValuesFrom xsd:decimal
                                         ] ,
                                         [ rdf:type owl:Restriction ;
                                           owl:onProperty time:months ;
                                           owl:allValuesFrom xsd:decimal
                                         ] ,
                                         [ rdf:type owl:Restriction ;
                                           owl:onProperty time:seconds ;
                                           owl:allValuesFrom xsd:decimal
                                         ] ,
                                         [ rdf:type owl:Restriction ;
                                           owl:onProperty time:weeks ;
                                           owl:allValuesFrom xsd:decimal
                                         ] ,
                                         [ rdf:type owl:Restriction ;
                                           owl:onProperty time:years ;
                                           owl:allValuesFrom xsd:decimal
                                         ] ;
                         rdfs:comment "Descripción de extensión temporal estructurada con valores separados para los distintos elementos de un sistema de horario-calendario. El sistema de referencia temporal se fija al calendario gregoriano, y el intervalo de cada una de las propiedades numéricas se restringe a xsd:decimal."@es ,
                                      "Description of temporal extent structured with separate values for the various elements of a calendar-clock system. The temporal reference system is fixed to Gregorian Calendar, and the range of each of the numeric properties is restricted to xsd:decimal"@en ;
                         rdfs:label "Duration description"@en ,
                                    "descripción de duración"@es ;
                         skos:definition "Descripción de extensión temporal estructurada con valores separados para los distintos elementos de un sistema de horario-calendario. El sistema de referencia temporal se fija al calendario gregoriano, y el intervalo de cada una de las propiedades numéricas se restringe a xsd:decimal."@es ,
                                         "Description of temporal extent structured with separate values for the various elements of a calendar-clock system. The temporal reference system is fixed to Gregorian Calendar, and the range of each of the numeric properties is restricted to xsd:decimal"@en ;
                         skos:note "En el calendario gregoriano la longitud de los meses no es fija. Por lo tanto, un valor como \"2,5 meses\" no se puede comparar exactamente con una duración similar expresada en términos de semanas o días."@es ,
                                   "In the Gregorian calendar the length of the month is not fixed. Therefore, a value like \"2.5 months\" cannot be exactly compared with a similar duration expressed in terms of weeks or days."@en .


###  http://www.w3.org/2006/time#GeneralDateTimeDescription
time:GeneralDateTimeDescription rdf:type owl:Class ;
                                rdfs:subClassOf time:TemporalPosition ,
                                                [ rdf:type owl:Restriction ;
                                                  owl:onProperty time:unitType ;
                                                  owl:cardinality "1"^^xsd:nonNegativeInteger
                                                ] ,
                                                [ rdf:type owl:Restriction ;
                                                  owl:onProperty time:dayOfWeek ;
                                                  owl:maxCardinality "1"^^xsd:nonNegativeInteger
                                                ] ,
                                                [ rdf:type owl:Restriction ;
                                                  owl:onProperty time:monthOfYear ;
                                                  owl:maxCardinality "1"^^xsd:nonNegativeInteger
                                                ] ,
                                                [ rdf:type owl:Restriction ;
                                                  owl:onProperty time:timeZone ;
                                                  owl:maxCardinality "1"^^xsd:nonNegativeInteger
                                                ] ,
                                                [ rdf:type owl:Restriction ;
                                                  owl:onProperty time:day ;
                                                  owl:maxCardinality "1"^^xsd:nonNegativeInteger
                                                ] ,
                                                [ rdf:type owl:Restriction ;
                                                  owl:onProperty time:dayOfYear ;
                                                  owl:maxCardinality "1"^^xsd:nonNegativeInteger
                                                ] ,
                                                [ rdf:type owl:Restriction ;
                                                  owl:onProperty time:hour ;
                                                  owl:maxCardinality "1"^^xsd:nonNegativeInteger
                                                ] ,
                                                [ rdf:type owl:Restriction ;
                                                  owl:onProperty time:minute ;
                                                  owl:maxCardinality "1"^^xsd:nonNegativeInteger
                                                ] ,
                                                [ rdf:type owl:Restriction ;
                                                  owl:onProperty time:month ;
                                                  owl:maxCardinality "1"^^xsd:nonNegativeInteger
                                                ] ,
                                                [ rdf:type owl:Restriction ;
                                                  owl:onProperty time:second ;
                                                  owl:maxCardinality "1"^^xsd:nonNegativeInteger
                                                ] ,
                                                [ rdf:type owl:Restriction ;
                                                  owl:onProperty time:week ;
                                                  owl:maxCardinality "1"^^xsd:nonNegativeInteger
                                                ] ,
                                                [ rdf:type owl:Restriction ;
                                                  owl:onProperty time:year ;
                                                  owl:maxCardinality "1"^^xsd:nonNegativeInteger
                                                ] ;
                                rdfs:comment "Descripción de fecha y hora estructurada con valores separados para los distintos elementos de un sistema calendario-reloj."@es ,
                                             "Description of date and time structured with separate values for the various elements of a calendar-clock system"@en ;
                                rdfs:label "Generalized date-time description"@en ,
                                           "descripción de fecha-hora generalizada"@es ;
                                skos:definition "Descripción de fecha y hora estructurada con valores separados para los distintos elementos de un sistema calendario-reloj." ,
                                                "Description of date and time structured with separate values for the various elements of a calendar-clock system"@en ;
                                skos:note "Algunas combinaciones de propiedades son redundantes - por ejemplo, dentro de un 'año' especificado si se proporciona 'día del año' entonces 'día' y 'mes' se pueden computar, y viceversa. Los valores individuales deberían ser consistentes entre ellos y con el calendario, indicado a través del valor de la propiedad 'tiene TRS'."@es ,
                                          "Some combinations of properties are redundant - for example, within a specified :year if :dayOfYear is provided then :day and :month can be computed, and vice versa. Individual values should be consistent with each other and the calendar, indicated through the value of the :hasTRS property." .


###  http://www.w3.org/2006/time#GeneralDurationDescription
time:GeneralDurationDescription rdf:type owl:Class ;
                                rdfs:subClassOf time:TemporalDuration ,
                                                [ rdf:type owl:Restriction ;
                                                  owl:onProperty time:hasTRS ;
                                                  owl:cardinality "1"^^xsd:nonNegativeInteger
                                                ] ,
                                                [ rdf:type owl:Restriction ;
                                                  owl:onProperty time:days ;
                                                  owl:maxCardinality "1"^^xsd:nonNegativeInteger
                                                ] ,
                                                [ rdf:type owl:Restriction ;
                                                  owl:onProperty time:hours ;
                                                  owl:maxCardinality "1"^^xsd:nonNegativeInteger
                                                ] ,
                                                [ rdf:type owl:Restriction ;
                                                  owl:onProperty time:minutes ;
                                                  owl:maxCardinality "1"^^xsd:nonNegativeInteger
                                                ] ,
                                                [ rdf:type owl:Restriction ;
                                                  owl:onProperty time:months ;
                                                  owl:maxCardinality "1"^^xsd:nonNegativeInteger
                                                ] ,
                                                [ rdf:type owl:Restriction ;
                                                  owl:onProperty time:seconds ;
                                                  owl:maxCardinality "1"^^xsd:nonNegativeInteger
                                                ] ,
                                                [ rdf:type owl:Restriction ;
                                                  owl:onProperty time:weeks ;
                                                  owl:maxCardinality "1"^^xsd:nonNegativeInteger
                                                ] ,
                                                [ rdf:type owl:Restriction ;
                                                  owl:onProperty time:years ;
                                                  owl:maxCardinality "1"^^xsd:nonNegativeInteger
                                                ] ;
                                rdfs:comment "Descripción de extensión temporal estructurada con valores separados para los distintos elementos de un sistema de horario-calendario."@es ,
                                             "Description of temporal extent structured with separate values for the various elements of a calendar-clock system."@en ;
                                rdfs:label "Generalized duration description"@en ,
                                           "descripción de duración generalizada"@es ;
                                skos:definition "Descripción de extensión temporal estructurada con valores separados para los distintos elementos de un sistema de horario-calendario."@es ,
                                                "Description of temporal extent structured with separate values for the various elements of a calendar-clock system."@en ;
                                skos:note "La extensión de una duración de tiempo expresada como una 'descripción de duración general' depende del Sistema de Referencia Temporal. En algunos calendarios la longitud de la semana o del mes no es constante a lo largo del año. Por tanto, un valor como \"25 meses\" puede no ser necesariamente ser comparado con un duración similar expresada en términos de semanas o días. Cuando se consideran calendarios que no están basados en el movimiento de la Tierra, se deben tomar incluso más precauciones en la comparación de duraciones."@es ,
                                          "The extent of a time duration expressed as a GeneralDurationDescription depends on the Temporal Reference System. In some calendars the length of the week or month is not constant within the year. Therefore, a value like \"2.5 months\" may not necessarily be exactly compared with a similar duration expressed in terms of weeks or days. When non-earth-based calendars are considered even more care must be taken in comparing durations."@en .


###  http://www.w3.org/2006/time#Instant
time:Instant rdf:type owl:Class ;
             rdfs:subClassOf time:TemporalEntity ;
             owl:disjointWith time:ProperInterval ;
             rdfs:comment "A temporal entity with zero extent or duration"@en ,
                          "Una entidad temporal con una extensión o duración cero."@es ;
             rdfs:isDefinedBy time: ;
             rdfs:label "Instant"@en ,
                        "Time instant"@en ,
                        "instante de tiempo."@es ;
             skos:definition "A temporal entity with zero extent or duration"@en ,
                             "Una entidad temporal con una extensión o duración cero."@es .


###  http://www.w3.org/2006/time#Interval
time:Interval rdf:type owl:Class ;
              rdfs:subClassOf time:TemporalEntity ;
              rdfs:comment "A temporal entity with an extent or duration"@en ,
                           "A temporal entity with an extent or duration."@en ,
                           "Una entidad temporal con una extensión o duración."@es ;
              rdfs:isDefinedBy time: ;
              rdfs:label "Interval"@en ,
                         "Time interval"@en ,
                         "intervalo de tiempo"@es ;
              skos:definition "A temporal entity with an extent or duration"@en ,
                              "Una entidad temporal con una extensión o duración."@es .


###  http://www.w3.org/2006/time#January
time:January rdf:type owl:Class ;
             rdfs:subClassOf time:DateTimeDescription ,
                             [ rdf:type owl:Restriction ;
                               owl:onProperty time:unitType ;
                               owl:hasValue time:unitMonth
                             ] ,
                             [ rdf:type owl:Restriction ;
                               owl:onProperty time:month ;
                               owl:hasValue "--01"
                             ] ;
             rdfs:label "January" ;
             owl:deprecated "true"^^xsd:boolean ;
             skos:historyNote "This class was present in the 2006 version of OWL-Time. It was presented as an example of how DateTimeDescription could be specialized, but does not belong in the revised ontology. " .


###  http://www.w3.org/2006/time#MonthOfYear
time:MonthOfYear rdf:type owl:Class ;
                 rdfs:subClassOf time:DateTimeDescription ,
                                 [ rdf:type owl:Restriction ;
                                   owl:onProperty time:unitType ;
                                   owl:hasValue time:unitMonth
                                 ] ,
                                 [ rdf:type owl:Restriction ;
                                   owl:onProperty time:day ;
                                   owl:cardinality "0"^^xsd:nonNegativeInteger
                                 ] ,
                                 [ rdf:type owl:Restriction ;
                                   owl:onProperty time:hour ;
                                   owl:cardinality "0"^^xsd:nonNegativeInteger
                                 ] ,
                                 [ rdf:type owl:Restriction ;
                                   owl:onProperty time:minute ;
                                   owl:cardinality "0"^^xsd:nonNegativeInteger
                                 ] ,
                                 [ rdf:type owl:Restriction ;
                                   owl:onProperty time:month ;
                                   owl:cardinality "1"^^xsd:nonNegativeInteger
                                 ] ,
                                 [ rdf:type owl:Restriction ;
                                   owl:onProperty time:second ;
                                   owl:cardinality "0"^^xsd:nonNegativeInteger
                                 ] ,
                                 [ rdf:type owl:Restriction ;
                                   owl:onProperty time:week ;
                                   owl:cardinality "0"^^xsd:nonNegativeInteger
                                 ] ,
                                 [ rdf:type owl:Restriction ;
                                   owl:onProperty time:year ;
                                   owl:cardinality "0"^^xsd:nonNegativeInteger
                                 ] ;
                 rdfs:comment "El mes del año."@es ,
                              "The month of the year"@en ;
                 rdfs:label "Month of year"@en ,
                            "mes del año"@es ;
                 skos:definition "El mes del año."@es ,
                                 "The month of the year"@en ;
                 skos:editorialNote "Característica en riesgo - añadida en la revisión de 2017, y no utilizada todavía de forma amplia."@es ,
                                    "Feature at risk - added in 2017 revision, and not yet widely used. "@en ;
                 skos:note "La pertenencia a la clase 'mes del año' está abierta, a permitir calendarios anuales alternativos y diferentes nombres de meses."@es ,
                           "Membership of the class :MonthOfYear is open, to allow for alternative annual calendars and different month names."@en .


###  http://www.w3.org/2006/time#ProperInterval
time:ProperInterval rdf:type owl:Class ;
                    rdfs:subClassOf time:Interval ;
                    rdfs:comment "A temporal entity with non-zero extent or duration, i.e. for which the value of the beginning and end are different"@en ,
                                 "Una entidad temporal con extensión o duración distinta de cero, es decir, para la cual los valores de principio y fin del intervalo son diferentes."@es ;
                    rdfs:label "Proper interval"@en ,
                               "intervalo propio"@es ;
                    skos:definition "A temporal entity with non-zero extent or duration, i.e. for which the value of the beginning and end are different"@en ,
                                    "Una entidad temporal con extensión o duración distinta de cero, es decir, para la cual los valores de principio y fin del intervalo son diferentes."@es .


###  http://www.w3.org/2006/time#TRS
time:TRS rdf:type owl:Class ;
         rdfs:comment """A temporal reference system, such as a temporal coordinate system (with an origin, direction, and scale), a calendar-clock combination, or a (possibly hierarchical) ordinal system. 

This is a stub class, representing the set of all temporal reference systems."""@en ,
                      """Un sistema de referencia temporal, tal como un sistema de coordenadas temporales (con un origen, una dirección y una escala), una combinación calendario-reloj, o un sistema ordinal (posiblemente jerárquico).
        Esta clase comodín representa el conjunto de todos los sistemas de referencia temporal."""@es ;
         rdfs:label "Temporal Reference System"@en ,
                    "sistema de referencia temporal"@es ;
         skos:definition """A temporal reference system, such as a temporal coordinate system (with an origin, direction, and scale), a calendar-clock combination, or a (possibly hierarchical) ordinal system. 

This is a stub class, representing the set of all temporal reference systems."""@en ,
                         """Un sistema de referencia temporal, tal como un sistema de coordenadas temporales (con un origen, una dirección y una escala), una combinación calendario-reloj, o un sistema ordinal (posiblemente jerárquico).
    Esta clase comodín representa el conjunto de todos los sistemas de referencia temporal."""@es ;
         skos:note "A taxonomy of temporal reference systems is provided in ISO 19108:2002 [ISO19108], including (a) calendar + clock systems; (b) temporal coordinate systems (i.e. numeric offset from an epoch); (c) temporal ordinal reference systems (i.e. ordered sequence of named intervals, not necessarily of equal duration)."@en ,
                   "En el ISO 19108:2002 [ISO19108] se proporciona una taxonomía de sistemas de referencia temporal, incluyendo (a) sistemas de calendario + reloj; (b) sistemas de coordenadas temporales (es decir, desplazamiento numérico a partir de una época); (c) sistemas de referencia ordinales temporales (es decir, secuencia ordenada de intervalos nombrados, no necesariamente de igual duración)."@es .


###  http://www.w3.org/2006/time#TemporalDuration
time:TemporalDuration rdf:type owl:Class ;
                      rdfs:comment "Extensión de tiempo; duración de un intervalo de tiempo independiente de su posición de inicio particular."@es ,
                                   "Time extent; duration of a time interval separate from its particular start position"@en ;
                      rdfs:isDefinedBy time: ;
                      rdfs:label "Temporal duration"@en ,
                                 "duración temporal"@es ;
                      skos:definition "Extensión de tiempo; duración de un intervalo de tiempo independiente de su posición de inicio particular."@es ,
                                      "Time extent; duration of a time interval separate from its particular start position"@en .


###  http://www.w3.org/2006/time#TemporalEntity
time:TemporalEntity rdf:type owl:Class ;
                    owl:equivalentClass [ rdf:type owl:Class ;
                                          owl:unionOf ( time:Instant
                                                        time:Interval
                                                      )
                                        ] ;
                    rdfs:subClassOf owl:Thing ;
                    rdfs:comment "A temporal interval or instant."@en ,
                                 "Un intervalo temporal o un instante."@es ;
                    rdfs:isDefinedBy time: ;
                    rdfs:label "Temporal entity"@en ,
                               "entidad temporal"@es ;
                    skos:definition "A temporal interval or instant."@en ,
                                    "Un intervalo temporal o un instante."@es .


###  http://www.w3.org/2006/time#TemporalPosition
time:TemporalPosition rdf:type owl:Class ;
                      rdfs:subClassOf [ rdf:type owl:Restriction ;
                                        owl:onProperty time:hasTRS ;
                                        owl:cardinality "1"^^xsd:nonNegativeInteger
                                      ] ;
                      rdfs:comment "A position on a time-line"@en ,
                                   "Una posición sobre una línea de tiempo."@es ;
                      rdfs:label "Temporal position"@en ,
                                 "posición temporal"@es ;
                      skos:definition "A position on a time-line"@en ,
                                      "Una posición sobre una línea de tiempo."@es .


###  http://www.w3.org/2006/time#TemporalUnit
time:TemporalUnit rdf:type owl:Class ;
                  rdfs:subClassOf time:TemporalDuration ;
                  rdfs:comment "A standard duration, which provides a scale factor for a time extent, or the granularity or precision for a time position."@en ,
                               "Una duración estándar, que proporciona un factor de escala para una extensión de tiempo, o la granularidad o precisión para una posición de tiempo."@es ;
                  rdfs:label "Temporal unit"@en ,
                             "unidad de tiempo"@es ;
                  skos:changeNote """Remove enumeration from definition, in order to allow other units to be used when required in other coordinate systems. 
NOTE: existing units are still present as members of the class, but the class membership is now open. 

In the original OWL-Time the following constraint appeared: 
  owl:oneOf (
      time:unitSecond
      time:unitMinute
      time:unitHour
      time:unitDay
      time:unitWeek
      time:unitMonth
      time:unitYear
    ) ;"""@en ;
                  skos:definition "A standard duration, which provides a scale factor for a time extent, or the granularity or precision for a time position."@en ,
                                  "Una duración estándar, que proporciona un factor de escala para una extensión de tiempo, o la granularidad o precisión para una posición de tiempo."@es ;
                  skos:note "La pertenencia de la clase 'unidad de tiempo' está abierta, para permitir otras unidades de tiempo utilizadas en algunas aplicaciones técnicas (por ejemplo, millones de años o el mes Baha'i)."@es ,
                            "Membership of the class TemporalUnit is open, to allow for other temporal units used in some technical applications (e.g. millions of years, Baha'i month)."@en .


###  http://www.w3.org/2006/time#TimePosition
time:TimePosition rdf:type owl:Class ;
                  rdfs:subClassOf time:TemporalPosition ,
                                  [ rdf:type owl:Class ;
                                    owl:unionOf ( [ rdf:type owl:Restriction ;
                                                    owl:onProperty time:nominalPosition ;
                                                    owl:cardinality "1"^^xsd:nonNegativeInteger
                                                  ]
                                                  [ rdf:type owl:Restriction ;
                                                    owl:onProperty time:numericPosition ;
                                                    owl:cardinality "1"^^xsd:nonNegativeInteger
                                                  ]
                                                )
                                  ] ;
                  rdfs:comment "A temporal position described using either a (nominal) value from an ordinal reference system, or a (numeric) value in a temporal coordinate system. "@en ,
                               "Una posición temporal descrita utilizando bien un valor (nominal) de un sistema de referencia ordinal, o un valor (numérico) en un sistema de coordenadas temporales."@es ;
                  rdfs:label "Time position"@en ,
                             "posición de tiempo"@es ;
                  skos:definition "A temporal position described using either a (nominal) value from an ordinal reference system, or a (numeric) value in a temporal coordinate system. "@en ,
                                  "Una posición temporal descrita utilizando bien un valor (nominal) de un sistema de referencia ordinal, o un valor (numérico) en un sistema de coordenadas temporales."@es .


###  http://www.w3.org/2006/time#TimeZone
time:TimeZone rdf:type owl:Class ;
              rdfs:comment """A Time Zone specifies the amount by which the local time is offset from UTC. 
	A time zone is usually denoted geographically (e.g. Australian Eastern Daylight Time), with a constant value in a given region. 
The region where it applies and the offset from UTC are specified by a locally recognised governing authority."""@en ,
                           """Un huso horario especifica la cantidad en que la hora local está desplazada con respecto a UTC.
        Un huso horario normalmente se denota geográficamente (p.ej. el horario de verano del este de Australia), con un valor constante en una región dada.
        La región donde aplica y el desplazamiento desde UTC las especifica una autoridad gubernamental localmente reconocida."""@es ;
              rdfs:label "Time Zone"@en ,
                         "huso horario"@es ;
              skos:definition """A Time Zone specifies the amount by which the local time is offset from UTC. 
	A time zone is usually denoted geographically (e.g. Australian Eastern Daylight Time), with a constant value in a given region. 
The region where it applies and the offset from UTC are specified by a locally recognised governing authority."""@en ,
                              """Un huso horario especifica la cantidad en que la hora local está desplazada con respecto a UTC.
    Un huso horario normalmente se denota geográficamente (p.ej. el horario de verano del este de Australia), con un valor constante en una región dada.
    La región donde aplica y el desplazamiento desde UTC las especifica una autoridad gubernamental localmente reconocida."""@es ;
              skos:historyNote """En la versión original de OWL-Time de 2006, se definió, en un espacio de nombres diferente \"http://www.w3.org/2006/timezone#\", la clase 'huso horario', con varias propiedades específicas correspondientes a un modelo específico de huso horario.
    En la versión actual hay una clase con el mismo nombre local en el espacio de nombres de OWL-Time, eliminando la dependencia del espacio de nombres externo.
    Un axioma de alineación permite que los datos codificados de acuerdo con la versión anterior sean consistentes con la ontología actualizada."""@es ,
                               """In the original 2006 version of OWL-Time, the TimeZone class, with several properties corresponding to a specific model of time-zones, was defined in a separate namespace \"http://www.w3.org/2006/timezone#\". 

In the current version a class with same local name is put into the main OWL-Time namespace, removing the dependency on the external namespace. 

An alignment axiom 
	tzont:TimeZone rdfs:subClassOf time:TimeZone . 
allows data encoded according to the previous version to be consistent with the updated ontology. """ ;
              skos:note """A designated timezone is associated with a geographic region. However, for a particular region the offset from UTC often varies seasonally, and the dates of the changes may vary from year to year. The timezone designation usually changes for the different seasons (e.g. Australian Eastern Standard Time vs. Australian Eastern Daylight Time). Furthermore, the offset for a timezone may change over longer timescales, though its designation might not.  

Detailed guidance about working with time zones is given in http://www.w3.org/TR/timezone/ ."""@en ,
                        "An ontology for time zone descriptions was described in [owl-time-20060927] and provided as RDF in a separate namespace tzont:. However, that ontology was incomplete in scope, and the example datasets were selective. Furthermore, since the use of a class from an external ontology as the range of an ObjectProperty in OWL-Time creates a dependency, reference to the time zone class has been replaced with the 'stub' class in the normative part of this version of OWL-Time."@en ,
                        """Un huso horario designado está asociado con una región geográfica. Sin embargo, para una región particular el desplazamiento desde UTC a menudo varía según las estaciones, y las fechas de los cambios pueden variar de un año a otro. La designación de huso horario  normalmente cambia de una estación a otra (por ejemplo, el horario estándar frente al horario de verano ambos del este de Australia). Además, del desplazamiento para un huso horario puede cambiar sobre escalas de tiempo mayores, aunque su designación no lo haga.
    Se puede encontrar una guía detallada sobre el funcionamiento de husos horarios en http://www.w3.org/TR/timezone/.\"@es , \"En [owl-time-20060927] se describió una ontología para descripciones de husos horarios, y se proporcionó en un espacio de nombres separado tzont:. Sin embargo, dicha ontología estaba incompleta en su alcance, y el ejemplo de conjuntos de datos (datasets) era selectivo. Además, puesto que el uso de una clase de una ontología externa como el rango de una propiedad de objeto en OWL-Time crea una dependencia, la referencia a la clase huso horario se ha reemplazado por una clase que viene a ser un \"cajón de sastre\" en la en la parte normativa de esta versión de OWL-Time."""@es ;
              skos:scopeNote "En esta implementación 'huso horario' no tiene definidas propiedades. Se debería pensar como una superclase \"abstracta\" de todas las implementaciones de huso horario específicas."@es ,
                             "In this implementation TimeZone has no properties defined. It should be thought of as an 'abstract' superclass of all specific timezone implementations." .


###  http://www.w3.org/2006/time#Year
time:Year rdf:type owl:Class ;
          rdfs:subClassOf time:DurationDescription ,
                          [ rdf:type owl:Restriction ;
                            owl:onProperty time:days ;
                            owl:cardinality "0"^^xsd:nonNegativeInteger
                          ] ,
                          [ rdf:type owl:Restriction ;
                            owl:onProperty time:hours ;
                            owl:cardinality "0"^^xsd:nonNegativeInteger
                          ] ,
                          [ rdf:type owl:Restriction ;
                            owl:onProperty time:minutes ;
                            owl:cardinality "0"^^xsd:nonNegativeInteger
                          ] ,
                          [ rdf:type owl:Restriction ;
                            owl:onProperty time:months ;
                            owl:cardinality "0"^^xsd:nonNegativeInteger
                          ] ,
                          [ rdf:type owl:Restriction ;
                            owl:onProperty time:seconds ;
                            owl:cardinality "0"^^xsd:nonNegativeInteger
                          ] ,
                          [ rdf:type owl:Restriction ;
                            owl:onProperty time:weeks ;
                            owl:cardinality "0"^^xsd:nonNegativeInteger
                          ] ,
                          [ rdf:type owl:Restriction ;
                            owl:onProperty time:years ;
                            owl:cardinality "1"^^xsd:nonNegativeInteger
                          ] ;
          rdfs:comment "Year duration" ;
          rdfs:label "Year"@en ;
          owl:deprecated "true"^^xsd:boolean ;
          skos:definition "Year duration" ;
          skos:historyNote """Year was proposed in the 2006 version of OWL-Time as an example of how DurationDescription could be specialized to allow for a duration to be restricted to a number of years. 

It is deprecated in this edition of OWL-Time. """ ;
          skos:prefLabel "Anno"@it ,
                         "Année (calendrier)"@fr ,
                         "Ano"@pt ,
                         "Año"@es ,
                         "Jaar"@nl ,
                         "Jahr"@de ,
                         "Rok"@pl ,
                         "Year"@en ,
                         "Год"@ru ,
                         "سنة"@ar ,
                         "年"@ja ,
                         "年"@zh .


###  http://www.w3.org/2015/03/inspire/cp#CadastralParcel
cp:CadastralParcel rdf:type owl:Class ;
                   rdfs:subClassOf geosp:SpatialObject ;
                   rdfs:comment "Areas defined by cadastral registers or equivalent."@en ;
                   rdfs:isDefinedBy <http://www.w3.org/2015/03/inspire/cp> ;
                   rdfs:label "Cadastral Parcel"@en .


###  http://www.w3.org/ns/sosa/Platform
sosa:Platform rdf:type owl:Class ;
              rdfs:comment "A Platform is an entity that hosts other entities, particularly Sensors, Actuators, Samplers, and other Platforms (definition taken from http://www.w3.org/ns/sosa/Platform)"@en ;
              rdfs:isDefinedBy sosa: ;
              rdfs:label "Platform"@en .


###  http://www.w3.org/ns/ssn/Deployment
ssn:Deployment rdf:type owl:Class ;
               rdfs:isDefinedBy ssn: ;
               rdfs:label "Deployment"@en .


###  http://www.w3.org/ns/ssn/System
ssn:System rdf:type owl:Class ;
           rdfs:comment "System is a unit of abstraction for pieces of infrastructure that implement Procedures. A System may have components, its subsystems, which are other Systems. (Definition taken from http://www.w3.org/ns/ssn/System)"@en ;
           rdfs:isDefinedBy ssn: ;
           rdfs:label "System"@en .


###  http://xmlns.com/foaf/0.1/Agent
foaf:Agent rdf:type owl:Class ;
           rdfs:subClassOf [ rdf:type owl:Restriction ;
                             owl:onProperty bigg:manages ;
                             owl:someValuesFrom bigg:Patrimony
                           ] ,
                           [ rdf:type owl:Restriction ;
                             owl:onProperty foaf:member ;
                             owl:someValuesFrom foaf:Agent
                           ] ;
           rdfs:label "Agent"@en .


###  http://xmlns.com/foaf/0.1/Person
foaf:Person rdf:type owl:Class ;
            rdfs:subClassOf foaf:Agent ;
            rdfs:label "Person"@en .


###  https://saref.etsi.org/core/ActuatingFunction
saref:ActuatingFunction rdf:type owl:Class ;
                        rdfs:subClassOf saref:Function ;
                        rdfs:comment "A function that allows to transmit data to actuators, such as level settings (e.g., temperature) or binary switching (e.g., open/close, on/off)"@en ;
                        rdfs:label "Actuating function"@en .


###  https://saref.etsi.org/core/Actuator
saref:Actuator rdf:type owl:Class ;
               rdfs:subClassOf saref:Device ,
                               [ rdf:type owl:Restriction ;
                                 owl:onProperty saref:hasFunction ;
                                 owl:someValuesFrom saref:ActuatingFunction
                               ] ;
               owl:disjointWith saref:Sensor ;
               rdfs:comment "A device responsible for moving or controlling a mechanism or system"@en ,
                            "A device responsible for moving or controlling a mechanism or system by performing an actuating function"@en ,
                            "A device responsible for moving or controlling a mechanism or system."@en ;
               rdfs:isDefinedBy saref: ;
               rdfs:label "Actuator"@en .


###  https://saref.etsi.org/core/Appliance
saref:Appliance rdf:type owl:Class ;
                rdfs:subClassOf saref:Device ;
                rdfs:comment "An electrical/mechanical machine that accomplish some household functions, such as cleaning or cooking"@en ;
                rdfs:label "Appliance"@en .


###  https://saref.etsi.org/core/CloseCommand
saref:CloseCommand rdf:type owl:Class ;
                   rdfs:subClassOf saref:Command ,
                                   [ rdf:type owl:Restriction ;
                                     owl:onProperty saref:actsUpon ;
                                     owl:someValuesFrom saref:OpenCloseState
                                   ] ,
                                   [ rdf:type owl:Restriction ;
                                     owl:onProperty saref:isCommandOf ;
                                     owl:allValuesFrom saref:OpenCloseFunction
                                   ] ;
                   owl:disjointWith saref:OpenCommand ;
                   rdfs:comment "A type of command"@en ;
                   rdfs:label "Close command"@en .


###  https://saref.etsi.org/core/CloseState
saref:CloseState rdf:type owl:Class ;
                 rdfs:subClassOf saref:OpenCloseState ;
                 rdfs:comment "The state of a device that is CLOSE"@en ;
                 rdfs:label "Close state"@en .


###  https://saref.etsi.org/core/Coal
saref:Coal rdf:type owl:Class ;
           rdfs:subClassOf saref:Commodity ;
           rdfs:comment "A type of commodity"@en ;
           rdfs:label "Coal"@en .


###  https://saref.etsi.org/core/Command
saref:Command rdf:type owl:Class ;
              rdfs:subClassOf [ rdf:type owl:Restriction ;
                                owl:onProperty saref:actsUpon ;
                                owl:allValuesFrom saref:State
                              ] ,
                              [ rdf:type owl:Restriction ;
                                owl:onProperty saref:isCommandOf ;
                                owl:minQualifiedCardinality "1"^^xsd:nonNegativeInteger ;
                                owl:onClass saref:Function
                              ] ,
                              [ rdf:type owl:Restriction ;
                                owl:onProperty saref:hasDescription ;
                                owl:maxCardinality "1"^^xsd:nonNegativeInteger
                              ] ;
              rdfs:comment "A directive that a device must support to perform a certain function. A command may act upon a state, but does not necessarily act upon a state. For example, the ON command acts upon the ON/OFF state, but the GET command does not act upon any state, it simply gives a directive to retrieve a certain value. We propose here a list of commands that are relevant for the purpose of SAREF, but this list can be extended."@en ;
              rdfs:label "Command"@en .


###  https://saref.etsi.org/core/Commodity
saref:Commodity rdf:type owl:Class ;
                rdfs:comment "A marketable item for which there is demand, but which is supplied without qualitative differentiation across a market. SAREF refers to energy commodities such as electricity, gas, coal and oil. "@en ;
                rdfs:label "Commodity"@en .


###  https://saref.etsi.org/core/Currency
saref:Currency rdf:type owl:Class ;
               rdfs:subClassOf saref:UnitOfMeasure ;
               rdfs:comment "The class of units of measure for price"@en ;
               rdfs:label "Currency"@en .


###  https://saref.etsi.org/core/Device
saref:Device rdf:type owl:Class ;
             rdfs:subClassOf ssn:System ,
                             s4bldg:PhysicalObject ,
                             [ rdf:type owl:Restriction ;
                               owl:onProperty saref:consistsOf ;
                               owl:allValuesFrom saref:Device
                             ] ,
                             [ rdf:type owl:Restriction ;
                               owl:onProperty saref:controlsProperty ;
                               owl:allValuesFrom saref:Property
                             ] ,
                             [ rdf:type owl:Restriction ;
                               owl:onProperty saref:hasProfile ;
                               owl:allValuesFrom saref:Profile
                             ] ,
                             [ rdf:type owl:Restriction ;
                               owl:onProperty saref:hasState ;
                               owl:allValuesFrom saref:State
                             ] ,
                             [ rdf:type owl:Restriction ;
                               owl:onProperty saref:isUsedFor ;
                               owl:allValuesFrom saref:Commodity
                             ] ,
                             [ rdf:type owl:Restriction ;
                               owl:onProperty saref:makesMeasurement ;
                               owl:allValuesFrom saref:Measurement
                             ] ,
                             [ rdf:type owl:Restriction ;
                               owl:onProperty saref:measuresProperty ;
                               owl:allValuesFrom saref:Property
                             ] ,
                             [ rdf:type owl:Restriction ;
                               owl:onProperty saref:offers ;
                               owl:allValuesFrom saref:Service
                             ] ,
                             [ rdf:type owl:Restriction ;
                               owl:onProperty saref:accomplishes ;
                               owl:minQualifiedCardinality "1"^^xsd:nonNegativeInteger ;
                               owl:onClass saref:Task
                             ] ,
                             [ rdf:type owl:Restriction ;
                               owl:onProperty saref:hasFunction ;
                               owl:minQualifiedCardinality "1"^^xsd:nonNegativeInteger ;
                               owl:onClass saref:Function
                             ] ,
                             [ rdf:type owl:Restriction ;
                               owl:onProperty saref:hasManufacturer ;
                               owl:maxCardinality "1"^^xsd:nonNegativeInteger
                             ] ,
                             [ rdf:type owl:Restriction ;
                               owl:onProperty saref:hasModel ;
                               owl:maxCardinality "1"^^xsd:nonNegativeInteger
                             ] ;
             rdfs:comment "A tangible object designed to accomplish a particular task in households, common public buildings or offices. In order to accomplish this task, the device performs one or more functions. For example, a washing machine is designed to wash (task) and to accomplish this task it performs a start and stop function. Devices can be structured in categories (subclasses) that reflect the different domain in which a device is used, e.g., smart appliances domain (subclass FunctionRelated) vs. building domain (subclass BuildingRelated) vs. smart grid domain (subclass EnergyRelated). New categories can be defined,if needed, to reflect other differences, for example different points of view, such as the point of view of the device's user vs. the point of view of the device's manufacturer. We propose a list of devices that are relevant for the purpose of SAREF, but this list can be extended."@en ,
                          "A tangible object designed to accomplish a particular task in households, common public buildings or offices. In order to accomplish this task, the device performs one or more functions. For example, a washing machine is designed to wash (task) and to accomplish this task it performs the start and stop function."@en ,
                          "A tangible object designed to accomplish a particular task. In order to accomplish this task, the device performs one or more functions. For example, a washing machine is designed to wash (task) and to accomplish this task it performs a start and stop function."@en ;
             rdfs:isDefinedBy saref: ;
             rdfs:label "Device"@en .


###  https://saref.etsi.org/core/DoorSwitch
saref:DoorSwitch rdf:type owl:Class ;
                 rdfs:subClassOf saref:Switch ,
                                 [ rdf:type owl:Restriction ;
                                   owl:onProperty saref:hasFunction ;
                                   owl:someValuesFrom saref:OpenCloseFunction
                                 ] ,
                                 [ rdf:type owl:Restriction ;
                                   owl:onProperty saref:hasState ;
                                   owl:someValuesFrom saref:OpenCloseState
                                 ] ;
                 rdfs:comment "A switch that performs the saref:OpenCloseFunction, is used for controlling a door, and can be found in the state saref:OpenCloseState. A saref:DoorSwitch is typically used to accomplish saref:Safety."@en ;
                 rdfs:label "Door switch"@en .


###  https://saref.etsi.org/core/Electricity
saref:Electricity rdf:type owl:Class ;
                  rdfs:subClassOf saref:Commodity ;
                  rdfs:comment "A type of commodity"@en ;
                  rdfs:label "Electricity"@en .


###  https://saref.etsi.org/core/Energy
saref:Energy rdf:type owl:Class ;
             rdfs:subClassOf saref:Property ;
             rdfs:comment "A saref:Property related to some measurements that are characterized by a certain value measured in an energy unit (such as Kilowatt_Hour or Watt_hour). Furter specializations of the saref:Energy class can be found in the SAREF4ENER extension, where classes such as EnergyMax, EnergyMin and EnergyExpected are defined. "@en ;
             rdfs:label "Energy"@en .


###  https://saref.etsi.org/core/EnergyUnit
saref:EnergyUnit rdf:type owl:Class ;
                 rdfs:subClassOf saref:UnitOfMeasure ;
                 rdfs:comment "The unit of measure for energy"@en ;
                 rdfs:label "Energy unit"@en .


###  https://saref.etsi.org/core/EventFunction
saref:EventFunction rdf:type owl:Class ;
                    rdfs:subClassOf saref:Function ,
                                    [ rdf:type owl:Restriction ;
                                      owl:onProperty saref:hasThresholdMeasurement ;
                                      owl:minQualifiedCardinality "1"^^xsd:nonNegativeInteger ;
                                      owl:onClass saref:Measurement
                                    ] ;
                    rdfs:comment "A function that allows to notify about some relevant activity; e.g., that a certain threshold value has been exceeded or that some object has moved."@en ;
                    rdfs:label "Event function"@en .


###  https://saref.etsi.org/core/FeatureOfInterest
saref:FeatureOfInterest rdf:type owl:Class ;
                        rdfs:subClassOf [ rdf:type owl:Restriction ;
                                          owl:onProperty saref:hasMeasurement ;
                                          owl:allValuesFrom saref:Measurement
                                        ] ,
                                        [ rdf:type owl:Restriction ;
                                          owl:onProperty saref:hasProperty ;
                                          owl:allValuesFrom saref:Property
                                        ] ;
                        rdfs:comment saref: ,
                                     "A feature of interest represents any real world entity from which a property is measured."@en ;
                        rdfs:isDefinedBy saref: ;
                        rdfs:label "Feature of interest"@en .


###  https://saref.etsi.org/core/Function
saref:Function rdf:type owl:Class ;
               rdfs:subClassOf [ rdf:type owl:Restriction ;
                                 owl:onProperty saref:hasCommand ;
                                 owl:minQualifiedCardinality "1"^^xsd:nonNegativeInteger ;
                                 owl:onClass saref:Command
                               ] ;
               rdfs:comment "The functionality necessary to accomplish the task for which a Device is designed. A device can be designed to perform more than one function. Functions can be structured in categories (subclasses) that reflect different points of view, for example, considering the specific application area for which a function can be used (e.g., light, temperature, motion, heat, power, etc.), or the capability that a function can support (e.g., receive, reply, notify, etc.), and so forth. "@en ,
                            "The functionality necessary to accomplish the task for which a device is designed. A device can be designed to perform more than one function. Functions can be structured in categories (subclasses) that reflect different points of view, for example, considering the specific application area for which a function can be used (e.g., light, temperature, motion, heat, power, etc.), or the capability that a function can support (e.g., receive, reply, notify, etc.), and so forth. "@en ;
               rdfs:label "Function"@en .


###  https://saref.etsi.org/core/Gas
saref:Gas rdf:type owl:Class ;
          rdfs:subClassOf saref:Commodity ;
          rdfs:comment "A type of commodity"@en ;
          rdfs:label "Gas"@en .


###  https://saref.etsi.org/core/GetCommand
saref:GetCommand rdf:type owl:Class ;
                 rdfs:subClassOf saref:Command ;
                 rdfs:comment "A type of command"@en ;
                 rdfs:label "Get command"@en .


###  https://saref.etsi.org/core/GetCurrentMeterValueCommand
saref:GetCurrentMeterValueCommand rdf:type owl:Class ;
                                  rdfs:subClassOf saref:GetCommand ,
                                                  [ rdf:type owl:Restriction ;
                                                    owl:onProperty saref:isCommandOf ;
                                                    owl:allValuesFrom saref:MeteringFunction
                                                  ] ;
                                  rdfs:comment "A type of get command"@en ;
                                  rdfs:label "Get current meter value command"@en .


###  https://saref.etsi.org/core/GetMeterDataCommand
saref:GetMeterDataCommand rdf:type owl:Class ;
                          rdfs:subClassOf saref:GetCommand ,
                                          [ rdf:type owl:Restriction ;
                                            owl:onProperty saref:isCommandOf ;
                                            owl:allValuesFrom saref:MeteringFunction
                                          ] ;
                          rdfs:comment "A type of get command"@en ;
                          rdfs:label "Get meter data command"@en .


###  https://saref.etsi.org/core/GetMeterHistoryCommand
saref:GetMeterHistoryCommand rdf:type owl:Class ;
                             rdfs:subClassOf saref:GetCommand ,
                                             [ rdf:type owl:Restriction ;
                                               owl:onProperty saref:isCommandOf ;
                                               owl:allValuesFrom saref:MeteringFunction
                                             ] ;
                             rdfs:comment "A type of get command"@en ;
                             rdfs:label "Get meter history command"@en .


###  https://saref.etsi.org/core/GetSensingDataCommand
saref:GetSensingDataCommand rdf:type owl:Class ;
                            rdfs:subClassOf saref:GetCommand ,
                                            [ rdf:type owl:Restriction ;
                                              owl:onProperty saref:isCommandOf ;
                                              owl:allValuesFrom saref:SensingFunction
                                            ] ;
                            rdfs:comment "A type of get command"@en ;
                            rdfs:label "Get sensing data command"@en .


###  https://saref.etsi.org/core/HVAC
saref:HVAC rdf:type owl:Class ;
           rdfs:subClassOf saref:Device ;
           rdfs:comment "Heating, Ventilation and Air Conditioning (HVAC) device that provides indoor environmental comfort. A saref:HVAC is typically used to accomplish saref:Comfort."@en ;
           rdfs:label "HVAC"@en .


###  https://saref.etsi.org/core/Humidity
saref:Humidity rdf:type owl:Class ;
               rdfs:subClassOf saref:Property ;
               rdfs:comment "A saref:Property related to some measurements that are characterized by a certain value that is measured in a humidity unit"@en ;
               rdfs:label "Humidity"@en ,
                          "Humidiy"@en .


###  https://saref.etsi.org/core/IlluminanceUnit
saref:IlluminanceUnit rdf:type owl:Class ;
                      rdfs:subClassOf saref:UnitOfMeasure ;
                      rdfs:comment "The unit of measure for light"@en ;
                      rdfs:label "Illuminance unit"@en .


###  https://saref.etsi.org/core/LevelControlFunction
saref:LevelControlFunction rdf:type owl:Class ;
                           rdfs:subClassOf saref:ActuatingFunction ;
                           rdfs:comment "An actuating function that allows to do level adjustments of a property in a certain range (e.g., 0%-100%), such as dimming a light in a room or setting the speed of an electric motor. "@en ;
                           rdfs:label "Level control function"@en .


###  https://saref.etsi.org/core/Light
saref:Light rdf:type owl:Class ;
            rdfs:subClassOf saref:Property ;
            rdfs:comment "A saref:Property related to some measurements that are characterized by a certain value that is measured in a illuminance unit (lux)"@en ;
            rdfs:label "Light"@en .


###  https://saref.etsi.org/core/LightSwitch
saref:LightSwitch rdf:type owl:Class ;
                  rdfs:subClassOf saref:Switch ,
                                  [ rdf:type owl:Restriction ;
                                    owl:onProperty saref:controlsProperty ;
                                    owl:someValuesFrom saref:Light
                                  ] ,
                                  [ rdf:type owl:Restriction ;
                                    owl:onProperty saref:hasFunction ;
                                    owl:someValuesFrom saref:OnOffFunction
                                  ] ,
                                  [ rdf:type owl:Restriction ;
                                    owl:onProperty saref:hasState ;
                                    owl:someValuesFrom saref:OnOffState
                                  ] ,
                                  [ rdf:type owl:Restriction ;
                                    owl:onProperty saref:offers ;
                                    owl:someValuesFrom saref:SwitchOnService
                                  ] ;
                  rdfs:comment "A switch that performs the saref:OnOffFunction, controls the property saref:Light, and can be found in the state saref:OnOffState. It can offer a switch on service. A saref:LightSwitch is typically used to accomplish saref:Lighting."@en ;
                  rdfs:label "Light switch"@en .


###  https://saref.etsi.org/core/Measurement
saref:Measurement rdf:type owl:Class ;
                  rdfs:subClassOf [ rdf:type owl:Restriction ;
                                    owl:onProperty saref:isMeasuredIn ;
                                    owl:allValuesFrom saref:UnitOfMeasure
                                  ] ,
                                  [ rdf:type owl:Restriction ;
                                    owl:onProperty saref:isMeasurementOf ;
                                    owl:allValuesFrom saref:FeatureOfInterest
                                  ] ,
                                  [ rdf:type owl:Restriction ;
                                    owl:onProperty saref:relatesToProperty ;
                                    owl:allValuesFrom saref:Property
                                  ] ,
                                  [ rdf:type owl:Restriction ;
                                    owl:onProperty saref:isMeasuredIn ;
                                    owl:qualifiedCardinality "1"^^xsd:nonNegativeInteger ;
                                    owl:onClass saref:UnitOfMeasure
                                  ] ,
                                  [ rdf:type owl:Restriction ;
                                    owl:onProperty saref:relatesToProperty ;
                                    owl:qualifiedCardinality "1"^^xsd:nonNegativeInteger ;
                                    owl:onClass saref:Property
                                  ] ,
                                  [ rdf:type owl:Restriction ;
                                    owl:onProperty saref:hasTimestamp ;
                                    owl:allValuesFrom xsd:dateTime
                                  ] ,
                                  [ rdf:type owl:Restriction ;
                                    owl:onProperty saref:hasValue ;
                                    owl:cardinality "1"^^xsd:nonNegativeInteger
                                  ] ,
                                  [ rdf:type owl:Restriction ;
                                    owl:onProperty saref:hasValue ;
                                    owl:qualifiedCardinality "1"^^xsd:nonNegativeInteger ;
                                    owl:onDataRange xsd:float
                                  ] ;
                  owl:disjointWith saref:Property ,
                                   saref:UnitOfMeasure ;
                  rdfs:comment "Represents the measured value made over a property. It is also linked to the unit of measure in which the value is expressed and the timestamp of the measurement."@en ;
                  rdfs:isDefinedBy saref: ,
                                   "https://saref.etsi.org/core/" ;
                  rdfs:label "Measurement"@en .


###  https://saref.etsi.org/core/Meter
saref:Meter rdf:type owl:Class ;
            rdfs:subClassOf saref:Device ,
                            saref:Sensor ,
                            [ rdf:type owl:Restriction ;
                              owl:onProperty saref:hasFunction ;
                              owl:someValuesFrom saref:MeteringFunction
                            ] ;
            rdfs:comment "A device built to accurately detect and display a quantity in a form readable by a human being. Further, a device of category saref:Meter that performs a saref:MeteringFunction."@en ;
            rdfs:isDefinedBy saref: ;
            rdfs:label "Meter"@en .


###  https://saref.etsi.org/core/MeteringFunction
saref:MeteringFunction rdf:type owl:Class ;
                       rdfs:subClassOf saref:Function ,
                                       [ rdf:type owl:Restriction ;
                                         owl:onProperty saref:hasMeterReading ;
                                         owl:allValuesFrom saref:Measurement
                                       ] ,
                                       [ rdf:type owl:Restriction ;
                                         owl:onProperty saref:hasMeterReadingType ;
                                         owl:allValuesFrom [ rdf:type owl:Class ;
                                                             owl:unionOf ( saref:Commodity
                                                                           saref:Property
                                                                         )
                                                           ]
                                       ] ;
                       rdfs:comment "A function that allows to get data from a meter, such as current meter reading or instantaneous demand"@en ;
                       rdfs:label "Metering function"@en .


###  https://saref.etsi.org/core/Motion
saref:Motion rdf:type owl:Class ;
             rdfs:subClassOf saref:Property ;
             rdfs:comment "A saref:Property related to some measurements that are characterized by a certain value that is measured in a unit of measure for motion"@en ;
             rdfs:label "Motion"@en .


###  https://saref.etsi.org/core/MultiLevelState
saref:MultiLevelState rdf:type owl:Class ;
                      rdfs:subClassOf saref:State ;
                      rdfs:comment "A type of state"@en ;
                      rdfs:label "Multi level state"@en .


###  https://saref.etsi.org/core/NotifyCommand
saref:NotifyCommand rdf:type owl:Class ;
                    rdfs:subClassOf saref:Command ,
                                    [ rdf:type owl:Restriction ;
                                      owl:onProperty saref:isCommandOf ;
                                      owl:allValuesFrom saref:EventFunction
                                    ] ;
                    rdfs:comment "A type of command"@en ;
                    rdfs:label "Notify command"@en .


###  https://saref.etsi.org/core/Occupancy
saref:Occupancy rdf:type owl:Class ;
                rdfs:subClassOf saref:Property ;
                rdfs:comment "A saref:Property related to some measurements that are characterized by a certain value (saref:hasValue property) that is measured in a unit of measure for occupancy"@en ;
                rdfs:label "Occupancy"@en .


###  https://saref.etsi.org/core/OffCommand
saref:OffCommand rdf:type owl:Class ;
                 rdfs:subClassOf saref:Command ,
                                 [ rdf:type owl:Restriction ;
                                   owl:onProperty saref:actsUpon ;
                                   owl:someValuesFrom saref:OnOffState
                                 ] ,
                                 [ rdf:type owl:Restriction ;
                                   owl:onProperty saref:isCommandOf ;
                                   owl:allValuesFrom saref:OnOffFunction
                                 ] ;
                 owl:disjointWith saref:OnCommand ;
                 rdfs:comment "A type of command"@en ;
                 rdfs:label "Off command"@en .


###  https://saref.etsi.org/core/OffState
saref:OffState rdf:type owl:Class ;
               rdfs:subClassOf saref:OnOffState ;
               rdfs:comment "The state of a device that is Off"@en ;
               rdfs:label "Off state"@en .


###  https://saref.etsi.org/core/OnCommand
saref:OnCommand rdf:type owl:Class ;
                rdfs:subClassOf saref:Command ,
                                [ rdf:type owl:Restriction ;
                                  owl:onProperty saref:actsUpon ;
                                  owl:someValuesFrom saref:OnOffState
                                ] ,
                                [ rdf:type owl:Restriction ;
                                  owl:onProperty saref:isCommandOf ;
                                  owl:allValuesFrom saref:OnOffFunction
                                ] ;
                rdfs:comment "A type of command"@en ;
                rdfs:label "On command"@en .


###  https://saref.etsi.org/core/OnOffFunction
saref:OnOffFunction rdf:type owl:Class ;
                    rdfs:subClassOf saref:ActuatingFunction ;
                    rdfs:comment "An actuating function that allows to switch on and off an actuator"@en ;
                    rdfs:label "On off function"@en .


###  https://saref.etsi.org/core/OnOffState
saref:OnOffState rdf:type owl:Class ;
                 rdfs:subClassOf saref:State ;
                 rdfs:comment "A type of state"@en ;
                 rdfs:label "On off state"@en .


###  https://saref.etsi.org/core/OnState
saref:OnState rdf:type owl:Class ;
              rdfs:subClassOf saref:OnOffState ;
              rdfs:comment "The state of a device that is On"@en ;
              rdfs:label "On state"@en .


###  https://saref.etsi.org/core/OpenCloseFunction
saref:OpenCloseFunction rdf:type owl:Class ;
                        rdfs:subClassOf saref:ActuatingFunction ;
                        rdfs:comment "An actuating function that allows to open and close a device"@en ;
                        rdfs:label "Open close function"@en .


###  https://saref.etsi.org/core/OpenCloseState
saref:OpenCloseState rdf:type owl:Class ;
                     rdfs:subClassOf saref:State ;
                     rdfs:comment "A type of state"@en ;
                     rdfs:label "Open close state"@en .


###  https://saref.etsi.org/core/OpenCommand
saref:OpenCommand rdf:type owl:Class ;
                  rdfs:subClassOf saref:Command ,
                                  [ rdf:type owl:Restriction ;
                                    owl:onProperty saref:actsUpon ;
                                    owl:someValuesFrom saref:OpenCloseState
                                  ] ,
                                  [ rdf:type owl:Restriction ;
                                    owl:onProperty saref:isCommandOf ;
                                    owl:allValuesFrom saref:OpenCloseFunction
                                  ] ;
                  rdfs:comment "A type of command"@en ;
                  rdfs:label "Open command"@en .


###  https://saref.etsi.org/core/OpenState
saref:OpenState rdf:type owl:Class ;
                rdfs:subClassOf saref:OpenCloseState ;
                rdfs:comment "The state of a device that is OPEN "@en ;
                rdfs:label "Open state"@en .


###  https://saref.etsi.org/core/PauseCommand
saref:PauseCommand rdf:type owl:Class ;
                   rdfs:subClassOf saref:Command ;
                   rdfs:comment "A type of command"@en ;
                   rdfs:label "Pause command"@en .


###  https://saref.etsi.org/core/Power
saref:Power rdf:type owl:Class ;
            rdfs:subClassOf saref:Property ;
            rdfs:comment "A saref:Property related to some measurements that are characterized by a certain value that is measured in a power unit (such as watt or kilowatt).  Further specializations of the saref:Power class can be found in the SAREF4ENER extension, where classes such as PowerMax, PowerMin and PowerExpected are defined."@en ;
            rdfs:label "Power"@en .


###  https://saref.etsi.org/core/PowerUnit
saref:PowerUnit rdf:type owl:Class ;
                rdfs:subClassOf saref:UnitOfMeasure ;
                rdfs:comment "The unit of measure for power"@en ;
                rdfs:label "Power unit"@en .


###  https://saref.etsi.org/core/Pressure
saref:Pressure rdf:type owl:Class ;
               rdfs:subClassOf saref:Property ;
               rdfs:comment "A saref:Property related to some measurements that are characterized by a certain value that is measured in a pressure unit (bar or pascal)"@en ;
               rdfs:label "Pressure"@en .


###  https://saref.etsi.org/core/PressureUnit
saref:PressureUnit rdf:type owl:Class ;
                   rdfs:subClassOf saref:UnitOfMeasure ;
                   rdfs:comment "The unit of measure for pressure"@en ;
                   rdfs:label "Pressure unit"@en .


###  https://saref.etsi.org/core/Price
saref:Price rdf:type owl:Class ;
            rdfs:subClassOf saref:Property ;
            rdfs:comment "A saref:Property crelated to some measurements that are characterized by a certain value that is measured using saref:Currency"@en ;
            rdfs:label "Price"@en .


###  https://saref.etsi.org/core/Profile
saref:Profile rdf:type owl:Class ;
              rdfs:subClassOf [ rdf:type owl:Restriction ;
                                owl:onProperty saref:consistsOf ;
                                owl:allValuesFrom saref:Profile
                              ] ,
                              [ rdf:type owl:Restriction ;
                                owl:onProperty saref:hasPrice ;
                                owl:allValuesFrom saref:Price
                              ] ,
                              [ rdf:type owl:Restriction ;
                                owl:onProperty saref:hasTime ;
                                owl:allValuesFrom saref:Time
                              ] ,
                              [ rdf:type owl:Restriction ;
                                owl:onProperty saref:isAbout ;
                                owl:allValuesFrom [ rdf:type owl:Class ;
                                                    owl:unionOf ( saref:Commodity
                                                                  saref:Property
                                                                )
                                                  ]
                              ] ;
              rdfs:comment "A specification associated to a device to collect information about a certain Property (e.g., Energy) for optimizing its usage in the home, office or building in which the device is located. This specification is about a certain Property (saref:isAbout), can be calculated over a time span (saref:hasTime) and can be associated to some costs (saref:hasPrice). An example is the Power Profile defined in the SAREF4ENER extension that can be associated to a device for optimizing the Energy efficiency in the home, office or building in which the device is located."@en ;
              rdfs:label "Profile"@en .


###  https://saref.etsi.org/core/Property
saref:Property rdf:type owl:Class ;
               rdfs:subClassOf [ rdf:type owl:Restriction ;
                                 owl:onProperty saref:isControlledByDevice ;
                                 owl:allValuesFrom saref:Device
                               ] ,
                               [ rdf:type owl:Restriction ;
                                 owl:onProperty saref:isMeasuredByDevice ;
                                 owl:allValuesFrom saref:Device
                               ] ,
                               [ rdf:type owl:Restriction ;
                                 owl:onProperty saref:isPropertyOf ;
                                 owl:allValuesFrom saref:FeatureOfInterest
                               ] ,
                               [ rdf:type owl:Restriction ;
                                 owl:onProperty saref:relatesToMeasurement ;
                                 owl:allValuesFrom saref:Measurement
                               ] ;
               owl:disjointWith saref:UnitOfMeasure ;
               rdfs:comment "A quality of a feature of interest that can be measured; an aspect of a feature of interest that is intrinsic to and cannot exist without the feature"@en ,
                            "An aspect of an entity that can be observable by a sensor."@en ,
                            "Anything that can be sensed, measured or controlled in households, common public buildings or offices. We propose here a list of properties that are relevant for the purpose of SAREF, but this list can be extended."@en ;
               rdfs:isDefinedBy saref: ,
                                "https://saref.etsi.org/core/" ;
               rdfs:label "Property"@en .


###  https://saref.etsi.org/core/SensingFunction
saref:SensingFunction rdf:type owl:Class ;
                      rdfs:subClassOf saref:Function ,
                                      [ rdf:type owl:Restriction ;
                                        owl:onProperty saref:hasSensingRange ;
                                        owl:someValuesFrom saref:Measurement
                                      ] ,
                                      [ rdf:type owl:Restriction ;
                                        owl:onProperty saref:hasSensorType ;
                                        owl:allValuesFrom saref:Property
                                      ] ;
                      rdfs:comment "A function that allows to transmit data from sensors, such as measurement values (e.g., temperature) or sensing data (e.g., occupancy)"@en ;
                      rdfs:label "Sensing function"@en .


###  https://saref.etsi.org/core/Sensor
saref:Sensor rdf:type owl:Class ;
             rdfs:subClassOf saref:Device ,
                             [ rdf:type owl:Restriction ;
                               owl:onProperty saref:hasFunction ;
                               owl:someValuesFrom saref:SensingFunction
                             ] ;
             rdfs:comment """A device that detects and responds to events or changes in the physical environment such as light, motion, or temperature changes.
A device that has category saref:Sensor and performs a saref:SensingFunction."""@en ,
                          "A device that detects and responds to events or changes in the physical environment such as light, motion, or temperature changes. A device that has category saref:Sensor and performs a saref:SensingFunction."@en ,
                          "A device that detects and responds to events or changes in the physical environment such as light, motion, or temperature changes. Further, a device of category saref:Sensor that performs a saref:SensingFunction."@en ;
             rdfs:isDefinedBy saref: ;
             rdfs:label "Sensor"@en .


###  https://saref.etsi.org/core/Service
saref:Service rdf:type owl:Class ;
              rdfs:subClassOf [ rdf:type owl:Restriction ;
                                owl:onProperty saref:isOfferedBy ;
                                owl:minQualifiedCardinality "1"^^xsd:nonNegativeInteger ;
                                owl:onClass saref:Device
                              ] ,
                              [ rdf:type owl:Restriction ;
                                owl:onProperty saref:represents ;
                                owl:minQualifiedCardinality "1"^^xsd:nonNegativeInteger ;
                                owl:onClass saref:Function
                              ] ;
              rdfs:comment "A service is a representation of a function to a network that makes the function discoverable, registerable, remotely controllable by other devices in the network. A service can represent one or more functions. A Service is offered by a device that wants (a certain set of) its function(s) to be discoverable, registerable, remotely controllable by other devices in the network. A Service must specify the device that is offering the service and the function(s) to be represented."@en ;
              rdfs:label "Service"@en .


###  https://saref.etsi.org/core/SetAbsoluteLevelCommand
saref:SetAbsoluteLevelCommand rdf:type owl:Class ;
                              rdfs:subClassOf saref:SetLevelCommand ;
                              rdfs:comment "A type of set level command"@en ;
                              rdfs:label "Set absolute level command"@en .


###  https://saref.etsi.org/core/SetLevelCommand
saref:SetLevelCommand rdf:type owl:Class ;
                      rdfs:subClassOf saref:Command ,
                                      [ rdf:type owl:Restriction ;
                                        owl:onProperty saref:actsUpon ;
                                        owl:someValuesFrom saref:MultiLevelState
                                      ] ,
                                      [ rdf:type owl:Restriction ;
                                        owl:onProperty saref:isCommandOf ;
                                        owl:allValuesFrom saref:LevelControlFunction
                                      ] ;
                      rdfs:comment "A type of command"@en ;
                      rdfs:label "Set level command"@en .


###  https://saref.etsi.org/core/SetRelativeLevelCommand
saref:SetRelativeLevelCommand rdf:type owl:Class ;
                              rdfs:subClassOf saref:SetLevelCommand ;
                              rdfs:comment "A type of set level command"@en ;
                              rdfs:label "Set relative level command"@en .


###  https://saref.etsi.org/core/Smoke
saref:Smoke rdf:type owl:Class ;
            rdfs:subClassOf saref:Property ;
            rdfs:comment "A saref:Property related to some measurements that are characterized by a certain value that is measured in a unit of measure for smoke"@en ;
            rdfs:label "Smoke"@en .


###  https://saref.etsi.org/core/SmokeSensor
saref:SmokeSensor rdf:type owl:Class ;
                  rdfs:subClassOf saref:Sensor ,
                                  [ rdf:type owl:Restriction ;
                                    owl:onProperty saref:hasFunction ;
                                    owl:someValuesFrom saref:EventFunction
                                  ] ,
                                  [ rdf:type owl:Restriction ;
                                    owl:onProperty saref:hasFunction ;
                                    owl:someValuesFrom saref:SensingFunction
                                  ] ,
                                  [ rdf:type owl:Restriction ;
                                    owl:onProperty saref:measuresProperty ;
                                    owl:someValuesFrom saref:Smoke
                                  ] ;
                  rdfs:comment "A sensor that performs the saref:SensingFunction and the saref:EventFunction, and is used for the purpose of sensing a property of type saref:Smoke. A saref:SmokeSensor is typically used to saref:accomplish saref:Safety."@en ;
                  rdfs:label "Smoke sensor"@en .


###  https://saref.etsi.org/core/StartCommand
saref:StartCommand rdf:type owl:Class ;
                   rdfs:subClassOf saref:Command ,
                                   [ rdf:type owl:Restriction ;
                                     owl:onProperty saref:actsUpon ;
                                     owl:someValuesFrom saref:StartStopState
                                   ] ,
                                   [ rdf:type owl:Restriction ;
                                     owl:onProperty saref:isCommandOf ;
                                     owl:allValuesFrom saref:StartStopFunction
                                   ] ;
                   owl:disjointWith saref:StopCommand ;
                   rdfs:comment "A type of command"@en ;
                   rdfs:label "Start command"@en .


###  https://saref.etsi.org/core/StartState
saref:StartState rdf:type owl:Class ;
                 rdfs:subClassOf saref:StartStopState ;
                 rdfs:comment "The state of a device that is STARTED"@en ;
                 rdfs:label "Start state"@en .


###  https://saref.etsi.org/core/StartStopFunction
saref:StartStopFunction rdf:type owl:Class ;
                        rdfs:subClassOf saref:ActuatingFunction ;
                        rdfs:comment "An actuating function that allows to start and stop a device"@en ;
                        rdfs:label "Start stop function"@en .


###  https://saref.etsi.org/core/StartStopState
saref:StartStopState rdf:type owl:Class ;
                     rdfs:subClassOf saref:State ;
                     rdfs:comment "A type of state"@en ;
                     rdfs:label "Start stop state"@en .


###  https://saref.etsi.org/core/State
saref:State rdf:type owl:Class ;
            rdfs:comment "The state in which a device can be found, e.g, ON/OFF/STANDBY, or ONLINE/OFFLINE. We propose here a list of states that are relevant for the purpose of SAREF, but this list can be extended."@en ;
            rdfs:label "State"@en .


###  https://saref.etsi.org/core/StepDownCommand
saref:StepDownCommand rdf:type owl:Class ;
                      rdfs:subClassOf saref:Command ,
                                      [ rdf:type owl:Restriction ;
                                        owl:onProperty saref:actsUpon ;
                                        owl:someValuesFrom saref:MultiLevelState
                                      ] ,
                                      [ rdf:type owl:Restriction ;
                                        owl:onProperty saref:isCommandOf ;
                                        owl:allValuesFrom saref:LevelControlFunction
                                      ] ;
                      owl:disjointWith saref:StepUpCommand ;
                      rdfs:comment "A type of command"@en ;
                      rdfs:label "Step down command"@en .


###  https://saref.etsi.org/core/StepUpCommand
saref:StepUpCommand rdf:type owl:Class ;
                    rdfs:subClassOf saref:Command ,
                                    [ rdf:type owl:Restriction ;
                                      owl:onProperty saref:actsUpon ;
                                      owl:someValuesFrom saref:MultiLevelState
                                    ] ,
                                    [ rdf:type owl:Restriction ;
                                      owl:onProperty saref:isCommandOf ;
                                      owl:allValuesFrom saref:LevelControlFunction
                                    ] ;
                    rdfs:comment "A type of command"@en ;
                    rdfs:label "Step up command"@en .


###  https://saref.etsi.org/core/StopCommand
saref:StopCommand rdf:type owl:Class ;
                  rdfs:subClassOf saref:Command ,
                                  [ rdf:type owl:Restriction ;
                                    owl:onProperty saref:actsUpon ;
                                    owl:someValuesFrom saref:StartStopState
                                  ] ,
                                  [ rdf:type owl:Restriction ;
                                    owl:onProperty saref:isCommandOf ;
                                    owl:allValuesFrom saref:StartStopFunction
                                  ] ;
                  rdfs:comment "A type of command"@en ;
                  rdfs:label "Stop command"@en .


###  https://saref.etsi.org/core/StopState
saref:StopState rdf:type owl:Class ;
                rdfs:subClassOf saref:StartStopState ;
                rdfs:comment "The state of a device that is STOPPED"@en ;
                rdfs:label "Stop state"@en .


###  https://saref.etsi.org/core/Switch
saref:Switch rdf:type owl:Class ;
             rdfs:subClassOf saref:Actuator ;
             rdfs:comment "A device of category saref:Actuator that performs an actuating function of type saref:OnOffFunction or saref:OpenCloseFunction"@en ;
             rdfs:label "Switch"@en .


###  https://saref.etsi.org/core/SwitchOnService
saref:SwitchOnService rdf:type owl:Class ;
                      rdfs:subClassOf saref:Service ,
                                      [ rdf:type owl:Restriction ;
                                        owl:onProperty saref:isOfferedBy ;
                                        owl:someValuesFrom saref:LightSwitch
                                      ] ,
                                      [ rdf:type owl:Restriction ;
                                        owl:onProperty saref:represents ;
                                        owl:someValuesFrom saref:OnOffFunction
                                      ] ;
                      rdfs:comment "A type of service that represents an on/off function to the network"@en ;
                      rdfs:label "Switch on service"@en .


###  https://saref.etsi.org/core/Task
saref:Task rdf:type owl:Class ;
           rdfs:subClassOf [ rdf:type owl:Restriction ;
                             owl:onProperty saref:isAccomplishedBy ;
                             owl:minQualifiedCardinality "1"^^xsd:nonNegativeInteger ;
                             owl:onClass saref:Device
                           ] ;
           rdfs:comment "The goal for which a device is designed (from a user perspective). For example, a washing machine is designed for the task of washing. We propose here a list of tasks that are relevant for the purpose of SAREF, but this list can be extended."@en ,
                        "The goal for which a device is designed (from a user perspective). For example, a washing machine is designed for the task of washing. We propose here a list of tasks that are relevant for the purpose of SAREF, but this list can be extended. Tasks can be accomplished by devices (saref:isAccomplishedBy)."@en ;
           rdfs:label "Task"@en .


###  https://saref.etsi.org/core/Temperature
saref:Temperature rdf:type owl:Class ;
                  rdfs:subClassOf saref:Property ;
                  rdfs:comment "A saref:Property related to some measurements that are characterized by a certain value that is measured in a temperature unit (degree_Celsius, degree_Fahrenheit, or degree_kelvin)"@en ;
                  rdfs:label "Temperature"@en .


###  https://saref.etsi.org/core/TemperatureSensor
saref:TemperatureSensor rdf:type owl:Class ;
                        rdfs:subClassOf saref:Sensor ,
                                        [ rdf:type owl:Restriction ;
                                          owl:onProperty saref:hasFunction ;
                                          owl:someValuesFrom saref:SensingFunction
                                        ] ,
                                        [ rdf:type owl:Restriction ;
                                          owl:onProperty saref:measuresProperty ;
                                          owl:someValuesFrom saref:Temperature
                                        ] ;
                        rdfs:comment "A sensor that is used for the purpose of sensing a property of type saref:Temperature. A saref:TemperatureSensor is typically used to saref:accomplish saref:Comfort."@en ;
                        rdfs:label "Temperature sensor"@en .


###  https://saref.etsi.org/core/TemperatureUnit
saref:TemperatureUnit rdf:type owl:Class ;
                      rdfs:subClassOf saref:UnitOfMeasure ;
                      rdfs:comment "The unit of measure for temperature"@en ;
                      rdfs:label "Temperature unit"@en .


###  https://saref.etsi.org/core/Time
saref:Time rdf:type owl:Class ;
           rdfs:subClassOf saref:Property ;
           rdfs:comment "A class that allows to specify the time concept."@en ,
                        "A saref:Property that allows to specify the time concept in terms of instants or intervals according to the imported W3C Time ontology."@en ;
           rdfs:label "Time"@en .


###  https://saref.etsi.org/core/ToggleCommand
saref:ToggleCommand rdf:type owl:Class ;
                    rdfs:subClassOf saref:Command ,
                                    [ rdf:type owl:Restriction ;
                                      owl:onProperty saref:isCommandOf ;
                                      owl:allValuesFrom saref:OnOffFunction
                                    ] ;
                    rdfs:comment "A type of command"@en ;
                    rdfs:label "Toggle command"@en .


###  https://saref.etsi.org/core/UnitOfMeasure
saref:UnitOfMeasure rdf:type owl:Class ;
                    rdfs:comment "The unit of measure is a standard for measurement of a quantity, such as a Property. For example,  Power is a property and Watt is a unit of power that represents a definite predetermined power: when we say 10 Watt, we actually mean 10 times the definite predetermined power called \"watt\". Our definition is based on the definition of unit of measure in the Ontology of units of Measure (OM). We propose here a list of some units of measure that are relevant for the purpose of SAREF, but this list can be extended, also using some other ontologies rather than the Ontology of units of Measure (OM)."@en ,
                                 "The unit of measure is a standard for measurement of a quantity, such as a Property. For example,  Power is a property and Watt is a unit of power that represents a definite predetermined power: when we say 10 Watt, we actually mean 10 times the definite predetermined power called \"watt\". Our definition is based on the definition of unit of measure in the Ontology of units of Measure (OM). We propose here a list of some units of measure that are relevant for the purpose of the Smart Appliances ontology, but this list can be extended."@en ,
                                 "The unit of measure is a standard for measurement of a quantity, such as a Property. For example, Power is a property and Watt is a unit of power that represents a definite predetermined power: when we say 10 Watt, we actually mean 10 times the definite predetermined power called \"watt\". Our definition is based on the definition of unit of measure in the Ontology of units of Measure (OM). We propose here a list of some units of measure that are relevant for the purpose of the Smart Appliances ontology, but this list can be extended."@en ;
                    rdfs:isDefinedBy <http://www.wurvoc.org/vocabularies/om-1.6/Unit_of_measure> ,
                                     saref: ;
                    rdfs:label "Unit of measure"@en .


###  https://saref.etsi.org/core/Water
saref:Water rdf:type owl:Class ;
            rdfs:subClassOf saref:Commodity ;
            rdfs:comment "A type of commodity"@en ;
            rdfs:label "Water"@en .


###  https://saref.etsi.org/saref4agri/Animal
s4agri:Animal rdf:type owl:Class ;
              rdfs:subClassOf saref:FeatureOfInterest ,
                              [ rdf:type owl:Restriction ;
                                owl:onProperty <http://purl.obolibrary.org/obo/TAXRANK_1000000> ;
                                owl:someValuesFrom <http://purl.obolibrary.org/obo/TAXRANK_0000000>
                              ] ,
                              [ rdf:type owl:Restriction ;
                                owl:onProperty s4agri:isLocatedIn ;
                                owl:someValuesFrom geosp:Feature
                              ] ,
                              [ rdf:type owl:Restriction ;
                                owl:onProperty s4agri:isMemberOf ;
                                owl:someValuesFrom s4agri:AnimalGroup
                              ] ,
                              [ rdf:type owl:Restriction ;
                                owl:onProperty s4agri:hasID ;
                                owl:maxQualifiedCardinality "1"^^xsd:nonNegativeInteger ;
                                owl:onClass s4agri:ID
                              ] ,
                              [ rdf:type owl:Restriction ;
                                owl:onProperty s4agri:hasBirthDate ;
                                owl:maxQualifiedCardinality "1"^^xsd:nonNegativeInteger ;
                                owl:onDataRange xsd:dateTime
                              ] ,
                              [ rdf:type owl:Restriction ;
                                owl:onProperty s4agri:hasDeathDate ;
                                owl:maxQualifiedCardinality "1"^^xsd:nonNegativeInteger ;
                                owl:onDataRange xsd:dateTime
                              ] ,
                              [ rdf:type owl:Restriction ;
                                owl:onProperty s4agri:hasName ;
                                owl:maxQualifiedCardinality "1"^^xsd:nonNegativeInteger ;
                                owl:onDataRange xsd:string
                              ] ;
              rdfs:comment "An individual and identifiable living organism that feeds on organic matter, typically having specialized sense organs and nervous system and able to respond rapidly to stimuli."@en ;
              rdfs:label "Animal"@en .


###  https://saref.etsi.org/saref4agri/AnimalGroup
s4agri:AnimalGroup rdf:type owl:Class ;
                   rdfs:subClassOf saref:FeatureOfInterest ,
                                   [ rdf:type owl:Restriction ;
                                     owl:onProperty s4agri:hasMember ;
                                     owl:someValuesFrom s4agri:Animal
                                   ] ,
                                   [ rdf:type owl:Restriction ;
                                     owl:onProperty s4agri:isLocatedIn ;
                                     owl:someValuesFrom geosp:Feature
                                   ] ,
                                   [ rdf:type owl:Restriction ;
                                     owl:onProperty s4agri:hasName ;
                                     owl:maxQualifiedCardinality "1"^^xsd:nonNegativeInteger ;
                                     owl:onDataRange xsd:string
                                   ] ;
                   rdfs:comment "A collection of one or multiple animals."@en ;
                   rdfs:label "Animal Group"@en .


###  https://saref.etsi.org/saref4agri/Building
s4agri:Building rdf:type owl:Class ;
                rdfs:subClassOf geosp:Feature ,
                                [ rdf:type owl:Restriction ;
                                  owl:onProperty s4agri:contains ;
                                  owl:someValuesFrom s4agri:BuildingSpace
                                ] ,
                                [ rdf:type owl:Restriction ;
                                  owl:onProperty s4agri:hasName ;
                                  owl:maxCardinality "1"^^xsd:nonNegativeInteger
                                ] ;
                rdfs:comment "A building represents a structure that provides shelter for its occupants or contents and stands in one place. The building is also used to provide a basic element within the spatial structure hierarchy for the components of a building project (together with site, storey, and space)."@en ;
                rdfs:label "Building"@en .


###  https://saref.etsi.org/saref4agri/BuildingSpace
s4agri:BuildingSpace rdf:type owl:Class ;
                     rdfs:subClassOf geosp:Feature ;
                     rdfs:comment "An entity used to define the physical spaces of the building. A building space contains devices or building objects."@en ;
                     rdfs:label "Building space"@en .


###  https://saref.etsi.org/saref4agri/Crop
s4agri:Crop rdf:type owl:Class ;
            rdfs:subClassOf saref:FeatureOfInterest ,
                            [ rdf:type owl:Restriction ;
                              owl:onProperty <http://purl.obolibrary.org/obo/TAXRANK_1000000> ;
                              owl:someValuesFrom <http://purl.obolibrary.org/obo/TAXRANK_0000000>
                            ] ,
                            [ rdf:type owl:Restriction ;
                              owl:onProperty s4agri:hasHarvestDate ;
                              owl:someValuesFrom xsd:dateTime
                            ] ,
                            [ rdf:type owl:Restriction ;
                              owl:onProperty s4agri:hasPlantDate ;
                              owl:someValuesFrom xsd:dateTime
                            ] ;
            rdfs:comment "A collection of cultivated plants that is grown on a large scale commercially, especially a cereal, fruit, or vegetable."@en ;
            rdfs:label "Crop"@en .


###  https://saref.etsi.org/saref4agri/Deployment
s4agri:Deployment rdf:type owl:Class ;
                  rdfs:subClassOf ssn:Deployment ,
                                  [ rdf:type owl:Restriction ;
                                    owl:onProperty ssn:deployedOnPlatform ;
                                    owl:someValuesFrom sosa:Platform
                                  ] ,
                                  [ rdf:type owl:Restriction ;
                                    owl:onProperty ssn:deployedSystem ;
                                    owl:someValuesFrom ssn:System
                                  ] ,
                                  [ rdf:type owl:Restriction ;
                                    owl:onProperty s4agri:hasDeploymentPeriod ;
                                    owl:someValuesFrom time:TemporalEntity
                                  ] ,
                                  [ rdf:type owl:Restriction ;
                                    owl:onProperty s4agri:isDeployedAtSpace ;
                                    owl:someValuesFrom geosp:SpatialObject
                                  ] ;
                  rdfs:comment "Deployment"@en ,
                               "The scenario, including temporal and spatial information, in which the systems and devices are installed."@en ;
                  rdfs:label "Deployment"@en .


###  https://saref.etsi.org/saref4agri/EatingActivitySensor
s4agri:EatingActivitySensor rdf:type owl:Class ;
                            rdfs:subClassOf saref:Sensor ;
                            rdfs:comment "Eating activity sensor"@en ;
                            rdfs:label "Eating activity sensor"@en .


###  https://saref.etsi.org/saref4agri/Farm
s4agri:Farm rdf:type owl:Class ;
            rdfs:subClassOf geosp:Feature ,
                            [ rdf:type owl:Restriction ;
                              owl:onProperty s4agri:contains ;
                              owl:someValuesFrom s4agri:Building
                            ] ,
                            [ rdf:type owl:Restriction ;
                              owl:onProperty s4agri:contains ;
                              owl:someValuesFrom s4agri:Parcel
                            ] ,
                            [ rdf:type owl:Restriction ;
                              owl:onProperty s4agri:hasName ;
                              owl:maxCardinality "1"^^xsd:nonNegativeInteger
                            ] ;
            rdfs:comment "A plot of land used for the scope of farming which can contain buildings and parcels."@en ;
            rdfs:label "Farm"@en .


###  https://saref.etsi.org/saref4agri/FarmHolding
s4agri:FarmHolding rdf:type owl:Class ;
                   rdfs:subClassOf schema:Organization ,
                                   [ rdf:type owl:Restriction ;
                                     owl:onProperty s4agri:managesFarm ;
                                     owl:someValuesFrom s4agri:Farm
                                   ] ,
                                   [ rdf:type owl:Restriction ;
                                     owl:onProperty s4agri:hasName ;
                                     owl:allValuesFrom xsd:string
                                   ] ;
                   rdfs:comment "A class to decsribe a saref4agri farm holding as subcass of an org:Organization"@en ;
                   rdfs:label "Farm holding"@en .


###  https://saref.etsi.org/saref4agri/Farmer
s4agri:Farmer rdf:type owl:Class ;
              rdfs:subClassOf foaf:Person ,
                              [ rdf:type owl:Restriction ;
                                owl:onProperty s4agri:managesFarm ;
                                owl:someValuesFrom s4agri:Farm
                              ] ,
                              [ rdf:type owl:Restriction ;
                                owl:onProperty s4agri:hasName ;
                                owl:allValuesFrom xsd:string
                              ] ;
              rdfs:comment "A class to decsribe a saref4agri farmer as subcass of a foaf:Person"@en ;
              rdfs:label "Farmer"@en .


###  https://saref.etsi.org/saref4agri/ID
s4agri:ID rdf:type owl:Class ;
          rdfs:comment "ID"@en ;
          rdfs:label "ID"@en .


###  https://saref.etsi.org/saref4agri/Intake
s4agri:Intake rdf:type owl:Class ;
              rdfs:comment "The amount of food or other substance taken into the body of an animal or into the soil."@en ;
              rdfs:label "Intake"@en .


###  https://saref.etsi.org/saref4agri/MilkingSensor
s4agri:MilkingSensor rdf:type owl:Class ;
                     rdfs:subClassOf saref:Sensor ;
                     rdfs:comment "Milking sensor"@en ;
                     rdfs:label "Milking sensor"@en .


###  https://saref.etsi.org/saref4agri/MovementActivitySensor
s4agri:MovementActivitySensor rdf:type owl:Class ;
                              rdfs:subClassOf saref:Sensor ;
                              rdfs:comment "Movement activity sensor"@en ;
                              rdfs:label "Movement activity sensor"@en .


###  https://saref.etsi.org/saref4agri/Parcel
s4agri:Parcel rdf:type owl:Class ;
              rdfs:subClassOf geosp:Feature ,
                              [ rdf:type owl:Restriction ;
                                owl:onProperty s4agri:contains ;
                                owl:someValuesFrom s4agri:Crop
                              ] ,
                              [ rdf:type owl:Restriction ;
                                owl:onProperty s4agri:hasName ;
                                owl:maxQualifiedCardinality "1"^^xsd:nonNegativeInteger ;
                                owl:onDataRange xsd:string
                              ] ;
              rdfs:comment "An area of land, which might be used for grazing animals or planting crops. The parcel is defined as an undividable logical area of land which contains homogeneous items."@en ;
              rdfs:label "Parcel"@en .


###  https://saref.etsi.org/saref4agri/Platform
s4agri:Platform rdf:type owl:Class ;
                rdfs:subClassOf sosa:Platform ;
                rdfs:comment "Platform"@en ;
                rdfs:label "Platform"@en .


###  https://saref.etsi.org/saref4agri/Pluviometer
s4agri:Pluviometer rdf:type owl:Class ;
                   rdfs:subClassOf saref:Sensor ;
                   rdfs:comment "A sensor that measures the rain fall."@en ;
                   rdfs:label "Pluviometer"@en .


###  https://saref.etsi.org/saref4agri/Soil
s4agri:Soil rdf:type owl:Class ;
            rdfs:subClassOf saref:FeatureOfInterest ;
            rdfs:comment "Upper layer of the earth in which plants grow."@en ;
            rdfs:label "Soil"@en .


###  https://saref.etsi.org/saref4agri/SoilTensiometer
s4agri:SoilTensiometer rdf:type owl:Class ;
                       rdfs:subClassOf saref:Sensor ;
                       rdfs:comment "A sensor that measures the soil moisture."@en ;
                       rdfs:label "Soil tensiometer"@en .


###  https://saref.etsi.org/saref4agri/Thermometer
s4agri:Thermometer rdf:type owl:Class ;
                   rdfs:subClassOf saref:Sensor ;
                   rdfs:comment "Thermometer"@en ;
                   rdfs:label "Thermometer"@en .


###  https://saref.etsi.org/saref4agri/WateringGun
s4agri:WateringGun rdf:type owl:Class ;
                   rdfs:subClassOf saref:Actuator ;
                   rdfs:comment "An actuator to irrigate an space."@en ;
                   rdfs:label "Watering gun"@en .


###  https://saref.etsi.org/saref4agri/WateringSystem
s4agri:WateringSystem rdf:type owl:Class ;
                      rdfs:subClassOf ssn:System ;
                      rdfs:comment "Watering system"@en ;
                      rdfs:label "Watering system"@en .


###  https://saref.etsi.org/saref4agri/WateringValve
s4agri:WateringValve rdf:type owl:Class ;
                     rdfs:subClassOf saref:Actuator ;
                     rdfs:comment "Watering valve"@en ;
                     rdfs:label "Watering valve"@en .


###  https://saref.etsi.org/saref4agri/WeatherStation
s4agri:WeatherStation rdf:type owl:Class ;
                      rdfs:subClassOf ssn:System ,
                                      saref:Sensor ;
                      rdfs:comment "A sensor o system that measure weather conditions."@en ;
                      rdfs:label "Weather station"@en .


###  https://saref.etsi.org/saref4agri/WeightSensor
s4agri:WeightSensor rdf:type owl:Class ;
                    rdfs:subClassOf saref:Sensor ;
                    rdfs:comment "Weight sensor"@en ;
                    rdfs:label "Weight sensor"@en .


###  https://saref.etsi.org/saref4agri/Yield
s4agri:Yield rdf:type owl:Class ;
             rdfs:comment "The produced amount of food for animals or of agricultural products."@en ;
             rdfs:label "Yield"@en .


###  https://saref.etsi.org/saref4bldg/Actuator
s4bldg:Actuator rdf:type owl:Class ;
                rdfs:subClassOf saref:Actuator ,
                                s4bldg:DistributionControlDevice ,
                                [ rdf:type owl:Restriction ;
                                  owl:onProperty s4bldg:failPosition ;
                                  owl:allValuesFrom xsd:string
                                ] ,
                                [ rdf:type owl:Restriction ;
                                  owl:onProperty s4bldg:manualOverride ;
                                  owl:allValuesFrom xsd:boolean
                                ] ;
                rdfs:comment "An actuator is a mechanical device for moving or controlling a mechanism or system. An actuator takes energy, usually created by air, electricity, or liquid, and converts that into some kind of motion."@en ;
                rdfs:label "Actuator"@en ;
                rdfs:seeAlso "https://w3id.org/ifc/IFC4_ADD1#IfcActuator" ;
                prov:hadPrimarySource <http://www.buildingsmart-tech.org/ifc/IFC4/Add1/html/schema/ifcbuildingcontrolsdomain/lexical/ifcactuator.htm> ,
                                      <http://www.buildingsmart-tech.org/ifc/IFC4/Add1/html/schema/ifcbuildingcontrolsdomain/pset/pset_actuatortypecommon.htm> .


###  https://saref.etsi.org/saref4bldg/AirToAirHeatRecovery
s4bldg:AirToAirHeatRecovery rdf:type owl:Class ;
                            rdfs:subClassOf s4bldg:EnergyConversionDevice ,
                                            [ rdf:type owl:Restriction ;
                                              owl:onProperty s4bldg:operationTemperatureMax ;
                                              owl:allValuesFrom saref:Measurement
                                            ] ,
                                            [ rdf:type owl:Restriction ;
                                              owl:onProperty s4bldg:operationTemperatureMin ;
                                              owl:allValuesFrom saref:Measurement
                                            ] ,
                                            [ rdf:type owl:Restriction ;
                                              owl:onProperty s4bldg:primaryAirFlowRateMax ;
                                              owl:allValuesFrom saref:Measurement
                                            ] ,
                                            [ rdf:type owl:Restriction ;
                                              owl:onProperty s4bldg:primaryAirFlowRateMin ;
                                              owl:allValuesFrom saref:Measurement
                                            ] ,
                                            [ rdf:type owl:Restriction ;
                                              owl:onProperty s4bldg:secondaryAirFlowRateMax ;
                                              owl:allValuesFrom saref:Measurement
                                            ] ,
                                            [ rdf:type owl:Restriction ;
                                              owl:onProperty s4bldg:secondaryAirFlowRateMin ;
                                              owl:allValuesFrom saref:Measurement
                                            ] ,
                                            [ rdf:type owl:Restriction ;
                                              owl:onProperty s4bldg:hasDefrost ;
                                              owl:allValuesFrom xsd:boolean
                                            ] ,
                                            [ rdf:type owl:Restriction ;
                                              owl:onProperty s4bldg:heatTransferTypeEnum ;
                                              owl:allValuesFrom xsd:string
                                            ] ;
                            rdfs:comment "An air-to-air heat recovery device employs a counter-flow heat exchanger between inbound and outbound air flow. It is typically used to transfer heat from warmer air in one chamber to cooler air in the second chamber (i.e., typically used to recover heat from the conditioned air being exhausted and the outside air being supplied to a building), resulting in energy savings from reduced heating (or cooling) requirements."@en ;
                            rdfs:label "Air to air heat recovery"@en ;
                            rdfs:seeAlso "https://w3id.org/ifc/IFC4_ADD1#IfcAirToAirHeatRecovery" ;
                            prov:hadPrimarySource <http://www.buildingsmart-tech.org/ifc/IFC4/Add1/html/schema/ifchvacdomain/lexical/ifcairtoairheatrecovery.htm> ,
                                                  <http://www.buildingsmart-tech.org/ifc/IFC4/Add1/html/schema/ifchvacdomain/pset/pset_airtoairheatrecoverytypecommon.htm> .


###  https://saref.etsi.org/saref4bldg/Alarm
s4bldg:Alarm rdf:type owl:Class ;
             rdfs:subClassOf s4bldg:DistributionControlDevice ;
             rdfs:comment """An alarm is a device that signals the existence of a condition or situation that is outside the boundaries of normal expectation or that activates such a device.

Alarms include the provision of break glass buttons and manual pull boxes that are used to activate alarms."""@en ;
             rdfs:label "Alarm"@en ;
             rdfs:seeAlso "https://w3id.org/ifc/IFC4_ADD1#IfcAlarm" ;
             prov:hadPrimarySource <http://www.buildingsmart-tech.org/ifc/IFC4/Add1/html/schema/ifcbuildingcontrolsdomain/lexical/ifcalarm.htm> ,
                                   <http://www.buildingsmart-tech.org/ifc/IFC4/Add1/html/schema/ifcbuildingcontrolsdomain/pset/pset_alarmtypecommon.htm> .


###  https://saref.etsi.org/saref4bldg/AudioVisualAppliance
s4bldg:AudioVisualAppliance rdf:type owl:Class ;
                            rdfs:subClassOf s4bldg:FlowTerminal ,
                                            [ rdf:type owl:Restriction ;
                                              owl:onProperty s4bldg:audioVolume ;
                                              owl:allValuesFrom saref:Measurement
                                            ] ,
                                            [ rdf:type owl:Restriction ;
                                              owl:onProperty s4bldg:mediaSource ;
                                              owl:allValuesFrom xsd:string
                                            ] ;
                            rdfs:comment """An audio-visual appliance is a device that displays, captures, transmits, or receives audio or video.

Audio-visual appliances may be fixed in place or may be able to be moved from one space to another. They may require an electrical supply that may be supplied either by an electrical circuit or provided from a local battery source. Audio-visual appliances may be connected to data circuits including specialist circuits for audio visual purposes only."""@en ;
                            rdfs:label "Audio visual appliance"@en ;
                            rdfs:seeAlso "https://w3id.org/ifc/IFC4_ADD1#IfcAudioVisualApplicance" ;
                            prov:hadPrimarySource <http://www.buildingsmart-tech.org/ifc/IFC4/Add1/html/schema/ifcelectricaldomain/lexical/ifcaudiovisualappliance.htm> ,
                                                  <http://www.buildingsmart-tech.org/ifc/IFC4/Add1/html/schema/ifcelectricaldomain/pset/pset_audiovisualappliancetypecommon.htm> .


###  https://saref.etsi.org/saref4bldg/Boiler
s4bldg:Boiler rdf:type owl:Class ;
              rdfs:subClassOf s4bldg:EnergyConversionDevice ,
                              [ rdf:type owl:Restriction ;
                                owl:onProperty s4bldg:heatTransferSurfaceArea ;
                                owl:allValuesFrom saref:Measurement
                              ] ,
                              [ rdf:type owl:Restriction ;
                                owl:onProperty s4bldg:nominalEnergyConsumption ;
                                owl:allValuesFrom saref:Measurement
                              ] ,
                              [ rdf:type owl:Restriction ;
                                owl:onProperty s4bldg:nominalPartLoadRatio ;
                                owl:allValuesFrom saref:Measurement
                              ] ,
                              [ rdf:type owl:Restriction ;
                                owl:onProperty s4bldg:outletTemperatureMax ;
                                owl:allValuesFrom saref:Measurement
                              ] ,
                              [ rdf:type owl:Restriction ;
                                owl:onProperty s4bldg:outletTemperatureMin ;
                                owl:allValuesFrom saref:Measurement
                              ] ,
                              [ rdf:type owl:Restriction ;
                                owl:onProperty s4bldg:pressureRating ;
                                owl:allValuesFrom saref:Measurement
                              ] ,
                              [ rdf:type owl:Restriction ;
                                owl:onProperty s4bldg:waterInletTemperatureMax ;
                                owl:allValuesFrom saref:Measurement
                              ] ,
                              [ rdf:type owl:Restriction ;
                                owl:onProperty s4bldg:waterInletTemperatureMin ;
                                owl:allValuesFrom saref:Measurement
                              ] ,
                              [ rdf:type owl:Restriction ;
                                owl:onProperty s4bldg:waterStorageCapacity ;
                                owl:allValuesFrom saref:Measurement
                              ] ,
                              [ rdf:type owl:Restriction ;
                                owl:onProperty s4bldg:energySource ;
                                owl:allValuesFrom xsd:string
                              ] ,
                              [ rdf:type owl:Restriction ;
                                owl:onProperty s4bldg:isWaterStorageHeater ;
                                owl:allValuesFrom xsd:boolean
                              ] ,
                              [ rdf:type owl:Restriction ;
                                owl:onProperty s4bldg:operatingMode ;
                                owl:allValuesFrom xsd:string
                              ] ;
              rdfs:comment "A boiler is a closed, pressure-rated vessel in which water or other fluid is heated using an energy source such as natural gas, heating oil, or electricity. The fluid in the vessel is then circulated out of the boiler for use in various processes or heating applications."@en ;
              rdfs:label "Boiler"@en ;
              rdfs:seeAlso "https://w3id.org/ifc/IFC4_ADD1#IfcBoiler" ;
              prov:hadPrimarySource <http://www.buildingsmart-tech.org/ifc/IFC4/Add1/html/schema/ifchvacdomain/lexical/ifcboiler.htm> ,
                                    <http://www.buildingsmart-tech.org/ifc/IFC4/Add1/html/schema/ifchvacdomain/pset/pset_boilertypecommon.htm> .


###  https://saref.etsi.org/saref4bldg/Building
s4bldg:Building rdf:type owl:Class ;
                rdfs:subClassOf [ rdf:type owl:Restriction ;
                                  owl:onProperty s4bldg:hasSpace ;
                                  owl:allValuesFrom s4bldg:BuildingSpace
                                ] ;
                rdfs:comment "A building represents a structure that provides shelter for its occupants or contents and stands in one place. The building is also used to provide a basic element within the spatial structure hierarchy for the components of a building project (together with site, storey, and space)."@en ;
                rdfs:label "Building"@en ;
                rdfs:seeAlso <https://w3id.org/ifc/IFC4_ADD1#IfcBuilding> ;
                prov:hadPrimarySource <http://www.buildingsmart-tech.org/ifc/IFC4/Add1/html/schema/ifcproductextension/lexical/ifcbuilding.htm> .


###  https://saref.etsi.org/saref4bldg/BuildingDevice
s4bldg:BuildingDevice rdf:type owl:Class ;
                      rdfs:subClassOf saref:Device ,
                                      s4bldg:BuildingObject ;
                      rdfs:comment "A tangible object designed to accomplish a particular task in a building."@en ;
                      rdfs:label "Building device"@en .


###  https://saref.etsi.org/saref4bldg/BuildingObject
s4bldg:BuildingObject rdf:type owl:Class ;
                      rdfs:subClassOf s4bldg:PhysicalObject ;
                      rdfs:comment "An object in the building that can be controlled by devices, such as a door or a window that can be automatically opened or closed by an actuator.  (Definition taken from SAREF 1.0)"@en ;
                      rdfs:label "Building object"@en .


###  https://saref.etsi.org/saref4bldg/BuildingSpace
s4bldg:BuildingSpace rdf:type owl:Class ;
                     rdfs:subClassOf [ rdf:type owl:Restriction ;
                                       owl:onProperty s4bldg:contains ;
                                       owl:allValuesFrom s4bldg:PhysicalObject
                                     ] ,
                                     [ rdf:type owl:Restriction ;
                                       owl:onProperty s4bldg:hasSpace ;
                                       owl:allValuesFrom s4bldg:BuildingSpace
                                     ] ,
                                     [ rdf:type owl:Restriction ;
                                       owl:onProperty s4bldg:isSpaceOf ;
                                       owl:allValuesFrom [ rdf:type owl:Class ;
                                                           owl:unionOf ( s4bldg:Building
                                                                         s4bldg:BuildingSpace
                                                                       )
                                                         ]
                                     ] ;
                     rdfs:comment "An entity used to define the physical spaces of the building. A building space contains devices or building objects."@en ;
                     rdfs:label "Building space"@en .


###  https://saref.etsi.org/saref4bldg/Burner
s4bldg:Burner rdf:type owl:Class ;
              rdfs:subClassOf s4bldg:EnergyConversionDevice ,
                              [ rdf:type owl:Restriction ;
                                owl:onProperty s4bldg:energySource ;
                                owl:allValuesFrom xsd:string
                              ] ;
              rdfs:comment "A burner is a device that converts fuel into heat through combustion. It includes gas, oil, and wood burners."@en ;
              rdfs:label "Burner"@en ;
              rdfs:seeAlso "https://w3id.org/ifc/IFC4_ADD1#IfcBurner" ;
              prov:hadPrimarySource <http://www.buildingsmart-tech.org/ifc/IFC4/Add1/html/schema/ifchvacdomain/lexical/ifcburner.htm> ,
                                    <http://www.buildingsmart-tech.org/ifc/IFC4/Add1/html/schema/ifchvacdomain/pset/pset_burnertypecommon.htm> .


###  https://saref.etsi.org/saref4bldg/Chiller
s4bldg:Chiller rdf:type owl:Class ;
               rdfs:subClassOf s4bldg:EnergyConversionDevice ,
                               [ rdf:type owl:Restriction ;
                                 owl:onProperty s4bldg:nominalCapacity ;
                                 owl:allValuesFrom saref:Measurement
                               ] ,
                               [ rdf:type owl:Restriction ;
                                 owl:onProperty s4bldg:nominalCondensingTemperature ;
                                 owl:allValuesFrom saref:Measurement
                               ] ,
                               [ rdf:type owl:Restriction ;
                                 owl:onProperty s4bldg:nominalEfficiency ;
                                 owl:allValuesFrom saref:Measurement
                               ] ,
                               [ rdf:type owl:Restriction ;
                                 owl:onProperty s4bldg:nominalEvaporatingTemmperature ;
                                 owl:allValuesFrom saref:Measurement
                               ] ,
                               [ rdf:type owl:Restriction ;
                                 owl:onProperty s4bldg:nominalHeatRejectionRate ;
                                 owl:allValuesFrom saref:Measurement
                               ] ,
                               [ rdf:type owl:Restriction ;
                                 owl:onProperty s4bldg:nominalPowerConsumption ;
                                 owl:allValuesFrom saref:Measurement
                               ] ;
               rdfs:comment "A chiller is a device used to remove heat from a liquid via a vapor-compression or absorption refrigeration cycle to cool a fluid, typically water or a mixture of water and glycol. The chilled fluid is then used to cool and dehumidify air in a building."@en ;
               rdfs:label "Chiller"@en ;
               rdfs:seeAlso "https://w3id.org/ifc/IFC4_ADD1#IfcChiller" ;
               prov:hadPrimarySource <http://www.buildingsmart-tech.org/ifc/IFC4/Add1/html/schema/ifchvacdomain/lexical/ifcchiller.htm> ,
                                     <http://www.buildingsmart-tech.org/ifc/IFC4/Add1/html/schema/ifchvacdomain/pset/pset_chillertypecommon.htm> .


###  https://saref.etsi.org/saref4bldg/Coil
s4bldg:Coil rdf:type owl:Class ;
            rdfs:subClassOf s4bldg:EnergyConversionDevice ,
                            [ rdf:type owl:Restriction ;
                              owl:onProperty s4bldg:airFlowRateMax ;
                              owl:allValuesFrom saref:Measurement
                            ] ,
                            [ rdf:type owl:Restriction ;
                              owl:onProperty s4bldg:airFlowRateMin ;
                              owl:allValuesFrom saref:Measurement
                            ] ,
                            [ rdf:type owl:Restriction ;
                              owl:onProperty s4bldg:nominalLatentCapacity ;
                              owl:allValuesFrom saref:Measurement
                            ] ,
                            [ rdf:type owl:Restriction ;
                              owl:onProperty s4bldg:nominalSensibleCapacity ;
                              owl:allValuesFrom saref:Measurement
                            ] ,
                            [ rdf:type owl:Restriction ;
                              owl:onProperty s4bldg:nominalUa ;
                              owl:allValuesFrom saref:Measurement
                            ] ,
                            [ rdf:type owl:Restriction ;
                              owl:onProperty s4bldg:operationTemperatureMax ;
                              owl:allValuesFrom saref:Measurement
                            ] ,
                            [ rdf:type owl:Restriction ;
                              owl:onProperty s4bldg:operationTemperatureMin ;
                              owl:allValuesFrom saref:Measurement
                            ] ,
                            [ rdf:type owl:Restriction ;
                              owl:onProperty s4bldg:placementType ;
                              owl:allValuesFrom xsd:string
                            ] ;
            rdfs:comment """A coil is a device used to provide heat transfer between non-mixing media. A common example is a cooling coil, which utilizes a finned coil in which circulates chilled water, antifreeze, or refrigerant that is used to remove heat from air moving across the surface of the coil. A coil may be used either for heating or cooling purposes by placing a series of tubes (the coil) carrying a heating or cooling fluid into an airstream. The coil may be constructed from tubes bundled in a serpentine form or from finned tubes that give a extended heat transfer surface.

Coils may also be used for non-airflow cases such as embedded in a floor slab."""@en ;
            rdfs:label "Coil"@en ;
            rdfs:seeAlso "https://w3id.org/ifc/IFC4_ADD1#IfcCoil" ;
            prov:hadPrimarySource <http://www.buildingsmart-tech.org/ifc/IFC4/Add1/html/schema/ifchvacdomain/lexical/ifccoil.htm> ,
                                  <http://www.buildingsmart-tech.org/ifc/IFC4/Add1/html/schema/ifchvacdomain/pset/pset_coiltypecommon.htm> .


###  https://saref.etsi.org/saref4bldg/CommunicationAppliance
s4bldg:CommunicationAppliance rdf:type owl:Class ;
                              rdfs:subClassOf s4bldg:FlowTerminal ;
                              rdfs:comment """A communications appliance transmits and receives electronic or digital information as data or sound.

Communication appliances may be fixed in place or may be able to be moved from one space to another. Communication appliances require an electrical supply that may be supplied either by an electrical circuit or provided from a local battery source."""@en ;
                              rdfs:label "Communication appliance"@en ;
                              rdfs:seeAlso "https://w3id.org/ifc/IFC4_ADD1#IfcCommunicationAppliance" ;
                              prov:hadPrimarySource <http://www.buildingsmart-tech.org/ifc/IFC4/Add1/html/schema/ifcelectricaldomain/lexical/ifccommunicationsappliance.htm> ,
                                                    <http://www.buildingsmart-tech.org/ifc/IFC4/Add1/html/schema/ifcelectricaldomain/pset/pset_communicationsappliancetypecommon.htm> .


###  https://saref.etsi.org/saref4bldg/Compressor
s4bldg:Compressor rdf:type owl:Class ;
                  rdfs:subClassOf s4bldg:FlowMovingDevice ,
                                  [ rdf:type owl:Restriction ;
                                    owl:onProperty s4bldg:compressorSpeed ;
                                    owl:allValuesFrom saref:Measurement
                                  ] ,
                                  [ rdf:type owl:Restriction ;
                                    owl:onProperty s4bldg:idealCapacity ;
                                    owl:allValuesFrom saref:Measurement
                                  ] ,
                                  [ rdf:type owl:Restriction ;
                                    owl:onProperty s4bldg:idealShaftPower ;
                                    owl:allValuesFrom saref:Measurement
                                  ] ,
                                  [ rdf:type owl:Restriction ;
                                    owl:onProperty s4bldg:impellerDiameter ;
                                    owl:allValuesFrom saref:Measurement
                                  ] ,
                                  [ rdf:type owl:Restriction ;
                                    owl:onProperty s4bldg:nominalCapacity ;
                                    owl:allValuesFrom saref:Measurement
                                  ] ,
                                  [ rdf:type owl:Restriction ;
                                    owl:onProperty s4bldg:partLoadRatioMax ;
                                    owl:allValuesFrom saref:Measurement
                                  ] ,
                                  [ rdf:type owl:Restriction ;
                                    owl:onProperty s4bldg:partLoadRatioMin ;
                                    owl:allValuesFrom saref:Measurement
                                  ] ,
                                  [ rdf:type owl:Restriction ;
                                    owl:onProperty s4bldg:hasHotGasBypass ;
                                    owl:allValuesFrom xsd:boolean
                                  ] ,
                                  [ rdf:type owl:Restriction ;
                                    owl:onProperty s4bldg:powerSource ;
                                    owl:allValuesFrom xsd:string
                                  ] ,
                                  [ rdf:type owl:Restriction ;
                                    owl:onProperty s4bldg:refrigerantClass ;
                                    owl:allValuesFrom xsd:string
                                  ] ;
                  rdfs:comment "A compressor is a device that compresses a fluid typically used in a refrigeration circuit."@en ;
                  rdfs:label "Compressor"@en ;
                  rdfs:seeAlso "https://w3id.org/ifc/IFC4_ADD1#IfcCompressor" ;
                  prov:hadPrimarySource <http://www.buildingsmart-tech.org/ifc/IFC4/Add1/html/schema/ifchvacdomain/lexical/ifccompressor.htm> ,
                                        <http://www.buildingsmart-tech.org/ifc/IFC4/Add1/html/schema/ifchvacdomain/pset/pset_compressortypecommon.htm> .


###  https://saref.etsi.org/saref4bldg/Condenser
s4bldg:Condenser rdf:type owl:Class ;
                 rdfs:subClassOf s4bldg:EnergyConversionDevice ,
                                 [ rdf:type owl:Restriction ;
                                   owl:onProperty s4bldg:externalSurfaceArea ;
                                   owl:allValuesFrom saref:Measurement
                                 ] ,
                                 [ rdf:type owl:Restriction ;
                                   owl:onProperty s4bldg:internalRefrigerantVolume ;
                                   owl:allValuesFrom saref:Measurement
                                 ] ,
                                 [ rdf:type owl:Restriction ;
                                   owl:onProperty s4bldg:internalSurfaceArea ;
                                   owl:allValuesFrom saref:Measurement
                                 ] ,
                                 [ rdf:type owl:Restriction ;
                                   owl:onProperty s4bldg:internalWaterVolume ;
                                   owl:allValuesFrom saref:Measurement
                                 ] ,
                                 [ rdf:type owl:Restriction ;
                                   owl:onProperty s4bldg:nominalHeatTransferArea ;
                                   owl:allValuesFrom saref:Measurement
                                 ] ,
                                 [ rdf:type owl:Restriction ;
                                   owl:onProperty s4bldg:nominalHeatTransferCoefficient ;
                                   owl:allValuesFrom saref:Measurement
                                 ] ,
                                 [ rdf:type owl:Restriction ;
                                   owl:onProperty s4bldg:refrigerantClass ;
                                   owl:allValuesFrom xsd:string
                                 ] ;
                 rdfs:comment "A condenser is a device that is used to dissipate heat, typically by condensing a substance such as a refrigerant from its gaseous to its liquid state."@en ;
                 rdfs:label "Condenser"@en ;
                 rdfs:seeAlso "https://w3id.org/ifc/IFC4_ADD1#IfcCondenser" ;
                 prov:hadPrimarySource <http://www.buildingsmart-tech.org/ifc/IFC4/Add1/html/schema/ifchvacdomain/lexical/ifccondenser.htm> ,
                                       <http://www.buildingsmart-tech.org/ifc/IFC4/Add1/html/schema/ifchvacdomain/pset/pset_condensertypecommon.htm> .


###  https://saref.etsi.org/saref4bldg/Controller
s4bldg:Controller rdf:type owl:Class ;
                  rdfs:subClassOf s4bldg:DistributionControlDevice ;
                  rdfs:comment """A controller is a device that monitors inputs and controls outputs within a building automation system.

A controller may be physical (having placement within a spatial structure) or logical (a software interface or aggregated within a programmable physical controller)."""@en ;
                  rdfs:label "Controller"@en ;
                  rdfs:seeAlso "https://w3id.org/ifc/IFC4_ADD1#IfcController" ;
                  prov:hadPrimarySource <http://www.buildingsmart-tech.org/ifc/IFC4/Add1/html/schema/ifcbuildingcontrolsdomain/lexical/ifccontroller.htm> ,
                                        <http://www.buildingsmart-tech.org/ifc/IFC4/Add1/html/schema/ifcbuildingcontrolsdomain/pset/pset_controllertypecommon.htm> .


###  https://saref.etsi.org/saref4bldg/CooledBeam
s4bldg:CooledBeam rdf:type owl:Class ;
                  rdfs:subClassOf s4bldg:EnergyConversionDevice ,
                                  [ rdf:type owl:Restriction ;
                                    owl:onProperty s4bldg:coilLength ;
                                    owl:allValuesFrom saref:Measurement
                                  ] ,
                                  [ rdf:type owl:Restriction ;
                                    owl:onProperty s4bldg:coilWidth ;
                                    owl:allValuesFrom saref:Measurement
                                  ] ,
                                  [ rdf:type owl:Restriction ;
                                    owl:onProperty s4bldg:nominalCoolingCapacity ;
                                    owl:allValuesFrom saref:Measurement
                                  ] ,
                                  [ rdf:type owl:Restriction ;
                                    owl:onProperty s4bldg:nominalHeatingCapacity ;
                                    owl:allValuesFrom saref:Measurement
                                  ] ,
                                  [ rdf:type owl:Restriction ;
                                    owl:onProperty s4bldg:nominalReturnWaterTemperatureCooling ;
                                    owl:allValuesFrom saref:Measurement
                                  ] ,
                                  [ rdf:type owl:Restriction ;
                                    owl:onProperty s4bldg:nominalReturnWaterTemperatureHeating ;
                                    owl:allValuesFrom saref:Measurement
                                  ] ,
                                  [ rdf:type owl:Restriction ;
                                    owl:onProperty s4bldg:nominalSorroundingHumidityCooling ;
                                    owl:allValuesFrom saref:Measurement
                                  ] ,
                                  [ rdf:type owl:Restriction ;
                                    owl:onProperty s4bldg:nominalSorroundingTemperatureCooling ;
                                    owl:allValuesFrom saref:Measurement
                                  ] ,
                                  [ rdf:type owl:Restriction ;
                                    owl:onProperty s4bldg:nominalSorroundingTemperatureHeating ;
                                    owl:allValuesFrom saref:Measurement
                                  ] ,
                                  [ rdf:type owl:Restriction ;
                                    owl:onProperty s4bldg:nominalSupplyWaterTemperatureCooling ;
                                    owl:allValuesFrom saref:Measurement
                                  ] ,
                                  [ rdf:type owl:Restriction ;
                                    owl:onProperty s4bldg:nominalSupplyWaterTemperatureHeating ;
                                    owl:allValuesFrom saref:Measurement
                                  ] ,
                                  [ rdf:type owl:Restriction ;
                                    owl:onProperty s4bldg:nominalWaterFlowCooling ;
                                    owl:allValuesFrom saref:Measurement
                                  ] ,
                                  [ rdf:type owl:Restriction ;
                                    owl:onProperty s4bldg:nominalWaterFlowHeating ;
                                    owl:allValuesFrom saref:Measurement
                                  ] ,
                                  [ rdf:type owl:Restriction ;
                                    owl:onProperty s4bldg:waterPressureMax ;
                                    owl:allValuesFrom saref:Measurement
                                  ] ,
                                  [ rdf:type owl:Restriction ;
                                    owl:onProperty s4bldg:waterPressureMin ;
                                    owl:allValuesFrom saref:Measurement
                                  ] ,
                                  [ rdf:type owl:Restriction ;
                                    owl:onProperty s4bldg:finishColor ;
                                    owl:allValuesFrom xsd:string
                                  ] ,
                                  [ rdf:type owl:Restriction ;
                                    owl:onProperty s4bldg:integratedLightingType ;
                                    owl:allValuesFrom xsd:string
                                  ] ,
                                  [ rdf:type owl:Restriction ;
                                    owl:onProperty s4bldg:isFreeHanging ;
                                    owl:allValuesFrom xsd:boolean
                                  ] ,
                                  [ rdf:type owl:Restriction ;
                                    owl:onProperty s4bldg:pipeConnectionEnum ;
                                    owl:allValuesFrom xsd:string
                                  ] ,
                                  [ rdf:type owl:Restriction ;
                                    owl:onProperty s4bldg:waterFlowControlSystemType ;
                                    owl:allValuesFrom xsd:string
                                  ] ;
                  rdfs:comment "A cooled beam (or chilled beam) is a device typically used to cool air by circulating a fluid such as chilled water through exposed finned tubes above a space. Typically mounted overhead near or within a ceiling, the cooled beam uses convection to cool the space below it by acting as a heat sink for the naturally rising warm air of the space. Once cooled, the air naturally drops back to the floor where the cycle begins again."@en ;
                  rdfs:label "Cooled beam"@en ;
                  rdfs:seeAlso "https://w3id.org/ifc/IFC4_ADD1#IfcCooledBeam" ;
                  prov:hadPrimarySource <http://www.buildingsmart-tech.org/ifc/IFC4/Add1/html/schema/ifchvacdomain/lexical/ifccooledbeam.htm> ,
                                        <http://www.buildingsmart-tech.org/ifc/IFC4/Add1/html/schema/ifchvacdomain/pset/pset_cooledbeamtypecommon.htm> .


###  https://saref.etsi.org/saref4bldg/CoolingTower
s4bldg:CoolingTower rdf:type owl:Class ;
                    rdfs:subClassOf s4bldg:EnergyConversionDevice ,
                                    [ rdf:type owl:Restriction ;
                                      owl:onProperty s4bldg:ambientDesignDryBulbTemperature ;
                                      owl:allValuesFrom saref:Measurement
                                    ] ,
                                    [ rdf:type owl:Restriction ;
                                      owl:onProperty s4bldg:ambientDesignWetBulbTemperature ;
                                      owl:allValuesFrom saref:Measurement
                                    ] ,
                                    [ rdf:type owl:Restriction ;
                                      owl:onProperty s4bldg:basinReserveVolume ;
                                      owl:allValuesFrom saref:Measurement
                                    ] ,
                                    [ rdf:type owl:Restriction ;
                                      owl:onProperty s4bldg:liftElevationDifference ;
                                      owl:allValuesFrom saref:Measurement
                                    ] ,
                                    [ rdf:type owl:Restriction ;
                                      owl:onProperty s4bldg:nominalCapacity ;
                                      owl:allValuesFrom saref:Measurement
                                    ] ,
                                    [ rdf:type owl:Restriction ;
                                      owl:onProperty s4bldg:operationTemperatureMax ;
                                      owl:allValuesFrom saref:Measurement
                                    ] ,
                                    [ rdf:type owl:Restriction ;
                                      owl:onProperty s4bldg:operationTemperatureMin ;
                                      owl:allValuesFrom saref:Measurement
                                    ] ,
                                    [ rdf:type owl:Restriction ;
                                      owl:onProperty s4bldg:waterRequirement ;
                                      owl:allValuesFrom saref:Measurement
                                    ] ,
                                    [ rdf:type owl:Restriction ;
                                      owl:onProperty s4bldg:capacityControl ;
                                      owl:allValuesFrom xsd:string
                                    ] ,
                                    [ rdf:type owl:Restriction ;
                                      owl:onProperty s4bldg:circuitType ;
                                      owl:allValuesFrom xsd:string
                                    ] ,
                                    [ rdf:type owl:Restriction ;
                                      owl:onProperty s4bldg:controlStrategy ;
                                      owl:allValuesFrom xsd:string
                                    ] ,
                                    [ rdf:type owl:Restriction ;
                                      owl:onProperty s4bldg:flowArrangement ;
                                      owl:allValuesFrom xsd:string
                                    ] ,
                                    [ rdf:type owl:Restriction ;
                                      owl:onProperty s4bldg:numberOfCells ;
                                      owl:allValuesFrom xsd:integer
                                    ] ,
                                    [ rdf:type owl:Restriction ;
                                      owl:onProperty s4bldg:sprayType ;
                                      owl:allValuesFrom xsd:string
                                    ] ;
                    rdfs:comment "A cooling tower is a device which rejects heat to ambient air by circulating a fluid such as water through it to reduce its temperature by partial evaporation."@en ;
                    rdfs:label "Cooling tower"@en ;
                    rdfs:seeAlso "https://w3id.org/ifc/IFC4_ADD1#IfcCoolingTower" ;
                    prov:hadPrimarySource <http://www.buildingsmart-tech.org/ifc/IFC4/Add1/html/schema/ifchvacdomain/lexical/ifccoolingtower.htm> ,
                                          <http://www.buildingsmart-tech.org/ifc/IFC4/Add1/html/schema/ifchvacdomain/pset/pset_coolingtowertypecommon.htm> .


###  https://saref.etsi.org/saref4bldg/Damper
s4bldg:Damper rdf:type owl:Class ;
              rdfs:subClassOf s4bldg:FlowController ,
                              [ rdf:type owl:Restriction ;
                                owl:onProperty s4bldg:airFlowRateMax ;
                                owl:allValuesFrom saref:Measurement
                              ] ,
                              [ rdf:type owl:Restriction ;
                                owl:onProperty s4bldg:bladeThickness ;
                                owl:allValuesFrom saref:Measurement
                              ] ,
                              [ rdf:type owl:Restriction ;
                                owl:onProperty s4bldg:closeOffRating ;
                                owl:allValuesFrom saref:Measurement
                              ] ,
                              [ rdf:type owl:Restriction ;
                                owl:onProperty s4bldg:faceArea ;
                                owl:allValuesFrom saref:Measurement
                              ] ,
                              [ rdf:type owl:Restriction ;
                                owl:onProperty s4bldg:frameDepth ;
                                owl:allValuesFrom saref:Measurement
                              ] ,
                              [ rdf:type owl:Restriction ;
                                owl:onProperty s4bldg:frameThickness ;
                                owl:allValuesFrom saref:Measurement
                              ] ,
                              [ rdf:type owl:Restriction ;
                                owl:onProperty s4bldg:leakageFullyClosed ;
                                owl:allValuesFrom saref:Measurement
                              ] ,
                              [ rdf:type owl:Restriction ;
                                owl:onProperty s4bldg:nominalAirFlowRate ;
                                owl:allValuesFrom saref:Measurement
                              ] ,
                              [ rdf:type owl:Restriction ;
                                owl:onProperty s4bldg:openPressureDrop ;
                                owl:allValuesFrom saref:Measurement
                              ] ,
                              [ rdf:type owl:Restriction ;
                                owl:onProperty s4bldg:operationTemperatureMax ;
                                owl:allValuesFrom saref:Measurement
                              ] ,
                              [ rdf:type owl:Restriction ;
                                owl:onProperty s4bldg:operationTemperatureMin ;
                                owl:allValuesFrom saref:Measurement
                              ] ,
                              [ rdf:type owl:Restriction ;
                                owl:onProperty s4bldg:temperatureRating ;
                                owl:allValuesFrom saref:Measurement
                              ] ,
                              [ rdf:type owl:Restriction ;
                                owl:onProperty s4bldg:workingPressureMax ;
                                owl:allValuesFrom saref:Measurement
                              ] ,
                              [ rdf:type owl:Restriction ;
                                owl:onProperty s4bldg:bladeAction ;
                                owl:allValuesFrom xsd:string
                              ] ,
                              [ rdf:type owl:Restriction ;
                                owl:onProperty s4bldg:bladeEdge ;
                                owl:allValuesFrom xsd:string
                              ] ,
                              [ rdf:type owl:Restriction ;
                                owl:onProperty s4bldg:bladeShape ;
                                owl:allValuesFrom xsd:string
                              ] ,
                              [ rdf:type owl:Restriction ;
                                owl:onProperty s4bldg:frameType ;
                                owl:allValuesFrom xsd:string
                              ] ,
                              [ rdf:type owl:Restriction ;
                                owl:onProperty s4bldg:numberOfBlades ;
                                owl:allValuesFrom xsd:integer
                              ] ,
                              [ rdf:type owl:Restriction ;
                                owl:onProperty s4bldg:operation ;
                                owl:allValuesFrom xsd:string
                              ] ,
                              [ rdf:type owl:Restriction ;
                                owl:onProperty s4bldg:orientation ;
                                owl:allValuesFrom xsd:string
                              ] ;
              rdfs:comment "A damper typically participates in an HVAC duct distribution system and is used to control or modulate the flow of air."@en ;
              rdfs:label "Damper"@en ;
              rdfs:seeAlso "https://w3id.org/ifc/IFC4_ADD1#IfcDamper" ;
              prov:hadPrimarySource <http://www.buildingsmart-tech.org/ifc/IFC4/Add1/html/schema/ifchvacdomain/lexical/ifcdamper.htm> ,
                                    <http://www.buildingsmart-tech.org/ifc/IFC4/Add1/html/schema/ifchvacdomain/pset/pset_dampertypecommon.htm> .


###  https://saref.etsi.org/saref4bldg/DistributionControlDevice
s4bldg:DistributionControlDevice rdf:type owl:Class ;
                                 rdfs:subClassOf s4bldg:DistributionDevice ;
                                 rdfs:comment "Represents devices of a building automation control system that are used to impart control over elements of a distribution system. (Definition adapated from http://www.buildingsmart-tech.org/ifc/IFC4/Add1/html/schema/ifcsharedbldgserviceelements/lexical/ifcdistributioncontrolelement.htm)"@en ;
                                 rdfs:label "Distribution control device"@en .


###  https://saref.etsi.org/saref4bldg/DistributionDevice
s4bldg:DistributionDevice rdf:type owl:Class ;
                          rdfs:subClassOf s4bldg:BuildingDevice ;
                          rdfs:comment "Generalization of all devices that participate in a distribution system. (Definition adapated from http://www.buildingsmart-tech.org/ifc/IFC4/Add1/html/schema/ifcproductextension/lexical/ifcdistributionelement.htm)"@en ;
                          rdfs:label "Distribution device"@en .


###  https://saref.etsi.org/saref4bldg/DistributionFlowDevice
s4bldg:DistributionFlowDevice rdf:type owl:Class ;
                              rdfs:subClassOf s4bldg:DistributionDevice ;
                              rdfs:comment "Represents devices of a distribution system that facilitate the distribution of energy or matter, such as air, water or power. (Definition adapated from http://www.buildingsmart-tech.org/ifc/IFC4/Add1/html/schema/ifcsharedbldgserviceelements/lexical/ifcdistributionflowelement.htm)"@en ;
                              rdfs:label "DistributionFlowDevice"@en .


###  https://saref.etsi.org/saref4bldg/DuctSilencer
s4bldg:DuctSilencer rdf:type owl:Class ;
                    rdfs:subClassOf s4bldg:FlowTreatmentDevice ,
                                    [ rdf:type owl:Restriction ;
                                      owl:onProperty s4bldg:airFlowRateMax ;
                                      owl:allValuesFrom saref:Measurement
                                    ] ,
                                    [ rdf:type owl:Restriction ;
                                      owl:onProperty s4bldg:airFlowRateMin ;
                                      owl:allValuesFrom saref:Measurement
                                    ] ,
                                    [ rdf:type owl:Restriction ;
                                      owl:onProperty s4bldg:hydraulicDiameter ;
                                      owl:allValuesFrom saref:Measurement
                                    ] ,
                                    [ rdf:type owl:Restriction ;
                                      owl:onProperty s4bldg:length ;
                                      owl:allValuesFrom saref:Measurement
                                    ] ,
                                    [ rdf:type owl:Restriction ;
                                      owl:onProperty s4bldg:operationTemperatureMax ;
                                      owl:allValuesFrom saref:Measurement
                                    ] ,
                                    [ rdf:type owl:Restriction ;
                                      owl:onProperty s4bldg:operationTemperatureMin ;
                                      owl:allValuesFrom saref:Measurement
                                    ] ,
                                    [ rdf:type owl:Restriction ;
                                      owl:onProperty s4bldg:weight ;
                                      owl:allValuesFrom saref:Measurement
                                    ] ,
                                    [ rdf:type owl:Restriction ;
                                      owl:onProperty s4bldg:workingPressureMax ;
                                      owl:allValuesFrom saref:Measurement
                                    ] ,
                                    [ rdf:type owl:Restriction ;
                                      owl:onProperty s4bldg:workingPressureMin ;
                                      owl:allValuesFrom saref:Measurement
                                    ] ,
                                    [ rdf:type owl:Restriction ;
                                      owl:onProperty s4bldg:hasExteriorInsulation ;
                                      owl:allValuesFrom xsd:boolean
                                    ] ;
                    rdfs:comment "A duct silencer is a device that is typically installed inside a duct distribution system for the purpose of reducing the noise levels from air movement, fan noise, etc. in the adjacent space or downstream of the duct silencer device."@en ;
                    rdfs:label "Duct silencer"@en ;
                    rdfs:seeAlso "https://w3id.org/ifc/IFC4_ADD1#IfcDuctSilencer" ;
                    prov:hadPrimarySource <http://www.buildingsmart-tech.org/ifc/IFC4/Add1/html/schema/ifchvacdomain/lexical/ifcductsilencer.htm> ,
                                          <http://www.buildingsmart-tech.org/ifc/IFC4/Add1/html/schema/ifchvacdomain/pset/pset_ductsilencertypecommon.htm> .


###  https://saref.etsi.org/saref4bldg/ElectricAppliance
s4bldg:ElectricAppliance rdf:type owl:Class ;
                         rdfs:subClassOf s4bldg:FlowTerminal ;
                         rdfs:comment """An electric appliance is a device intended for consumer usage that is powered by electricity.

Electric appliances may be fixed in place or may be able to be moved from one space to another. Electric appliances require an electrical supply that may be supplied either by an electrical circuit or provided from a local battery source."""@en ;
                         rdfs:label "Electric appliance"@en ;
                         rdfs:seeAlso "https://w3id.org/ifc/IFC4_ADD1#IfcElectricAppliance" ;
                         prov:hadPrimarySource <http://www.buildingsmart-tech.org/ifc/IFC4/Add1/html/schema/ifcelectricaldomain/lexical/ifcelectricappliance.htm> ,
                                               <http://www.buildingsmart-tech.org/ifc/IFC4/Add1/html/schema/ifcelectricaldomain/pset/pset_electricappliancetypecommon.htm> .


###  https://saref.etsi.org/saref4bldg/ElectricFlowStorageDevice
s4bldg:ElectricFlowStorageDevice rdf:type owl:Class ;
                                 rdfs:subClassOf s4bldg:FlowStorageDevice ,
                                                 [ rdf:type owl:Restriction ;
                                                   owl:onProperty s4bldg:nominalFrequency ;
                                                   owl:allValuesFrom saref:Measurement
                                                 ] ,
                                                 [ rdf:type owl:Restriction ;
                                                   owl:onProperty s4bldg:nominalSupplyVoltage ;
                                                   owl:allValuesFrom saref:Measurement
                                                 ] ,
                                                 [ rdf:type owl:Restriction ;
                                                   owl:onProperty s4bldg:nominalSupplyVoltageMin ;
                                                   owl:allValuesFrom saref:Measurement
                                                 ] ;
                                 rdfs:comment "An electric flow storage device is a device in which electrical energy is stored and from which energy may be progressively released."@en ;
                                 rdfs:label "Electric flow storage device"@en ;
                                 rdfs:seeAlso "https://w3id.org/ifc/IFC4_ADD1#IfcElectricFlowStorageDevice" ;
                                 prov:hadPrimarySource <http://www.buildingsmart-tech.org/ifc/IFC4/Add1/html/schema/ifcelectricaldomain/lexical/ifcelectricflowstoragedevice.htm> ,
                                                       <http://www.buildingsmart-tech.org/ifc/IFC4/Add1/html/schema/ifcelectricaldomain/pset/pset_electricflowstoragedevicetypecommon.htm> .


###  https://saref.etsi.org/saref4bldg/ElectricGenerator
s4bldg:ElectricGenerator rdf:type owl:Class ;
                         rdfs:subClassOf s4bldg:EnergyConversionDevice ,
                                         [ rdf:type owl:Restriction ;
                                           owl:onProperty s4bldg:electricGeneratorEfficiency ;
                                           owl:allValuesFrom saref:Measurement
                                         ] ,
                                         [ rdf:type owl:Restriction ;
                                           owl:onProperty s4bldg:powerOutputMax ;
                                           owl:allValuesFrom saref:Measurement
                                         ] ,
                                         [ rdf:type owl:Restriction ;
                                           owl:onProperty s4bldg:startCurrentFactor ;
                                           owl:allValuesFrom saref:Measurement
                                         ] ;
                         rdfs:comment "An electric generator is an engine that is a machine for converting mechanical energy into electrical energy."@en ;
                         rdfs:label "Electric generator"@en ;
                         rdfs:seeAlso "https://w3id.org/ifc/IFC4_ADD1#IfcElectricGenerator" ;
                         prov:hadPrimarySource <http://www.buildingsmart-tech.org/ifc/IFC4/Add1/html/schema/ifcelectricaldomain/lexical/ifcelectricgenerator.htm> ,
                                               <http://www.buildingsmart-tech.org/ifc/IFC4/Add1/html/schema/ifcelectricaldomain/pset/pset_electricgeneratortypecommon.htm> .


###  https://saref.etsi.org/saref4bldg/ElectricMotor
s4bldg:ElectricMotor rdf:type owl:Class ;
                     rdfs:subClassOf s4bldg:EnergyConversionDevice ,
                                     [ rdf:type owl:Restriction ;
                                       owl:onProperty s4bldg:electricMotorEfficiency ;
                                       owl:allValuesFrom saref:Measurement
                                     ] ,
                                     [ rdf:type owl:Restriction ;
                                       owl:onProperty s4bldg:lockedRotorCurrent ;
                                       owl:allValuesFrom saref:Measurement
                                     ] ,
                                     [ rdf:type owl:Restriction ;
                                       owl:onProperty s4bldg:powerOutputMax ;
                                       owl:allValuesFrom saref:Measurement
                                     ] ,
                                     [ rdf:type owl:Restriction ;
                                       owl:onProperty s4bldg:startCurrentFactor ;
                                       owl:allValuesFrom saref:Measurement
                                     ] ,
                                     [ rdf:type owl:Restriction ;
                                       owl:onProperty s4bldg:startingTime ;
                                       owl:allValuesFrom saref:Measurement
                                     ] ,
                                     [ rdf:type owl:Restriction ;
                                       owl:onProperty s4bldg:teTime ;
                                       owl:allValuesFrom saref:Measurement
                                     ] ,
                                     [ rdf:type owl:Restriction ;
                                       owl:onProperty s4bldg:frameSize ;
                                       owl:allValuesFrom xsd:string
                                     ] ,
                                     [ rdf:type owl:Restriction ;
                                       owl:onProperty s4bldg:hasPartWinding ;
                                       owl:allValuesFrom xsd:boolean
                                     ] ,
                                     [ rdf:type owl:Restriction ;
                                       owl:onProperty s4bldg:isGuarded ;
                                       owl:allValuesFrom xsd:boolean
                                     ] ,
                                     [ rdf:type owl:Restriction ;
                                       owl:onProperty s4bldg:motorEnclosureType ;
                                       owl:allValuesFrom xsd:string
                                     ] ;
                     rdfs:comment "An electric motor is an engine that is a machine for converting electrical energy into mechanical energy."@en ;
                     rdfs:label "Electric motor"@en ;
                     rdfs:seeAlso "https://w3id.org/ifc/IFC4_ADD1#IfcElectricMotor" ;
                     prov:hadPrimarySource <http://www.buildingsmart-tech.org/ifc/IFC4/Add1/html/schema/ifcelectricaldomain/lexical/ifcelectricmotor.htm> ,
                                           <http://www.buildingsmart-tech.org/ifc/IFC4/Add1/html/schema/ifcelectricaldomain/pset/pset_electricmotortypecommon.htm> .


###  https://saref.etsi.org/saref4bldg/ElectricTimeControl
s4bldg:ElectricTimeControl rdf:type owl:Class ;
                           rdfs:subClassOf s4bldg:FlowController ;
                           rdfs:comment "An electric time control is a device that applies control to the provision or flow of electrical energy over time."@en ;
                           rdfs:label "Electric time control"@en ;
                           rdfs:seeAlso "https://w3id.org/ifc/IFC4_ADD1#IfcElectricTimeControl" ;
                           prov:hadPrimarySource <http://www.buildingsmart-tech.org/ifc/IFC4/Add1/html/schema/ifcelectricaldomain/lexical/ifcelectrictimecontrol.htm> ,
                                                 <http://www.buildingsmart-tech.org/ifc/IFC4/Add1/html/schema/ifcelectricaldomain/pset/pset_electrictimecontroltypecommon.htm> .


###  https://saref.etsi.org/saref4bldg/EnergyConversionDevice
s4bldg:EnergyConversionDevice rdf:type owl:Class ;
                              rdfs:subClassOf s4bldg:DistributionFlowDevice ;
                              rdfs:comment "The distribution flow element EnergyConversionDevice defines the occurrence of a device used to perform energy conversion or heat transfer and typically participates in a flow distribution system."@en ;
                              rdfs:label "Energy conversion device"@en ;
                              rdfs:seeAlso "https://w3id.org/ifc/IFC4_ADD1#IfcEnergyConversionDevice" ;
                              prov:hadPrimarySource <http://www.buildingsmart-tech.org/ifc/IFC4/Add1/html/schema/ifcsharedbldgserviceelements/lexical/ifcenergyconversiondevice.htm> .


###  https://saref.etsi.org/saref4bldg/Engine
s4bldg:Engine rdf:type owl:Class ;
              rdfs:subClassOf s4bldg:EnergyConversionDevice ,
                              [ rdf:type owl:Restriction ;
                                owl:onProperty s4bldg:energySource ;
                                owl:allValuesFrom xsd:string
                              ] ;
              rdfs:comment "An engine is a device that converts fuel into mechanical energy through combustion."@en ;
              rdfs:label "Engine"@en ;
              rdfs:seeAlso "https://w3id.org/ifc/IFC4_ADD1#IfcEngine" ;
              prov:hadPrimarySource <http://www.buildingsmart-tech.org/ifc/IFC4/Add1/html/schema/ifchvacdomain/lexical/ifcengine.htm> ,
                                    <http://www.buildingsmart-tech.org/ifc/IFC4/Add1/html/schema/ifchvacdomain/pset/pset_enginetypecommon.htm> .


###  https://saref.etsi.org/saref4bldg/EvaporativeCooler
s4bldg:EvaporativeCooler rdf:type owl:Class ;
                         rdfs:subClassOf s4bldg:EnergyConversionDevice ,
                                         [ rdf:type owl:Restriction ;
                                           owl:onProperty s4bldg:heatExchangeArea ;
                                           owl:allValuesFrom saref:Measurement
                                         ] ,
                                         [ rdf:type owl:Restriction ;
                                           owl:onProperty s4bldg:operationTemperatureMax ;
                                           owl:allValuesFrom saref:Measurement
                                         ] ,
                                         [ rdf:type owl:Restriction ;
                                           owl:onProperty s4bldg:operationTemperatureMin ;
                                           owl:allValuesFrom saref:Measurement
                                         ] ,
                                         [ rdf:type owl:Restriction ;
                                           owl:onProperty s4bldg:waterRequirement ;
                                           owl:allValuesFrom saref:Measurement
                                         ] ,
                                         [ rdf:type owl:Restriction ;
                                           owl:onProperty s4bldg:flowArrangement ;
                                           owl:allValuesFrom xsd:string
                                         ] ;
                         rdfs:comment "An evaporative cooler is a device that cools air by saturating it with water vapor."@en ;
                         rdfs:label "Evaporative cooler"@en ;
                         rdfs:seeAlso "https://w3id.org/ifc/IFC4_ADD1#IfcEvaporativeCooler" ;
                         prov:hadPrimarySource <http://www.buildingsmart-tech.org/ifc/IFC4/Add1/html/schema/ifchvacdomain/lexical/ifcevaporativecooler.htm> ,
                                               <http://www.buildingsmart-tech.org/ifc/IFC4/Add1/html/schema/ifchvacdomain/pset/pset_evaporativecoolertypecommon.htm> .


###  https://saref.etsi.org/saref4bldg/Evaporator
s4bldg:Evaporator rdf:type owl:Class ;
                  rdfs:subClassOf s4bldg:EnergyConversionDevice ,
                                  [ rdf:type owl:Restriction ;
                                    owl:onProperty s4bldg:externalSurfaceArea ;
                                    owl:allValuesFrom saref:Measurement
                                  ] ,
                                  [ rdf:type owl:Restriction ;
                                    owl:onProperty s4bldg:internalRefrigerantVolume ;
                                    owl:allValuesFrom saref:Measurement
                                  ] ,
                                  [ rdf:type owl:Restriction ;
                                    owl:onProperty s4bldg:internalSurfaceArea ;
                                    owl:allValuesFrom saref:Measurement
                                  ] ,
                                  [ rdf:type owl:Restriction ;
                                    owl:onProperty s4bldg:internalWaterVolume ;
                                    owl:allValuesFrom saref:Measurement
                                  ] ,
                                  [ rdf:type owl:Restriction ;
                                    owl:onProperty s4bldg:nominalHeatTransferArea ;
                                    owl:allValuesFrom saref:Measurement
                                  ] ,
                                  [ rdf:type owl:Restriction ;
                                    owl:onProperty s4bldg:nominalHeatTransferCoefficient ;
                                    owl:allValuesFrom saref:Measurement
                                  ] ,
                                  [ rdf:type owl:Restriction ;
                                    owl:onProperty s4bldg:evaporationCoolant ;
                                    owl:allValuesFrom xsd:string
                                  ] ,
                                  [ rdf:type owl:Restriction ;
                                    owl:onProperty s4bldg:evaporationMediumType ;
                                    owl:allValuesFrom xsd:string
                                  ] ,
                                  [ rdf:type owl:Restriction ;
                                    owl:onProperty s4bldg:refrigerantClass ;
                                    owl:allValuesFrom xsd:string
                                  ] ;
                  rdfs:comment "An evaporator is a device in which a liquid refrigerent is vaporized and absorbs heat from the surrounding fluid."@en ;
                  rdfs:label "Evaporator"@en ;
                  rdfs:seeAlso "https://w3id.org/ifc/IFC4_ADD1#IfcEvaporator" ;
                  prov:hadPrimarySource <http://www.buildingsmart-tech.org/ifc/IFC4/Add1/html/schema/ifchvacdomain/lexical/ifcevaporator.htm> ,
                                        <http://www.buildingsmart-tech.org/ifc/IFC4/Add1/html/schema/ifchvacdomain/pset/pset_evaporatortypecommon.htm> .


###  https://saref.etsi.org/saref4bldg/Fan
s4bldg:Fan rdf:type owl:Class ;
           rdfs:subClassOf s4bldg:FlowMovingDevice ,
                           [ rdf:type owl:Restriction ;
                             owl:onProperty s4bldg:nominalAirFlowRate ;
                             owl:allValuesFrom saref:Measurement
                           ] ,
                           [ rdf:type owl:Restriction ;
                             owl:onProperty s4bldg:nominalPowerRate ;
                             owl:allValuesFrom saref:Measurement
                           ] ,
                           [ rdf:type owl:Restriction ;
                             owl:onProperty s4bldg:nominalRotationSpeed ;
                             owl:allValuesFrom saref:Measurement
                           ] ,
                           [ rdf:type owl:Restriction ;
                             owl:onProperty s4bldg:nominalStaticPressure ;
                             owl:allValuesFrom saref:Measurement
                           ] ,
                           [ rdf:type owl:Restriction ;
                             owl:onProperty s4bldg:nominalTotalPressure ;
                             owl:allValuesFrom saref:Measurement
                           ] ,
                           [ rdf:type owl:Restriction ;
                             owl:onProperty s4bldg:operationTemperatureMax ;
                             owl:allValuesFrom saref:Measurement
                           ] ,
                           [ rdf:type owl:Restriction ;
                             owl:onProperty s4bldg:operationTemperatureMin ;
                             owl:allValuesFrom saref:Measurement
                           ] ,
                           [ rdf:type owl:Restriction ;
                             owl:onProperty s4bldg:operationalRiterial ;
                             owl:allValuesFrom saref:Measurement
                           ] ,
                           [ rdf:type owl:Restriction ;
                             owl:onProperty s4bldg:capacityControlType ;
                             owl:allValuesFrom xsd:string
                           ] ,
                           [ rdf:type owl:Restriction ;
                             owl:onProperty s4bldg:motorDriveType ;
                             owl:allValuesFrom xsd:string
                           ] ;
           rdfs:comment "A fan is a device which imparts mechanical work on a gas. A typical usage of a fan is to induce airflow in a building services air distribution system."@en ;
           rdfs:label "Fan"@en ;
           rdfs:seeAlso "https://w3id.org/ifc/IFC4_ADD1#IfcFan" ;
           prov:hadPrimarySource <http://www.buildingsmart-tech.org/ifc/IFC4/Add1/html/schema/ifchvacdomain/lexical/ifcfan.htm> ,
                                 <http://www.buildingsmart-tech.org/ifc/IFC4/Add1/html/schema/ifchvacdomain/pset/pset_fantypecommon.htm> .


###  https://saref.etsi.org/saref4bldg/Filter
s4bldg:Filter rdf:type owl:Class ;
              rdfs:subClassOf s4bldg:FlowTreatmentDevice ,
                              [ rdf:type owl:Restriction ;
                                owl:onProperty s4bldg:finalResistance ;
                                owl:allValuesFrom saref:Measurement
                              ] ,
                              [ rdf:type owl:Restriction ;
                                owl:onProperty s4bldg:fluidFlowRateMax ;
                                owl:allValuesFrom saref:Measurement
                              ] ,
                              [ rdf:type owl:Restriction ;
                                owl:onProperty s4bldg:fluidFlowRateMin ;
                                owl:allValuesFrom saref:Measurement
                              ] ,
                              [ rdf:type owl:Restriction ;
                                owl:onProperty s4bldg:initialResistance ;
                                owl:allValuesFrom saref:Measurement
                              ] ,
                              [ rdf:type owl:Restriction ;
                                owl:onProperty s4bldg:nominalFilterFaceVelocity ;
                                owl:allValuesFrom saref:Measurement
                              ] ,
                              [ rdf:type owl:Restriction ;
                                owl:onProperty s4bldg:nominalFlowRate ;
                                owl:allValuesFrom saref:Measurement
                              ] ,
                              [ rdf:type owl:Restriction ;
                                owl:onProperty s4bldg:nominalMediaSurfaceVelocity ;
                                owl:allValuesFrom saref:Measurement
                              ] ,
                              [ rdf:type owl:Restriction ;
                                owl:onProperty s4bldg:nominalParticleGeometricMeanDiameter ;
                                owl:allValuesFrom saref:Measurement
                              ] ,
                              [ rdf:type owl:Restriction ;
                                owl:onProperty s4bldg:nominalParticleGeometricStandardDeviation ;
                                owl:allValuesFrom saref:Measurement
                              ] ,
                              [ rdf:type owl:Restriction ;
                                owl:onProperty s4bldg:nominalPressureDrop ;
                                owl:allValuesFrom saref:Measurement
                              ] ,
                              [ rdf:type owl:Restriction ;
                                owl:onProperty s4bldg:operationTemperatureMax ;
                                owl:allValuesFrom saref:Measurement
                              ] ,
                              [ rdf:type owl:Restriction ;
                                owl:onProperty s4bldg:operationTemperatureMin ;
                                owl:allValuesFrom saref:Measurement
                              ] ,
                              [ rdf:type owl:Restriction ;
                                owl:onProperty s4bldg:weight ;
                                owl:allValuesFrom saref:Measurement
                              ] ;
              rdfs:comment "A filter is an apparatus used to remove particulate or gaseous matter from fluids and gases."@en ;
              rdfs:label "Filter"@en ;
              rdfs:seeAlso "https://w3id.org/ifc/IFC4_ADD1#IfcFilter" ;
              prov:hadPrimarySource <http://www.buildingsmart-tech.org/ifc/IFC4/Add1/html/schema/ifchvacdomain/lexical/ifcfilter.htm> ,
                                    <http://www.buildingsmart-tech.org/ifc/IFC4/Add1/html/schema/ifchvacdomain/pset/pset_filtertypecommon.htm> .


###  https://saref.etsi.org/saref4bldg/FireSuppressionTerminal
s4bldg:FireSuppressionTerminal rdf:type owl:Class ;
                               rdfs:subClassOf s4bldg:FlowTerminal ;
                               rdfs:comment """A fire suppression terminal has the purpose of delivering a fluid (gas or liquid) that will suppress a fire.

A fire suppression terminal provides for all forms of sprinkler, spreader and other form of terminal that is connected to a pipework system and intended to act in the role of suppressing a fire."""@en ;
                               rdfs:label "Fire suppression terminal"@en ;
                               rdfs:seeAlso "https://w3id.org/ifc/IFC4_ADD1#IfcFireSuppressionTerminal" ;
                               prov:hadPrimarySource <http://www.buildingsmart-tech.org/ifc/IFC4/Add1/html/schema/ifcplumbingfireprotectiondomain/lexical/ifcfiresuppressionterminal.htm> ,
                                                     <http://www.buildingsmart-tech.org/ifc/IFC4/Add1/html/schema/ifcplumbingfireprotectiondomain/pset/pset_firesuppressionterminaltypecommon.htm> .


###  https://saref.etsi.org/saref4bldg/FlowController
s4bldg:FlowController rdf:type owl:Class ;
                      rdfs:subClassOf s4bldg:DistributionFlowDevice ;
                      rdfs:comment "The distribution flow element FlowController defines the occurrence of elements of a distribution system that are used to regulate flow through a distribution system. Examples include dampers, valves, switches, and relays."@en ;
                      rdfs:label "Flow controller"@en ;
                      rdfs:seeAlso "https://w3id.org/ifc/IFC4_ADD1#IfcFlowController" ;
                      prov:hadPrimarySource <http://www.buildingsmart-tech.org/ifc/IFC4/Add1/html/schema/ifcsharedbldgserviceelements/lexical/ifcflowcontroller.htm> .


###  https://saref.etsi.org/saref4bldg/FlowInstrument
s4bldg:FlowInstrument rdf:type owl:Class ;
                      rdfs:subClassOf s4bldg:DistributionControlDevice ;
                      rdfs:comment """A flow instrument reads and displays the value of a particular property of a system at a point, or displays the difference in the value of a property between two points.

Instrumentation is typically for the purpose of determining the value of the property at a point in time. It is not the purpose of an instrument to record or integrate the values over time (although they may be connected to recording devices that do perform such a function). This entity provides for all forms of mechanical flow instrument (thermometers, pressure gauges etc.) and electrical flow instruments (ammeters, voltmeters etc.)"""@en ;
                      rdfs:label "Flow instrument"@en ;
                      rdfs:seeAlso "https://w3id.org/ifc/IFC4_ADD1#IfcFlowInstrument" ;
                      prov:hadPrimarySource <http://www.buildingsmart-tech.org/ifc/IFC4/Add1/html/schema/ifcbuildingcontrolsdomain/lexical/ifcflowinstrument.htm> ,
                                            <http://www.buildingsmart-tech.org/ifc/IFC4/Add1/html/schema/ifcbuildingcontrolsdomain/pset/pset_flowinstrumenttypecommon.htm> .


###  https://saref.etsi.org/saref4bldg/FlowMeter
s4bldg:FlowMeter rdf:type owl:Class ;
                 rdfs:subClassOf s4bldg:FlowController ,
                                 [ rdf:type owl:Restriction ;
                                   owl:onProperty s4bldg:readOutType ;
                                   owl:allValuesFrom xsd:string
                                 ] ,
                                 [ rdf:type owl:Restriction ;
                                   owl:onProperty s4bldg:remoteReading ;
                                   owl:allValuesFrom xsd:boolean
                                 ] ;
                 rdfs:comment "A flow meter is a device that is used to measure the flow rate in a system."@en ;
                 rdfs:label "Flow meter"@en ;
                 rdfs:seeAlso "https://w3id.org/ifc/IFC4_ADD1#IfcFlowMeter" ;
                 prov:hadPrimarySource <http://www.buildingsmart-tech.org/ifc/IFC4/Add1/html/schema/ifchvacdomain/lexical/ifcflowmeter.htm> ,
                                       <http://www.buildingsmart-tech.org/ifc/IFC4/Add1/html/schema/ifchvacdomain/pset/pset_flowmetertypecommon.htm> .


###  https://saref.etsi.org/saref4bldg/FlowMovingDevice
s4bldg:FlowMovingDevice rdf:type owl:Class ;
                        rdfs:subClassOf s4bldg:DistributionFlowDevice ;
                        rdfs:comment "The distribution flow element FlowMovingDevice defines the occurrence of an apparatus used to distribute, circulate or perform conveyance of fluids, including liquids and gases (such as a pump or fan), and typically participates in a flow distribution system."@en ;
                        rdfs:label "Flow moving device"@en ;
                        rdfs:seeAlso "https://w3id.org/ifc/IFC4_ADD1#IfcFlowMovingDevice" ;
                        prov:hadPrimarySource <http://www.buildingsmart-tech.org/ifc/IFC4/Add1/html/schema/ifcsharedbldgserviceelements/lexical/ifcflowmovingdevice.htm> .


###  https://saref.etsi.org/saref4bldg/FlowStorageDevice
s4bldg:FlowStorageDevice rdf:type owl:Class ;
                         rdfs:subClassOf s4bldg:DistributionFlowDevice ;
                         rdfs:comment "The distribution flow element FlowStorageDevice defines the occurrence of a device that participates in a distribution system and is used for temporary storage (such as a tank)."@en ;
                         rdfs:label "Flow storage device"@en ;
                         rdfs:seeAlso "https://w3id.org/ifc/IFC4_ADD1#IfcFlowStorageDevice" ;
                         prov:hadPrimarySource <http://www.buildingsmart-tech.org/ifc/IFC4/Add1/html/schema/ifcsharedbldgserviceelements/lexical/ifcflowstoragedevice.htm> .


###  https://saref.etsi.org/saref4bldg/FlowTerminal
s4bldg:FlowTerminal rdf:type owl:Class ;
                    rdfs:subClassOf s4bldg:DistributionFlowDevice ;
                    rdfs:comment "The distribution flow element FlowTerminal defines the occurrence of a permanently attached element that acts as a terminus or beginning of a distribution system (such as an air outlet, drain, water closet, or sink). A terminal is typically a point at which a system interfaces with an external environment."@en ;
                    rdfs:label "Flow terminal"@en ;
                    rdfs:seeAlso "https://w3id.org/ifc/IFC4_ADD1#IfcFlowTerminal" ;
                    prov:hadPrimarySource <http://www.buildingsmart-tech.org/ifc/IFC4/Add1/html/schema/ifcsharedbldgserviceelements/lexical/ifcflowterminal.htm> .


###  https://saref.etsi.org/saref4bldg/FlowTreatmentDevice
s4bldg:FlowTreatmentDevice rdf:type owl:Class ;
                           rdfs:subClassOf s4bldg:DistributionFlowDevice ;
                           rdfs:comment "The distribution flow element FlowTreatmentDevice defines the occurrence of a device typically used to remove unwanted matter from a fluid, either liquid or gas, and typically participates in a flow distribution system."@en ;
                           rdfs:label "Flow treatment device"@en ;
                           rdfs:seeAlso "https://w3id.org/ifc/IFC4_ADD1#IfcFlowTreatmentDevice" ;
                           prov:hadPrimarySource <http://www.buildingsmart-tech.org/ifc/IFC4/Add1/html/schema/ifcsharedbldgserviceelements/lexical/ifcflowtreatmentdevice.htm> .


###  https://saref.etsi.org/saref4bldg/HeatExchanger
s4bldg:HeatExchanger rdf:type owl:Class ;
                     rdfs:subClassOf s4bldg:EnergyConversionDevice ,
                                     [ rdf:type owl:Restriction ;
                                       owl:onProperty s4bldg:arrangement ;
                                       owl:allValuesFrom xsd:string
                                     ] ;
                     rdfs:comment "A heat exchanger is a device used to provide heat transfer between non-mixing media such as plate and shell and tube heat exchangers. HeatExchanger is commonly used on water-side distribution systems to recover energy from a liquid to another liquid (typically water-based), whereas AirToAirHeatRecovery is commonly used on air-side distribution systems to recover energy from a gas to a gas (usually air)."@en ;
                     rdfs:label "Heat exchanger"@en ;
                     rdfs:seeAlso "https://w3id.org/ifc/IFC4_ADD1#IfcHeatExchanger" ;
                     prov:hadPrimarySource <http://www.buildingsmart-tech.org/ifc/IFC4/Add1/html/schema/ifchvacdomain/lexical/ifcheatexchanger.htm> ,
                                           <http://www.buildingsmart-tech.org/ifc/IFC4/Add1/html/schema/ifchvacdomain/pset/pset_heatexchangertypecommon.htm> .


###  https://saref.etsi.org/saref4bldg/Humidifier
s4bldg:Humidifier rdf:type owl:Class ;
                  rdfs:subClassOf s4bldg:EnergyConversionDevice ,
                                  [ rdf:type owl:Restriction ;
                                    owl:onProperty s4bldg:nominalAirFlowRate ;
                                    owl:allValuesFrom saref:Measurement
                                  ] ,
                                  [ rdf:type owl:Restriction ;
                                    owl:onProperty s4bldg:nominalMoistureGain ;
                                    owl:allValuesFrom saref:Measurement
                                  ] ,
                                  [ rdf:type owl:Restriction ;
                                    owl:onProperty s4bldg:waterRequirement ;
                                    owl:allValuesFrom saref:Measurement
                                  ] ,
                                  [ rdf:type owl:Restriction ;
                                    owl:onProperty s4bldg:weight ;
                                    owl:allValuesFrom saref:Measurement
                                  ] ,
                                  [ rdf:type owl:Restriction ;
                                    owl:onProperty s4bldg:application ;
                                    owl:allValuesFrom xsd:string
                                  ] ,
                                  [ rdf:type owl:Restriction ;
                                    owl:onProperty s4bldg:internalControl ;
                                    owl:allValuesFrom xsd:string
                                  ] ;
                  rdfs:comment "A humidifier is a device that adds moisture into the air."@en ;
                  rdfs:label "Humidifier"@en ;
                  rdfs:seeAlso "https://w3id.org/ifc/IFC4_ADD1#IfcHumidifier" ;
                  prov:hadPrimarySource <http://www.buildingsmart-tech.org/ifc/IFC4/Add1/html/schema/ifchvacdomain/lexical/ifchumidifier.htm> ,
                                        <http://www.buildingsmart-tech.org/ifc/IFC4/Add1/html/schema/ifchvacdomain/pset/pset_humidifiertypecommon.htm> .


###  https://saref.etsi.org/saref4bldg/Interceptor
s4bldg:Interceptor rdf:type owl:Class ;
                   rdfs:subClassOf s4bldg:FlowTreatmentDevice ,
                                   [ rdf:type owl:Restriction ;
                                     owl:onProperty s4bldg:coverLength ;
                                     owl:allValuesFrom saref:Measurement
                                   ] ,
                                   [ rdf:type owl:Restriction ;
                                     owl:onProperty s4bldg:coverWidth ;
                                     owl:allValuesFrom saref:Measurement
                                   ] ,
                                   [ rdf:type owl:Restriction ;
                                     owl:onProperty s4bldg:inletConnectionSize ;
                                     owl:allValuesFrom saref:Measurement
                                   ] ,
                                   [ rdf:type owl:Restriction ;
                                     owl:onProperty s4bldg:nominalBodyDepth ;
                                     owl:allValuesFrom saref:Measurement
                                   ] ,
                                   [ rdf:type owl:Restriction ;
                                     owl:onProperty s4bldg:nominalBodyLength ;
                                     owl:allValuesFrom saref:Measurement
                                   ] ,
                                   [ rdf:type owl:Restriction ;
                                     owl:onProperty s4bldg:nominalBodyWidth ;
                                     owl:allValuesFrom saref:Measurement
                                   ] ,
                                   [ rdf:type owl:Restriction ;
                                     owl:onProperty s4bldg:outletConnectionSize ;
                                     owl:allValuesFrom saref:Measurement
                                   ] ,
                                   [ rdf:type owl:Restriction ;
                                     owl:onProperty s4bldg:ventilatingPipeSize ;
                                     owl:allValuesFrom saref:Measurement
                                   ] ;
                   rdfs:comment "An interceptor is a device designed and installed in order to separate and retain deleterious, hazardous or undesirable matter while permitting normal sewage or liquids to discharge into a collection system by gravity."@en ;
                   rdfs:label "Interceptor"@en ;
                   rdfs:seeAlso "https://w3id.org/ifc/IFC4_ADD1#IfcInterceptor" ;
                   prov:hadPrimarySource <http://www.buildingsmart-tech.org/ifc/IFC4/Add1/html/schema/ifcplumbingfireprotectiondomain/lexical/ifcinterceptor.htm> ,
                                         <http://www.buildingsmart-tech.org/ifc/IFC4/Add1/html/schema/ifcplumbingfireprotectiondomain/pset/pset_interceptortypecommon.htm> .


###  https://saref.etsi.org/saref4bldg/Lamp
s4bldg:Lamp rdf:type owl:Class ;
            rdfs:subClassOf s4bldg:FlowTerminal ,
                            [ rdf:type owl:Restriction ;
                              owl:onProperty s4bldg:colorTemperature ;
                              owl:allValuesFrom saref:Measurement
                            ] ,
                            [ rdf:type owl:Restriction ;
                              owl:onProperty s4bldg:contributedLuminousFlux ;
                              owl:allValuesFrom saref:Measurement
                            ] ,
                            [ rdf:type owl:Restriction ;
                              owl:onProperty s4bldg:lampMaintenanceFactor ;
                              owl:allValuesFrom saref:Measurement
                            ] ,
                            [ rdf:type owl:Restriction ;
                              owl:onProperty s4bldg:lightEmitterNominalPower ;
                              owl:allValuesFrom saref:Measurement
                            ] ,
                            [ rdf:type owl:Restriction ;
                              owl:onProperty s4bldg:spectrumMax ;
                              owl:allValuesFrom saref:Measurement
                            ] ,
                            [ rdf:type owl:Restriction ;
                              owl:onProperty s4bldg:spectrumMin ;
                              owl:allValuesFrom saref:Measurement
                            ] ,
                            [ rdf:type owl:Restriction ;
                              owl:onProperty s4bldg:colorAppearance ;
                              owl:allValuesFrom xsd:string
                            ] ,
                            [ rdf:type owl:Restriction ;
                              owl:onProperty s4bldg:colorRenderingIndex ;
                              owl:allValuesFrom xsd:integer
                            ] ,
                            [ rdf:type owl:Restriction ;
                              owl:onProperty s4bldg:lampBallastType ;
                              owl:allValuesFrom xsd:string
                            ] ,
                            [ rdf:type owl:Restriction ;
                              owl:onProperty s4bldg:lampCompensationType ;
                              owl:allValuesFrom xsd:string
                            ] ;
            rdfs:comment "A lamp is an artificial light source such as a light bulb or tube."@en ;
            rdfs:label "Lamp"@en ;
            rdfs:seeAlso "https://w3id.org/ifc/IFC4_ADD1#IfcLamp" ;
            prov:hadPrimarySource <http://www.buildingsmart-tech.org/ifc/IFC4/Add1/html/schema/ifcelectricaldomain/lexical/ifclamp.htm> ,
                                  <http://www.buildingsmart-tech.org/ifc/IFC4/Add1/html/schema/ifcelectricaldomain/pset/pset_lamptypecommon.htm> .


###  https://saref.etsi.org/saref4bldg/MedicalDevice
s4bldg:MedicalDevice rdf:type owl:Class ;
                     rdfs:subClassOf s4bldg:FlowTerminal ;
                     rdfs:comment "A medical device is attached to a medical piping system and operates upon medical gases to perform a specific function. Medical gases include medical air, medical vacuum, oxygen, carbon dioxide, nitrogen, and nitrous oxide."@en ;
                     rdfs:label "Medical device"@en ;
                     rdfs:seeAlso "https://w3id.org/ifc/IFC4_ADD1#IfcMedicalDevice" ;
                     prov:hadPrimarySource <http://www.buildingsmart-tech.org/ifc/IFC4/Add1/html/schema/ifchvacdomain/lexical/ifcmedicaldevice.htm> ,
                                           <http://www.buildingsmart-tech.org/ifc/IFC4/Add1/html/schema/ifchvacdomain/pset/pset_medicaldevicetypecommon.htm> .


###  https://saref.etsi.org/saref4bldg/Outlet
s4bldg:Outlet rdf:type owl:Class ;
              rdfs:subClassOf s4bldg:FlowTerminal ,
                              [ rdf:type owl:Restriction ;
                                owl:onProperty s4bldg:isPluggableOutlet ;
                                owl:allValuesFrom xsd:boolean
                              ] ,
                              [ rdf:type owl:Restriction ;
                                owl:onProperty s4bldg:numberOsSockets ;
                                owl:allValuesFrom xsd:integer
                              ] ;
              rdfs:comment """An outlet is a device installed at a point to receive one or more inserted plugs for electrical power or communications.

Power outlets are commonly connected within a junction box; data outlets may be directly connected to a wall. For power outlets sharing the same circuit within a junction box, the ports should indicate the logical wiring relationship to the enclosing junction box, even though they may be physically connected to a cable going to another outlet, switch, or fixture."""@en ;
              rdfs:label "Outlet"@en ;
              rdfs:seeAlso "https://w3id.org/ifc/IFC4_ADD1#IfcOutlet" ;
              prov:hadPrimarySource <http://www.buildingsmart-tech.org/ifc/IFC4/Add1/html/schema/ifcelectricaldomain/lexical/ifcoutlet.htm> ,
                                    <http://www.buildingsmart-tech.org/ifc/IFC4/Add1/html/schema/ifcelectricaldomain/pset/pset_outlettypecommon.htm> .


###  https://saref.etsi.org/saref4bldg/PhysicalObject
s4bldg:PhysicalObject rdf:type owl:Class ;
                      rdfs:subClassOf [ rdf:type owl:Restriction ;
                                        owl:onProperty s4bldg:contains ;
                                        owl:allValuesFrom s4bldg:PhysicalObject
                                      ] ,
                                      [ rdf:type owl:Restriction ;
                                        owl:onProperty s4bldg:isContainedIn ;
                                        owl:allValuesFrom [ rdf:type owl:Class ;
                                                            owl:unionOf ( s4bldg:BuildingSpace
                                                                          s4bldg:PhysicalObject
                                                                        )
                                                          ]
                                      ] ;
                      rdfs:comment "Any Object that has a proper space region.  (Definition extracted from DUL ontology)"@en ;
                      rdfs:label "Physical object"@en .


###  https://saref.etsi.org/saref4bldg/ProtectiveDevice
s4bldg:ProtectiveDevice rdf:type owl:Class ;
                        rdfs:subClassOf s4bldg:FlowController ;
                        rdfs:comment """A protective device breaks an electrical circuit when a stated electric current that passes through it is exceeded.

A protective device provides protection against electrical current only (not as a general protective device). It may be used to represent the complete set of elements including both the tripping unit and the breaking unit that provide the protection. This may be particularly useful at earlier stages of design where the approach to breaking the electrical supply may be determined but the method of tripping may not. Alternatively, this entity may be used to specifically represent the breaking unit alone (in which case the tripping unit will also be specifically identified). This entity is specific to dedicated protective devices and excludes electrical outlets that may have circuit protection."""@en ;
                        rdfs:label "Protective device"@en ;
                        rdfs:seeAlso "https://w3id.org/ifc/IFC4_ADD1#IfcProtectiveDevice" ;
                        prov:hadPrimarySource <http://www.buildingsmart-tech.org/ifc/IFC4/Add1/html/schema/ifcelectricaldomain/lexical/ifcprotectivedevice.htm> ,
                                              <http://www.buildingsmart-tech.org/ifc/IFC4/Add1/html/schema/ifcelectricaldomain/pset/pset_protectivedevicetypecommon.htm> .


###  https://saref.etsi.org/saref4bldg/ProtectiveDeviceTrippingUnit
s4bldg:ProtectiveDeviceTrippingUnit rdf:type owl:Class ;
                                    rdfs:subClassOf s4bldg:DistributionControlDevice ,
                                                    [ rdf:type owl:Restriction ;
                                                      owl:onProperty s4bldg:limitingTerminalSize ;
                                                      owl:allValuesFrom saref:Measurement
                                                    ] ,
                                                    [ rdf:type owl:Restriction ;
                                                      owl:onProperty s4bldg:standard ;
                                                      owl:allValuesFrom xsd:string
                                                    ] ;
                                    rdfs:comment "A protective device tripping unit breaks an electrical circuit at a separate breaking unit when a stated electric current that passes through the unit is exceeded."@en ;
                                    rdfs:label "Protective device tripping unit"@en ;
                                    rdfs:seeAlso "https://w3id.org/ifc/IFC4_ADD1#IfcProtectiveDeviceTrippingUnit" ;
                                    prov:hadPrimarySource <http://www.buildingsmart-tech.org/ifc/IFC4/Add1/html/schema/ifcelectricaldomain/lexical/ifcprotectivedevicetrippingunit.htm> ,
                                                          <http://www.buildingsmart-tech.org/ifc/IFC4/Add1/html/schema/ifcelectricaldomain/pset/pset_protectivedevicetrippingunittypecommon.htm> .


###  https://saref.etsi.org/saref4bldg/Pump
s4bldg:Pump rdf:type owl:Class ;
            rdfs:subClassOf s4bldg:FlowMovingDevice ,
                            [ rdf:type owl:Restriction ;
                              owl:onProperty s4bldg:connectionSize ;
                              owl:allValuesFrom saref:Measurement
                            ] ,
                            [ rdf:type owl:Restriction ;
                              owl:onProperty s4bldg:flowResistanceMax ;
                              owl:allValuesFrom saref:Measurement
                            ] ,
                            [ rdf:type owl:Restriction ;
                              owl:onProperty s4bldg:flowResistanceMin ;
                              owl:allValuesFrom saref:Measurement
                            ] ,
                            [ rdf:type owl:Restriction ;
                              owl:onProperty s4bldg:netPositiveSuctionHead ;
                              owl:allValuesFrom saref:Measurement
                            ] ,
                            [ rdf:type owl:Restriction ;
                              owl:onProperty s4bldg:nomminalRotationSpeed ;
                              owl:allValuesFrom saref:Measurement
                            ] ,
                            [ rdf:type owl:Restriction ;
                              owl:onProperty s4bldg:operationTemperatureMax ;
                              owl:allValuesFrom saref:Measurement
                            ] ,
                            [ rdf:type owl:Restriction ;
                              owl:onProperty s4bldg:operationTemperatureMin ;
                              owl:allValuesFrom saref:Measurement
                            ] ,
                            [ rdf:type owl:Restriction ;
                              owl:onProperty s4bldg:pumpFlowRateMax ;
                              owl:allValuesFrom saref:Measurement
                            ] ,
                            [ rdf:type owl:Restriction ;
                              owl:onProperty s4bldg:pumpFlowRateMin ;
                              owl:allValuesFrom saref:Measurement
                            ] ;
            rdfs:comment "A pump is a device which imparts mechanical work on fluids or slurries to move them through a channel or pipeline. A typical use of a pump is to circulate chilled water or heating hot water in a building services distribution system."@en ;
            rdfs:label "Pump"@en ;
            rdfs:seeAlso "https://w3id.org/ifc/IFC4_ADD1#IfcPump" ;
            prov:hadPrimarySource <http://www.buildingsmart-tech.org/ifc/IFC4/Add1/html/schema/ifchvacdomain/lexical/ifcpump.htm> ,
                                  <http://www.buildingsmart-tech.org/ifc/IFC4/Add1/html/schema/ifchvacdomain/pset/pset_pumptypecommon.htm> .


###  https://saref.etsi.org/saref4bldg/SanitaryTerminal
s4bldg:SanitaryTerminal rdf:type owl:Class ;
                        rdfs:subClassOf s4bldg:FlowTerminal ;
                        rdfs:comment "A sanitary terminal is a fixed appliance or terminal usually supplied with water and used for drinking, cleaning or foul water disposal or that is an item of equipment directly used with such an appliance or terminal."@en ;
                        rdfs:label "Sanitary terminal"@en ;
                        rdfs:seeAlso "https://w3id.org/ifc/IFC4_ADD1#IfcSanitaryTerminal" ;
                        prov:hadPrimarySource <http://www.buildingsmart-tech.org/ifc/IFC4/Add1/html/schema/ifcplumbingfireprotectiondomain/lexical/ifcsanitaryterminal.htm> ,
                                              <http://www.buildingsmart-tech.org/ifc/IFC4/Add1/html/schema/ifcplumbingfireprotectiondomain/pset/pset_sanitaryterminaltypecommon.htm> .


###  https://saref.etsi.org/saref4bldg/Sensor
s4bldg:Sensor rdf:type owl:Class ;
              rdfs:subClassOf saref:Sensor ,
                              s4bldg:DistributionControlDevice ;
              rdfs:comment "A sensor is a device that measures a physical quantity and converts it into a signal which can be read by an observer or by an instrument."@en ;
              rdfs:label "Sensor"@en ;
              rdfs:seeAlso "https://w3id.org/ifc/IFC4_ADD1#IfcSensor" ;
              prov:hadPrimarySource <http://www.buildingsmart-tech.org/ifc/IFC4/Add1/html/schema/ifcbuildingcontrolsdomain/lexical/ifcsensor.htm> ,
                                    <http://www.buildingsmart-tech.org/ifc/IFC4/Add1/html/schema/ifcbuildingcontrolsdomain/pset/pset_sensortypecommon.htm> .


###  https://saref.etsi.org/saref4bldg/ShadingDevice
s4bldg:ShadingDevice rdf:type owl:Class ;
                     rdfs:subClassOf s4bldg:BuildingDevice ,
                                     [ rdf:type owl:Restriction ;
                                       owl:onProperty s4bldg:solarReflectance ;
                                       owl:allValuesFrom saref:Measurement
                                     ] ,
                                     [ rdf:type owl:Restriction ;
                                       owl:onProperty s4bldg:solarTransmittance ;
                                       owl:allValuesFrom saref:Measurement
                                     ] ,
                                     [ rdf:type owl:Restriction ;
                                       owl:onProperty s4bldg:thermalTransmittance ;
                                       owl:allValuesFrom saref:Measurement
                                     ] ,
                                     [ rdf:type owl:Restriction ;
                                       owl:onProperty s4bldg:visibleLightReflectance ;
                                       owl:allValuesFrom saref:Measurement
                                     ] ,
                                     [ rdf:type owl:Restriction ;
                                       owl:onProperty s4bldg:visibleLightTransmittance ;
                                       owl:allValuesFrom saref:Measurement
                                     ] ,
                                     [ rdf:type owl:Restriction ;
                                       owl:onProperty s4bldg:isExternal ;
                                       owl:allValuesFrom xsd:boolean
                                     ] ,
                                     [ rdf:type owl:Restriction ;
                                       owl:onProperty s4bldg:mechanicalOperated ;
                                       owl:allValuesFrom xsd:boolean
                                     ] ,
                                     [ rdf:type owl:Restriction ;
                                       owl:onProperty s4bldg:roughness ;
                                       owl:allValuesFrom xsd:string
                                     ] ,
                                     [ rdf:type owl:Restriction ;
                                       owl:onProperty s4bldg:shadingDeviceType ;
                                       owl:allValuesFrom xsd:string
                                     ] ;
                     rdfs:comment "Shading devices are purpose built devices to protect from the sunlight, from natural light, or screening them from view. Shading devices can form part of the facade or can be mounted inside the building, they can be fixed or operable."@en ;
                     rdfs:label "Shading device"@en ;
                     rdfs:seeAlso "https://w3id.org/ifc/IFC4_ADD1#IfcShadingDevice" ;
                     prov:hadPrimarySource <http://www.buildingsmart-tech.org/ifc/IFC4/Add1/html/schema/ifcsharedbldgelements/lexical/ifcshadingdevice.htm> ,
                                           <http://www.buildingsmart-tech.org/ifc/IFC4/Add1/html/schema/ifcsharedbldgelements/pset/pset_shadingdevicecommon.htm> .


###  https://saref.etsi.org/saref4bldg/SolarDevice
s4bldg:SolarDevice rdf:type owl:Class ;
                   rdfs:subClassOf s4bldg:EnergyConversionDevice ;
                   rdfs:comment "A solar device converts solar radiation into other energy such as electric current or thermal energy."@en ;
                   rdfs:label "Solar device"@en ;
                   rdfs:seeAlso "https://w3id.org/ifc/IFC4_ADD1#IfcSolarDevice" ;
                   prov:hadPrimarySource <http://www.buildingsmart-tech.org/ifc/IFC4/Add1/html/schema/ifcelectricaldomain/lexical/ifcsolardevicetypeenum.htm> ,
                                         <http://www.buildingsmart-tech.org/ifc/IFC4/Add1/html/schema/ifcelectricaldomain/pset/pset_solardevicetypecommon.htm> .


###  https://saref.etsi.org/saref4bldg/SpaceHeater
s4bldg:SpaceHeater rdf:type owl:Class ;
                   rdfs:subClassOf s4bldg:FlowTerminal ,
                                   [ rdf:type owl:Restriction ;
                                     owl:onProperty s4bldg:bodyMass ;
                                     owl:allValuesFrom saref:Measurement
                                   ] ,
                                   [ rdf:type owl:Restriction ;
                                     owl:onProperty s4bldg:outputCapacity ;
                                     owl:allValuesFrom saref:Measurement
                                   ] ,
                                   [ rdf:type owl:Restriction ;
                                     owl:onProperty s4bldg:thermalEfficiency ;
                                     owl:allValuesFrom saref:Measurement
                                   ] ,
                                   [ rdf:type owl:Restriction ;
                                     owl:onProperty s4bldg:thermalMassHeatCapacity ;
                                     owl:allValuesFrom saref:Measurement
                                   ] ,
                                   [ rdf:type owl:Restriction ;
                                     owl:onProperty s4bldg:energySource ;
                                     owl:allValuesFrom xsd:string
                                   ] ,
                                   [ rdf:type owl:Restriction ;
                                     owl:onProperty s4bldg:heatTransferDimension ;
                                     owl:allValuesFrom xsd:string
                                   ] ,
                                   [ rdf:type owl:Restriction ;
                                     owl:onProperty s4bldg:heatTransferMedium ;
                                     owl:allValuesFrom xsd:string
                                   ] ,
                                   [ rdf:type owl:Restriction ;
                                     owl:onProperty s4bldg:numberOfPanels ;
                                     owl:allValuesFrom xsd:integer
                                   ] ,
                                   [ rdf:type owl:Restriction ;
                                     owl:onProperty s4bldg:numberOfSections ;
                                     owl:allValuesFrom xsd:integer
                                   ] ,
                                   [ rdf:type owl:Restriction ;
                                     owl:onProperty s4bldg:placementType ;
                                     owl:allValuesFrom xsd:string
                                   ] ,
                                   [ rdf:type owl:Restriction ;
                                     owl:onProperty s4bldg:temperatureClassification ;
                                     owl:allValuesFrom xsd:string
                                   ] ;
                   rdfs:comment """Space heaters utilize a combination of radiation and/or natural convection using a heating source such as electricity, steam or hot water to heat a limited space or area. Examples of space heaters include radiators, convectors, baseboard and finned-tube heaters.

UnitaryEquipment should be used for packaged units supporting a combination of heating, cooling, and/or dehumidification; Coil should be used for coil-based floor heating."""@en ;
                   rdfs:label "Space heater"@en ;
                   rdfs:seeAlso "https://w3id.org/ifc/IFC4_ADD1#IfcSpaceHeater" ;
                   prov:hadPrimarySource <http://www.buildingsmart-tech.org/ifc/IFC4/Add1/html/schema/ifchvacdomain/lexical/ifcspaceheater.htm> ,
                                         <http://www.buildingsmart-tech.org/ifc/IFC4/Add1/html/schema/ifchvacdomain/pset/pset_spaceheatertypecommon.htm> .


###  https://saref.etsi.org/saref4bldg/SwitchingDevice
s4bldg:SwitchingDevice rdf:type owl:Class ;
                       rdfs:subClassOf s4bldg:FlowController ,
                                       [ rdf:type owl:Restriction ;
                                         owl:onProperty s4bldg:hasLock ;
                                         owl:allValuesFrom xsd:boolean
                                       ] ,
                                       [ rdf:type owl:Restriction ;
                                         owl:onProperty s4bldg:isIlluminated ;
                                         owl:allValuesFrom xsd:boolean
                                       ] ,
                                       [ rdf:type owl:Restriction ;
                                         owl:onProperty s4bldg:legend ;
                                         owl:allValuesFrom xsd:string
                                       ] ,
                                       [ rdf:type owl:Restriction ;
                                         owl:onProperty s4bldg:numberOfGangs ;
                                         owl:allValuesFrom xsd:integer
                                       ] ,
                                       [ rdf:type owl:Restriction ;
                                         owl:onProperty s4bldg:switchFunction ;
                                         owl:allValuesFrom xsd:string
                                       ] ;
                       rdfs:comment """A switch is used in a cable distribution system (electrical circuit) to control or modulate the flow of electricity.

Switches include those used for electrical power, communications, audio-visual, or other distribution system types as determined by the available ports."""@en ;
                       rdfs:label "Switching device"@en ;
                       rdfs:seeAlso "https://w3id.org/ifc/IFC4_ADD1#IfcSwitchingDevice" ;
                       prov:hadPrimarySource <http://www.buildingsmart-tech.org/ifc/IFC4/Add1/html/schema/ifcelectricaldomain/lexical/ifcswitchingdevice.htm> ,
                                             <http://www.buildingsmart-tech.org/ifc/IFC4/Add1/html/schema/ifcelectricaldomain/pset/pset_switchingdevicetypecommon.htm> .


###  https://saref.etsi.org/saref4bldg/Tank
s4bldg:Tank rdf:type owl:Class ;
            rdfs:subClassOf s4bldg:FlowStorageDevice ,
                            [ rdf:type owl:Restriction ;
                              owl:onProperty s4bldg:effectiveCapacity ;
                              owl:allValuesFrom saref:Measurement
                            ] ,
                            [ rdf:type owl:Restriction ;
                              owl:onProperty s4bldg:firstCurvatureRadius ;
                              owl:allValuesFrom saref:Measurement
                            ] ,
                            [ rdf:type owl:Restriction ;
                              owl:onProperty s4bldg:nominalDepth ;
                              owl:allValuesFrom saref:Measurement
                            ] ,
                            [ rdf:type owl:Restriction ;
                              owl:onProperty s4bldg:nominalLengthOrDiameter ;
                              owl:allValuesFrom saref:Measurement
                            ] ,
                            [ rdf:type owl:Restriction ;
                              owl:onProperty s4bldg:nominalVolumetricCapacity ;
                              owl:allValuesFrom saref:Measurement
                            ] ,
                            [ rdf:type owl:Restriction ;
                              owl:onProperty s4bldg:nominalWidthOrDiameter ;
                              owl:allValuesFrom saref:Measurement
                            ] ,
                            [ rdf:type owl:Restriction ;
                              owl:onProperty s4bldg:operatingWeight ;
                              owl:allValuesFrom saref:Measurement
                            ] ,
                            [ rdf:type owl:Restriction ;
                              owl:onProperty s4bldg:secondCurvatureRadius ;
                              owl:allValuesFrom saref:Measurement
                            ] ,
                            [ rdf:type owl:Restriction ;
                              owl:onProperty s4bldg:accessType ;
                              owl:allValuesFrom xsd:string
                            ] ,
                            [ rdf:type owl:Restriction ;
                              owl:onProperty s4bldg:endShapeType ;
                              owl:allValuesFrom xsd:string
                            ] ,
                            [ rdf:type owl:Restriction ;
                              owl:onProperty s4bldg:numberOfSections ;
                              owl:allValuesFrom xsd:integer
                            ] ,
                            [ rdf:type owl:Restriction ;
                              owl:onProperty s4bldg:patternType ;
                              owl:allValuesFrom xsd:string
                            ] ,
                            [ rdf:type owl:Restriction ;
                              owl:onProperty s4bldg:storageType ;
                              owl:allValuesFrom xsd:string
                            ] ;
            rdfs:comment "A tank is a vessel or container in which a fluid or gas is stored for later use."@en ;
            rdfs:label "Tank"@en ;
            rdfs:seeAlso "https://w3id.org/ifc/IFC4_ADD1#IfcTank" ;
            prov:hadPrimarySource <http://www.buildingsmart-tech.org/ifc/IFC4/Add1/html/schema/ifchvacdomain/lexical/ifctank.htm> ,
                                  <http://www.buildingsmart-tech.org/ifc/IFC4/Add1/html/schema/ifchvacdomain/pset/pset_tanktypecommon.htm> .


###  https://saref.etsi.org/saref4bldg/Transformer
s4bldg:Transformer rdf:type owl:Class ;
                   rdfs:subClassOf s4bldg:EnergyConversionDevice ,
                                   [ rdf:type owl:Restriction ;
                                     owl:onProperty s4bldg:apparentPowerMax ;
                                     owl:allValuesFrom saref:Measurement
                                   ] ,
                                   [ rdf:type owl:Restriction ;
                                     owl:onProperty s4bldg:imaginaryImpedanceRatio ;
                                     owl:allValuesFrom saref:Measurement
                                   ] ,
                                   [ rdf:type owl:Restriction ;
                                     owl:onProperty s4bldg:primaryApparentPower ;
                                     owl:allValuesFrom saref:Measurement
                                   ] ,
                                   [ rdf:type owl:Restriction ;
                                     owl:onProperty s4bldg:primaryCurrent ;
                                     owl:allValuesFrom saref:Measurement
                                   ] ,
                                   [ rdf:type owl:Restriction ;
                                     owl:onProperty s4bldg:primaryFrequency ;
                                     owl:allValuesFrom saref:Measurement
                                   ] ,
                                   [ rdf:type owl:Restriction ;
                                     owl:onProperty s4bldg:primaryVoltage ;
                                     owl:allValuesFrom saref:Measurement
                                   ] ,
                                   [ rdf:type owl:Restriction ;
                                     owl:onProperty s4bldg:realImpedanceRatio ;
                                     owl:allValuesFrom saref:Measurement
                                   ] ,
                                   [ rdf:type owl:Restriction ;
                                     owl:onProperty s4bldg:secondaryApparentPower ;
                                     owl:allValuesFrom saref:Measurement
                                   ] ,
                                   [ rdf:type owl:Restriction ;
                                     owl:onProperty s4bldg:secondaryCurrent ;
                                     owl:allValuesFrom saref:Measurement
                                   ] ,
                                   [ rdf:type owl:Restriction ;
                                     owl:onProperty s4bldg:secondaryFrequency ;
                                     owl:allValuesFrom saref:Measurement
                                   ] ,
                                   [ rdf:type owl:Restriction ;
                                     owl:onProperty s4bldg:secondaryVoltage ;
                                     owl:allValuesFrom saref:Measurement
                                   ] ,
                                   [ rdf:type owl:Restriction ;
                                     owl:onProperty s4bldg:isNeutralPrimaryTerminalAvailable ;
                                     owl:allValuesFrom xsd:boolean
                                   ] ,
                                   [ rdf:type owl:Restriction ;
                                     owl:onProperty s4bldg:isNeutralSecondaryTerminalAvailable ;
                                     owl:allValuesFrom xsd:boolean
                                   ] ,
                                   [ rdf:type owl:Restriction ;
                                     owl:onProperty s4bldg:secondaryCurrentType ;
                                     owl:allValuesFrom xsd:string
                                   ] ,
                                   [ rdf:type owl:Restriction ;
                                     owl:onProperty s4bldg:transformerVectorGroup ;
                                     owl:allValuesFrom xsd:string
                                   ] ;
                   rdfs:comment """A transformer is an inductive stationary device that transfers electrical energy from one circuit to another.

Transformer is used to transform electric power; conversion of electric signals for other purposes is handled at other entities: Controller converts arbitrary signals, AudioVisualAppliance converts signals for audio or video streams, and CommunicationsAppliance converts signals for data or other communications usage."""@en ;
                   rdfs:label "Transformer"@en ;
                   rdfs:seeAlso "https://w3id.org/ifc/IFC4_ADD1#IfcTransformer" ;
                   prov:hadPrimarySource <http://www.buildingsmart-tech.org/ifc/IFC4/Add1/html/schema/ifcelectricaldomain/lexical/ifctransformer.htm> ,
                                         <http://www.buildingsmart-tech.org/ifc/IFC4/Add1/html/schema/ifcelectricaldomain/pset/pset_transformertypecommon.htm> .


###  https://saref.etsi.org/saref4bldg/TransportElement
s4bldg:TransportElement rdf:type owl:Class ;
                        rdfs:subClassOf saref:Device ,
                                        [ rdf:type owl:Restriction ;
                                          owl:onProperty s4bldg:capacityWeight ;
                                          owl:allValuesFrom saref:Measurement
                                        ] ,
                                        [ rdf:type owl:Restriction ;
                                          owl:onProperty s4bldg:capacityPeople ;
                                          owl:allValuesFrom xsd:positiveInteger
                                        ] ,
                                        [ rdf:type owl:Restriction ;
                                          owl:onProperty s4bldg:fireExit ;
                                          owl:allValuesFrom xsd:boolean
                                        ] ;
                        rdfs:comment "A transport element is a generalization of all transport related objects that move people, animals or goods within a building or building complex. The TransportElement defines the occurrence of a transport element. "@en ;
                        rdfs:label "Transport element"@en ;
                        rdfs:seeAlso "https://w3id.org/ifc/IFC4_ADD1#IfcTransportElement" ;
                        prov:hadPrimarySource <http://www.buildingsmart-tech.org/ifc/IFC4/Add1/html/schema/ifcproductextension/lexical/ifctransportelement.htm> ,
                                              <http://www.buildingsmart-tech.org/ifc/IFC4/Add1/html/schema/ifcproductextension/pset/pset_transportelementcommon.htm> .


###  https://saref.etsi.org/saref4bldg/TubeBundle
s4bldg:TubeBundle rdf:type owl:Class ;
                  rdfs:subClassOf s4bldg:EnergyConversionDevice ,
                                  [ rdf:type owl:Restriction ;
                                    owl:onProperty s4bldg:foulingFactor ;
                                    owl:allValuesFrom saref:Measurement
                                  ] ,
                                  [ rdf:type owl:Restriction ;
                                    owl:onProperty s4bldg:horizontalSpacing ;
                                    owl:allValuesFrom saref:Measurement
                                  ] ,
                                  [ rdf:type owl:Restriction ;
                                    owl:onProperty s4bldg:inLineRowSpacing ;
                                    owl:allValuesFrom saref:Measurement
                                  ] ,
                                  [ rdf:type owl:Restriction ;
                                    owl:onProperty s4bldg:insideDiameter ;
                                    owl:allValuesFrom saref:Measurement
                                  ] ,
                                  [ rdf:type owl:Restriction ;
                                    owl:onProperty s4bldg:length ;
                                    owl:allValuesFrom saref:Measurement
                                  ] ,
                                  [ rdf:type owl:Restriction ;
                                    owl:onProperty s4bldg:nominalDiameter ;
                                    owl:allValuesFrom saref:Measurement
                                  ] ,
                                  [ rdf:type owl:Restriction ;
                                    owl:onProperty s4bldg:outsideDiameter ;
                                    owl:allValuesFrom saref:Measurement
                                  ] ,
                                  [ rdf:type owl:Restriction ;
                                    owl:onProperty s4bldg:staggeredRowSpacing ;
                                    owl:allValuesFrom saref:Measurement
                                  ] ,
                                  [ rdf:type owl:Restriction ;
                                    owl:onProperty s4bldg:thermalConductivity ;
                                    owl:allValuesFrom saref:Measurement
                                  ] ,
                                  [ rdf:type owl:Restriction ;
                                    owl:onProperty s4bldg:verticalSpacing ;
                                    owl:allValuesFrom saref:Measurement
                                  ] ,
                                  [ rdf:type owl:Restriction ;
                                    owl:onProperty s4bldg:volumen ;
                                    owl:allValuesFrom saref:Measurement
                                  ] ,
                                  [ rdf:type owl:Restriction ;
                                    owl:onProperty s4bldg:hasTurbulator ;
                                    owl:allValuesFrom xsd:boolean
                                  ] ,
                                  [ rdf:type owl:Restriction ;
                                    owl:onProperty s4bldg:numberOfCircuits ;
                                    owl:allValuesFrom xsd:integer
                                  ] ,
                                  [ rdf:type owl:Restriction ;
                                    owl:onProperty s4bldg:numberOfRows ;
                                    owl:allValuesFrom xsd:integer
                                  ] ;
                  rdfs:comment "A tube bundle is a device consisting of tubes and bundles of tubes used for heat transfer and contained typically within other energy conversion devices, such as a chiller or coil."@en ;
                  rdfs:label "Tube bundle"@en ;
                  rdfs:seeAlso "https://w3id.org/ifc/IFC4_ADD1#IfcTubeBundle" ;
                  prov:hadPrimarySource <http://www.buildingsmart-tech.org/ifc/IFC4/Add1/html/schema/ifchvacdomain/lexical/ifctubebundle.htm> ,
                                        <http://www.buildingsmart-tech.org/ifc/IFC4/Add1/html/schema/ifchvacdomain/pset/pset_tubebundletypecommon.htm> .


###  https://saref.etsi.org/saref4bldg/UnitaryControlElement
s4bldg:UnitaryControlElement rdf:type owl:Class ;
                             rdfs:subClassOf s4bldg:DistributionControlDevice ;
                             rdfs:comment """A unitary control element combines a number of control components into a single product, such as a thermostat or humidistat.

A unitary control element provides a housing for an aggregation of control or electrical distribution elements that, in combination, perform a singular (unitary) purpose. Each item in the aggregation may have its own geometric representation and location."""@en ;
                             rdfs:label "Unitary control element"@en ;
                             rdfs:seeAlso "https://w3id.org/ifc/IFC4_ADD1#IfcUnitaryControlElement" ;
                             prov:hadPrimarySource <http://www.buildingsmart-tech.org/ifc/IFC4/Add1/html/schema/ifcbuildingcontrolsdomain/lexical/ifcunitarycontrolelement.htm> ,
                                                   <http://www.buildingsmart-tech.org/ifc/IFC4/Add1/html/schema/ifcbuildingcontrolsdomain/pset/pset_unitarycontrolelementtypecommon.htm> .


###  https://saref.etsi.org/saref4bldg/Valve
s4bldg:Valve rdf:type owl:Class ;
             rdfs:subClassOf s4bldg:FlowController ,
                             [ rdf:type owl:Restriction ;
                               owl:onProperty s4bldg:closeOffRating ;
                               owl:allValuesFrom saref:Measurement
                             ] ,
                             [ rdf:type owl:Restriction ;
                               owl:onProperty s4bldg:flowCoefficient ;
                               owl:allValuesFrom saref:Measurement
                             ] ,
                             [ rdf:type owl:Restriction ;
                               owl:onProperty s4bldg:size ;
                               owl:allValuesFrom saref:Measurement
                             ] ,
                             [ rdf:type owl:Restriction ;
                               owl:onProperty s4bldg:testPressure ;
                               owl:allValuesFrom saref:Measurement
                             ] ,
                             [ rdf:type owl:Restriction ;
                               owl:onProperty s4bldg:workingPressure ;
                               owl:allValuesFrom saref:Measurement
                             ] ,
                             [ rdf:type owl:Restriction ;
                               owl:onProperty s4bldg:valveMechanism ;
                               owl:allValuesFrom xsd:string
                             ] ,
                             [ rdf:type owl:Restriction ;
                               owl:onProperty s4bldg:valveOperation ;
                               owl:allValuesFrom xsd:string
                             ] ,
                             [ rdf:type owl:Restriction ;
                               owl:onProperty s4bldg:valvePattern ;
                               owl:allValuesFrom xsd:string
                             ] ;
             rdfs:comment "A valve is used in a building services piping distribution system to control or modulate the flow of the fluid."@en ;
             rdfs:label "Valve"@en ;
             rdfs:seeAlso "https://w3id.org/ifc/IFC4_ADD1#IfcValve" ;
             prov:hadPrimarySource <http://www.buildingsmart-tech.org/ifc/IFC4/Add1/html/schema/ifchvacdomain/lexical/ifcvalve.htm> ,
                                   <http://www.buildingsmart-tech.org/ifc/IFC4/Add1/html/schema/ifchvacdomain/pset/pset_valvetypecommon.htm> .


###  https://saref.etsi.org/saref4bldg/VibrationIsolator
s4bldg:VibrationIsolator rdf:type owl:Class ;
                         rdfs:subClassOf saref:Device ,
                                         [ rdf:type owl:Restriction ;
                                           owl:onProperty s4bldg:height ;
                                           owl:allValuesFrom saref:Measurement
                                         ] ,
                                         [ rdf:type owl:Restriction ;
                                           owl:onProperty s4bldg:isolatorCompressibility ;
                                           owl:allValuesFrom saref:Measurement
                                         ] ,
                                         [ rdf:type owl:Restriction ;
                                           owl:onProperty s4bldg:isolatorStaticDeflection ;
                                           owl:allValuesFrom saref:Measurement
                                         ] ,
                                         [ rdf:type owl:Restriction ;
                                           owl:onProperty s4bldg:supportedWeightMax ;
                                           owl:allValuesFrom saref:Measurement
                                         ] ,
                                         [ rdf:type owl:Restriction ;
                                           owl:onProperty s4bldg:vibrationTransmissibility ;
                                           owl:allValuesFrom saref:Measurement
                                         ] ;
                         rdfs:comment "A vibration isolator is a device used to minimize the effects of vibration transmissibility in a building."@en ;
                         rdfs:label "Vibration isolator"@en ;
                         rdfs:seeAlso "https://w3id.org/ifc/IFC4_ADD1#IfcVibrationIsolator" ;
                         prov:hadPrimarySource <http://www.buildingsmart-tech.org/ifc/IFC4/Add1/html/schema/ifchvacdomain/lexical/ifcvibrationisolator.htm> ,
                                               <http://www.buildingsmart-tech.org/ifc/IFC4/Add1/html/schema/ifchvacdomain/pset/pset_vibrationisolatortypecommon.htm> .


###  https://saref.etsi.org/saref4city/Agent
s4city:Agent rdf:type owl:Class ;
             rdfs:comment "An agent making an action in the context of a city. An agent could be a person, software, etc."@en ;
             rdfs:isDefinedBy s4city: ;
             rdfs:label "Agent"@en .


###  https://saref.etsi.org/saref4city/KeyPerformanceIndicator
s4city:KeyPerformanceIndicator rdf:type owl:Class ;
                               rdfs:subClassOf [ rdf:type owl:Restriction ;
                                                 owl:onProperty s4city:hasCalculationPeriod ;
                                                 owl:allValuesFrom time:TemporalDuration
                                               ] ,
                                               [ rdf:type owl:Restriction ;
                                                 owl:onProperty s4city:isKPIOf ;
                                                 owl:allValuesFrom saref:FeatureOfInterest
                                               ] ;
                               rdfs:comment "A Key Performance Indicator (KPI) is a type of performance measurement. KPIs evaluate the success of an organization or of a particular activity in which it engages. (Definition taken from FIWARE)"@en ;
                               rdfs:isDefinedBy s4city: ;
                               rdfs:label "Key Performance Indicator"@en ;
                               rdfs:seeAlso <http://fiware-datamodels.readthedocs.io/en/latest/KeyPerformanceIndicator/doc/spec/index.html> .


###  https://saref.etsi.org/saref4city/KeyPerformanceIndicatorAssessment
s4city:KeyPerformanceIndicatorAssessment rdf:type owl:Class ;
                                         rdfs:subClassOf [ rdf:type owl:Restriction ;
                                                           owl:onProperty saref:isMeasuredIn ;
                                                           owl:allValuesFrom saref:UnitOfMeasure
                                                         ] ,
                                                         [ rdf:type owl:Restriction ;
                                                           owl:onProperty s4city:assesses ;
                                                           owl:allValuesFrom saref:FeatureOfInterest
                                                         ] ,
                                                         [ rdf:type owl:Restriction ;
                                                           owl:onProperty s4city:isAssessedBy ;
                                                           owl:allValuesFrom s4city:Agent
                                                         ] ,
                                                         [ rdf:type owl:Restriction ;
                                                           owl:onProperty s4city:isDerivedFrom ;
                                                           owl:allValuesFrom saref:Measurement
                                                         ] ,
                                                         [ rdf:type owl:Restriction ;
                                                           owl:onProperty s4city:quantifiesKPI ;
                                                           owl:allValuesFrom s4city:KeyPerformanceIndicator
                                                         ] ,
                                                         [ rdf:type owl:Restriction ;
                                                           owl:onProperty s4city:refersToTime ;
                                                           owl:allValuesFrom time:TemporalEntity
                                                         ] ,
                                                         [ rdf:type owl:Restriction ;
                                                           owl:onProperty s4city:hasCreationDate ;
                                                           owl:allValuesFrom xsd:dateTime
                                                         ] ,
                                                         [ rdf:type owl:Restriction ;
                                                           owl:onProperty s4city:hasExpirationDate ;
                                                           owl:allValuesFrom xsd:dateTime
                                                         ] ,
                                                         [ rdf:type owl:Restriction ;
                                                           owl:onProperty s4city:hasLastUpdateDate ;
                                                           owl:allValuesFrom xsd:dateTime
                                                         ] ,
                                                         [ rdf:type owl:Restriction ;
                                                           owl:onProperty saref:hasValue ;
                                                           owl:cardinality "1"^^xsd:nonNegativeInteger
                                                         ] ;
                                         rdfs:comment "A Key Performance Indicator assessment represents the assessment of a KPI calculated by a given agent in a given time."@en ;
                                         rdfs:isDefinedBy s4city: ;
                                         rdfs:label "Key performance indicator assessment"@en .


###  https://saref.etsi.org/saref4syst/Connection
s4syst:Connection rdf:type owl:Class ;
                  rdfs:subClassOf [ rdf:type owl:Restriction ;
                                    owl:onProperty s4syst:connectsSystem ;
                                    owl:someValuesFrom s4syst:System
                                  ] ,
                                  [ rdf:type owl:Restriction ;
                                    owl:onProperty s4syst:connectsSystemAt ;
                                    owl:someValuesFrom s4syst:ConnectionPoint
                                  ] ;
                  owl:disjointWith s4syst:ConnectionPoint ,
                                   s4syst:System ;
                  rdfs:comment "The class of connections between systems. This class qualifies property s4syst:connectedTo. A connection describes potential interactions between systems. Any two connected systems are connected through a connection. A connection can connect more than two systems at the same time."@en ;
                  rdfs:label "Connection"@en .


###  https://saref.etsi.org/saref4syst/ConnectionPoint
s4syst:ConnectionPoint rdf:type owl:Class ;
                       rdfs:subClassOf [ rdf:type owl:Restriction ;
                                         owl:onProperty s4syst:connectionPointOf ;
                                         owl:cardinality "1"^^xsd:nonNegativeInteger
                                       ] ;
                       owl:disjointWith s4syst:System ;
                       rdfs:comment "The class of connection points of systems, at which they may be connected to other systems. This class qualifies properties s4syst:connectsSystem and s4syst:connectedThrough. A connection point belongs to exactly one system. Any system connected through a connection is connected at one of its connection points to the connection. The system of a connection point that is connected through a connection is itself connected through the connection."@en ;
                       rdfs:label "Connection Point"@en .


###  https://saref.etsi.org/saref4syst/System
s4syst:System rdf:type owl:Class ;
              rdfs:comment "The class of systems, i.e., systems virtually isolated from the environment, whose behaviour and interactions with the environment are modeled. Systems can be connected to other systems. Connected systems interact in some ways. Systems can also have subsystems. Properties of subsystems somehow contribute to the properties of the supersystem."@en ;
              rdfs:isDefinedBy s4syst: ;
              rdfs:label "System"@en .


###  https://saref.etsi.org/saref4watr/AcceptabilityProperty
s4watr:AcceptabilityProperty rdf:type owl:Class ;
                             rdfs:subClassOf s4watr:WaterProperty ;
                             rdfs:comment "An acceptability property is a property of water that is related to its acceptability."@en ;
                             rdfs:label "Acceptability property"@en .


###  https://saref.etsi.org/saref4watr/Aquifer
s4watr:Aquifer rdf:type owl:Class ;
               rdfs:subClassOf s4watr:StorageAsset ;
               rdfs:comment "An aquifer is an underground layer of water-bearing permeable rock, rock fractures or unconsolidated materials."@en ;
               rdfs:label "Aquifer"@en .


###  https://saref.etsi.org/saref4watr/BacterialProperty
s4watr:BacterialProperty rdf:type owl:Class ;
                         rdfs:subClassOf s4watr:MicrobialProperty ;
                         rdfs:comment "A bacterial property is a property of water that is related to bacteria."@en ;
                         rdfs:label "Bacterial property"@en .


###  https://saref.etsi.org/saref4watr/Channel
s4watr:Channel rdf:type owl:Class ;
               rdfs:subClassOf s4watr:Main ;
               rdfs:comment "A channel is a passage of water flowing in an open conduit (i.e., subject to atmospheric pressure)."@en ;
               rdfs:label "Channel"@en .


###  https://saref.etsi.org/saref4watr/ChemicalProperty
s4watr:ChemicalProperty rdf:type owl:Class ;
                        rdfs:subClassOf s4watr:WaterProperty ;
                        rdfs:comment "A chemical property is a property of water that is related to chemical components."@en ;
                        rdfs:label "ChemicalProperty"@en .


###  https://saref.etsi.org/saref4watr/ConsumptionBasedTariff
s4watr:ConsumptionBasedTariff rdf:type owl:Class ;
                              rdfs:subClassOf s4watr:Tariff ;
                              rdfs:comment "A consumption-based tariff is a tariff that is based on consumption."@en ;
                              rdfs:label "Consumption-based tariff"@en .


###  https://saref.etsi.org/saref4watr/DistributionSystem
s4watr:DistributionSystem rdf:type owl:Class ;
                          rdfs:subClassOf s4watr:WaterInfrastructure ;
                          rdfs:comment "A water distribution system is an infrastructure to carry potable water from a centralized treatment plant or wells to water consumers in order to adequately deliver water to satisfy residential, commercial, industrial and fire fighting requirements."@en ;
                          rdfs:label "Distribution system"@en .


###  https://saref.etsi.org/saref4watr/EnvironmentalProperty
s4watr:EnvironmentalProperty rdf:type owl:Class ;
                             rdfs:subClassOf saref:Property ;
                             rdfs:comment "Class to group those properties related to the environment."@en ;
                             rdfs:label "Environmental property"@en .


###  https://saref.etsi.org/saref4watr/Estuary
s4watr:Estuary rdf:type owl:Class ;
               rdfs:subClassOf s4watr:SinkAsset ;
               rdfs:comment "An estuary is a partially enclosed coastal body of brackish water with one or more rivers or streams flowing into it, and with a free connection to the open sea."@en ;
               rdfs:label "Estuary"@en .


###  https://saref.etsi.org/saref4watr/FireHydrant
s4watr:FireHydrant rdf:type owl:Class ;
                   rdfs:subClassOf s4watr:WaterDevice ;
                   rdfs:comment "A fire hydrant is a fitting in a street or other public place with a nozzle by which a fire hose may be attached to a water main."@en ;
                   rdfs:label "Fire hydrant"@en .


###  https://saref.etsi.org/saref4watr/GaugingStation
s4watr:GaugingStation rdf:type owl:Class ;
                      rdfs:subClassOf s4watr:MonitoringInfrastructure ;
                      rdfs:comment "A gauging station is an infrastructure to monitor and test terrestrial bodies of water."@en ;
                      rdfs:label "Gauging station"@en .


###  https://saref.etsi.org/saref4watr/Glacier
s4watr:Glacier rdf:type owl:Class ;
               rdfs:subClassOf s4watr:SourceAsset ;
               rdfs:comment "A glacier is a persistent body of dense ice that is constantly moving under its own weight."@en ;
               rdfs:label "Glacier"@en .


###  https://saref.etsi.org/saref4watr/HydroelectricPowerPlant
s4watr:HydroelectricPowerPlant rdf:type owl:Class ;
                               rdfs:subClassOf s4watr:WaterInfrastructure ;
                               rdfs:comment "A hydroelectric power plant is an infrastructure to generate electricity by conversion of the energy of running water."@en ;
                               rdfs:label "Hydroelectric power plant"@en .


###  https://saref.etsi.org/saref4watr/Intake
s4watr:Intake rdf:type owl:Class ;
              rdfs:subClassOf s4watr:TransportAsset ;
              rdfs:comment "An intake is an installation for obtaining water from a source of supply (river, lake, reservoir, and so on)."@en ;
              rdfs:label "Intake"@en .


###  https://saref.etsi.org/saref4watr/Lagoon
s4watr:Lagoon rdf:type owl:Class ;
              rdfs:subClassOf s4watr:SourceAsset ;
              rdfs:comment "A lagoon is a shallow body of water separated from a larger body of water by barrier islands or reefs."@en ;
              rdfs:label "Lagoon"@en .


###  https://saref.etsi.org/saref4watr/Lake
s4watr:Lake rdf:type owl:Class ;
            rdfs:subClassOf s4watr:SourceAsset ;
            rdfs:comment "A lake is an area filled with water, localized in a basin, surrounded by land, apart from any river or other outlet that serves to feed or drain the lake."@en ;
            rdfs:label "Lake"@en .


###  https://saref.etsi.org/saref4watr/Main
s4watr:Main rdf:type owl:Class ;
            rdfs:subClassOf s4watr:TransportAsset ;
            rdfs:comment "A main is a passage of water to flow through."@en ;
            rdfs:label "Main"@en .


###  https://saref.etsi.org/saref4watr/Manhole
s4watr:Manhole rdf:type owl:Class ;
               rdfs:subClassOf s4watr:TransportAsset ;
               rdfs:comment "A maintenance hole is an enclosure that facilitates human access to and working space for equipment."@en ;
               rdfs:label "Maintenance hole"@en ,
                          "Manhole"@en .


###  https://saref.etsi.org/saref4watr/MicrobialProperty
s4watr:MicrobialProperty rdf:type owl:Class ;
                         rdfs:subClassOf s4watr:WaterProperty ;
                         rdfs:comment "A microbial property is a property of water that is related to microbes."@en ;
                         rdfs:label "Microbial property"@en .


###  https://saref.etsi.org/saref4watr/MonitoringInfrastructure
s4watr:MonitoringInfrastructure rdf:type owl:Class ;
                                rdfs:subClassOf s4watr:WaterInfrastructure ;
                                rdfs:comment "A monitoring infrastructure is an infrastructure to monitor water."@en ;
                                rdfs:label "Monitoring infrastructure"@en .


###  https://saref.etsi.org/saref4watr/Ocean
s4watr:Ocean rdf:type owl:Class ;
             rdfs:subClassOf s4watr:SinkAsset ;
             rdfs:comment "An ocean is a large body of salt water."@en ;
             rdfs:label "Ocean"@en .


###  https://saref.etsi.org/saref4watr/Pipe
s4watr:Pipe rdf:type owl:Class ;
            rdfs:subClassOf s4watr:Main ;
            rdfs:comment "A pipe is a passage of water flowing in a closed conduit (i.e., not subject to atmospheric pressure)."@en ;
            rdfs:label "Pipe"@en .


###  https://saref.etsi.org/saref4watr/Pit
s4watr:Pit rdf:type owl:Class ;
           rdfs:subClassOf s4watr:TransportAsset ;
           rdfs:comment "A pit is a well or hole sunk in the ground to procure, store or drain water."@en ;
           rdfs:label "Pit"@en .


###  https://saref.etsi.org/saref4watr/Pump
s4watr:Pump rdf:type owl:Class ;
            rdfs:subClassOf saref:Actuator ,
                            s4watr:WaterDevice ;
            rdfs:comment "A pump is a device for moving water by mechanical action."@en ;
            rdfs:label "Pump"@en .


###  https://saref.etsi.org/saref4watr/Reservoir
s4watr:Reservoir rdf:type owl:Class ;
                 rdfs:subClassOf s4watr:StorageAsset ;
                 rdfs:comment "A reservoir is an enlarged natural or artificial lake, pond or impoundment created using a dam or lock to store water."@en ;
                 rdfs:label "Reservoir"@en .


###  https://saref.etsi.org/saref4watr/River
s4watr:River rdf:type owl:Class ;
             rdfs:subClassOf s4watr:SinkAsset ;
             rdfs:comment "A river is a natural flowing watercourse, usually freshwater, flowing towards an ocean, sea, lake or another river."@en ;
             rdfs:label "River"@en .


###  https://saref.etsi.org/saref4watr/Sea
s4watr:Sea rdf:type owl:Class ;
           rdfs:subClassOf s4watr:SinkAsset ;
           rdfs:comment "A sea is a body of salt water partly or fully enclosed by land."@en ;
           rdfs:label "Sea"@en .


###  https://saref.etsi.org/saref4watr/SinkAsset
s4watr:SinkAsset rdf:type owl:Class ;
                 rdfs:subClassOf s4watr:WaterAsset ;
                 rdfs:comment "A sink asset is a water asset where water sinks."@en ;
                 rdfs:label "Sink asset"@en .


###  https://saref.etsi.org/saref4watr/SourceAsset
s4watr:SourceAsset rdf:type owl:Class ;
                   rdfs:subClassOf s4watr:WaterAsset ;
                   rdfs:comment "A source asset is a water asset that is a natural source of water."@en ;
                   rdfs:label "Source asset"@en .


###  https://saref.etsi.org/saref4watr/StorageAsset
s4watr:StorageAsset rdf:type owl:Class ;
                    rdfs:subClassOf s4watr:WaterAsset ;
                    rdfs:comment "A storage asset is a water asset used to store water."@en ;
                    rdfs:label "Storage asset"@en .


###  https://saref.etsi.org/saref4watr/StorageInfrastructure
s4watr:StorageInfrastructure rdf:type owl:Class ;
                             rdfs:subClassOf s4watr:WaterInfrastructure ;
                             rdfs:comment "An storage infrastructure is an infrastructure to storage both potable water for consumption, and non potable water for use in agriculture."@en ;
                             rdfs:label "Storage infrastructure"@en .


###  https://saref.etsi.org/saref4watr/Tank
s4watr:Tank rdf:type owl:Class ;
            rdfs:subClassOf s4watr:StorageAsset ;
            rdfs:comment "A tank is a container for storing water."@en ;
            rdfs:label "Tank"@en .


###  https://saref.etsi.org/saref4watr/Tariff
s4watr:Tariff rdf:type owl:Class ;
              rdfs:comment "A tariff is a schedule of rates or charges of a business or a public utility. Tariffs can be based on time, thresholds or consumption; however, combined tariffs may also exist that mix more than one of these types."@en ;
              rdfs:label "Tariff"@en .


###  https://saref.etsi.org/saref4watr/ThresholdBasedTariff
s4watr:ThresholdBasedTariff rdf:type owl:Class ;
                            rdfs:subClassOf s4watr:Tariff ;
                            rdfs:comment "A threshold-based tariff is a tariff that is based on a threshold."@en ;
                            rdfs:label "Threshold-based tariff"@en .


###  https://saref.etsi.org/saref4watr/TimeBasedTariff
s4watr:TimeBasedTariff rdf:type owl:Class ;
                       rdfs:subClassOf s4watr:Tariff ;
                       rdfs:comment "A time-based tariff is a tariff that is based on time."@en ;
                       rdfs:label "Time-based tariff"@en .


###  https://saref.etsi.org/saref4watr/TransportAsset
s4watr:TransportAsset rdf:type owl:Class ;
                      rdfs:subClassOf s4watr:WaterAsset ;
                      rdfs:comment "A transport asset is a water asset used to enable and support the transport and distribution of water."@en ;
                      rdfs:label "Transport asset"@en .


###  https://saref.etsi.org/saref4watr/TreatmentPlant
s4watr:TreatmentPlant rdf:type owl:Class ;
                      rdfs:subClassOf s4watr:WaterInfrastructure ;
                      rdfs:comment "A treatment plant is an infrastructure to improve the quality of water to make it more acceptable for a specific end-use."@en ;
                      rdfs:label "Treatment plant"@en .


###  https://saref.etsi.org/saref4watr/Valve
s4watr:Valve rdf:type owl:Class ;
             rdfs:subClassOf saref:Actuator ,
                             s4watr:WaterDevice ;
             rdfs:comment "A valve is a device designed to control water flow, pressure or volume."@en ;
             rdfs:label "Valve"@en .


###  https://saref.etsi.org/saref4watr/Vent
s4watr:Vent rdf:type owl:Class ;
            rdfs:subClassOf s4watr:TransportAsset ;
            rdfs:comment "A vent is the part of a system that allows air to enter a plumbing system to maintain proper air pressure and sewer gases to escape to the outside."@en ;
            rdfs:label "Vent"@en .


###  https://saref.etsi.org/saref4watr/Water
s4watr:Water rdf:type owl:Class ;
             rdfs:subClassOf saref:FeatureOfInterest ,
                             [ rdf:type owl:Restriction ;
                               owl:onProperty saref:hasProperty ;
                               owl:allValuesFrom s4watr:WaterProperty
                             ] ;
             rdfs:comment "This class is used to define a particular quantity or body of water."@en ;
             rdfs:label "Water"@en .


###  https://saref.etsi.org/saref4watr/WaterAsset
s4watr:WaterAsset rdf:type owl:Class ;
                  rdfs:subClassOf geosp:Feature ,
                                  saref:FeatureOfInterest ,
                                  s4syst:System ;
                  rdfs:comment "A water asset is a physical entity used in the process of transporting, treating, storing and distributing water."@en ;
                  rdfs:label "Water asset"@en .


###  https://saref.etsi.org/saref4watr/WaterDevice
s4watr:WaterDevice rdf:type owl:Class ;
                   rdfs:subClassOf saref:Device ,
                                   s4watr:WaterAsset ;
                   rdfs:comment "A water device is a device that is also a water asset."@en ;
                   rdfs:label "Water device"@en .


###  https://saref.etsi.org/saref4watr/WaterFlowProperty
s4watr:WaterFlowProperty rdf:type owl:Class ;
                         rdfs:subClassOf saref:Property ;
                         rdfs:comment "Class to group those properties related to water flow."@en ;
                         rdfs:label "Water flow property"@en .


###  https://saref.etsi.org/saref4watr/WaterInfrastructure
s4watr:WaterInfrastructure rdf:type owl:Class ;
                           rdfs:subClassOf geosp:Feature ,
                                           saref:FeatureOfInterest ,
                                           s4syst:System ,
                                           [ rdf:type owl:Restriction ;
                                             owl:onProperty s4watr:isDesignedFor ;
                                             owl:someValuesFrom s4watr:Water
                                           ] ,
                                           [ rdf:type owl:Restriction ;
                                             owl:onProperty s4watr:isIntendedFor ;
                                             owl:someValuesFrom s4watr:WaterUse
                                           ] ;
                           rdfs:comment "A water infrastructure is the set of facilities, services, and installations needed for water management."@en ;
                           rdfs:label "Water infrastructure"@en .


###  https://saref.etsi.org/saref4watr/WaterMeter
s4watr:WaterMeter rdf:type owl:Class ;
                  rdfs:subClassOf saref:Meter ,
                                  s4watr:WaterDevice ,
                                  [ rdf:type owl:Restriction ;
                                    owl:onProperty saref:measuresProperty ;
                                    owl:someValuesFrom s4watr:WaterFlowProperty
                                  ] ,
                                  [ rdf:type owl:Restriction ;
                                    owl:onProperty saref:hasProperty ;
                                    owl:allValuesFrom s4watr:WaterMeterProperty
                                  ] ,
                                  [ rdf:type owl:Restriction ;
                                    owl:onProperty s4watr:hasFabricationNumber ;
                                    owl:maxCardinality "1"^^xsd:nonNegativeInteger
                                  ] ,
                                  [ rdf:type owl:Restriction ;
                                    owl:onProperty s4watr:hasFirmwareVersion ;
                                    owl:maxCardinality "1"^^xsd:nonNegativeInteger
                                  ] ,
                                  [ rdf:type owl:Restriction ;
                                    owl:onProperty s4watr:hasHardwareVersion ;
                                    owl:maxCardinality "1"^^xsd:nonNegativeInteger
                                  ] ,
                                  [ rdf:type owl:Restriction ;
                                    owl:onProperty s4watr:hasVersion ;
                                    owl:maxCardinality "1"^^xsd:nonNegativeInteger
                                  ] ;
                  rdfs:comment "A water meter is an instrument intended to measure continuously, memorize, and display the volume of water passing through the meter."@en ;
                  rdfs:label "Water meter"@en .


###  https://saref.etsi.org/saref4watr/WaterMeterProperty
s4watr:WaterMeterProperty rdf:type owl:Class ;
                          rdfs:subClassOf saref:Property ;
                          rdfs:comment "Class to group those properties related to water meters."@en ;
                          rdfs:label "Water meter property"@en .


###  https://saref.etsi.org/saref4watr/WaterProperty
s4watr:WaterProperty rdf:type owl:Class ;
                     rdfs:subClassOf saref:Property ;
                     rdfs:comment "Class to group those properties related to the water."@en ;
                     rdfs:label "Water property"@en .


###  https://saref.etsi.org/saref4watr/WaterUse
s4watr:WaterUse rdf:type owl:Class ;
                rdfs:comment "This class is used to define the different uses of water."@en ;
                rdfs:label "Water use"@en .


###  https://schema.org/Organization
schema:Organization rdf:type owl:Class ;
                    rdfs:subClassOf foaf:Agent ;
                    rdfs:label "Organization"@en .


###  https://schema.org/Person
schema:Person rdf:type owl:Class .


#################################################################
#    Individuals
#################################################################

###  http://dbpedia.org/resource/DBM
<http://dbpedia.org/resource/DBM> rdf:type owl:NamedIndividual ,
                                           saref:UnitOfMeasure ;
                                  rdfs:label "decibel-milliwatts"@en .


###  http://qudt.org/vocab/unit/KiloW-HR
<http://qudt.org/vocab/unit/KiloW-HR> rdf:type owl:NamedIndividual ,
                                               saref:EnergyUnit .


###  http://qudt.org/vocab/unit/M2
<http://qudt.org/vocab/unit/M2> rdf:type owl:NamedIndividual .


###  http://www.ontology-of-units-of-measure.org/resource/om-2/degreeCelsius
<http://www.ontology-of-units-of-measure.org/resource/om-2/degreeCelsius> rdf:type owl:NamedIndividual ,
                                                                                   saref:UnitOfMeasure ;
                                                                          rdfs:label "degree Celsius"@en .


###  http://www.ontology-of-units-of-measure.org/resource/om-2/millibar
<http://www.ontology-of-units-of-measure.org/resource/om-2/millibar> rdf:type owl:NamedIndividual ,
                                                                              saref:UnitOfMeasure ;
                                                                     rdfs:label "millibar"@en .


###  http://www.ontology-of-units-of-measure.org/resource/om-2/millimetre
<http://www.ontology-of-units-of-measure.org/resource/om-2/millimetre> rdf:type owl:NamedIndividual ,
                                                                                saref:UnitOfMeasure ;
                                                                       rdfs:label "millimetre"@en .


###  http://www.ontology-of-units-of-measure.org/resource/om-2/millivolt
<http://www.ontology-of-units-of-measure.org/resource/om-2/millivolt> rdf:type owl:NamedIndividual ,
                                                                               saref:UnitOfMeasure ;
                                                                      rdfs:label "millivolt"@en .


###  http://www.opengis.net/def/uom/ISO-8601/0/Gregorian
<http://www.opengis.net/def/uom/ISO-8601/0/Gregorian> rdf:type owl:NamedIndividual .


###  http://www.w3.org/2006/time#Friday
time:Friday rdf:type owl:NamedIndividual ,
                     time:DayOfWeek ;
            rdfs:label "Friday"@en ;
            skos:prefLabel "Freitag"@de ,
                           "Friday"@en ,
                           "Piątek"@pl ,
                           "Sexta-feira"@pt ,
                           "Vendredi"@fr ,
                           "Venerdì"@it ,
                           "Viernes"@es ,
                           "Vrijdag"@nl ,
                           "Пятница"@ru ,
                           "الجمعة"@ar ,
                           "星期五"@zh ,
                           "金曜日"@ja .


###  http://www.w3.org/2006/time#Monday
time:Monday rdf:type owl:NamedIndividual ,
                     time:DayOfWeek ;
            rdfs:label "Monday"@en ;
            skos:prefLabel "Lundi"@fr ,
                           "Lunedì"@it ,
                           "Lunes"@es ,
                           "Maandag"@nl ,
                           "Monday"@en ,
                           "Montag"@de ,
                           "Poniedziałek"@pl ,
                           "Segunda-feira"@pt ,
                           "Понедельник"@ru ,
                           "الاثنين"@ar ,
                           "星期一"@zh ,
                           "月曜日"@ja .


###  http://www.w3.org/2006/time#Saturday
time:Saturday rdf:type owl:NamedIndividual ,
                       time:DayOfWeek ;
              rdfs:label "Saturday"@en ;
              skos:prefLabel "Sabato"@it ,
                             "Samedi"@fr ,
                             "Samstag"@de ,
                             "Saturday"@en ,
                             "Sobota"@pl ,
                             "Sábado"@es ,
                             "Sábado"@pt ,
                             "Zaterdag"@nl ,
                             "Суббота"@ru ,
                             "السبت"@ar ,
                             "土曜日"@ja ,
                             "星期六"@zh .


###  http://www.w3.org/2006/time#Sunday
time:Sunday rdf:type owl:NamedIndividual ,
                     time:DayOfWeek ;
            rdfs:label "Sunday"@en ;
            skos:prefLabel "Dimanche"@fr ,
                           "Domenica"@it ,
                           "Domingo"@es ,
                           "Domingo"@pt ,
                           "Niedziela"@pl ,
                           "Sonntag"@de ,
                           "Sunday"@en ,
                           "Zondag"@nl ,
                           "Воскресенье"@ru ,
                           "الأحد (يوم)"@ar ,
                           "日曜日"@ja ,
                           "星期日"@zh .


###  http://www.w3.org/2006/time#Thursday
time:Thursday rdf:type owl:NamedIndividual ,
                       time:DayOfWeek ;
              rdfs:label "Thursday"@en ;
              skos:prefLabel "Czwartek"@pl ,
                             "Donderdag"@nl ,
                             "Donnerstag"@de ,
                             "Giovedì"@it ,
                             "Jeudi"@fr ,
                             "Jueves"@es ,
                             "Quinta-feira"@pt ,
                             "Thursday"@en ,
                             "Четверг"@ru ,
                             "الخميس"@ar ,
                             "星期四"@zh ,
                             "木曜日"@ja .


###  http://www.w3.org/2006/time#Tuesday
time:Tuesday rdf:type owl:NamedIndividual ,
                      time:DayOfWeek ;
             rdfs:label "Tuesday"@en ;
             skos:prefLabel "Dienstag"@de ,
                            "Dinsdag"@nl ,
                            "Mardi"@fr ,
                            "Martedì"@it ,
                            "Martes"@es ,
                            "Terça-feira"@pt ,
                            "Tuesday"@en ,
                            "Wtorek"@pl ,
                            "Вторник"@ru ,
                            "الثلاثاء"@ar ,
                            "星期二"@zh ,
                            "火曜日"@ja .


###  http://www.w3.org/2006/time#Wednesday
time:Wednesday rdf:type owl:NamedIndividual ,
                        time:DayOfWeek ;
               rdfs:label "Wednesday"@en ;
               skos:prefLabel "Mercoledì"@it ,
                              "Mercredi"@fr ,
                              "Mittwoch"@de ,
                              "Miércoles"@es ,
                              "Quarta-feira"@pt ,
                              "Wednesday"@en ,
                              "Woensdag"@nl ,
                              "Środa"@pl ,
                              "Среда"@ru ,
                              "الأربعاء"@ar ,
                              "星期三"@zh ,
                              "水曜日"@ja .


###  http://www.w3.org/2006/time#unitDay
time:unitDay rdf:type owl:NamedIndividual ,
                      time:TemporalUnit ;
             time:days 1 ;
             time:hours 0 ;
             time:minutes 0 ;
             time:months 0 ;
             time:seconds 0 ;
             time:weeks 0 ;
             time:years 0 ;
             rdfs:label "Day (unit of temporal duration)"@en ;
             skos:prefLabel "Tag"@de ,
                            "dag"@nl ,
                            "day"@en ,
                            "dia"@pt ,
                            "doba"@pl ,
                            "día"@es ,
                            "giorno"@it ,
                            "jour"@fr ,
                            "يوماً ما"@ar ,
                            "ある日"@jp ,
                            "一天"@zh ,
                            "언젠가"@kr .


###  http://www.w3.org/2006/time#unitHour
time:unitHour rdf:type owl:NamedIndividual ,
                       time:TemporalUnit ;
              time:days 0 ;
              time:hours 1 ;
              time:minutes 0 ;
              time:months 0 ;
              time:seconds 0 ;
              time:weeks 0 ;
              time:years 0 ;
              rdfs:label "Hour (unit of temporal duration)"@en ;
              skos:prefLabel "Stunde"@de ,
                             "godzina"@pl ,
                             "heure"@fr ,
                             "hora"@es ,
                             "hora"@pt ,
                             "hour"@en ,
                             "ora"@it ,
                             "uur"@nl ,
                             "один час\"@ru" ,
                             "ساعة واحدة"@ar ,
                             "一小時"@zh ,
                             "一時間"@jp ,
                             "한 시간"@kr .


###  http://www.w3.org/2006/time#unitMinute
time:unitMinute rdf:type owl:NamedIndividual ,
                         time:TemporalUnit ;
                time:days 0 ;
                time:hours 0 ;
                time:minutes 1 ;
                time:months 0 ;
                time:seconds 0 ;
                time:weeks 0 ;
                time:years 0 ;
                rdfs:label "Minute (unit of temporal duration)"@en ;
                skos:prefLabel "Minute"@de ,
                               "minuta"@pl ,
                               "minute"@en ,
                               "minute"@fr ,
                               "minuto"@es ,
                               "minuto"@it ,
                               "minuto"@pt ,
                               "minuut"@nl ,
                               "одна минута"@ru ,
                               "دقيقة واحدة"@ar ,
                               "一分"@jp ,
                               "等一下"@zh ,
                               "분"@kr .


###  http://www.w3.org/2006/time#unitMonth
time:unitMonth rdf:type owl:NamedIndividual ,
                        time:TemporalUnit ;
               time:days 0 ;
               time:hours 0 ;
               time:minutes 0 ;
               time:months 1 ;
               time:seconds 0 ;
               time:weeks 0 ;
               time:years 0 ;
               rdfs:label "Month (unit of temporal duration)"@en ;
               skos:prefLabel "Monat"@de ,
                              "maand"@nl ,
                              "mes"@es ,
                              "mese"@it ,
                              "miesiąc"@pl ,
                              "mois"@fr ,
                              "month"@en ,
                              "один месяц"@ru ,
                              "شهر واحد"@ar ,
                              "一か月"@jp ,
                              "一個月"@zh ,
                              "한달"@kr .


###  http://www.w3.org/2006/time#unitSecond
time:unitSecond rdf:type owl:NamedIndividual ,
                         time:TemporalUnit ;
                time:days 0 ;
                time:hours 0 ;
                time:minutes 0 ;
                time:months 0 ;
                time:seconds 1 ;
                time:weeks 0 ;
                time:years 0 ;
                rdfs:label "Second (unit of temporal duration)"@en ;
                skos:prefLabel "Sekunde"@de ,
                               "Sekundę"@pl ,
                               "second"@en ,
                               "seconde"@fr ,
                               "seconde"@nl ,
                               "secondo"@it ,
                               "segundo"@es ,
                               "segundo"@pt ,
                               "ثانية واحدة"@ar ,
                               "一秒"@jp ,
                               "一秒"@zh ,
                               "일초"@kr .


###  http://www.w3.org/2006/time#unitWeek
time:unitWeek rdf:type owl:NamedIndividual ,
                       time:TemporalUnit ;
              time:days 0 ;
              time:hours 0 ;
              time:minutes 0 ;
              time:months 0 ;
              time:seconds 0 ;
              time:weeks 1 ;
              time:years 0 ;
              rdfs:label "Week (unit of temporal duration)"@en ;
              skos:prefLabel "Woche"@de ,
                             "semaine"@fr ,
                             "semana"@es ,
                             "semana"@pt ,
                             "settimana"@it ,
                             "tydzień"@pl ,
                             "week"@en ,
                             "week"@nl ,
                             "одна неделя"@ru ,
                             "سبوع واحد"@ar ,
                             "一周"@zh ,
                             "一週間"@jp ,
                             "일주일"@kr .


###  http://www.w3.org/2006/time#unitYear
time:unitYear rdf:type owl:NamedIndividual ,
                       time:TemporalUnit ;
              time:days 0 ;
              time:hours 0 ;
              time:minutes 0 ;
              time:months 0 ;
              time:seconds 0 ;
              time:weeks 0 ;
              time:years 1 ;
              rdfs:label "Year (unit of temporal duration)"@en ;
              skos:prefLabel "1 년"@kr ,
                             "1年"@jp ,
                             "Jahr"@de ,
                             "an"@fr ,
                             "anno"@it ,
                             "ano"@pt ,
                             "jaar"@nl ,
                             "rok"@pl ,
                             "un año"@es ,
                             "year"@en ,
                             "один год"@ru ,
                             "سنة واحدة"@ar ,
                             "一年"@zh .


###  https://saref.etsi.org/core/Cleaning
saref:Cleaning rdf:type owl:NamedIndividual ,
                        saref:Task ;
               rdfs:comment "A type of task for which a device is designed"@en ;
               rdfs:label "Cleaning"@en .


###  https://saref.etsi.org/core/Comfort
saref:Comfort rdf:type owl:NamedIndividual ,
                       saref:Task ;
              rdfs:comment "A type of task for which a device is designed"@en ;
              rdfs:label "Comfort"@en .


###  https://saref.etsi.org/core/Drying
saref:Drying rdf:type owl:NamedIndividual ,
                      saref:Task ;
             rdfs:comment "A type of task for which a device is designed"@en ;
             rdfs:label "Drying"@en .


###  https://saref.etsi.org/core/EnergyEfficiency
saref:EnergyEfficiency rdf:type owl:NamedIndividual ,
                                saref:Task ;
                       rdfs:comment "A type of task for which a device is designed"@en ;
                       rdfs:label "EnergyEfficiency"@en .


###  https://saref.etsi.org/core/Entertainment
saref:Entertainment rdf:type owl:NamedIndividual ,
                             saref:Task ;
                    rdfs:comment "A type of task for which a device is designed"@en ;
                    rdfs:label "Entertainment"@en .


###  https://saref.etsi.org/core/Lighting
saref:Lighting rdf:type owl:NamedIndividual ,
                        saref:Task ;
               rdfs:comment "A type of task for which a device is designed"@en ;
               rdfs:label "Lighting"@en .


###  https://saref.etsi.org/core/MeterReading
saref:MeterReading rdf:type owl:NamedIndividual ,
                            saref:Task ;
                   rdfs:comment "A type of task for which a device is designed"@en ;
                   rdfs:label "Meter reading"@en .


###  https://saref.etsi.org/core/Safety
saref:Safety rdf:type owl:NamedIndividual ,
                      saref:Task ;
             rdfs:comment "A type of task for which a device is designed"@en ;
             rdfs:label "Safety"@en .


###  https://saref.etsi.org/core/Washing
saref:Washing rdf:type owl:NamedIndividual ,
                       saref:Task ;
              rdfs:comment "A type of task for which a device is designed"@en ;
              rdfs:label "Washing"@en .


###  https://saref.etsi.org/core/WellBeing
saref:WellBeing rdf:type owl:NamedIndividual ,
                         saref:Task ;
                rdfs:comment "A type of task for which a device is designed"@en ;
                rdfs:label "WellBeing"@en .


###  https://saref.etsi.org/saref4agri/AirTemperature
s4agri:AirTemperature rdf:type owl:NamedIndividual ,
                               saref:Temperature ;
                      rdfs:comment "The degree or intensity of heat present in the air."@en ;
                      rdfs:label "Air temperature"@en .


###  https://saref.etsi.org/saref4agri/AmbientHumidity
s4agri:AmbientHumidity rdf:type owl:NamedIndividual ,
                                saref:Humidity ;
                       rdfs:comment "The amount of water vapour in the air."@en ;
                       rdfs:label "Ambient humidity"@en .


###  https://saref.etsi.org/saref4agri/IrrigationWater
s4agri:IrrigationWater rdf:type owl:NamedIndividual ,
                                saref:Property ;
                       rdfs:comment "The amount of water falling in the soil by irrigation methods."@en ;
                       rdfs:label "Irrigation water"@en .


###  https://saref.etsi.org/saref4agri/PlantGrowthStage
s4agri:PlantGrowthStage rdf:type owl:NamedIndividual ,
                                 saref:Property ;
                        rdfs:comment "The level or stage of growth of the plant."@en ;
                        rdfs:label "Plant growth stage"@en .


###  https://saref.etsi.org/saref4agri/Precipitation
s4agri:Precipitation rdf:type owl:NamedIndividual ,
                              saref:Property ;
                     rdfs:comment "The amount of water falling in the soil by natural process (e.g. rain)."@en ;
                     rdfs:label "Precipitation"@en .


###  https://saref.etsi.org/saref4agri/SoilMoisture
s4agri:SoilMoisture rdf:type owl:NamedIndividual ,
                             saref:Property ;
                    rdfs:comment "The amount of water or humidity contained in the soil."@en ;
                    rdfs:label "Soil moisture"@en .


###  https://saref.etsi.org/saref4agri/SoilTemperature
s4agri:SoilTemperature rdf:type owl:NamedIndividual ,
                                saref:Temperature ;
                       rdfs:comment "The degree or intensity of heat present in the soil."@en ;
                       rdfs:label "Soil temperature"@en .


###  https://saref.etsi.org/saref4watr/Acrylamide
s4watr:Acrylamide rdf:type owl:NamedIndividual ,
                           s4watr:ChemicalProperty ;
                  rdfs:comment "Property of the water indicating its concentration of acrylamide."@en ;
                  rdfs:label "Acrylamide"@en .


###  https://saref.etsi.org/saref4watr/Agriculture
s4watr:Agriculture rdf:type owl:NamedIndividual ,
                            s4watr:WaterUse ;
                   rdfs:comment "Use of water for the farming of plants and livestock."@en ;
                   rdfs:label "Agriculture"@en .


###  https://saref.etsi.org/saref4watr/Aluminium
s4watr:Aluminium rdf:type owl:NamedIndividual ,
                          s4watr:ChemicalProperty ;
                 rdfs:comment "Property of the water indicating its concentration of aluminium."@en ;
                 rdfs:label "Aluminium"@en .


###  https://saref.etsi.org/saref4watr/Ammonium
s4watr:Ammonium rdf:type owl:NamedIndividual ,
                         s4watr:ChemicalProperty ;
                rdfs:comment "Property of the water indicating its concentration of ammonium."@en ;
                rdfs:label "Ammonium"@en .


###  https://saref.etsi.org/saref4watr/Antimony
s4watr:Antimony rdf:type owl:NamedIndividual ,
                         s4watr:ChemicalProperty ;
                rdfs:comment "Property of the water indicating its concentration of antimony."@en ;
                rdfs:label "Antimony"@en .


###  https://saref.etsi.org/saref4watr/Aquaculture
s4watr:Aquaculture rdf:type owl:NamedIndividual ,
                            s4watr:WaterUse ;
                   rdfs:comment "Use of water for the farming of fish, crustaceans, molluscs, aquatic plants, algae, and other organisms."@en ;
                   rdfs:label "Aquaculture"@en .


###  https://saref.etsi.org/saref4watr/Arsenic
s4watr:Arsenic rdf:type owl:NamedIndividual ,
                        s4watr:ChemicalProperty ;
               rdfs:comment "Property of the water indicating its concentration of arsenic."@en ;
               rdfs:label "Arsenic"@en .


###  https://saref.etsi.org/saref4watr/AtmosphericPressure
s4watr:AtmosphericPressure rdf:type owl:NamedIndividual ,
                                    s4watr:EnvironmentalProperty ;
                           rdfs:comment "Property of the environment indicating the atmospheric pressure."@en ;
                           rdfs:label "Atmospheric pressure"@en .


###  https://saref.etsi.org/saref4watr/BatteryLastChange
s4watr:BatteryLastChange rdf:type owl:NamedIndividual ,
                                  s4watr:WaterMeterProperty ;
                         rdfs:comment "The time in which the battery was last changed."@en ;
                         rdfs:label "Battery last change"@en .


###  https://saref.etsi.org/saref4watr/BatteryOperatingTime
s4watr:BatteryOperatingTime rdf:type owl:NamedIndividual ,
                                     s4watr:WaterMeterProperty ;
                            rdfs:comment "The time for which the battery has been operating since the last charge."@en ;
                            rdfs:label "Battery operating time"@en .


###  https://saref.etsi.org/saref4watr/BatteryRemainingTime
s4watr:BatteryRemainingTime rdf:type owl:NamedIndividual ,
                                     s4watr:WaterMeterProperty ;
                            rdfs:comment "The time until the battery is discharged."@en ;
                            rdfs:label "Battery remaining time"@en .


###  https://saref.etsi.org/saref4watr/Benzene
s4watr:Benzene rdf:type owl:NamedIndividual ,
                        s4watr:ChemicalProperty ;
               rdfs:comment "Property of the water indicating its concentration of benzene."@en ;
               rdfs:label "Benzene"@en .


###  https://saref.etsi.org/saref4watr/Benzoapyrene
s4watr:Benzoapyrene rdf:type owl:NamedIndividual ,
                             s4watr:ChemicalProperty ;
                    rdfs:comment "Property of the water indicating its concentration of benzo(a)pyrene."@en ;
                    rdfs:label "Benzo(a)pyrene"@en .


###  https://saref.etsi.org/saref4watr/Boron
s4watr:Boron rdf:type owl:NamedIndividual ,
                      s4watr:ChemicalProperty ;
             rdfs:comment "Property of the water indicating its concentration of boron."@en ;
             rdfs:label "Boron"@en .


###  https://saref.etsi.org/saref4watr/Bromate
s4watr:Bromate rdf:type owl:NamedIndividual ,
                        s4watr:ChemicalProperty ;
               rdfs:comment "Property of the water indicating its concentration of bromate."@en ;
               rdfs:label "Bromate"@en .


###  https://saref.etsi.org/saref4watr/Cadmium
s4watr:Cadmium rdf:type owl:NamedIndividual ,
                        s4watr:ChemicalProperty ;
               rdfs:comment "Property of the water indicating its concentration of cadmium."@en ;
               rdfs:label "Cadmium"@en .


###  https://saref.etsi.org/saref4watr/Chloride
s4watr:Chloride rdf:type owl:NamedIndividual ,
                         s4watr:ChemicalProperty ;
                rdfs:comment "Property of the water indicating its concentration of chloride."@en ;
                rdfs:label "Chloride"@en .


###  https://saref.etsi.org/saref4watr/Chromium
s4watr:Chromium rdf:type owl:NamedIndividual ,
                         s4watr:ChemicalProperty ;
                rdfs:comment "Property of the water indicating its concentration of chromium."@en ;
                rdfs:label "Chromium"@en .


###  https://saref.etsi.org/saref4watr/ClostridiumPerfringens
s4watr:ClostridiumPerfringens rdf:type owl:NamedIndividual ,
                                       s4watr:BacterialProperty ;
                              rdfs:comment "Property of the water indicating its concentration of clostridium perfringens."@en ;
                              rdfs:label "Clostridium perfringens"@en .


###  https://saref.etsi.org/saref4watr/ColiformBacteria
s4watr:ColiformBacteria rdf:type owl:NamedIndividual ,
                                 s4watr:BacterialProperty ;
                        rdfs:comment "Property of the water indicating its concentration of coliform bacteria."@en ;
                        rdfs:label "Coliform bacteria"@en .


###  https://saref.etsi.org/saref4watr/ColonyCount22C
s4watr:ColonyCount22C rdf:type owl:NamedIndividual ,
                               s4watr:BacterialProperty ;
                      rdfs:comment "Property of the water indicating its colony count at 22 ºC."@en ;
                      rdfs:label "Colony count at 22 °C"@en .


###  https://saref.etsi.org/saref4watr/ColonyCount37C
s4watr:ColonyCount37C rdf:type owl:NamedIndividual ,
                               s4watr:BacterialProperty ;
                      rdfs:comment "Property of the water indicating its colony count at 37 ºC."@en ;
                      rdfs:label "Colony count at 37 °C"@en .


###  https://saref.etsi.org/saref4watr/Colour
s4watr:Colour rdf:type owl:NamedIndividual ,
                       s4watr:AcceptabilityProperty ;
              rdfs:comment "Property of the water indicating its colour."@en ;
              rdfs:label "Colour"@en .


###  https://saref.etsi.org/saref4watr/Conductivity
s4watr:Conductivity rdf:type owl:NamedIndividual ,
                             s4watr:AcceptabilityProperty ;
                    rdfs:comment "Property of the water indicating its conductivity."@en ;
                    rdfs:label "Conductivity"@en .


###  https://saref.etsi.org/saref4watr/Copper
s4watr:Copper rdf:type owl:NamedIndividual ,
                       s4watr:ChemicalProperty ;
              rdfs:comment "Property of the water indicating its concentration of copper."@en ;
              rdfs:label "Copper"@en .


###  https://saref.etsi.org/saref4watr/Cyanide
s4watr:Cyanide rdf:type owl:NamedIndividual ,
                        s4watr:ChemicalProperty ;
               rdfs:comment "Property of the water indicating its concentration of cyanide."@en ;
               rdfs:label "Cyanide"@en .


###  https://saref.etsi.org/saref4watr/Domestic
s4watr:Domestic rdf:type owl:NamedIndividual ,
                         s4watr:WaterUse ;
                rdfs:comment "Use of water for domestic purposes."@en ;
                rdfs:label "Domestic"@en .


###  https://saref.etsi.org/saref4watr/DrinkingWater
s4watr:DrinkingWater rdf:type owl:NamedIndividual ,
                              s4watr:Water ;
                     rdfs:comment "Drinking water is water that is treated to comply with drinking water standards."@en ;
                     rdfs:label "Drinking water"@en ,
                                "Potable water"@en .


###  https://saref.etsi.org/saref4watr/Enterococci
s4watr:Enterococci rdf:type owl:NamedIndividual ,
                            s4watr:BacterialProperty ;
                   rdfs:comment "Property of the water indicating its concentration of enterococci."@en ;
                   rdfs:label "Enterococci"@en .


###  https://saref.etsi.org/saref4watr/Epichlorohydrin
s4watr:Epichlorohydrin rdf:type owl:NamedIndividual ,
                                s4watr:ChemicalProperty ;
                       rdfs:comment "Property of the water indicating its concentration of epichlorohydrin."@en ;
                       rdfs:label "Epichlorohydrin"@en .


###  https://saref.etsi.org/saref4watr/EscherichiaColi
s4watr:EscherichiaColi rdf:type owl:NamedIndividual ,
                                s4watr:BacterialProperty ;
                       rdfs:comment "Property of the water indicating its concentration of escherichia coli."@en ;
                       rdfs:label "E. coli"@en ,
                                  "Escherichia coli"@en .


###  https://saref.etsi.org/saref4watr/ExternalTemperature
s4watr:ExternalTemperature rdf:type owl:NamedIndividual ,
                                    s4watr:EnvironmentalProperty ;
                           rdfs:comment "Property of the environment indicating the temperature."@en ;
                           rdfs:label "External temperature"@en .


###  https://saref.etsi.org/saref4watr/FlowPressure
s4watr:FlowPressure rdf:type owl:NamedIndividual ,
                             s4watr:WaterFlowProperty ;
                    rdfs:comment "Property indicating the pressure of a water flow."@en ;
                    rdfs:label "Flow pressure"@en .


###  https://saref.etsi.org/saref4watr/FlowRate
s4watr:FlowRate rdf:type owl:NamedIndividual ,
                         s4watr:WaterFlowProperty ;
                rdfs:comment "Property indicating the rate of a water flow."@en ;
                rdfs:label "Flow rate"@en .


###  https://saref.etsi.org/saref4watr/FlowTemperature
s4watr:FlowTemperature rdf:type owl:NamedIndividual ,
                                s4watr:WaterFlowProperty ;
                       rdfs:comment "Property indicating the temperature of a water flow."@en ;
                       rdfs:label "Flow temperature"@en .


###  https://saref.etsi.org/saref4watr/FlowVolume
s4watr:FlowVolume rdf:type owl:NamedIndividual ,
                           s4watr:WaterFlowProperty ;
                  rdfs:comment "Property indicating the volume of a water flow."@en ;
                  rdfs:label "Flow volume"@en .


###  https://saref.etsi.org/saref4watr/Fluoride
s4watr:Fluoride rdf:type owl:NamedIndividual ,
                         s4watr:ChemicalProperty ;
                rdfs:comment "Property of the water indicating its concentration of fluoride."@en ;
                rdfs:label "Fluoride"@en .


###  https://saref.etsi.org/saref4watr/Hardness
s4watr:Hardness rdf:type owl:NamedIndividual ,
                         s4watr:AcceptabilityProperty ;
                rdfs:comment "Property of the water indicating its hardness."@en ;
                rdfs:label "Hardness"@en .


###  https://saref.etsi.org/saref4watr/Humidity
s4watr:Humidity rdf:type owl:NamedIndividual ,
                         s4watr:EnvironmentalProperty ;
                rdfs:comment "Property of the environment indicating the humidity."@en ;
                rdfs:label "Humidity"@en .


###  https://saref.etsi.org/saref4watr/HydrogenIonConcentration
s4watr:HydrogenIonConcentration rdf:type owl:NamedIndividual ,
                                         s4watr:AcceptabilityProperty ;
                                rdfs:comment "Property of the water indicating its hydrogen ion concentration."@en ;
                                rdfs:label "Hydrogen ion concentration"@en ,
                                           "pH"@en .


###  https://saref.etsi.org/saref4watr/Industry
s4watr:Industry rdf:type owl:NamedIndividual ,
                         s4watr:WaterUse ;
                rdfs:comment "Use of water for industrial purposes."@en ;
                rdfs:label "Industry"@en .


###  https://saref.etsi.org/saref4watr/Iron
s4watr:Iron rdf:type owl:NamedIndividual ,
                     s4watr:ChemicalProperty ;
            rdfs:comment "Property of the water indicating its concentration of iron."@en ;
            rdfs:label "Iron"@en .


###  https://saref.etsi.org/saref4watr/Lead
s4watr:Lead rdf:type owl:NamedIndividual ,
                     s4watr:ChemicalProperty ;
            rdfs:comment "Property of the water indicating its concentration of lead."@en ;
            rdfs:label "Lead"@en .


###  https://saref.etsi.org/saref4watr/Manganese
s4watr:Manganese rdf:type owl:NamedIndividual ,
                          s4watr:ChemicalProperty ;
                 rdfs:comment "Property of the water indicating its concentration of manganese."@en ;
                 rdfs:label "Manganese"@en .


###  https://saref.etsi.org/saref4watr/Mercury
s4watr:Mercury rdf:type owl:NamedIndividual ,
                        s4watr:ChemicalProperty ;
               rdfs:comment "Property of the water indicating its concentration of mercury."@en ;
               rdfs:label "Mercury"@en .


###  https://saref.etsi.org/saref4watr/MeterOnTime
s4watr:MeterOnTime rdf:type owl:NamedIndividual ,
                            s4watr:WaterMeterProperty ;
                   rdfs:comment "The duration of the meter power up."@en ;
                   rdfs:label "Meter on time"@en .


###  https://saref.etsi.org/saref4watr/MeterOperatingTime
s4watr:MeterOperatingTime rdf:type owl:NamedIndividual ,
                                   s4watr:WaterMeterProperty ;
                          rdfs:comment "The time for which the meter has been operating."@en ;
                          rdfs:label "Meter operating time"@en .


###  https://saref.etsi.org/saref4watr/Nickel
s4watr:Nickel rdf:type owl:NamedIndividual ,
                       s4watr:ChemicalProperty ;
              rdfs:comment "Property of the water indicating its concentration of nickel."@en ;
              rdfs:label "Nickel"@en .


###  https://saref.etsi.org/saref4watr/Nitrate
s4watr:Nitrate rdf:type owl:NamedIndividual ,
                        s4watr:ChemicalProperty ;
               rdfs:comment "Property of the water indicating its concentration of nitrate."@en ;
               rdfs:label "Nitrate"@en .


###  https://saref.etsi.org/saref4watr/Nitrite
s4watr:Nitrite rdf:type owl:NamedIndividual ,
                        s4watr:ChemicalProperty ;
               rdfs:comment "Property of the water indicating its concentration of nitrite."@en ;
               rdfs:label "Nitrite"@en .


###  https://saref.etsi.org/saref4watr/Odour
s4watr:Odour rdf:type owl:NamedIndividual ,
                      s4watr:AcceptabilityProperty ;
             rdfs:comment "Property of the water indicating its odour."@en ;
             rdfs:label "Odour"@en .


###  https://saref.etsi.org/saref4watr/Oxidisability
s4watr:Oxidisability rdf:type owl:NamedIndividual ,
                              s4watr:AcceptabilityProperty ;
                     rdfs:comment "Property of the water indicating its oxidisability."@en ;
                     rdfs:label "Oxidisability"@en .


###  https://saref.etsi.org/saref4watr/Oxygen
s4watr:Oxygen rdf:type owl:NamedIndividual ,
                       s4watr:ChemicalProperty ;
              rdfs:comment "Property of the water indicating its oxygen saturation."@en ;
              rdfs:label "Dissolved oxygen"@en ,
                         "Oxygen"@en ,
                         "Oxygen saturation"@en .


###  https://saref.etsi.org/saref4watr/PolycyclicAromaticHydrocarbons
s4watr:PolycyclicAromaticHydrocarbons rdf:type owl:NamedIndividual ,
                                               s4watr:ChemicalProperty ;
                                      rdfs:comment "Property of the water indicating its concentration of polycyclic aromatic hydrocarbons."@en ;
                                      rdfs:label "Polycyclic aromatic hydrocarbons"@en .


###  https://saref.etsi.org/saref4watr/Precipitation
s4watr:Precipitation rdf:type owl:NamedIndividual ,
                              s4watr:EnvironmentalProperty ;
                     rdfs:comment "Property of the environment indicating the precipitation."@en ;
                     rdfs:label "Precipitation"@en .


###  https://saref.etsi.org/saref4watr/PseudomonasAeruginosa
s4watr:PseudomonasAeruginosa rdf:type owl:NamedIndividual ,
                                      s4watr:BacterialProperty ;
                             rdfs:comment "Property of the water indicating its concentration of pseudomonas aeruginosa."@en ;
                             rdfs:label "Pseudomonas aeruginosa"@en .


###  https://saref.etsi.org/saref4watr/RawWater
s4watr:RawWater rdf:type owl:NamedIndividual ,
                         s4watr:Water ;
                rdfs:comment "Raw water is water found in the environment that has not been treated and does not have any of its minerals, ions, particles, bacteria, or parasites removed."@en ;
                rdfs:label "Raw water"@en .


###  https://saref.etsi.org/saref4watr/Recreation
s4watr:Recreation rdf:type owl:NamedIndividual ,
                           s4watr:WaterUse ;
                  rdfs:comment "Use of water for recreational purposes."@en ;
                  rdfs:label "Recreation"@en .


###  https://saref.etsi.org/saref4watr/Selenium
s4watr:Selenium rdf:type owl:NamedIndividual ,
                         s4watr:ChemicalProperty ;
                rdfs:comment "Property of the water indicating its concentration of selenium."@en ;
                rdfs:label "Selenium"@en .


###  https://saref.etsi.org/saref4watr/Sodium
s4watr:Sodium rdf:type owl:NamedIndividual ,
                       s4watr:ChemicalProperty ;
              rdfs:comment "Property of the water indicating its concentration of sodium."@en ;
              rdfs:label "Sodium"@en .


###  https://saref.etsi.org/saref4watr/Stormwater
s4watr:Stormwater rdf:type owl:NamedIndividual ,
                           s4watr:Water ;
                  rdfs:comment "Stormwater is water that originates during precipitation events and snow/ice melt."@en ;
                  rdfs:label "Storm water"@en .


###  https://saref.etsi.org/saref4watr/Sulphate
s4watr:Sulphate rdf:type owl:NamedIndividual ,
                         s4watr:ChemicalProperty ;
                rdfs:comment "Property of the water indicating its concentration of sulphate."@en ;
                rdfs:label "Sulphate"@en .


###  https://saref.etsi.org/saref4watr/Taste
s4watr:Taste rdf:type owl:NamedIndividual ,
                      s4watr:AcceptabilityProperty ;
             rdfs:comment "Property of the water indicating its taste."@en ;
             rdfs:label "Taste"@en .


###  https://saref.etsi.org/saref4watr/Temperature
s4watr:Temperature rdf:type owl:NamedIndividual ,
                            s4watr:AcceptabilityProperty ;
                   rdfs:comment "Property of the water indicating its temperature."@en ;
                   rdfs:label "Temperature"@en .


###  https://saref.etsi.org/saref4watr/Tetrachloroethene
s4watr:Tetrachloroethene rdf:type owl:NamedIndividual ,
                                  s4watr:ChemicalProperty ;
                         rdfs:comment "Property of the water indicating its concentration of tetrachloroethene."@en ;
                         rdfs:label "Tetrachloroethene"@en .


###  https://saref.etsi.org/saref4watr/TotalDissolvedSolids
s4watr:TotalDissolvedSolids rdf:type owl:NamedIndividual ,
                                     s4watr:AcceptabilityProperty ;
                            rdfs:comment "Property of the water indicating the dissolved combined content of all inorganic and organic substances present in a sample of water."@en ;
                            rdfs:label "Total dissolved solids"@en .


###  https://saref.etsi.org/saref4watr/TotalIndicativeDose
s4watr:TotalIndicativeDose rdf:type owl:NamedIndividual ,
                                    s4watr:AcceptabilityProperty ;
                           rdfs:comment "Property of the water indicating its total indicative dose."@en ;
                           rdfs:label "Total indicative dose"@en .


###  https://saref.etsi.org/saref4watr/TotalOrganicCarbon
s4watr:TotalOrganicCarbon rdf:type owl:NamedIndividual ,
                                   s4watr:ChemicalProperty ;
                          rdfs:comment "Property of the water indicating its concentration of total organic carbon."@en ;
                          rdfs:label "TOC"@en ,
                                     "Total organic carbon"@en .


###  https://saref.etsi.org/saref4watr/TotalSuspendedSolids
s4watr:TotalSuspendedSolids rdf:type owl:NamedIndividual ,
                                     s4watr:AcceptabilityProperty ;
                            rdfs:comment "Property of the water indicating the dry-weight of suspended particles, that are not dissolved, in a sample of water."@en ;
                            rdfs:label "Total suspended solids"@en .


###  https://saref.etsi.org/saref4watr/Trichloroethene
s4watr:Trichloroethene rdf:type owl:NamedIndividual ,
                                s4watr:ChemicalProperty ;
                       rdfs:comment "Property of the water indicating its concentration of trichloroethene."@en ;
                       rdfs:label "Trichloroethene"@en .


###  https://saref.etsi.org/saref4watr/Trihalomethanes
s4watr:Trihalomethanes rdf:type owl:NamedIndividual ,
                                s4watr:ChemicalProperty ;
                       rdfs:comment "Property of the water indicating its concentration of trihalomethanes."@en ;
                       rdfs:label "Trihalomethanes"@en .


###  https://saref.etsi.org/saref4watr/Tritium
s4watr:Tritium rdf:type owl:NamedIndividual ,
                        s4watr:ChemicalProperty ;
               rdfs:comment "Property of the water indicating its concentration of tritium."@en ;
               rdfs:label "Tritium"@en .


###  https://saref.etsi.org/saref4watr/Turbidity
s4watr:Turbidity rdf:type owl:NamedIndividual ,
                          s4watr:AcceptabilityProperty ;
                 rdfs:comment "Property of the water indicating its turbidity."@en ;
                 rdfs:label "Turbidity"@en .


###  https://saref.etsi.org/saref4watr/VinylChloride
s4watr:VinylChloride rdf:type owl:NamedIndividual ,
                              s4watr:ChemicalProperty ;
                     rdfs:comment "Property of the water indicating its concentration of vinyl chloride."@en ;
                     rdfs:label "Vinyl chloride"@en .


###  https://saref.etsi.org/saref4watr/Wastewater
s4watr:Wastewater rdf:type owl:NamedIndividual ,
                           s4watr:Water ;
                  rdfs:comment "Wastewater is water that has been used in the home, in a business, or as part of an industrial process."@en ;
                  rdfs:label "Waste water"@en .


###  https://saref.etsi.org/saref4watr/12Dichloroethane
<https://saref.etsi.org/saref4watr/12Dichloroethane> rdf:type owl:NamedIndividual ,
                                                              s4watr:ChemicalProperty ;
                                                     rdfs:comment "Property of the water indicating its concentration of 1,2-dichloroethane."@en ;
                                                     rdfs:label "1,2-dichloroethane"@en .


[ foaf:PersonalProfileDocument <https://www.linkedin.com/in/tatianatarasova>
] .

[ foaf:homepage <http://www.smartopendata.eu> ;
   foaf:name "SmartOpenData project"
 ] .

[ schema:affiliation "Australian National University" ,
                      "SURROUND Australia Pty Ltd" ;
   schema:email "nicholas.car@surroundaustralia.com"^^xsd:anyURI ;
   schema:name "Nicholas J. Car" ;
   schema:url "https://orcid.org/0000-0002-8742-7730"^^xsd:anyURI
 ] .

[ schema:name "Open Geospatial Consortium" ;
   schema:url "https://www.ogc.org"^^xsd:anyURI
 ] .

[ schema:affiliation "Geoscape Australia" ;
   schema:email "joseph.abhayaratna@geoscape.com.au"^^xsd:anyURI ;
   schema:name "Joseph Abhayaratna" ;
   schema:url "https://orcid.org/0000-0001-5075-6234"^^xsd:anyURI
 ] .

[ schema:affiliation "CSIRO Australia" ;
   schema:email "simon.cox@csiro.au"^^xsd:anyURI ;
   schema:name "Simon J D Cox" ;
   schema:url "https://orcid.org/0000-0002-3884-3420"^^xsd:anyURI
 ] .

[ schema:email "fjknibbe@gmail.com"^^xsd:anyURI ;
   schema:name "Frans Knibbe" ;
   schema:url "https://orcid.org/0000-0003-3789-2260"^^xsd:anyURI
 ] .

[ schema:affiliation "Oracle Corporation" ;
   schema:email "matthew.perry@oracle.com"^^xsd:anyURI ;
   schema:name "Matthew Perry" ;
   schema:url "https://orcid.org/0000-0003-1988-462X"^^xsd:anyURI
 ] .

[ schema:affiliation "Mainz University Of Applied Sciences" ;
   schema:email "timo.homburg@hs-mainz.de"^^xsd:anyURI ;
   schema:name "Timo Homburg" ;
   schema:url "https://orcid.org/0000-0002-9499-5840"^^xsd:anyURI
 ] .

[ schema:affiliation "Oracle Corporation" ;
   schema:email "john.herring@oracle.com"^^xsd:anyURI ;
   schema:name "John Herring"
 ] .

[ schema:affiliation "KU Leuven" ,
                      "Neanex Technologies" ;
   schema:email "mathias.bonduel@neanex.com"^^xsd:anyURI ;
   schema:name "Mathias Bonduel" ;
   schema:url "https://orcid.org/0000-0002-3313-924X"^^xsd:anyURI
 ] .

[ xsd:pattern "-?([1-9][0-9]{3,}|0[0-9]{3})(Z|(\\+|-)((0[0-9]|1[0-3]):[0-5][0-9]|14:00))?"
 ] .

[ xsd:pattern "--(0[1-9]|1[0-9]|20)(Z|(\\+|-)((0[0-9]|1[0-3]):[0-5][0-9]|14:00))?"
 ] .

[ xsd:pattern "---(0[1-9]|[1-9][0-9])(Z|(\\+|-)((0[0-9]|1[0-3]):[0-5][0-9]|14:00))?"
 ] .

#################################################################
#    Annotations
#################################################################

wgs84: dc:date "$Date: 2009/04/20 15:00:30 $" ;
        rdfs:label "geo" ;
        dc:description """A vocabulary for representing latitude, longitude and 
 altitude information in the WGS84 geodetic reference datum. 
 Version $Id: wgs84_pos.rdf,v 1.22 2009/04/20 15:00:30 timbl Exp $. See http://www.w3.org/2003/01/geo/ for more details.""" ;
        rdfs:comment """
Recent changes to this namespace:
$Log: wgs84_pos.rdf,v $
Revision 1.22  2009/04/20 15:00:30  timbl
Remove the time bits which have been deal with elsewhere eg in iCal.

Revision 1.21  2009/04/20 12:52:47  timbl
try again

Revision 1.20  2009/04/20 12:42:11  timbl
Add Event (edited ages ago and never checked in), and location (following discussion http://chatlogs.planetrdf.com/swig/2009-04-20#T12-36-09)

Revision 1.19  2009/04/20 12:36:31  timbl
Add Event (edited ages ago and never checked in), and location (following discussion http://chatlogs.planetrdf.com/swig/2009-04-20#T12-36-09)

Revision 1.18  2006/02/01 22:01:04  danbri
Clarified that lat and long are decimal degrees, and that alt is decimal metres about local reference ellipsoid

Revision 1.17  2004/02/06 17:38:12  danbri
Fixed a bad commit screwup

Revision 1.15  2003/04/19 11:24:08  danbri
Fixed the typo even more.

Revision 1.14  2003/04/19 11:16:56  danbri
fixed a typo

Revision 1.13  2003/02/19 22:27:27  connolly
relaxed domain constraints on lat/long/alt from Point to SpatialThing

Revision 1.12  2003/01/12 01:41:41  danbri
Trying local copy of XSLT doc.

Revision 1.11  2003/01/12 01:20:18  danbri
added a link to morten's xslt rdfs viewer.

Revision 1.10  2003/01/11 18:56:49  danbri
Removed datatype range from lat and long properties, since they would
have required each occurance of the property to mention the datatype.

Revision 1.9  2003/01/11 11:41:31  danbri
Another typo; repaired rdfs:Property to rdf:Property x4

Revision 1.8  2003/01/11 11:05:02  danbri
Added an rdfs:range for each lat/long/alt property,
http://www.w3.org/2001/XMLSchema#float

Revision 1.7  2003/01/10 20:25:16  danbri
Longer rdfs:comment for Point, trying to be Earth-centric and neutral about
coordinate system(s) at the same time. Feedback welcomed.

Revision 1.6  2003/01/10 20:18:30  danbri
Added CVS log comments into the RDF/XML as an rdfs:comment property of the
vocabulary. Note that this is not common practice (but seems both harmless
and potentially useful).


revision 1.5
date: 2003/01/10 20:14:31;  author: danbri;  state: Exp;  lines: +16 -5
Updated schema:
Added a dc:date, added url for more info. Changed the rdfs:label of the
namespace from gp to geo. Added a class Point, set as the rdfs:domain of
each property. Added XML comment on the lat_long property suggesting that
we might not need it (based on #rdfig commentary from implementors).

revision 1.4
date: 2003/01/10 20:01:07;  author: danbri;  state: Exp;  lines: +6 -5
Fixed typo; several rdfs:about attributes are now rdf:about. Thanks to MortenF in
#rdfig for catching this error.

revision 1.3
date: 2003/01/10 11:59:03;  author: danbri;  state: Exp;  lines: +4 -3
fixed buglet in vocab, added more wgs links

revision 1.2
date: 2003/01/10 11:01:11;  author: danbri;  state: Exp;  lines: +4 -4
Removed alt from the as-a-flat-string property, and switched from
space separated to comma separated.

revision 1.1
date: 2003/01/10 10:53:23;  author: danbri;  state: Exp;
basic geo vocab

""" ;
        dc:title "WGS84 Geo Positioning: an RDF vocabulary" .


wgs84:alt rdfs:comment "The WGS84 altitude of a SpatialThing (decimal meters above the local reference ellipsoid)."@en ;
          rdfs:label "altitude" ,
                     "altitude"@en ;
          rdfs:comment """The WGS84 altitude of a SpatialThing (decimal meters 
above the local reference ellipsoid).""" .


wgs84:lat rdfs:comment "The WGS84 latitude of a SpatialThing (decimal degrees)." ;
          rdfs:label "latitude"@en ,
                     "latitude" ;
          rdfs:comment "The WGS84 latitude of a SpatialThing (decimal degrees)."@en .


wgs84:lat_long rdfs:comment "A comma-separated representation of a latitude, longitude coordinate." ;
               rdfs:label "lat/long" .


wgs84:location rdfs:isDefinedBy wgs84: ;
               rdfs:label "location" ;
               rdfs:comment """The relation between something and the point, 
 or other geometrical thing in space, where it is.  For example, the realtionship between
 a radio tower and a Point with a given lat and long.
 Or a relationship between a park and its outline as a closed arc of points, or a road and
 its location as a arc (a sequence of points).
 Clearly in practice there will be limit to the accuracy of any such statement, but one would expect
 an accuracy appropriate for the size of the object and uses such as mapping .
 """ ,
                            """The relation between something and the point, 
 or other geometrical thing in space, where it is.  For example, the realtionship between
 a radio tower and a Point with a given lat and long.
 Or a relationship between a park and its outline as a closed arc of points, or a road and
 its location as a arc (a sequence of points).
 Clearly in practice there will be limit to the accuracy of any such statement, but one would expect
 an accuracy appropriate for the size of the object and uses such as mapping .
 """@en ,
                            "The relation between something and the point,  or other geometrical thing in space, where it is.  For example, the realtionship between a radio tower and a Point with a given lat and long. Or a relationship between a park and its outline as a closed arc of points, or a road and its location as a arc (a sequence of points). Clearly in practice there will be limit to the accuracy of any such statement, but one would expect an accuracy appropriate for the size of the object and uses such as mapping ."@en ;
               rdfs:label "location"@en .


wgs84:long rdfs:comment "The WGS84 longitude of a SpatialThing (decimal degrees)."@en ;
           rdfs:label "longitude"@en ,
                      "longitude" ;
           rdfs:comment "The WGS84 longitude of a SpatialThing (decimal degrees)." .


###  Generated by the OWL API (version 4.5.9.2019-02-01T07:24:44Z) https://github.com/owlcs/owlapi
